@prefix adms: <http://www.w3.org/ns/adms#> .
@prefix dc: <http://purl.org/dc/elements/1.1/> .
@prefix dcat: <http://www.w3.org/ns/dcat#> .
@prefix dct: <http://purl.org/dc/terms/> .
@prefix doap: <http://usefulinc.com/ns/doap#> .
@prefix euvoc: <http://publications.europa.eu/ontology/euvoc#> .
@prefix foaf: <http://xmlns.com/foaf/0.1/> .
@prefix org: <http://www.w3.org/ns/org#> .
@prefix owl: <http://www.w3.org/2002/07/owl#> .
@prefix prov: <http://www.w3.org/ns/prov#> .
@prefix qb: <http://purl.org/linked-data/cube#> .
@prefix rdf: <http://www.w3.org/1999/02/22-rdf-syntax-ns#> .
@prefix rdfs: <http://www.w3.org/2000/01/rdf-schema#> .
@prefix schema: <http://schema.org/> .
@prefix sh: <http://www.w3.org/ns/shacl#> .
@prefix skos: <http://www.w3.org/2004/02/skos/core#> .
@prefix skosthes: <http://purl.org/iso25964/skos-thes#> .
@prefix skosxl: <http://www.w3.org/2008/05/skos-xl#> .
@prefix xsd: <http://www.w3.org/2001/XMLSchema#> .

<https://w3id.org/permafrost/v/nrcglossary/scheme> a skos:ConceptScheme;
  dct:created "2022-10-25"^^xsd:date;
  dct:description "Glossary of permafrost and related ground-ice terms";
  dct:identifier "ipaglossary"^^xsd:token;
  dct:modified "2022-10-25"^^xsd:date;
  dct:references <https://nrc-publications.canada.ca/fra/voir/objet/?id=549123c3-092c-4fca-8dea-99d53eac06dd;https://nrc-publications.canada.ca/eng/view/object/?id=69fb8993-1baa-4225-b33a-6a02341d383d>;
  dct:source "https://nrc-publications.canada.ca/fra/voir/objet/?id=549123c3-092c-4fca-8dea-99d53eac06dd;https://nrc-publications.canada.ca/eng/view/object/?id=69fb8993-1baa-4225-b33a-6a02341d383d"^^xsd:anyURI;
  dct:title "NRC Permafrost Glossary";
  owl:versionInfo "1";
  skos:definition "Glossary of permafrost and related ground-ice terms";
  skos:hasTopConcept <https://w3id.org/permafrost/v/nrcglossary/t0001>, <https://w3id.org/permafrost/v/nrcglossary/t0002>,
    <https://w3id.org/permafrost/v/nrcglossary/t0003>, <https://w3id.org/permafrost/v/nrcglossary/t0004>,
    <https://w3id.org/permafrost/v/nrcglossary/t0005>, <https://w3id.org/permafrost/v/nrcglossary/t0006>,
    <https://w3id.org/permafrost/v/nrcglossary/t0007>, <https://w3id.org/permafrost/v/nrcglossary/t0008>,
    <https://w3id.org/permafrost/v/nrcglossary/t0009>, <https://w3id.org/permafrost/v/nrcglossary/t0010>,
    <https://w3id.org/permafrost/v/nrcglossary/t0011>, <https://w3id.org/permafrost/v/nrcglossary/t0012>,
    <https://w3id.org/permafrost/v/nrcglossary/t0013>, <https://w3id.org/permafrost/v/nrcglossary/t0014>,
    <https://w3id.org/permafrost/v/nrcglossary/t0015>, <https://w3id.org/permafrost/v/nrcglossary/t0016>,
    <https://w3id.org/permafrost/v/nrcglossary/t0017>, <https://w3id.org/permafrost/v/nrcglossary/t0018>,
    <https://w3id.org/permafrost/v/nrcglossary/t0019>, <https://w3id.org/permafrost/v/nrcglossary/t0020>,
    <https://w3id.org/permafrost/v/nrcglossary/t0021>, <https://w3id.org/permafrost/v/nrcglossary/t0022>,
    <https://w3id.org/permafrost/v/nrcglossary/t0023>, <https://w3id.org/permafrost/v/nrcglossary/t0024>,
    <https://w3id.org/permafrost/v/nrcglossary/t0025>, <https://w3id.org/permafrost/v/nrcglossary/t0026>,
    <https://w3id.org/permafrost/v/nrcglossary/t0027>, <https://w3id.org/permafrost/v/nrcglossary/t0028>,
    <https://w3id.org/permafrost/v/nrcglossary/t0029>, <https://w3id.org/permafrost/v/nrcglossary/t0030>,
    <https://w3id.org/permafrost/v/nrcglossary/t0031>, <https://w3id.org/permafrost/v/nrcglossary/t0032>,
    <https://w3id.org/permafrost/v/nrcglossary/t0033>, <https://w3id.org/permafrost/v/nrcglossary/t0034>,
    <https://w3id.org/permafrost/v/nrcglossary/t0035>, <https://w3id.org/permafrost/v/nrcglossary/t0036>,
    <https://w3id.org/permafrost/v/nrcglossary/t0037>, <https://w3id.org/permafrost/v/nrcglossary/t0038>,
    <https://w3id.org/permafrost/v/nrcglossary/t0039>, <https://w3id.org/permafrost/v/nrcglossary/t0040>,
    <https://w3id.org/permafrost/v/nrcglossary/t0041>, <https://w3id.org/permafrost/v/nrcglossary/t0042>,
    <https://w3id.org/permafrost/v/nrcglossary/t0043>, <https://w3id.org/permafrost/v/nrcglossary/t0044>,
    <https://w3id.org/permafrost/v/nrcglossary/t0045>, <https://w3id.org/permafrost/v/nrcglossary/t0046>,
    <https://w3id.org/permafrost/v/nrcglossary/t0047>, <https://w3id.org/permafrost/v/nrcglossary/t0048>,
    <https://w3id.org/permafrost/v/nrcglossary/t0049>, <https://w3id.org/permafrost/v/nrcglossary/t0050>,
    <https://w3id.org/permafrost/v/nrcglossary/t0051>, <https://w3id.org/permafrost/v/nrcglossary/t0052>,
    <https://w3id.org/permafrost/v/nrcglossary/t0053>, <https://w3id.org/permafrost/v/nrcglossary/t0054>,
    <https://w3id.org/permafrost/v/nrcglossary/t0055>, <https://w3id.org/permafrost/v/nrcglossary/t0056>,
    <https://w3id.org/permafrost/v/nrcglossary/t0057>, <https://w3id.org/permafrost/v/nrcglossary/t0058>,
    <https://w3id.org/permafrost/v/nrcglossary/t0059>, <https://w3id.org/permafrost/v/nrcglossary/t0060>,
    <https://w3id.org/permafrost/v/nrcglossary/t0061>, <https://w3id.org/permafrost/v/nrcglossary/t0062>,
    <https://w3id.org/permafrost/v/nrcglossary/t0063>, <https://w3id.org/permafrost/v/nrcglossary/t0064>,
    <https://w3id.org/permafrost/v/nrcglossary/t0065>, <https://w3id.org/permafrost/v/nrcglossary/t0066>,
    <https://w3id.org/permafrost/v/nrcglossary/t0067>, <https://w3id.org/permafrost/v/nrcglossary/t0068>,
    <https://w3id.org/permafrost/v/nrcglossary/t0069>, <https://w3id.org/permafrost/v/nrcglossary/t0070>,
    <https://w3id.org/permafrost/v/nrcglossary/t0071>, <https://w3id.org/permafrost/v/nrcglossary/t0072>,
    <https://w3id.org/permafrost/v/nrcglossary/t0073>, <https://w3id.org/permafrost/v/nrcglossary/t0074>,
    <https://w3id.org/permafrost/v/nrcglossary/t0075>, <https://w3id.org/permafrost/v/nrcglossary/t0076>,
    <https://w3id.org/permafrost/v/nrcglossary/t0077>, <https://w3id.org/permafrost/v/nrcglossary/t0078>,
    <https://w3id.org/permafrost/v/nrcglossary/t0079>, <https://w3id.org/permafrost/v/nrcglossary/t0080>,
    <https://w3id.org/permafrost/v/nrcglossary/t0081>, <https://w3id.org/permafrost/v/nrcglossary/t0082>,
    <https://w3id.org/permafrost/v/nrcglossary/t0083>, <https://w3id.org/permafrost/v/nrcglossary/t0084>,
    <https://w3id.org/permafrost/v/nrcglossary/t0085>, <https://w3id.org/permafrost/v/nrcglossary/t0086>,
    <https://w3id.org/permafrost/v/nrcglossary/t0087>, <https://w3id.org/permafrost/v/nrcglossary/t0088>,
    <https://w3id.org/permafrost/v/nrcglossary/t0089>, <https://w3id.org/permafrost/v/nrcglossary/t0090>,
    <https://w3id.org/permafrost/v/nrcglossary/t0091>, <https://w3id.org/permafrost/v/nrcglossary/t0092>,
    <https://w3id.org/permafrost/v/nrcglossary/t0093>, <https://w3id.org/permafrost/v/nrcglossary/t0094>,
    <https://w3id.org/permafrost/v/nrcglossary/t0095>, <https://w3id.org/permafrost/v/nrcglossary/t0096>,
    <https://w3id.org/permafrost/v/nrcglossary/t0097>, <https://w3id.org/permafrost/v/nrcglossary/t0098>,
    <https://w3id.org/permafrost/v/nrcglossary/t0099>, <https://w3id.org/permafrost/v/nrcglossary/t0100>,
    <https://w3id.org/permafrost/v/nrcglossary/t0101>, <https://w3id.org/permafrost/v/nrcglossary/t0102>,
    <https://w3id.org/permafrost/v/nrcglossary/t0103>, <https://w3id.org/permafrost/v/nrcglossary/t0104>,
    <https://w3id.org/permafrost/v/nrcglossary/t0105>, <https://w3id.org/permafrost/v/nrcglossary/t0106>,
    <https://w3id.org/permafrost/v/nrcglossary/t0107>, <https://w3id.org/permafrost/v/nrcglossary/t0108>,
    <https://w3id.org/permafrost/v/nrcglossary/t0109>, <https://w3id.org/permafrost/v/nrcglossary/t0110>,
    <https://w3id.org/permafrost/v/nrcglossary/t0111>, <https://w3id.org/permafrost/v/nrcglossary/t0112>,
    <https://w3id.org/permafrost/v/nrcglossary/t0113>, <https://w3id.org/permafrost/v/nrcglossary/t0114>,
    <https://w3id.org/permafrost/v/nrcglossary/t0115>, <https://w3id.org/permafrost/v/nrcglossary/t0116>,
    <https://w3id.org/permafrost/v/nrcglossary/t0117>, <https://w3id.org/permafrost/v/nrcglossary/t0118>,
    <https://w3id.org/permafrost/v/nrcglossary/t0119>, <https://w3id.org/permafrost/v/nrcglossary/t0120>,
    <https://w3id.org/permafrost/v/nrcglossary/t0121>, <https://w3id.org/permafrost/v/nrcglossary/t0122>,
    <https://w3id.org/permafrost/v/nrcglossary/t0123>, <https://w3id.org/permafrost/v/nrcglossary/t0124>,
    <https://w3id.org/permafrost/v/nrcglossary/t0125>, <https://w3id.org/permafrost/v/nrcglossary/t0126>,
    <https://w3id.org/permafrost/v/nrcglossary/t0127>, <https://w3id.org/permafrost/v/nrcglossary/t0128>,
    <https://w3id.org/permafrost/v/nrcglossary/t0129>, <https://w3id.org/permafrost/v/nrcglossary/t0130>,
    <https://w3id.org/permafrost/v/nrcglossary/t0131>, <https://w3id.org/permafrost/v/nrcglossary/t0132>,
    <https://w3id.org/permafrost/v/nrcglossary/t0133>, <https://w3id.org/permafrost/v/nrcglossary/t0134>,
    <https://w3id.org/permafrost/v/nrcglossary/t0135>, <https://w3id.org/permafrost/v/nrcglossary/t0136>,
    <https://w3id.org/permafrost/v/nrcglossary/t0137>, <https://w3id.org/permafrost/v/nrcglossary/t0138>,
    <https://w3id.org/permafrost/v/nrcglossary/t0139>, <https://w3id.org/permafrost/v/nrcglossary/t0140>,
    <https://w3id.org/permafrost/v/nrcglossary/t0141>, <https://w3id.org/permafrost/v/nrcglossary/t0142>,
    <https://w3id.org/permafrost/v/nrcglossary/t0143>, <https://w3id.org/permafrost/v/nrcglossary/t0144>,
    <https://w3id.org/permafrost/v/nrcglossary/t0145>, <https://w3id.org/permafrost/v/nrcglossary/t0146>,
    <https://w3id.org/permafrost/v/nrcglossary/t0147>, <https://w3id.org/permafrost/v/nrcglossary/t0148>,
    <https://w3id.org/permafrost/v/nrcglossary/t0149>, <https://w3id.org/permafrost/v/nrcglossary/t0150>,
    <https://w3id.org/permafrost/v/nrcglossary/t0151>, <https://w3id.org/permafrost/v/nrcglossary/t0152>,
    <https://w3id.org/permafrost/v/nrcglossary/t0153>, <https://w3id.org/permafrost/v/nrcglossary/t0154>,
    <https://w3id.org/permafrost/v/nrcglossary/t0155>, <https://w3id.org/permafrost/v/nrcglossary/t0156>,
    <https://w3id.org/permafrost/v/nrcglossary/t0157>, <https://w3id.org/permafrost/v/nrcglossary/t0158>,
    <https://w3id.org/permafrost/v/nrcglossary/t0159>, <https://w3id.org/permafrost/v/nrcglossary/t0160>,
    <https://w3id.org/permafrost/v/nrcglossary/t0161>, <https://w3id.org/permafrost/v/nrcglossary/t0162>,
    <https://w3id.org/permafrost/v/nrcglossary/t0163>, <https://w3id.org/permafrost/v/nrcglossary/t0164>,
    <https://w3id.org/permafrost/v/nrcglossary/t0165>, <https://w3id.org/permafrost/v/nrcglossary/t0166>,
    <https://w3id.org/permafrost/v/nrcglossary/t0167>, <https://w3id.org/permafrost/v/nrcglossary/t0168>,
    <https://w3id.org/permafrost/v/nrcglossary/t0169>, <https://w3id.org/permafrost/v/nrcglossary/t0170>,
    <https://w3id.org/permafrost/v/nrcglossary/t0171>, <https://w3id.org/permafrost/v/nrcglossary/t0172>,
    <https://w3id.org/permafrost/v/nrcglossary/t0173>, <https://w3id.org/permafrost/v/nrcglossary/t0174>,
    <https://w3id.org/permafrost/v/nrcglossary/t0175>, <https://w3id.org/permafrost/v/nrcglossary/t0176>,
    <https://w3id.org/permafrost/v/nrcglossary/t0177>, <https://w3id.org/permafrost/v/nrcglossary/t0178>,
    <https://w3id.org/permafrost/v/nrcglossary/t0179>, <https://w3id.org/permafrost/v/nrcglossary/t0180>,
    <https://w3id.org/permafrost/v/nrcglossary/t0181>, <https://w3id.org/permafrost/v/nrcglossary/t0182>,
    <https://w3id.org/permafrost/v/nrcglossary/t0183>, <https://w3id.org/permafrost/v/nrcglossary/t0184>,
    <https://w3id.org/permafrost/v/nrcglossary/t0185>, <https://w3id.org/permafrost/v/nrcglossary/t0186>,
    <https://w3id.org/permafrost/v/nrcglossary/t0187>, <https://w3id.org/permafrost/v/nrcglossary/t0188>,
    <https://w3id.org/permafrost/v/nrcglossary/t0189>, <https://w3id.org/permafrost/v/nrcglossary/t0190>,
    <https://w3id.org/permafrost/v/nrcglossary/t0191>, <https://w3id.org/permafrost/v/nrcglossary/t0192>,
    <https://w3id.org/permafrost/v/nrcglossary/t0193>, <https://w3id.org/permafrost/v/nrcglossary/t0194>,
    <https://w3id.org/permafrost/v/nrcglossary/t0195>, <https://w3id.org/permafrost/v/nrcglossary/t0196>,
    <https://w3id.org/permafrost/v/nrcglossary/t0197>, <https://w3id.org/permafrost/v/nrcglossary/t0198>,
    <https://w3id.org/permafrost/v/nrcglossary/t0199>, <https://w3id.org/permafrost/v/nrcglossary/t0200>,
    <https://w3id.org/permafrost/v/nrcglossary/t0201>, <https://w3id.org/permafrost/v/nrcglossary/t0202>,
    <https://w3id.org/permafrost/v/nrcglossary/t0203>, <https://w3id.org/permafrost/v/nrcglossary/t0204>,
    <https://w3id.org/permafrost/v/nrcglossary/t0205>, <https://w3id.org/permafrost/v/nrcglossary/t0206>,
    <https://w3id.org/permafrost/v/nrcglossary/t0207>, <https://w3id.org/permafrost/v/nrcglossary/t0208>,
    <https://w3id.org/permafrost/v/nrcglossary/t0209>, <https://w3id.org/permafrost/v/nrcglossary/t0210>,
    <https://w3id.org/permafrost/v/nrcglossary/t0211>, <https://w3id.org/permafrost/v/nrcglossary/t0212>,
    <https://w3id.org/permafrost/v/nrcglossary/t0213>, <https://w3id.org/permafrost/v/nrcglossary/t0214>,
    <https://w3id.org/permafrost/v/nrcglossary/t0215>, <https://w3id.org/permafrost/v/nrcglossary/t0216>,
    <https://w3id.org/permafrost/v/nrcglossary/t0217>, <https://w3id.org/permafrost/v/nrcglossary/t0218>,
    <https://w3id.org/permafrost/v/nrcglossary/t0219>, <https://w3id.org/permafrost/v/nrcglossary/t0220>,
    <https://w3id.org/permafrost/v/nrcglossary/t0221>, <https://w3id.org/permafrost/v/nrcglossary/t0222>,
    <https://w3id.org/permafrost/v/nrcglossary/t0223>, <https://w3id.org/permafrost/v/nrcglossary/t0224>,
    <https://w3id.org/permafrost/v/nrcglossary/t0225>, <https://w3id.org/permafrost/v/nrcglossary/t0226>,
    <https://w3id.org/permafrost/v/nrcglossary/t0227>, <https://w3id.org/permafrost/v/nrcglossary/t0228>,
    <https://w3id.org/permafrost/v/nrcglossary/t0229>, <https://w3id.org/permafrost/v/nrcglossary/t0230>,
    <https://w3id.org/permafrost/v/nrcglossary/t0231>, <https://w3id.org/permafrost/v/nrcglossary/t0232>,
    <https://w3id.org/permafrost/v/nrcglossary/t0233>, <https://w3id.org/permafrost/v/nrcglossary/t0234>,
    <https://w3id.org/permafrost/v/nrcglossary/t0235>, <https://w3id.org/permafrost/v/nrcglossary/t0236>,
    <https://w3id.org/permafrost/v/nrcglossary/t0237>, <https://w3id.org/permafrost/v/nrcglossary/t0238>,
    <https://w3id.org/permafrost/v/nrcglossary/t0239>, <https://w3id.org/permafrost/v/nrcglossary/t0240>,
    <https://w3id.org/permafrost/v/nrcglossary/t0241>, <https://w3id.org/permafrost/v/nrcglossary/t0242>,
    <https://w3id.org/permafrost/v/nrcglossary/t0243>, <https://w3id.org/permafrost/v/nrcglossary/t0244>,
    <https://w3id.org/permafrost/v/nrcglossary/t0245>, <https://w3id.org/permafrost/v/nrcglossary/t0246>,
    <https://w3id.org/permafrost/v/nrcglossary/t0247>, <https://w3id.org/permafrost/v/nrcglossary/t0248>,
    <https://w3id.org/permafrost/v/nrcglossary/t0249>, <https://w3id.org/permafrost/v/nrcglossary/t0250>,
    <https://w3id.org/permafrost/v/nrcglossary/t0251>, <https://w3id.org/permafrost/v/nrcglossary/t0252>,
    <https://w3id.org/permafrost/v/nrcglossary/t0253>, <https://w3id.org/permafrost/v/nrcglossary/t0254>,
    <https://w3id.org/permafrost/v/nrcglossary/t0255>, <https://w3id.org/permafrost/v/nrcglossary/t0256>,
    <https://w3id.org/permafrost/v/nrcglossary/t0257>, <https://w3id.org/permafrost/v/nrcglossary/t0258>,
    <https://w3id.org/permafrost/v/nrcglossary/t0259>, <https://w3id.org/permafrost/v/nrcglossary/t0260>,
    <https://w3id.org/permafrost/v/nrcglossary/t0261>, <https://w3id.org/permafrost/v/nrcglossary/t0262>,
    <https://w3id.org/permafrost/v/nrcglossary/t0263>, <https://w3id.org/permafrost/v/nrcglossary/t0264>,
    <https://w3id.org/permafrost/v/nrcglossary/t0265>, <https://w3id.org/permafrost/v/nrcglossary/t0266>,
    <https://w3id.org/permafrost/v/nrcglossary/t0267>, <https://w3id.org/permafrost/v/nrcglossary/t0268>,
    <https://w3id.org/permafrost/v/nrcglossary/t0269>, <https://w3id.org/permafrost/v/nrcglossary/t0270>,
    <https://w3id.org/permafrost/v/nrcglossary/t0271>, <https://w3id.org/permafrost/v/nrcglossary/t0272>,
    <https://w3id.org/permafrost/v/nrcglossary/t0273>, <https://w3id.org/permafrost/v/nrcglossary/t0274>,
    <https://w3id.org/permafrost/v/nrcglossary/t0275>, <https://w3id.org/permafrost/v/nrcglossary/t0276>,
    <https://w3id.org/permafrost/v/nrcglossary/t0277>, <https://w3id.org/permafrost/v/nrcglossary/t0278>,
    <https://w3id.org/permafrost/v/nrcglossary/t0279>, <https://w3id.org/permafrost/v/nrcglossary/t0280>,
    <https://w3id.org/permafrost/v/nrcglossary/t0281>, <https://w3id.org/permafrost/v/nrcglossary/t0282>,
    <https://w3id.org/permafrost/v/nrcglossary/t0283>, <https://w3id.org/permafrost/v/nrcglossary/t0284>,
    <https://w3id.org/permafrost/v/nrcglossary/t0285>, <https://w3id.org/permafrost/v/nrcglossary/t0286>,
    <https://w3id.org/permafrost/v/nrcglossary/t0287>, <https://w3id.org/permafrost/v/nrcglossary/t0288>,
    <https://w3id.org/permafrost/v/nrcglossary/t0289>, <https://w3id.org/permafrost/v/nrcglossary/t0290>,
    <https://w3id.org/permafrost/v/nrcglossary/t0291>, <https://w3id.org/permafrost/v/nrcglossary/t0292>,
    <https://w3id.org/permafrost/v/nrcglossary/t0293>, <https://w3id.org/permafrost/v/nrcglossary/t0294>,
    <https://w3id.org/permafrost/v/nrcglossary/t0295>, <https://w3id.org/permafrost/v/nrcglossary/t0296>,
    <https://w3id.org/permafrost/v/nrcglossary/t0297>, <https://w3id.org/permafrost/v/nrcglossary/t0298>,
    <https://w3id.org/permafrost/v/nrcglossary/t0299>, <https://w3id.org/permafrost/v/nrcglossary/t0300>,
    <https://w3id.org/permafrost/v/nrcglossary/t0301>, <https://w3id.org/permafrost/v/nrcglossary/t0302>,
    <https://w3id.org/permafrost/v/nrcglossary/t0303>, <https://w3id.org/permafrost/v/nrcglossary/t0304>,
    <https://w3id.org/permafrost/v/nrcglossary/t0305>, <https://w3id.org/permafrost/v/nrcglossary/t0306>,
    <https://w3id.org/permafrost/v/nrcglossary/t0307>, <https://w3id.org/permafrost/v/nrcglossary/t0308>,
    <https://w3id.org/permafrost/v/nrcglossary/t0309>, <https://w3id.org/permafrost/v/nrcglossary/t0310>,
    <https://w3id.org/permafrost/v/nrcglossary/t0311>, <https://w3id.org/permafrost/v/nrcglossary/t0312>,
    <https://w3id.org/permafrost/v/nrcglossary/t0313>, <https://w3id.org/permafrost/v/nrcglossary/t0314>,
    <https://w3id.org/permafrost/v/nrcglossary/t0315>, <https://w3id.org/permafrost/v/nrcglossary/t0316>,
    <https://w3id.org/permafrost/v/nrcglossary/t0317>, <https://w3id.org/permafrost/v/nrcglossary/t0318>,
    <https://w3id.org/permafrost/v/nrcglossary/t0319>, <https://w3id.org/permafrost/v/nrcglossary/t0320>,
    <https://w3id.org/permafrost/v/nrcglossary/t0321>, <https://w3id.org/permafrost/v/nrcglossary/t0322>,
    <https://w3id.org/permafrost/v/nrcglossary/t0323>, <https://w3id.org/permafrost/v/nrcglossary/t0324>,
    <https://w3id.org/permafrost/v/nrcglossary/t0325>, <https://w3id.org/permafrost/v/nrcglossary/t0326>,
    <https://w3id.org/permafrost/v/nrcglossary/t0327>, <https://w3id.org/permafrost/v/nrcglossary/t0328>,
    <https://w3id.org/permafrost/v/nrcglossary/t0329>, <https://w3id.org/permafrost/v/nrcglossary/t0330>,
    <https://w3id.org/permafrost/v/nrcglossary/t0331>, <https://w3id.org/permafrost/v/nrcglossary/t0332>,
    <https://w3id.org/permafrost/v/nrcglossary/t0333>, <https://w3id.org/permafrost/v/nrcglossary/t0334>,
    <https://w3id.org/permafrost/v/nrcglossary/t0335>, <https://w3id.org/permafrost/v/nrcglossary/t0336>,
    <https://w3id.org/permafrost/v/nrcglossary/t0337>, <https://w3id.org/permafrost/v/nrcglossary/t0338>,
    <https://w3id.org/permafrost/v/nrcglossary/t0339>, <https://w3id.org/permafrost/v/nrcglossary/t0340>,
    <https://w3id.org/permafrost/v/nrcglossary/t0341>, <https://w3id.org/permafrost/v/nrcglossary/t0342>,
    <https://w3id.org/permafrost/v/nrcglossary/t0343>, <https://w3id.org/permafrost/v/nrcglossary/t0344>,
    <https://w3id.org/permafrost/v/nrcglossary/t0345>, <https://w3id.org/permafrost/v/nrcglossary/t0346>,
    <https://w3id.org/permafrost/v/nrcglossary/t0347>, <https://w3id.org/permafrost/v/nrcglossary/t0348>,
    <https://w3id.org/permafrost/v/nrcglossary/t0349>, <https://w3id.org/permafrost/v/nrcglossary/t0350>,
    <https://w3id.org/permafrost/v/nrcglossary/t0351>, <https://w3id.org/permafrost/v/nrcglossary/t0352>,
    <https://w3id.org/permafrost/v/nrcglossary/t0353>, <https://w3id.org/permafrost/v/nrcglossary/t0354>,
    <https://w3id.org/permafrost/v/nrcglossary/t0355>, <https://w3id.org/permafrost/v/nrcglossary/t0356>,
    <https://w3id.org/permafrost/v/nrcglossary/t0357>, <https://w3id.org/permafrost/v/nrcglossary/t0358>,
    <https://w3id.org/permafrost/v/nrcglossary/t0359>, <https://w3id.org/permafrost/v/nrcglossary/t0360>,
    <https://w3id.org/permafrost/v/nrcglossary/t0361>, <https://w3id.org/permafrost/v/nrcglossary/t0362>,
    <https://w3id.org/permafrost/v/nrcglossary/t0363>, <https://w3id.org/permafrost/v/nrcglossary/t0364>,
    <https://w3id.org/permafrost/v/nrcglossary/t0365>, <https://w3id.org/permafrost/v/nrcglossary/t0366>,
    <https://w3id.org/permafrost/v/nrcglossary/t0367>, <https://w3id.org/permafrost/v/nrcglossary/t0368>,
    <https://w3id.org/permafrost/v/nrcglossary/t0369>, <https://w3id.org/permafrost/v/nrcglossary/t0370>,
    <https://w3id.org/permafrost/v/nrcglossary/t0371>, <https://w3id.org/permafrost/v/nrcglossary/t0372>,
    <https://w3id.org/permafrost/v/nrcglossary/t0373>, <https://w3id.org/permafrost/v/nrcglossary/t0374>,
    <https://w3id.org/permafrost/v/nrcglossary/t0375>, <https://w3id.org/permafrost/v/nrcglossary/t0376>,
    <https://w3id.org/permafrost/v/nrcglossary/t0377>, <https://w3id.org/permafrost/v/nrcglossary/t0378>,
    <https://w3id.org/permafrost/v/nrcglossary/t0379>, <https://w3id.org/permafrost/v/nrcglossary/t0380>,
    <https://w3id.org/permafrost/v/nrcglossary/t0381>, <https://w3id.org/permafrost/v/nrcglossary/t0382>,
    <https://w3id.org/permafrost/v/nrcglossary/t0383>, <https://w3id.org/permafrost/v/nrcglossary/t0384>,
    <https://w3id.org/permafrost/v/nrcglossary/t0385>, <https://w3id.org/permafrost/v/nrcglossary/t0386>,
    <https://w3id.org/permafrost/v/nrcglossary/t0387>, <https://w3id.org/permafrost/v/nrcglossary/t0388>,
    <https://w3id.org/permafrost/v/nrcglossary/t0389>, <https://w3id.org/permafrost/v/nrcglossary/t0390>,
    <https://w3id.org/permafrost/v/nrcglossary/t0391>, <https://w3id.org/permafrost/v/nrcglossary/t0392>,
    <https://w3id.org/permafrost/v/nrcglossary/t0393>, <https://w3id.org/permafrost/v/nrcglossary/t0394>,
    <https://w3id.org/permafrost/v/nrcglossary/t0395>, <https://w3id.org/permafrost/v/nrcglossary/t0396>,
    <https://w3id.org/permafrost/v/nrcglossary/t0397>;
  skos:prefLabel "NRC Permafrost Glossary" .

<https://w3id.org/permafrost/v/nrcglossary/t0001> a skos:Concept;
  dct:identifier "t0001"^^xsd:token;
  dct:source "https://nrc-publications.canada.ca/eng/view/object/?id=69fb8993-1baa-4225-b33a-6a02341d383d"^^xsd:anyURI,
    "https://nrc-publications.canada.ca/fra/voir/objet/?id=549123c3-092c-4fca-8dea-99d53eac06dd"^^xsd:anyURI;
  skos:definition "A foundation pile on which a cold air refrigeration system has been installed to remove heat from the ground."@en;
  skos:inScheme <https://w3id.org/permafrost/v/nrcglossary/scheme>;
  skos:prefLabel "active air-cooled thermal pile"@en;
  skos:scopeNote "The refrigeration system may be fastened to, or form part of the pile or, if the pile is a sealed unit (e.g. steel pipe), the pile itself may serve as both a heat-removal device and a structural unit."@en;
  skos:topConceptOf <https://w3id.org/permafrost/v/nrcglossary/scheme> .

<https://w3id.org/permafrost/v/nrcglossary/t0002> a skos:Concept;
  dct:identifier "t0002"^^xsd:token;
  dct:source "https://nrc-publications.canada.ca/eng/view/object/?id=69fb8993-1baa-4225-b33a-6a02341d383d"^^xsd:anyURI,
    "https://nrc-publications.canada.ca/fra/voir/objet/?id=549123c3-092c-4fca-8dea-99d53eac06dd"^^xsd:anyURI;
  skos:definition "Special design and construction methods used for engineering works in permafrost areas where permafrost degradation cannot be prevented."@en;
  skos:inScheme <https://w3id.org/permafrost/v/nrcglossary/scheme>;
  skos:prefLabel "active construction methods in permafrost"@en;
  skos:scopeNote "Two main approaches are possible. Unfavourable foundation materials can be thawed and compacted or replaced with more suitable materials before the structure is erected. Alternatively, the foundations and structure may be designed to accommodate any thaw settlement that will occur."@en;
  skos:topConceptOf <https://w3id.org/permafrost/v/nrcglossary/scheme> .

<https://w3id.org/permafrost/v/nrcglossary/t0003> a skos:Concept;
  dct:identifier "t0003"^^xsd:token;
  dct:source "https://nrc-publications.canada.ca/eng/view/object/?id=69fb8993-1baa-4225-b33a-6a02341d383d"^^xsd:anyURI,
    "https://nrc-publications.canada.ca/fra/voir/objet/?id=549123c3-092c-4fca-8dea-99d53eac06dd"^^xsd:anyURI;
  skos:definition "An ice wedge that is growing as a result of repeated (but not necessarily annual) winter cracking."@en;
  skos:inScheme <https://w3id.org/permafrost/v/nrcglossary/scheme>;
  skos:prefLabel "active ice wedge"@en;
  skos:scopeNote "Active ice wedges developed in mineral soil occur primarily in areas of continuous permafrost."@en;
  skos:topConceptOf <https://w3id.org/permafrost/v/nrcglossary/scheme> .

<https://w3id.org/permafrost/v/nrcglossary/t0004> a skos:Concept;
  dct:identifier "t0004"^^xsd:token;
  dct:source "https://nrc-publications.canada.ca/eng/view/object/?id=69fb8993-1baa-4225-b33a-6a02341d383d"^^xsd:anyURI,
    "https://nrc-publications.canada.ca/fra/voir/objet/?id=549123c3-092c-4fca-8dea-99d53eac06dd"^^xsd:anyURI;
  skos:definition "The layer of ground that is subject to annual thawing and freezing in areas underlain by permafrost (see Figure 2)."@en;
  skos:inScheme <https://w3id.org/permafrost/v/nrcglossary/scheme>;
  skos:prefLabel "active layer"@en, "mollisol"@fr;
  skos:topConceptOf <https://w3id.org/permafrost/v/nrcglossary/scheme> .

<https://w3id.org/permafrost/v/nrcglossary/t0005> a skos:Concept;
  dct:identifier "t0005"^^xsd:token;
  dct:source "https://nrc-publications.canada.ca/eng/view/object/?id=69fb8993-1baa-4225-b33a-6a02341d383d"^^xsd:anyURI,
    "https://nrc-publications.canada.ca/fra/voir/objet/?id=549123c3-092c-4fca-8dea-99d53eac06dd"^^xsd:anyURI;
  skos:altLabel "skin flow"@en;
  skos:definition "A general term referring to several forms of slope failures or failure mechanisms commonly occurring in the active layer overlying permafrost (see Figure 21a)."@en;
  skos:inScheme <https://w3id.org/permafrost/v/nrcglossary/scheme>;
  skos:prefLabel "active-layer failure"@en;
  skos:scopeNote "These include detachment failures but not retrogressive thaw slumps and thaw slumping since these involve permafrost."@en;
  skos:topConceptOf <https://w3id.org/permafrost/v/nrcglossary/scheme> .

<https://w3id.org/permafrost/v/nrcglossary/t0006> a skos:Concept;
  dct:identifier "t0006"^^xsd:token;
  dct:source "https://nrc-publications.canada.ca/eng/view/object/?id=69fb8993-1baa-4225-b33a-6a02341d383d"^^xsd:anyURI,
    "https://nrc-publications.canada.ca/fra/voir/objet/?id=549123c3-092c-4fca-8dea-99d53eac06dd"^^xsd:anyURI;
  skos:definition "The thickness of the layer of the ground that is subject to annual thawing and freeing in areas underlain by permafrost."@en;
  skos:inScheme <https://w3id.org/permafrost/v/nrcglossary/scheme>;
  skos:prefLabel "active-layer thickness"@en;
  skos:scopeNote "The thickness of the active layer depends on such factors as the ambient air temperature, vegetation, drainage, soil or rock type and total water content, snowcover, and degree and orientation of slope. As a rule, the active layer is thin in the High Arctic (it can be less than 15 cm) and becomes thicker farther south (1 m or more). The thickness of the active layer can vary from year to year, primarily due to variations in the mean annual air temperature, distribution of soil moisture, and snowcover. The thickness of the active layer includes the uppermost part of the permafrost wherever either the salinity or clay content of the permafrost allows it to thaw and refreeze annually, even though the material remains cryotic (T < 0°C). Use of the term \"depth to permafrost\" as a synonym for the thickness of the active layer is misleading, especially in areas where the active layer is separated from the permafrost by a residual thaw layer, that is, by a thawed or noncryotic (T> 0°C) layer of ground."@en;
  skos:topConceptOf <https://w3id.org/permafrost/v/nrcglossary/scheme> .

<https://w3id.org/permafrost/v/nrcglossary/t0007> a skos:Concept;
  dct:identifier "t0007"^^xsd:token;
  dct:source "https://nrc-publications.canada.ca/eng/view/object/?id=69fb8993-1baa-4225-b33a-6a02341d383d"^^xsd:anyURI,
    "https://nrc-publications.canada.ca/fra/voir/objet/?id=549123c3-092c-4fca-8dea-99d53eac06dd"^^xsd:anyURI;
  skos:definition "A foundation pile on which a liquid coolant refrigeration system has been installed to remove heat from the ground."@en;
  skos:inScheme <https://w3id.org/permafrost/v/nrcglossary/scheme>;
  skos:prefLabel "active liquid refrigerant pile"@en;
  skos:scopeNote "The refrigeration system may be fastened to, or form part of the pile or, if the pile is a sealed unit (e.g. steel pipe), the pile itself may serve as both a heat-removal device and a structural unit."@en;
  skos:topConceptOf <https://w3id.org/permafrost/v/nrcglossary/scheme> .

<https://w3id.org/permafrost/v/nrcglossary/t0008> a skos:Concept;
  dct:identifier "t0008"^^xsd:token;
  dct:source "https://nrc-publications.canada.ca/eng/view/object/?id=69fb8993-1baa-4225-b33a-6a02341d383d"^^xsd:anyURI,
    "https://nrc-publications.canada.ca/fra/voir/objet/?id=549123c3-092c-4fca-8dea-99d53eac06dd"^^xsd:anyURI;
  skos:definition "A mass of rock fragments and finer material, on a slope, that contains either an ice core or interstitial ice, and shows evidence of present movement."@en;
  skos:inScheme <https://w3id.org/permafrost/v/nrcglossary/scheme>;
  skos:prefLabel "active rock glacier"@en;
  skos:scopeNote "Active rock glaciers possess steep fronts with slope angles that may exceed the angle of repose. Gradual elimination of such oversteepening of the frontal portion may suggest some movement long after the ice has melted and the main body of the rock glacier has stopped moving."@en;
  skos:topConceptOf <https://w3id.org/permafrost/v/nrcglossary/scheme> .

<https://w3id.org/permafrost/v/nrcglossary/t0009> a skos:Concept;
  dct:identifier "t0009"^^xsd:token;
  dct:source "https://nrc-publications.canada.ca/eng/view/object/?id=69fb8993-1baa-4225-b33a-6a02341d383d"^^xsd:anyURI,
    "https://nrc-publications.canada.ca/fra/voir/objet/?id=549123c3-092c-4fca-8dea-99d53eac06dd"^^xsd:anyURI;
  skos:definition "The process by which characteristic landforms are currently developing as a result of thawing of ice-rich permafrost or melting of massive ice."@en;
  skos:inScheme <https://w3id.org/permafrost/v/nrcglossary/scheme>;
  skos:prefLabel "active thermokarst"@en;
  skos:scopeNote "The occurrence of active thermokarst indicates the presence of disequilibrium permafrost."@en;
  skos:topConceptOf <https://w3id.org/permafrost/v/nrcglossary/scheme> .

<https://w3id.org/permafrost/v/nrcglossary/t0010> a skos:Concept;
  dct:identifier "t0010"^^xsd:token;
  dct:source "https://nrc-publications.canada.ca/eng/view/object/?id=69fb8993-1baa-4225-b33a-6a02341d383d"^^xsd:anyURI,
    "https://nrc-publications.canada.ca/fra/voir/objet/?id=549123c3-092c-4fca-8dea-99d53eac06dd"^^xsd:anyURI;
  skos:altLabel "frost grip"@en;
  skos:definition "The process by which two objects are bonded together by ice formed between them."@en;
  skos:inScheme <https://w3id.org/permafrost/v/nrcglossary/scheme>;
  skos:prefLabel "adfreeze/adfreezing"@en, "congélation adhérente"@fr;
  skos:scopeNote "Adfreezing is the process that anchors piles or buried foundations in permafrost, so that they can be unaffected by frost heave occurring in the active layer."@en;
  skos:topConceptOf <https://w3id.org/permafrost/v/nrcglossary/scheme> .

<https://w3id.org/permafrost/v/nrcglossary/t0011> a skos:Concept;
  dct:identifier "t0011"^^xsd:token;
  dct:source "https://nrc-publications.canada.ca/eng/view/object/?id=69fb8993-1baa-4225-b33a-6a02341d383d"^^xsd:anyURI,
    "https://nrc-publications.canada.ca/fra/voir/objet/?id=549123c3-092c-4fca-8dea-99d53eac06dd"^^xsd:anyURI;
  skos:definition "The tensile or shear strength which has to be overcome to separate two objects that are bonded together by ice."@en;
  skos:inScheme <https://w3id.org/permafrost/v/nrcglossary/scheme>;
  skos:prefLabel "adfreeze strength"@en;
  skos:scopeNote "The term is usually used to describe the resistance to the force that is required to separate frozen ground or an ice mass from an object (frequently a foundation unit) to which it is frozen. The shear stress required to separate an object from frozen ground is frequently referred to as the \"tangential adfreeze strength\"."@en;
  skos:topConceptOf <https://w3id.org/permafrost/v/nrcglossary/scheme> .

<https://w3id.org/permafrost/v/nrcglossary/t0012> a skos:Concept;
  dct:identifier "t0012"^^xsd:token;
  dct:source "https://nrc-publications.canada.ca/eng/view/object/?id=69fb8993-1baa-4225-b33a-6a02341d383d"^^xsd:anyURI,
    "https://nrc-publications.canada.ca/fra/voir/objet/?id=549123c3-092c-4fca-8dea-99d53eac06dd"^^xsd:anyURI;
  skos:definition "The additional ground ice formed as a direct result of permafrost aggradation (see Figure 10a)."@en;
  skos:inScheme <https://w3id.org/permafrost/v/nrcglossary/scheme>;
  skos:prefLabel "aggradational ice"@en;
  skos:scopeNote "Ice lenses form seasonally, especially in the lower part of the active layer, and can be incorporated into the permafrost if they do not melt over a period of years."@en;
  skos:topConceptOf <https://w3id.org/permafrost/v/nrcglossary/scheme> .

<https://w3id.org/permafrost/v/nrcglossary/t0013> a skos:Concept;
  dct:identifier "t0013"^^xsd:token;
  dct:source "https://nrc-publications.canada.ca/eng/view/object/?id=69fb8993-1baa-4225-b33a-6a02341d383d"^^xsd:anyURI,
    "https://nrc-publications.canada.ca/fra/voir/objet/?id=549123c3-092c-4fca-8dea-99d53eac06dd"^^xsd:anyURI;
  skos:definition "The cumulative number of degree-days below 0°C for the air temperature during a given time period."@en;
  skos:inScheme <https://w3id.org/permafrost/v/nrcglossary/scheme>;
  skos:prefLabel "air freezing index"@en;
  skos:scopeNote "The air freezing index differs from the corresponding surface freezing index. (see n-factor)."@en;
  skos:topConceptOf <https://w3id.org/permafrost/v/nrcglossary/scheme> .

<https://w3id.org/permafrost/v/nrcglossary/t0014> a skos:Concept;
  dct:identifier "t0014"^^xsd:token;
  dct:source "https://nrc-publications.canada.ca/eng/view/object/?id=69fb8993-1baa-4225-b33a-6a02341d383d"^^xsd:anyURI,
    "https://nrc-publications.canada.ca/fra/voir/objet/?id=549123c3-092c-4fca-8dea-99d53eac06dd"^^xsd:anyURI;
  skos:definition "The cumulative number of degree-days above 0°C for the air temperature during a given period."@en;
  skos:inScheme <https://w3id.org/permafrost/v/nrcglossary/scheme>;
  skos:prefLabel "air thawing index"@en;
  skos:scopeNote "The air thawing index differs from the corresponding surface thawing index. (see n-factor)."@en;
  skos:topConceptOf <https://w3id.org/permafrost/v/nrcglossary/scheme> .

<https://w3id.org/permafrost/v/nrcglossary/t0015> a skos:Concept;
  dct:identifier "t0015"^^xsd:token;
  dct:source "https://nrc-publications.canada.ca/eng/view/object/?id=69fb8993-1baa-4225-b33a-6a02341d383d"^^xsd:anyURI,
    "https://nrc-publications.canada.ca/fra/voir/objet/?id=549123c3-092c-4fca-8dea-99d53eac06dd"^^xsd:anyURI;
  skos:definition "A large depression of the ground surface produced by thawing of a large area of very thick and exceedingly ice-rich permafrost."@en;
  skos:inScheme <https://w3id.org/permafrost/v/nrcglossary/scheme>;
  skos:prefLabel "alas/alass"@en;
  skos:scopeNote "Typically, alasses are large depressions ranging from 0.5 to more than 100 km2 in area and from 5 to 20 m in depth. In the early stages of formation, a shallow (? 2 m) circular \"alas lake\" forms in a steep-sided depression. Enlargement and ultimate drainage of a number of such lakes may leave low interalas plateaus (termed \"mezhalasye\" in Russian). Ultimately, the plateaus disappear and mass wasting produces gentle side slopes. The term is of Yakut origin. The term is of Yakut origin. An analogous term of Nenets (northwestern Siberia) origin is \"khasyrey\"."@en;
  skos:topConceptOf <https://w3id.org/permafrost/v/nrcglossary/scheme> .

<https://w3id.org/permafrost/v/nrcglossary/t0016> a skos:Concept;
  dct:identifier "t0016"^^xsd:token;
  dct:source "https://nrc-publications.canada.ca/eng/view/object/?id=69fb8993-1baa-4225-b33a-6a02341d383d"^^xsd:anyURI,
    "https://nrc-publications.canada.ca/fra/voir/objet/?id=549123c3-092c-4fca-8dea-99d53eac06dd"^^xsd:anyURI;
  skos:definition "Albedo is a measure of the reflecting power of a surface, expressed as the fraction of the incoming solar radiation reflected by the surface."@en;
  skos:inScheme <https://w3id.org/permafrost/v/nrcglossary/scheme>;
  skos:prefLabel "albedo"@en;
  skos:scopeNote "The albedo of natural land surfaces varies over a wide range, and it changes with the seasons, primarily due to changes in vegetation and snowcover."@en;
  skos:topConceptOf <https://w3id.org/permafrost/v/nrcglossary/scheme> .

<https://w3id.org/permafrost/v/nrcglossary/t0017> a skos:Concept;
  dct:identifier "t0017"^^xsd:token;
  dct:source "https://nrc-publications.canada.ca/eng/view/object/?id=69fb8993-1baa-4225-b33a-6a02341d383d"^^xsd:anyURI,
    "https://nrc-publications.canada.ca/fra/voir/objet/?id=549123c3-092c-4fca-8dea-99d53eac06dd"^^xsd:anyURI;
  skos:definition "The lowest altitude at which mountain permafrost occurs in a given highland area outside the general permafrost region."@en;
  skos:inScheme <https://w3id.org/permafrost/v/nrcglossary/scheme>;
  skos:prefLabel "altitudinal limit of permafrost"@en;
  skos:scopeNote "The altitudinal limit of mountain permafrost generally rises progressively with decreasing latitude."@en;
  skos:topConceptOf <https://w3id.org/permafrost/v/nrcglossary/scheme> .

<https://w3id.org/permafrost/v/nrcglossary/t0018> a skos:Concept;
  dct:identifier "t0018"^^xsd:token;
  dct:source "https://nrc-publications.canada.ca/eng/view/object/?id=69fb8993-1baa-4225-b33a-6a02341d383d"^^xsd:anyURI,
    "https://nrc-publications.canada.ca/fra/voir/objet/?id=549123c3-092c-4fca-8dea-99d53eac06dd"^^xsd:anyURI;
  skos:definition "The vertical subdivision of an area of mountain permafrost into permafrost zones, based on the proportion of the ground that is perennially cryotic."@en;
  skos:inScheme <https://w3id.org/permafrost/v/nrcglossary/scheme>;
  skos:prefLabel "altitudinal zonation of permafrost"@en;
  skos:scopeNote "As mean annual temperatures decrease with increasing elevation, mountain permafrost can normally be expected to be more extensive, thicker and colder at higher elevations, although exposure and the extent of vegetation and snow cover will moderate this effect. A noteable exception is found in the southwestern portion of Yukon, where (1) the high St. Elias Mountains block the circulation of moist and warm maritime air from the Pacific Ocean, particularly in winter, and (2) the deeply dissected nature of the terrain promotes cold-air drainage and ponding in the valleys. As a result, permafrost is more extensive, thicker and colder in valley bottoms than at higher elevations."@en;
  skos:topConceptOf <https://w3id.org/permafrost/v/nrcglossary/scheme> .

<https://w3id.org/permafrost/v/nrcglossary/t0019> a skos:Concept;
  dct:identifier "t0019"^^xsd:token;
  dct:source "https://nrc-publications.canada.ca/eng/view/object/?id=69fb8993-1baa-4225-b33a-6a02341d383d"^^xsd:anyURI,
    "https://nrc-publications.canada.ca/fra/voir/objet/?id=549123c3-092c-4fca-8dea-99d53eac06dd"^^xsd:anyURI;
  skos:definition "An ice wedge that grows progressively downwards into a receding slope, in a direction normal to the surface (see Figure 17i)."@en;
  skos:inScheme <https://w3id.org/permafrost/v/nrcglossary/scheme>;
  skos:prefLabel "anti-syngenetic ice wedge"@en;
  skos:scopeNote "The younger portions of the wedge extend farthest down. The downward rate of growth is a function of the rate of slope recession and the rate of formation of new ice veinlets."@en;
  skos:topConceptOf <https://w3id.org/permafrost/v/nrcglossary/scheme> .

<https://w3id.org/permafrost/v/nrcglossary/t0020> a skos:Concept;
  dct:identifier "t0020"^^xsd:token;
  dct:source "https://nrc-publications.canada.ca/eng/view/object/?id=69fb8993-1baa-4225-b33a-6a02341d383d"^^xsd:anyURI,
    "https://nrc-publications.canada.ca/fra/voir/objet/?id=549123c3-092c-4fca-8dea-99d53eac06dd"^^xsd:anyURI;
  skos:definition "The amount of heat required to raise the temperature of a unit mass of frozen ground by one degree."@en;
  skos:inScheme <https://w3id.org/permafrost/v/nrcglossary/scheme>;
  skos:prefLabel "apparent heat capacity"@en;
  skos:scopeNote "Because the phase change in frozen ground often occurs gradually over a range of temperatures, the apparent heat capacity (which is the sum of the specific heat capacity and the latent heat released) may vary significantly with temperature. Apparent heat capacity is commonly expressed in Joules per kg per degree K."@en;
  skos:topConceptOf <https://w3id.org/permafrost/v/nrcglossary/scheme> .

<https://w3id.org/permafrost/v/nrcglossary/t0021> a skos:Concept;
  dct:identifier "t0021"^^xsd:token;
  dct:source "https://nrc-publications.canada.ca/eng/view/object/?id=69fb8993-1baa-4225-b33a-6a02341d383d"^^xsd:anyURI,
    "https://nrc-publications.canada.ca/fra/voir/objet/?id=549123c3-092c-4fca-8dea-99d53eac06dd"^^xsd:anyURI;
  skos:definition "The cumulative number of degree-days below 0°C for a given time period, calculated from the mean monthly temperatures for a specific station without making corrections for positive degree-days in spring and fall."@en;
  skos:inScheme <https://w3id.org/permafrost/v/nrcglossary/scheme>;
  skos:prefLabel "approximate freezing index"@en;
  skos:topConceptOf <https://w3id.org/permafrost/v/nrcglossary/scheme> .

<https://w3id.org/permafrost/v/nrcglossary/t0022> a skos:Concept;
  dct:identifier "t0022"^^xsd:token;
  dct:source "https://nrc-publications.canada.ca/eng/view/object/?id=69fb8993-1baa-4225-b33a-6a02341d383d"^^xsd:anyURI,
    "https://nrc-publications.canada.ca/fra/voir/objet/?id=549123c3-092c-4fca-8dea-99d53eac06dd"^^xsd:anyURI;
  skos:definition "The cumulative number of degree-days above 0°C for a given time period, calculated from the mean monthly temperatures for a specific station without making corrections for negative degree-days in spring and fall."@en;
  skos:inScheme <https://w3id.org/permafrost/v/nrcglossary/scheme>;
  skos:prefLabel "approximate thawing index"@en;
  skos:topConceptOf <https://w3id.org/permafrost/v/nrcglossary/scheme> .

<https://w3id.org/permafrost/v/nrcglossary/t0023> a skos:Concept;
  dct:identifier "t0023"^^xsd:token;
  dct:source "https://nrc-publications.canada.ca/eng/view/object/?id=69fb8993-1baa-4225-b33a-6a02341d383d"^^xsd:anyURI,
    "https://nrc-publications.canada.ca/fra/voir/objet/?id=549123c3-092c-4fca-8dea-99d53eac06dd"^^xsd:anyURI;
  skos:definition "The process of inducing or maintaining a frozen condition in earth materials by artificial means."@en;
  skos:inScheme <https://w3id.org/permafrost/v/nrcglossary/scheme>;
  skos:prefLabel "artificial ground freezing"@en;
  skos:scopeNote "The frozen condition can be induced or maintained by natural convection movement of air, gases or liquids (e.g., through or in ventilation ducts, thermal piles, thermosyphons), or by forced (mechanical) circulation of cold air or a refrigerant through a system of ducts or freeze pipes in the ground."@en;
  skos:topConceptOf <https://w3id.org/permafrost/v/nrcglossary/scheme> .

<https://w3id.org/permafrost/v/nrcglossary/t0024> a skos:Concept;
  dct:identifier "t0024"^^xsd:token;
  dct:source "https://nrc-publications.canada.ca/eng/view/object/?id=69fb8993-1baa-4225-b33a-6a02341d383d"^^xsd:anyURI,
    "https://nrc-publications.canada.ca/fra/voir/objet/?id=549123c3-092c-4fca-8dea-99d53eac06dd"^^xsd:anyURI;
  skos:definition "A distinct soil micromorphology, resulting from the effects of freezing and thawing processes, in which soil particles form subhorizontal layers (see Figure 8c)."@en;
  skos:inScheme <https://w3id.org/permafrost/v/nrcglossary/scheme>;
  skos:prefLabel "banded cryogenic fabric"@en;
  skos:scopeNote "This fabric, found in cryosols, results from freeze-thaw processes accompanied by eluviation."@en;
  skos:topConceptOf <https://w3id.org/permafrost/v/nrcglossary/scheme> .

<https://w3id.org/permafrost/v/nrcglossary/t0025> a skos:Concept;
  dct:identifier "t0025"^^xsd:token;
  dct:source "https://nrc-publications.canada.ca/eng/view/object/?id=69fb8993-1baa-4225-b33a-6a02341d383d"^^xsd:anyURI,
    "https://nrc-publications.canada.ca/fra/voir/objet/?id=549123c3-092c-4fca-8dea-99d53eac06dd"^^xsd:anyURI;
  skos:definition "Areas of discontinuous vegetation cover in the polar semi-desert of the High Arctic."@en;
  skos:inScheme <https://w3id.org/permafrost/v/nrcglossary/scheme>;
  skos:prefLabel "barrens"@en;
  skos:scopeNote "Unvegetated areas of polar desert may be caused by climatic factors (too cold and/or too dry), or edaphic factors (low soil nutrients or toxic substrate), or a combination of those."@en;
  skos:topConceptOf <https://w3id.org/permafrost/v/nrcglossary/scheme> .

<https://w3id.org/permafrost/v/nrcglossary/t0026> a skos:Concept;
  dct:identifier "t0026"^^xsd:token;
  dct:source "https://nrc-publications.canada.ca/eng/view/object/?id=69fb8993-1baa-4225-b33a-6a02341d383d"^^xsd:anyURI,
    "https://nrc-publications.canada.ca/fra/voir/objet/?id=549123c3-092c-4fca-8dea-99d53eac06dd"^^xsd:anyURI;
  skos:definition "A layer of unfrozen ground that is perennially cryotic (T < 0°C), forming the basal portion of the permafrost (see Figures 2, 4 and 11)."@en;
  skos:inScheme <https://w3id.org/permafrost/v/nrcglossary/scheme>;
  skos:prefLabel "basal cryopeg"@en;
  skos:scopeNote "In a basal cryopeg, freezing is prevented by freezing-point depression due to the dissolved-solids content of its pore water."@en;
  skos:topConceptOf <https://w3id.org/permafrost/v/nrcglossary/scheme> .

<https://w3id.org/permafrost/v/nrcglossary/t0027> a skos:Concept;
  dct:identifier "t0027"^^xsd:token;
  dct:source "https://nrc-publications.canada.ca/eng/view/object/?id=69fb8993-1baa-4225-b33a-6a02341d383d"^^xsd:anyURI,
    "https://nrc-publications.canada.ca/fra/voir/objet/?id=549123c3-092c-4fca-8dea-99d53eac06dd"^^xsd:anyURI;
  skos:definition "The cryostructure of a frozen deposit of boulders that is saturated with ice (see Figure 9e)."@en;
  skos:inScheme <https://w3id.org/permafrost/v/nrcglossary/scheme>;
  skos:prefLabel "basal cryostructure"@en;
  skos:topConceptOf <https://w3id.org/permafrost/v/nrcglossary/scheme> .

<https://w3id.org/permafrost/v/nrcglossary/t0028> a skos:Concept;
  dct:identifier "t0028"^^xsd:token;
  dct:source "https://nrc-publications.canada.ca/eng/view/object/?id=69fb8993-1baa-4225-b33a-6a02341d383d"^^xsd:anyURI,
    "https://nrc-publications.canada.ca/fra/voir/objet/?id=549123c3-092c-4fca-8dea-99d53eac06dd"^^xsd:anyURI;
  skos:definition "The cryostructure of a frozen layered deposit of gravel and boulders that is saturated with ice (see Figure 9e)."@en;
  skos:inScheme <https://w3id.org/permafrost/v/nrcglossary/scheme>;
  skos:prefLabel "basal-layered cryostructure"@en;
  skos:topConceptOf <https://w3id.org/permafrost/v/nrcglossary/scheme> .

<https://w3id.org/permafrost/v/nrcglossary/t0029> a skos:Concept;
  dct:identifier "t0029"^^xsd:token;
  dct:source "https://nrc-publications.canada.ca/eng/view/object/?id=69fb8993-1baa-4225-b33a-6a02341d383d"^^xsd:anyURI,
    "https://nrc-publications.canada.ca/fra/voir/objet/?id=549123c3-092c-4fca-8dea-99d53eac06dd"^^xsd:anyURI;
  skos:definition "A stream characterized by narrow reaches linking pools or small lakes (see Figure 22a)."@en;
  skos:hiddenLabel "beaded drainage"@en, "button drainage"@en;
  skos:inScheme <https://w3id.org/permafrost/v/nrcglossary/scheme>;
  skos:prefLabel "beaded stream"@en, "cours d'eau en chapelet"@fr;
  skos:scopeNote "A characteristic pattern of small streams in areas underlain by ice wedges. The course of the stream channel is controlled by the pattern of the wedges, with the beads (pools) occurring at the junctions of the wedges. When the intervening channels are dry, they may be called \"beaded channels\"."@en;
  skos:topConceptOf <https://w3id.org/permafrost/v/nrcglossary/scheme> .

<https://w3id.org/permafrost/v/nrcglossary/t0030> a skos:Concept;
  dct:identifier "t0030"^^xsd:token;
  dct:source "https://nrc-publications.canada.ca/eng/view/object/?id=69fb8993-1baa-4225-b33a-6a02341d383d"^^xsd:anyURI,
    "https://nrc-publications.canada.ca/fra/voir/objet/?id=549123c3-092c-4fca-8dea-99d53eac06dd"^^xsd:anyURI;
  skos:altLabel "stone field"@en;
  skos:definition "A surficial layer of angular shattered rocks formed in either modern or Pleistocene periglacial environments."@en;
  skos:hiddenLabel "blockmeer"@en, "felsenmeer"@en;
  skos:inScheme <https://w3id.org/permafrost/v/nrcglossary/scheme>;
  skos:prefLabel "block field"@en;
  skos:topConceptOf <https://w3id.org/permafrost/v/nrcglossary/scheme> .

<https://w3id.org/permafrost/v/nrcglossary/t0031> a skos:Concept;
  dct:identifier "t0031"^^xsd:token;
  dct:source "https://nrc-publications.canada.ca/eng/view/object/?id=69fb8993-1baa-4225-b33a-6a02341d383d"^^xsd:anyURI,
    "https://nrc-publications.canada.ca/fra/voir/objet/?id=549123c3-092c-4fca-8dea-99d53eac06dd"^^xsd:anyURI;
  skos:definition "Temperature measured at the base of the snow cover during mid- to late- winter (February/March)."@en;
  skos:inScheme <https://w3id.org/permafrost/v/nrcglossary/scheme>;
  skos:prefLabel "bottom temperature of snow cover (BTS)"@en;
  skos:scopeNote "Such measurements are used in the BTS method to predict the presence or absence of permafrost in mountain areas where the winter snow cover is thicker than about 1.0 m"@en;
  skos:topConceptOf <https://w3id.org/permafrost/v/nrcglossary/scheme> .

<https://w3id.org/permafrost/v/nrcglossary/t0032> a skos:Concept;
  dct:identifier "t0032"^^xsd:token;
  dct:source "https://nrc-publications.canada.ca/eng/view/object/?id=69fb8993-1baa-4225-b33a-6a02341d383d"^^xsd:anyURI,
    "https://nrc-publications.canada.ca/fra/voir/objet/?id=549123c3-092c-4fca-8dea-99d53eac06dd"^^xsd:anyURI;
  skos:definition "Method to predict the presence or absence of permafrost in a mountain area, using measurements of the bottom temperature of snow cover in mid- to late-winter."@en;
  skos:inScheme <https://w3id.org/permafrost/v/nrcglossary/scheme>;
  skos:prefLabel "BTS method"@en;
  skos:scopeNote "Snow cover, with its low thermal conductivity, insulates the soil from short- term fluctuations in air temperature. In those mountain areas where snow-cover thickness equals or exceeds 1 m and surface melting is still negligible in mid- to late-winter, BTS values remain virtually constant, mainly controlled by heat transfer from the upper ground layers, which in turn is strongly influenced by the presence or absence of permafrost. According to published data, BTS values below -3?C, between -3?C and -1.7?C, and above -1.7C? suggest, respectively, the presence, possible presence, and absence of permafrost."@en;
  skos:topConceptOf <https://w3id.org/permafrost/v/nrcglossary/scheme> .

<https://w3id.org/permafrost/v/nrcglossary/t0033> a skos:Concept;
  dct:identifier "t0033"^^xsd:token;
  dct:source "https://nrc-publications.canada.ca/eng/view/object/?id=69fb8993-1baa-4225-b33a-6a02341d383d"^^xsd:anyURI,
    "https://nrc-publications.canada.ca/fra/voir/objet/?id=549123c3-092c-4fca-8dea-99d53eac06dd"^^xsd:anyURI;
  skos:definition "Ice formed or deposited on the ground surface and later covered by sediments."@en;
  skos:inScheme <https://w3id.org/permafrost/v/nrcglossary/scheme>;
  skos:prefLabel "buried ice"@en;
  skos:scopeNote "Buried ice likely represents buried glacier ice or snowbanks; or less likely, lake, river or sea ice, or icings."@en;
  skos:topConceptOf <https://w3id.org/permafrost/v/nrcglossary/scheme> .

<https://w3id.org/permafrost/v/nrcglossary/t0034> a skos:Concept;
  dct:identifier "t0034"^^xsd:token;
  dct:source "https://nrc-publications.canada.ca/eng/view/object/?id=69fb8993-1baa-4225-b33a-6a02341d383d"^^xsd:anyURI,
    "https://nrc-publications.canada.ca/fra/voir/objet/?id=549123c3-092c-4fca-8dea-99d53eac06dd"^^xsd:anyURI;
  skos:definition "Ice formed in a closed or open cave."@en;
  skos:inScheme <https://w3id.org/permafrost/v/nrcglossary/scheme>;
  skos:prefLabel "cave ice"@en;
  skos:scopeNote "Cave ice can form and persist in an area of temperate climatic conditions where the configuration of the cave or cave system permits an influx of cold winter air by gravity flow but limits access of warm summer air."@en;
  skos:topConceptOf <https://w3id.org/permafrost/v/nrcglossary/scheme> .

<https://w3id.org/permafrost/v/nrcglossary/t0035> a skos:Concept;
  dct:identifier "t0035"^^xsd:token;
  dct:source "https://nrc-publications.canada.ca/eng/view/object/?id=69fb8993-1baa-4225-b33a-6a02341d383d"^^xsd:anyURI,
    "https://nrc-publications.canada.ca/fra/voir/objet/?id=549123c3-092c-4fca-8dea-99d53eac06dd"^^xsd:anyURI;
  skos:definition "Ice formed in a closed space, cavity or cave in permafrost."@en;
  skos:inScheme <https://w3id.org/permafrost/v/nrcglossary/scheme>;
  skos:prefLabel "closed-cavity ice"@en;
  skos:scopeNote "Along the western Arctic coast of Canada for example, underground cavities, apparently formed by pockets of methane gas, have been found filled with ice crystals. The water from which the crystals have grown probably entered the cavities through vapour diffusion."@en;
  skos:topConceptOf <https://w3id.org/permafrost/v/nrcglossary/scheme> .

<https://w3id.org/permafrost/v/nrcglossary/t0036> a skos:Concept;
  dct:identifier "t0036"^^xsd:token;
  dct:source "https://nrc-publications.canada.ca/eng/view/object/?id=69fb8993-1baa-4225-b33a-6a02341d383d"^^xsd:anyURI,
    "https://nrc-publications.canada.ca/fra/voir/objet/?id=549123c3-092c-4fca-8dea-99d53eac06dd"^^xsd:anyURI;
  skos:definition "Freezing that occurs under conditions that preclude the gain or loss of any water by the system (see Figure 7)."@en;
  skos:inScheme <https://w3id.org/permafrost/v/nrcglossary/scheme>;
  skos:prefLabel "closed-system freezing"@en;
  skos:scopeNote "Pure closed-system conditions, in which water is neither added to nor removed from the system, are sometimes referred to as \"in situ freezing\". Closed-system freezing of water-saturated soil causes expansion equal to about 9 percent of the original pore volume of the unfrozen soil. Inside closed systems, some redistribution of water may take place during freezing."@en;
  skos:topConceptOf <https://w3id.org/permafrost/v/nrcglossary/scheme> .

<https://w3id.org/permafrost/v/nrcglossary/t0037> a skos:Concept;
  dct:identifier "t0037"^^xsd:token;
  dct:source "https://nrc-publications.canada.ca/eng/view/object/?id=69fb8993-1baa-4225-b33a-6a02341d383d"^^xsd:anyURI,
    "https://nrc-publications.canada.ca/fra/voir/objet/?id=549123c3-092c-4fca-8dea-99d53eac06dd"^^xsd:anyURI;
  skos:altLabel "hydrostatic pingo"@en;
  skos:definition "A pingo formed by doming of frozen ground due to freezing of injected water supplied by expulsion of pore water during permafrost aggradation in the closed talik under a former water body (see Figures 18 and 19a)."@en;
  skos:hiddenLabel "Mackenzie Delta pingo"@en;
  skos:inScheme <https://w3id.org/permafrost/v/nrcglossary/scheme>;
  skos:prefLabel "closed-system pingo"@en;
  skos:scopeNote "Most closed-system pingos are found in flat, poorly-drained terrain in the zone of continuous permafrost. Repeated injections of expelled water into the overlying permafrost, followed by freezing of the injected water, cause progressive doming, and produce the massive ice forming the core of the pingo. Progressive formation of segregated ice and dilation crack ice can also contribute to the process."@en;
  skos:topConceptOf <https://w3id.org/permafrost/v/nrcglossary/scheme> .

<https://w3id.org/permafrost/v/nrcglossary/t0038> a skos:Concept;
  dct:identifier "t0038"^^xsd:token;
  dct:source "https://nrc-publications.canada.ca/eng/view/object/?id=69fb8993-1baa-4225-b33a-6a02341d383d"^^xsd:anyURI,
    "https://nrc-publications.canada.ca/fra/voir/objet/?id=549123c3-092c-4fca-8dea-99d53eac06dd"^^xsd:anyURI;
  skos:definition "A layer or body of unfrozen ground occupying a depression in the permafrost table below a lake or river (see Figure 11)."@en;
  skos:inScheme <https://w3id.org/permafrost/v/nrcglossary/scheme>;
  skos:prefLabel "closed talik"@en;
  skos:scopeNote "The temperature of closed lake taliks and river taliks remains above 0°C because of the heat storage effect of the surface water."@en;
  skos:topConceptOf <https://w3id.org/permafrost/v/nrcglossary/scheme> .

<https://w3id.org/permafrost/v/nrcglossary/t0039> a skos:Concept;
  dct:identifier "t0039"^^xsd:token;
  dct:source "https://nrc-publications.canada.ca/eng/view/object/?id=69fb8993-1baa-4225-b33a-6a02341d383d"^^xsd:anyURI,
    "https://nrc-publications.canada.ca/fra/voir/objet/?id=549123c3-092c-4fca-8dea-99d53eac06dd"^^xsd:anyURI;
  skos:definition "The volume change per unit volume of a substance per unit increase in effective compressive stress, under isothermal conditions."@en;
  skos:inScheme <https://w3id.org/permafrost/v/nrcglossary/scheme>;
  skos:prefLabel "coefficient of compressibility"@en;
  skos:scopeNote "Frozen soils are usually considered to be practically incompressible, and volume-change deformations can therefore be neglected. Numerous investigations have shown, however, that the compressibility of frozen soils can be significant and should not be neglected in some cases, especially when large areas are to be loaded. Compressibility and its time dependence in frozen soils are due to several causes, such as instantaneous compression of the gaseous phase, creep of the pore ice due to shear stresses at the grain contacts, and hydrodynamic consolidation due to the expulsion of unfrozen water under stress, the amount of which varies with the applied pressure."@en;
  skos:topConceptOf <https://w3id.org/permafrost/v/nrcglossary/scheme> .

<https://w3id.org/permafrost/v/nrcglossary/t0040> a skos:Concept;
  dct:identifier "t0040"^^xsd:token;
  dct:source "https://nrc-publications.canada.ca/eng/view/object/?id=69fb8993-1baa-4225-b33a-6a02341d383d"^^xsd:anyURI,
    "https://nrc-publications.canada.ca/fra/voir/objet/?id=549123c3-092c-4fca-8dea-99d53eac06dd"^^xsd:anyURI;
  skos:definition "That portion of a peatland where the whole or part of a palsa or peat plateau has thawed and collapsed to the level of the surrounding peatland (see Figures 14 and 15e)."@en;
  skos:inScheme <https://w3id.org/permafrost/v/nrcglossary/scheme>;
  skos:prefLabel "cicatriced'affaissement"@fr, "collapse scar"@en;
  skos:scopeNote "A collapse scar is not a depression but is marked by vegetation different from the peatland that did not contain permafrost. Irregular topography (hence thermokarst terrain) may be present on the peatland as a whole but the collapse scars are only part of that thermokarst terrain, marked by the absence of permafrost, and by vegetation different from that on both the previously unfrozen peatlands and the remnant permafrost peat landforms."@en;
  skos:topConceptOf <https://w3id.org/permafrost/v/nrcglossary/scheme> .

<https://w3id.org/permafrost/v/nrcglossary/t0041> a skos:Concept;
  dct:identifier "t0041"^^xsd:token;
  dct:source "https://nrc-publications.canada.ca/eng/view/object/?id=69fb8993-1baa-4225-b33a-6a02341d383d"^^xsd:anyURI,
    "https://nrc-publications.canada.ca/fra/voir/objet/?id=549123c3-092c-4fca-8dea-99d53eac06dd"^^xsd:anyURI;
  skos:definition "A wedge showing evidence of both primary and secondary filling."@en;
  skos:inScheme <https://w3id.org/permafrost/v/nrcglossary/scheme>;
  skos:prefLabel "composite wedge"@en, "fente en coin à remplissage composé"@fr;
  skos:scopeNote "When used with reference to thermal contraction crack phenomena in permafrost, it describes a wedge filled by a combination of ice and soil (usually sand). The term is also frequently used to describe Pleistocene sand wedges and ice-wedge casts. Typically, composite wedges are filled with material very similar in structure and texture to sands in a typical fissure of primary filling (i.e., sand wedge). However, there may be inclusions of material from the fissure walls and some distortion of the adjacent sediments bordering the wedge, reflecting the presence of ice in the original fill material."@en;
  skos:topConceptOf <https://w3id.org/permafrost/v/nrcglossary/scheme> .

<https://w3id.org/permafrost/v/nrcglossary/t0042> a skos:Concept;
  dct:identifier "t0042"^^xsd:token;
  dct:source "https://nrc-publications.canada.ca/eng/view/object/?id=69fb8993-1baa-4225-b33a-6a02341d383d"^^xsd:anyURI,
    "https://nrc-publications.canada.ca/fra/voir/objet/?id=549123c3-092c-4fca-8dea-99d53eac06dd"^^xsd:anyURI;
  skos:definition "A distinct soil micromorphology, resulting from the effects of freezing and thawing processes, in which coarser soil particles form compound arrangements (see Figure 8f)."@en;
  skos:inScheme <https://w3id.org/permafrost/v/nrcglossary/scheme>;
  skos:prefLabel "conglomeric cryogenic fabric"@en;
  skos:scopeNote "This fabric, found in cryosols, results from freeze-thaw processes probably accompanied by cryoturbation."@en;
  skos:topConceptOf <https://w3id.org/permafrost/v/nrcglossary/scheme> .

<https://w3id.org/permafrost/v/nrcglossary/t0043> a skos:Concept;
  dct:identifier "t0043"^^xsd:token;
  dct:source "https://nrc-publications.canada.ca/eng/view/object/?id=69fb8993-1baa-4225-b33a-6a02341d383d"^^xsd:anyURI,
    "https://nrc-publications.canada.ca/fra/voir/objet/?id=549123c3-092c-4fca-8dea-99d53eac06dd"^^xsd:anyURI;
  skos:definition "Special design and construction procedures required when engineering works are undertaken in permafrost areas."@en;
  skos:inScheme <https://w3id.org/permafrost/v/nrcglossary/scheme>;
  skos:prefLabel "construction methods in permafrost"@en;
  skos:scopeNote "Design and construction of engineering works on permafrost normally follow one of two broad principles which are based on whether or not the frozen foundation soil or rock is thaw-stable (thaw-stable permafrost) or thaw-unstable (thaw-sensitive permafrost). Permafrost conditions can be neglected, and conventional designs and construction methods used when foundation materials are stable upon thawing. When the foundation materials are thaw-sensitive, however, then either the \"passive\" or \"active\" design and construction method is selected. The passive method maintains the foundation materials in a frozen state. Preservation of the frozen condition or permafrost aggradation can be accomplished using thermal piles or thermosyphons, or by using either a ventilation or an insulation construction technique; often a combination of these techniques is used. The ventilation technique requires that there is a clear space left between the bottom of the structure and the ground surface, or that the structure is placed on a fill pad with ducts incorporated in the pad or the floor system. Movement of cold air through the air space or ducts dissipates heat from the structure above and removes heat from the ground below. Using the insulation technique, a relatively thick fill (sometimes containing a layer of insulation) is placed on the ground surface to prevent thawing or to reduce or control the depth of thaw below the original ground surface. When permafrost degradation cannot be prevented, then one of the active methods must be considered. Two main approaches are possible. Unfavourable foundation materials are thawed and compacted or replaced with more suitable materials before the structure is erected. Alternatively, the foundations and structure are designed to accommodate the thaw settlements that will occur."@en;
  skos:topConceptOf <https://w3id.org/permafrost/v/nrcglossary/scheme> .

<https://w3id.org/permafrost/v/nrcglossary/t0044> a skos:Concept;
  dct:identifier "t0044"^^xsd:token;
  dct:source "https://nrc-publications.canada.ca/eng/view/object/?id=69fb8993-1baa-4225-b33a-6a02341d383d"^^xsd:anyURI,
    "https://nrc-publications.canada.ca/fra/voir/objet/?id=549123c3-092c-4fca-8dea-99d53eac06dd"^^xsd:anyURI;
  skos:definition "Permafrost occurring everywhere beneath the exposed land surface throughout a geographic region with the exception of widely scattered sites, such as newly deposited unconsolidated sediments, where the climate has just begun to impose its influence on the thermal regime of the ground, causing the development of continuous permafrost (see Figure 1)."@en;
  skos:inScheme <https://w3id.org/permafrost/v/nrcglossary/scheme>;
  skos:prefLabel "continuous permafrost"@en;
  skos:scopeNote "For practical purposes, the existence of small taliks within continuous permafrost has to be recognized. The term, therefore, generally refers to areas where more than 90 percent of the ground surface is underlain by permafrost."@en;
  skos:topConceptOf <https://w3id.org/permafrost/v/nrcglossary/scheme> .

<https://w3id.org/permafrost/v/nrcglossary/t0045> a skos:Concept;
  dct:identifier "t0045"^^xsd:token;
  dct:source "https://nrc-publications.canada.ca/eng/view/object/?id=69fb8993-1baa-4225-b33a-6a02341d383d"^^xsd:anyURI,
    "https://nrc-publications.canada.ca/fra/voir/objet/?id=549123c3-092c-4fca-8dea-99d53eac06dd"^^xsd:anyURI;
  skos:definition "The major subdivision of a permafrost region in which permafrost occurs everywhere beneath the exposed land surface with the exception of widely scattered sites."@en;
  skos:inScheme <https://w3id.org/permafrost/v/nrcglossary/scheme>;
  skos:prefLabel "continuous permafrost zone"@en;
  skos:scopeNote "Taliks associated with rivers and lakes may occur in the continuous permafrost zone."@en;
  skos:topConceptOf <https://w3id.org/permafrost/v/nrcglossary/scheme> .

<https://w3id.org/permafrost/v/nrcglossary/t0046> a skos:Concept;
  dct:identifier "t0046"^^xsd:token;
  dct:source "https://nrc-publications.canada.ca/eng/view/object/?id=69fb8993-1baa-4225-b33a-6a02341d383d"^^xsd:anyURI,
    "https://nrc-publications.canada.ca/fra/voir/objet/?id=549123c3-092c-4fca-8dea-99d53eac06dd"^^xsd:anyURI;
  skos:definition "The slow deformation (or time-dependent shear strain) that results from long-term application of a stress too small to produce failure in the frozen material."@en;
  skos:inScheme <https://w3id.org/permafrost/v/nrcglossary/scheme>;
  skos:prefLabel "creep of frozen ground"@en, "fluage du gélisol"@fr;
  skos:scopeNote "In frozen soils, creep deformations are due mainly to the creep of pore ice and the migration of unfrozen pore water. In ice-saturated frozen soils, most creep deformations are distortional with little or no volume change. In frozen soils with large unfrozen water contents or in unsaturated frozen soils, slow deformations due to consolidation, and creep due to volume change, may also occur. Usually, a large portion of the creep deformation is permanent."@en;
  skos:topConceptOf <https://w3id.org/permafrost/v/nrcglossary/scheme> .

<https://w3id.org/permafrost/v/nrcglossary/t0047> a skos:Concept;
  dct:identifier "t0047"^^xsd:token;
  dct:source "https://nrc-publications.canada.ca/eng/view/object/?id=69fb8993-1baa-4225-b33a-6a02341d383d"^^xsd:anyURI,
    "https://nrc-publications.canada.ca/fra/voir/objet/?id=549123c3-092c-4fca-8dea-99d53eac06dd"^^xsd:anyURI;
  skos:definition "The failure strength of a material at a given strain rate or after a given period under deviatoric stress."@en;
  skos:inScheme <https://w3id.org/permafrost/v/nrcglossary/scheme>;
  skos:prefLabel "creep strength"@en;
  skos:scopeNote "Under high confining stress and at relatively high freezing temperatures, most frozen soils creep and eventually fail in a plastic manner."@en;
  skos:topConceptOf <https://w3id.org/permafrost/v/nrcglossary/scheme> .

<https://w3id.org/permafrost/v/nrcglossary/t0048> a skos:Concept;
  dct:identifier "t0048"^^xsd:token;
  dct:source "https://nrc-publications.canada.ca/eng/view/object/?id=69fb8993-1baa-4225-b33a-6a02341d383d"^^xsd:anyURI,
    "https://nrc-publications.canada.ca/fra/voir/objet/?id=549123c3-092c-4fca-8dea-99d53eac06dd"^^xsd:anyURI;
  skos:definition "The cryostructure of a frozen deposit of angular blocks that are coated with ice, whereas large spaces between the blocks are not filled with ice (see Figure 9e)."@en;
  skos:inScheme <https://w3id.org/permafrost/v/nrcglossary/scheme>;
  skos:prefLabel "crust-like cryostructure"@en;
  skos:scopeNote "A deposit with a crust-like cryostructure has a relatively low ice content."@en;
  skos:topConceptOf <https://w3id.org/permafrost/v/nrcglossary/scheme> .

<https://w3id.org/permafrost/v/nrcglossary/t0049> a skos:Concept;
  dct:identifier "t0049"^^xsd:token;
  dct:source "https://nrc-publications.canada.ca/eng/view/object/?id=69fb8993-1baa-4225-b33a-6a02341d383d"^^xsd:anyURI,
    "https://nrc-publications.canada.ca/fra/voir/objet/?id=549123c3-092c-4fca-8dea-99d53eac06dd"^^xsd:anyURI;
  skos:definition "The boundary between cryotic and noncryotic ground as indicated by the position of the 0°C isotherm in the ground (see Figures 4 and 5)."@en;
  skos:inScheme <https://w3id.org/permafrost/v/nrcglossary/scheme>;
  skos:prefLabel "cryofront"@en, "cryofront"@fr;
  skos:scopeNote "The permafrost base and the boundaries between noncryotic and cryotic portions of the active layer constitute cryofronts. As a result of freezing-point depression, the freezing front usually lags behind the cryofront as it moves downwards during annual freezing of the active layer."@en;
  skos:topConceptOf <https://w3id.org/permafrost/v/nrcglossary/scheme> .

<https://w3id.org/permafrost/v/nrcglossary/t0050> a skos:Concept;
  dct:identifier "t0050"^^xsd:token;
  dct:source "https://nrc-publications.canada.ca/eng/view/object/?id=69fb8993-1baa-4225-b33a-6a02341d383d"^^xsd:anyURI,
    "https://nrc-publications.canada.ca/fra/voir/objet/?id=549123c3-092c-4fca-8dea-99d53eac06dd"^^xsd:anyURI;
  skos:definition "The combination of thermophysical, physico-chemical and physico- mechanical processes occurring in freezing, frozen and thawing earth materials."@en;
  skos:inScheme <https://w3id.org/permafrost/v/nrcglossary/scheme>;
  skos:prefLabel "cryogenesis"@en, "cryogenèse"@fr;
  skos:scopeNote "Specific processes of cryogenesis include water migration during freezing and thawing of the ground, frost heave, heat and mass (moisture) exchange, regelation and gelifluction. In the Russian permafrost literature, cryogenesis includes mainly processes that lead to development of permafrost cryostructure and landforms."@en;
  skos:topConceptOf <https://w3id.org/permafrost/v/nrcglossary/scheme> .

<https://w3id.org/permafrost/v/nrcglossary/t0051> a skos:Concept;
  dct:identifier "t0051"^^xsd:token;
  dct:source "https://nrc-publications.canada.ca/eng/view/object/?id=69fb8993-1baa-4225-b33a-6a02341d383d"^^xsd:anyURI,
    "https://nrc-publications.canada.ca/fra/voir/objet/?id=549123c3-092c-4fca-8dea-99d53eac06dd"^^xsd:anyURI;
  skos:definition "A layer of ground which, because of its frozen state, has a low enough permeability to act as a confining bed for an aquifer."@en;
  skos:inScheme <https://w3id.org/permafrost/v/nrcglossary/scheme>;
  skos:prefLabel "cryogenic aquiclude"@en;
  skos:scopeNote "Annual freezing can turn the active layer into a cryogenic aquiclude."@en;
  skos:topConceptOf <https://w3id.org/permafrost/v/nrcglossary/scheme> .

<https://w3id.org/permafrost/v/nrcglossary/t0052> a skos:Concept;
  dct:identifier "t0052"^^xsd:token;
  dct:source "https://nrc-publications.canada.ca/eng/view/object/?id=69fb8993-1baa-4225-b33a-6a02341d383d"^^xsd:anyURI,
    "https://nrc-publications.canada.ca/fra/voir/objet/?id=549123c3-092c-4fca-8dea-99d53eac06dd"^^xsd:anyURI;
  skos:definition "The distinct soil micromorphology resulting from the effects of freezing and thawing processes (see Figure 8)."@en;
  skos:inScheme <https://w3id.org/permafrost/v/nrcglossary/scheme>;
  skos:prefLabel "cryogenic fabric"@en;
  skos:scopeNote "The following cryogenic fabrics, found in cryosols, can be distinguished under a microscope: 1. granic and granoidic fabrics - soil particles form discrete loosely packed units. These fabrics are generally attributed to freeze-thaw processes and the formation of needle ice near the ground surface. 2. fragmic and fragmoidal fabrics - soil particles form discrete units that are either densely packed or coalescing. These fabrics commonly occur in subsurface soil horizons, usually close to the freezing front where soil material is subject to ice lens formation. 3. banded and isoband fabrics - soil particles form subhorizontal layers which result from freeze-thaw processes accompanied by eluviation. 4. orbiculic, suscitic and conglomeric fabrics - coarser soil particles form circular to ellipsoidal patterns (orbiculic), vertical or near-vertical orientation (suscitic), and compound arrangements (conglomeric), probably as a result of cryoturbation activity."@en;
  skos:topConceptOf <https://w3id.org/permafrost/v/nrcglossary/scheme> .

<https://w3id.org/permafrost/v/nrcglossary/t0053> a skos:Concept;
  dct:identifier "t0053"^^xsd:token;
  dct:source "https://nrc-publications.canada.ca/eng/view/object/?id=69fb8993-1baa-4225-b33a-6a02341d383d"^^xsd:anyURI,
    "https://nrc-publications.canada.ca/fra/voir/objet/?id=549123c3-092c-4fca-8dea-99d53eac06dd"^^xsd:anyURI;
  skos:definition "In international materials science, this term refers to temperatures generally below -50°C, but usually to temperatures within a few degrees of absolute zero (-273?C)."@en;
  skos:inScheme <https://w3id.org/permafrost/v/nrcglossary/scheme>;
  skos:prefLabel "cryogenic temperature"@en, "température cryogenique"@fr;
  skos:topConceptOf <https://w3id.org/permafrost/v/nrcglossary/scheme> .

<https://w3id.org/permafrost/v/nrcglossary/t0054> a skos:Concept;
  dct:identifier "t0054"^^xsd:token;
  dct:source "https://nrc-publications.canada.ca/eng/view/object/?id=69fb8993-1baa-4225-b33a-6a02341d383d"^^xsd:anyURI,
    "https://nrc-publications.canada.ca/fra/voir/objet/?id=549123c3-092c-4fca-8dea-99d53eac06dd"^^xsd:anyURI;
  skos:definition "The study of the genesis, structure and lithology of frozen earth materials."@en;
  skos:inScheme <https://w3id.org/permafrost/v/nrcglossary/scheme>;
  skos:prefLabel "cryolithologie"@fr, "cryolithology"@en;
  skos:scopeNote "This is a Russian term not widely used in North America. It is a branch of geocryology in which lithological and ground-ice conditions are emphasized."@en;
  skos:topConceptOf <https://w3id.org/permafrost/v/nrcglossary/scheme> .

<https://w3id.org/permafrost/v/nrcglossary/t0055> a skos:Concept;
  dct:identifier "t0055"^^xsd:token;
  dct:source "https://nrc-publications.canada.ca/eng/view/object/?id=69fb8993-1baa-4225-b33a-6a02341d383d"^^xsd:anyURI,
    "https://nrc-publications.canada.ca/fra/voir/objet/?id=549123c3-092c-4fca-8dea-99d53eac06dd"^^xsd:anyURI;
  skos:definition "The study of soils at temperatures below 0°C, with particular reference to soils subject to intensive frost action, and to soils overlying permafrost."@en;
  skos:inScheme <https://w3id.org/permafrost/v/nrcglossary/scheme>;
  skos:prefLabel "cryopedology"@en, "cryopédologie"@fr;
  skos:scopeNote "As originally defined (Bryan, 1946), the term comprised the whole science of geocryology, including the civil engineering methods used to overcome difficulties resulting from intensive frost action and the existence of permafrost."@en;
  skos:topConceptOf <https://w3id.org/permafrost/v/nrcglossary/scheme> .

<https://w3id.org/permafrost/v/nrcglossary/t0056> a skos:Concept;
  dct:identifier "t0056"^^xsd:token;
  dct:source "https://nrc-publications.canada.ca/eng/view/object/?id=69fb8993-1baa-4225-b33a-6a02341d383d"^^xsd:anyURI,
    "https://nrc-publications.canada.ca/fra/voir/objet/?id=549123c3-092c-4fca-8dea-99d53eac06dd"^^xsd:anyURI;
  skos:definition "A layer of unfrozen ground that is perennially cryotic (forming part of the permafrost), in which freezing is prevented by freezing-point depression due to the dissolved-solids content of the pore water (see Figures 2, 4 and 11)."@en;
  skos:inScheme <https://w3id.org/permafrost/v/nrcglossary/scheme>;
  skos:prefLabel "cryopeg"@en, "cryopeg"@fr;
  skos:scopeNote "Three types of cryopeg can be distinguished on the basis of their position with respect to permafrost: 1. a basal cryopeg forms the basal portion of the permafrost; 2. an isolated cryopeg is entirely surrounded by perennially frozen ground;; 3. a marine cryopeg is found in coastal or subsea perennially frozen ground; marine cryopegs may also be basal and/or isolated. In Russian literature cryopegs are defined as lenses of \"cryosaline water\" (supercooled brine) found within saline cryotic soils or rock."@en;
  skos:topConceptOf <https://w3id.org/permafrost/v/nrcglossary/scheme> .

<https://w3id.org/permafrost/v/nrcglossary/t0057> a skos:Concept;
  dct:identifier "t0057"^^xsd:token;
  dct:source "https://nrc-publications.canada.ca/eng/view/object/?id=69fb8993-1baa-4225-b33a-6a02341d383d"^^xsd:anyURI,
    "https://nrc-publications.canada.ca/fra/voir/objet/?id=549123c3-092c-4fca-8dea-99d53eac06dd"^^xsd:anyURI;
  skos:definition "The process through which cryoplanation terraces form."@en;
  skos:inScheme <https://w3id.org/permafrost/v/nrcglossary/scheme>;
  skos:prefLabel "cryoplanation"@en;
  skos:scopeNote "Cryoplanation occurs most frequently in periglacial areas of moderate aridity underlain by permafrost, under conditions of intense frost wedging associated with snowbanks."@en;
  skos:topConceptOf <https://w3id.org/permafrost/v/nrcglossary/scheme> .

<https://w3id.org/permafrost/v/nrcglossary/t0058> a skos:Concept;
  dct:identifier "t0058"^^xsd:token;
  dct:source "https://nrc-publications.canada.ca/eng/view/object/?id=69fb8993-1baa-4225-b33a-6a02341d383d"^^xsd:anyURI,
    "https://nrc-publications.canada.ca/fra/voir/objet/?id=549123c3-092c-4fca-8dea-99d53eac06dd"^^xsd:anyURI;
  skos:definition "A step-like or table-like bench cut in bedrock in cold climate regions."@en;
  skos:inScheme <https://w3id.org/permafrost/v/nrcglossary/scheme>;
  skos:prefLabel "cryoplanation terrace"@en, "terrasse d'altiplanatïon"@fr;
  skos:scopeNote "Cryoplanation terraces may occur as both hillside benches or bevelled summit surfaces and often lack structural control. They are thought to form under conditions of intense frost wedging associated with snowbanks. Cryoplanation terraces are more frequently reported from periglacial areas of moderate aridity. As these areas are usually underlain by permafrost, cryoplanation terraces are regarded by some as diagnostic landforms of permafrost terrain."@en;
  skos:topConceptOf <https://w3id.org/permafrost/v/nrcglossary/scheme> .

<https://w3id.org/permafrost/v/nrcglossary/t0059> a skos:Concept;
  dct:identifier "t0059"^^xsd:token;
  dct:source "https://nrc-publications.canada.ca/eng/view/object/?id=69fb8993-1baa-4225-b33a-6a02341d383d"^^xsd:anyURI,
    "https://nrc-publications.canada.ca/fra/voir/objet/?id=549123c3-092c-4fca-8dea-99d53eac06dd"^^xsd:anyURI;
  skos:definition "Soil formed in either mineral or organic materials having permafrost either within 1 m below the surface or, if the soil is strongly cryoturbated, within 2 m below the surface, and having a mean annual ground temperature below 0°C."@en;
  skos:hiddenLabel "cryosolic soil"@en, "pergelic soil"@en;
  skos:inScheme <https://w3id.org/permafrost/v/nrcglossary/scheme>;
  skos:prefLabel "cryosol"@en, "cryosol"@fr;
  skos:scopeNote "This is a pedological term for a major soil order. Cryosols are divided into three groups: 1. organic cryosols developed in organic (peat) materials; 2. static cryosols developed in mineral soils and showing little or no evidence of cryoturbation; 3. turbic cryosols developed in mineral soils and showing strong evidence of cryoturbation."@en;
  skos:topConceptOf <https://w3id.org/permafrost/v/nrcglossary/scheme> .

<https://w3id.org/permafrost/v/nrcglossary/t0060> a skos:Concept;
  dct:identifier "t0060"^^xsd:token;
  dct:source "https://nrc-publications.canada.ca/eng/view/object/?id=69fb8993-1baa-4225-b33a-6a02341d383d"^^xsd:anyURI,
    "https://nrc-publications.canada.ca/fra/voir/objet/?id=549123c3-092c-4fca-8dea-99d53eac06dd"^^xsd:anyURI;
  skos:definition "That part of the earth's crust, hydrosphere and atmosphere subject to temperatures below 0°C for at least part of each year."@en;
  skos:inScheme <https://w3id.org/permafrost/v/nrcglossary/scheme>;
  skos:prefLabel "cryosphere"@en, "cryosphère"@fr;
  skos:scopeNote "The cryosphere may be divided into the cryoatmosphere, the cryohydrosphere (snowcover, glaciers, and river, lake and sea ice) and the cryolithosphere (perennially and seasonally cryotic ground). Some authorities exclude the earth's atmosphere from the cryosphere; others restrict the term \"cryosphere\" to the regions of the earth's crust where permafrost exists."@en;
  skos:topConceptOf <https://w3id.org/permafrost/v/nrcglossary/scheme> .

<https://w3id.org/permafrost/v/nrcglossary/t0061> a skos:Concept;
  dct:identifier "t0061"^^xsd:token;
  dct:source "https://nrc-publications.canada.ca/eng/view/object/?id=69fb8993-1baa-4225-b33a-6a02341d383d"^^xsd:anyURI,
    "https://nrc-publications.canada.ca/fra/voir/objet/?id=549123c3-092c-4fca-8dea-99d53eac06dd"^^xsd:anyURI;
  skos:definition "The structural characteristics of frozen earth materials (see Figure 9)."@en;
  skos:inScheme <https://w3id.org/permafrost/v/nrcglossary/scheme>;
  skos:prefLabel "cryostructure"@en, "cryostructure"@fr;
  skos:scopeNote "The cryostructure is determined by the amount and distribution of pore ice (or ice cement) and lenses of segregated ice. The type and arrangement of ice in the frozen material will depend largely on the initial total water content of the material and the extent of moisture migration during subsequent freezing. For engineering purposes, the structure of frozen soil may be described as massive, layered or reticulate, based on the type and distribution of ice in the soil. A massive structure (not to be confused with massive ground-ice forms) is characterized by the predominant presence of pore ice and by a relatively low total ice content. In soils with a reticulate structure, ice veins generally form a random net, whereas in those with a layered structure, well-oriented horizontal ice lenses alternate with soil layers having a massive structure. In both cases their total ice content is relatively high. Russian permafrost scientists identify ten cryogenic structures or cryostructures: basal, basal-layered, crust-like, layered, lens-type, massive- agglomerate, massive, massive-porous, reticulate and reticulate-blocky."@en;
  skos:topConceptOf <https://w3id.org/permafrost/v/nrcglossary/scheme> .

<https://w3id.org/permafrost/v/nrcglossary/t0062> a skos:Concept;
  dct:identifier "t0062"^^xsd:token;
  dct:source "https://nrc-publications.canada.ca/eng/view/object/?id=69fb8993-1baa-4225-b33a-6a02341d383d"^^xsd:anyURI,
    "https://nrc-publications.canada.ca/fra/voir/objet/?id=549123c3-092c-4fca-8dea-99d53eac06dd"^^xsd:anyURI;
  skos:definition "A suction developed in freezing or partially frozen fine-grained materials as a result of temperature-dependent differences in unfrozen water content."@en;
  skos:hiddenLabel "frost suction"@en;
  skos:inScheme <https://w3id.org/permafrost/v/nrcglossary/scheme>;
  skos:prefLabel "cryosuccion"@fr, "cryosuction"@en;
  skos:scopeNote "Cryosuction occurs where gradients of the temperature-dependent unfrozen water content in a freezing or partially frozen fine-grained earth material cause hydraulic gradients large enough to induce migration of pore water from unfrozen soil into the partially frozen soil via unfrozen water films."@en;
  skos:topConceptOf <https://w3id.org/permafrost/v/nrcglossary/scheme> .

<https://w3id.org/permafrost/v/nrcglossary/t0063> a skos:Concept;
  dct:identifier "t0063"^^xsd:token;
  dct:source "https://nrc-publications.canada.ca/eng/view/object/?id=69fb8993-1baa-4225-b33a-6a02341d383d"^^xsd:anyURI,
    "https://nrc-publications.canada.ca/fra/voir/objet/?id=549123c3-092c-4fca-8dea-99d53eac06dd"^^xsd:anyURI;
  skos:definition "The textural characteristics of frozen, fine-grained organic and mineral earth materials cemented together with ice."@en;
  skos:inScheme <https://w3id.org/permafrost/v/nrcglossary/scheme>;
  skos:prefLabel "cryotexture"@en, "cryotexture"@fr;
  skos:scopeNote "Cryotextures may be useful in determining the nature of the freezing process and the conditions under which the sediments accumulated."@en;
  skos:topConceptOf <https://w3id.org/permafrost/v/nrcglossary/scheme> .

<https://w3id.org/permafrost/v/nrcglossary/t0064> a skos:Concept;
  dct:identifier "t0064"^^xsd:token;
  dct:source "https://nrc-publications.canada.ca/eng/view/object/?id=69fb8993-1baa-4225-b33a-6a02341d383d"^^xsd:anyURI,
    "https://nrc-publications.canada.ca/fra/voir/objet/?id=549123c3-092c-4fca-8dea-99d53eac06dd"^^xsd:anyURI;
  skos:definition "Soil or rock at temperatures of 0°C or lower."@en;
  skos:inScheme <https://w3id.org/permafrost/v/nrcglossary/scheme>;
  skos:prefLabel "cryotic ground"@en, "sol cryotique"@fr;
  skos:scopeNote "The terms \"cryotic\" and \"noncryotic\" were introduced to solve a major semantic problem identified by Brown and Kupsch (1974), namely the lack of specific separate terms to designate \"above 0°C\" and \"below 0°C\" as opposed to \"unfrozen\" (not containing ice) and \"frozen\" (containing ice) (see Figure 3). Cryotic and noncryotic refer solely to the temperature of the material described, independent of its water or ice content. Perennially cryotic ground refers to ground that remains at or below 0°C continuously for two or more years and is therefore synonymous with permafrost."@en;
  skos:topConceptOf <https://w3id.org/permafrost/v/nrcglossary/scheme> .

<https://w3id.org/permafrost/v/nrcglossary/t0065> a skos:Concept;
  dct:identifier "t0065"^^xsd:token;
  dct:source "https://nrc-publications.canada.ca/eng/view/object/?id=69fb8993-1baa-4225-b33a-6a02341d383d"^^xsd:anyURI,
    "https://nrc-publications.canada.ca/fra/voir/objet/?id=549123c3-092c-4fca-8dea-99d53eac06dd"^^xsd:anyURI;
  skos:altLabel "cryoturbations"@en;
  skos:definition "A body of earth material moved or disturbed by frost action."@en;
  skos:hiddenLabel "congeliturbate"@en;
  skos:inScheme <https://w3id.org/permafrost/v/nrcglossary/scheme>;
  skos:prefLabel "cryoturbate"@en, "matériaux géliturbés"@fr;
  skos:scopeNote "The process of cryoturbation results in the disruption and distortion of soil horizons and structures, the formation of patterned ground, the growth of involutions, and the redistribution of organic-rich subsurface masses and layers. Downslope soil movements are more properly termed solifluction, gelifluction and frost creep, although many authors include the products of solifluction within the term cryoturbate."@en;
  skos:topConceptOf <https://w3id.org/permafrost/v/nrcglossary/scheme> .

<https://w3id.org/permafrost/v/nrcglossary/t0066> a skos:Concept;
  dct:identifier "t0066"^^xsd:token;
  dct:source "https://nrc-publications.canada.ca/eng/view/object/?id=69fb8993-1baa-4225-b33a-6a02341d383d"^^xsd:anyURI,
    "https://nrc-publications.canada.ca/fra/voir/objet/?id=549123c3-092c-4fca-8dea-99d53eac06dd"^^xsd:anyURI;
  skos:definition "1. (Singular) A collective term used to describe all soil movements due to frost action. 2. (Plural) Irregular structures formed in earth materials by deep frost penetration and frost action processes, and characterized by folded, broken and dislocated beds and lenses of unconsolidated deposits, included organic horizons and even bedrock."@en;
  skos:inScheme <https://w3id.org/permafrost/v/nrcglossary/scheme>;
  skos:prefLabel "cryoturbation"@en, "géliturbat"@fr;
  skos:scopeNote "Cryoturbation encompasses frost heave, thaw settlement and all differential movements, including expansion and contraction due to temperature changes and the growth and disappearance of ground ice bodies, whether perennial or seasonal. Low temperatures alone are not enough to produce cryoturbation; the water-ice phase change is necessary. Cryoturbation is an important process in the development of patterned ground."@en;
  skos:topConceptOf <https://w3id.org/permafrost/v/nrcglossary/scheme> .

<https://w3id.org/permafrost/v/nrcglossary/t0067> a skos:Concept;
  dct:identifier "t0067"^^xsd:token;
  dct:source "https://nrc-publications.canada.ca/eng/view/object/?id=69fb8993-1baa-4225-b33a-6a02341d383d"^^xsd:anyURI,
    "https://nrc-publications.canada.ca/fra/voir/objet/?id=549123c3-092c-4fca-8dea-99d53eac06dd"^^xsd:anyURI;
  skos:definition "A sudden and destructive variety of landslide, in which loose material on a slope, with more than 50 percent of particles larger than sand size, is mobilized by saturation and flows down a channel or canyon."@en;
  skos:inScheme <https://w3id.org/permafrost/v/nrcglossary/scheme>;
  skos:prefLabel "debris flow"@en;
  skos:scopeNote "The water content of debris flows may range from 10 to over 50 percent by volume. They may transport huge boulders for great distances down gentle slopes. Debris flows also occur in non-permafrost areas."@en;
  skos:topConceptOf <https://w3id.org/permafrost/v/nrcglossary/scheme> .

<https://w3id.org/permafrost/v/nrcglossary/t0068> a skos:Concept;
  dct:identifier "t0068"^^xsd:token;
  dct:source "https://nrc-publications.canada.ca/eng/view/object/?id=69fb8993-1baa-4225-b33a-6a02341d383d"^^xsd:anyURI,
    "https://nrc-publications.canada.ca/fra/voir/objet/?id=549123c3-092c-4fca-8dea-99d53eac06dd"^^xsd:anyURI;
  skos:definition "The ability of a material to change its shape or size under the influence of an external or internal agency, such as stress, temperature, or pore pressure."@en;
  skos:inScheme <https://w3id.org/permafrost/v/nrcglossary/scheme>;
  skos:prefLabel "deformability"@en;
  skos:topConceptOf <https://w3id.org/permafrost/v/nrcglossary/scheme> .

<https://w3id.org/permafrost/v/nrcglossary/t0069> a skos:Concept;
  dct:identifier "t0069"^^xsd:token;
  dct:source "https://nrc-publications.canada.ca/eng/view/object/?id=69fb8993-1baa-4225-b33a-6a02341d383d"^^xsd:anyURI,
    "https://nrc-publications.canada.ca/fra/voir/objet/?id=549123c3-092c-4fca-8dea-99d53eac06dd"^^xsd:anyURI;
  skos:definition "A derived unit of measurement used to express the departure of the mean temperature for a day from a given reference (or base) temperature."@en;
  skos:inScheme <https://w3id.org/permafrost/v/nrcglossary/scheme>;
  skos:prefLabel "degree-day (C or F)"@en;
  skos:scopeNote "The freezing index and the thawing index are expressed in degree-days with respect to a reference temperature of 0°C (32?F); units: degree-day Celsius or degree-day Fahrenheit."@en;
  skos:topConceptOf <https://w3id.org/permafrost/v/nrcglossary/scheme> .

<https://w3id.org/permafrost/v/nrcglossary/t0070> a skos:Concept;
  dct:identifier "t0070"^^xsd:token;
  dct:source "https://nrc-publications.canada.ca/eng/view/object/?id=69fb8993-1baa-4225-b33a-6a02341d383d"^^xsd:anyURI,
    "https://nrc-publications.canada.ca/fra/voir/objet/?id=549123c3-092c-4fca-8dea-99d53eac06dd"^^xsd:anyURI;
  skos:definition "1. The total degree of saturation of frozen soil is the ratio of the volume of ice and unfrozen water in the soil pores to the volume of the pores. 2. The degree of saturation of frozen soil by ice is the ratio of the volume of ice in the soil pores to the volume of the pores."@en;
  skos:inScheme <https://w3id.org/permafrost/v/nrcglossary/scheme>;
  skos:prefLabel "degree of saturation"@en;
  skos:scopeNote "Neither definition is the equivalent of the standard definition used in soil mechanics where the degree of saturation is the ratio of the volume of water in a soil to the volume of the pores."@en;
  skos:topConceptOf <https://w3id.org/permafrost/v/nrcglossary/scheme> .

<https://w3id.org/permafrost/v/nrcglossary/t0071> a skos:Concept;
  dct:identifier "t0071"^^xsd:token;
  dct:source "https://nrc-publications.canada.ca/eng/view/object/?id=69fb8993-1baa-4225-b33a-6a02341d383d"^^xsd:anyURI,
    "https://nrc-publications.canada.ca/fra/voir/objet/?id=549123c3-092c-4fca-8dea-99d53eac06dd"^^xsd:anyURI;
  skos:definition "The failure strength of a material at a given strain rate or after a given period under deviatoric stress."@en;
  skos:inScheme <https://w3id.org/permafrost/v/nrcglossary/scheme>;
  skos:prefLabel "delayed strength"@en;
  skos:topConceptOf <https://w3id.org/permafrost/v/nrcglossary/scheme> .

<https://w3id.org/permafrost/v/nrcglossary/t0072> a skos:Concept;
  dct:identifier "t0072"^^xsd:token;
  dct:source "https://nrc-publications.canada.ca/eng/view/object/?id=69fb8993-1baa-4225-b33a-6a02341d383d"^^xsd:anyURI,
    "https://nrc-publications.canada.ca/fra/voir/objet/?id=549123c3-092c-4fca-8dea-99d53eac06dd"^^xsd:anyURI;
  skos:definition "The mass of a unit volume of frozen soil or rock."@en;
  skos:inScheme <https://w3id.org/permafrost/v/nrcglossary/scheme>;
  skos:prefLabel "density of frozen ground"@en, "densité du gélisol"@fr;
  skos:topConceptOf <https://w3id.org/permafrost/v/nrcglossary/scheme> .

<https://w3id.org/permafrost/v/nrcglossary/t0073> a skos:Concept;
  dct:identifier "t0073"^^xsd:token;
  dct:source "https://nrc-publications.canada.ca/eng/view/object/?id=69fb8993-1baa-4225-b33a-6a02341d383d"^^xsd:anyURI,
    "https://nrc-publications.canada.ca/fra/voir/objet/?id=549123c3-092c-4fca-8dea-99d53eac06dd"^^xsd:anyURI;
  skos:definition "The maximum thickness of the seasonally frozen layer."@en;
  skos:inScheme <https://w3id.org/permafrost/v/nrcglossary/scheme>;
  skos:prefLabel "depth of seasonal frost penetration"@en;
  skos:scopeNote "This term is primarily used in areas without permafrost, but also in areas with permafrost where the seasonal frost does not reach the permafrost table."@en;
  skos:topConceptOf <https://w3id.org/permafrost/v/nrcglossary/scheme> .

<https://w3id.org/permafrost/v/nrcglossary/t0074> a skos:Concept;
  dct:identifier "t0074"^^xsd:token;
  dct:source "https://nrc-publications.canada.ca/eng/view/object/?id=69fb8993-1baa-4225-b33a-6a02341d383d"^^xsd:anyURI,
    "https://nrc-publications.canada.ca/fra/voir/objet/?id=549123c3-092c-4fca-8dea-99d53eac06dd"^^xsd:anyURI;
  skos:definition "The minimum distance between the ground surface and frozen ground at any time during the thawing season in an area subject to seasonal freezing and thawing (see Figure 4)."@en;
  skos:inScheme <https://w3id.org/permafrost/v/nrcglossary/scheme>;
  skos:prefLabel "depth of thaw"@en, "profondeur de dégel"@fr;
  skos:scopeNote "When no frozen ground remains, thawing is complete, and depth of thaw cannot be determined."@en;
  skos:topConceptOf <https://w3id.org/permafrost/v/nrcglossary/scheme> .

<https://w3id.org/permafrost/v/nrcglossary/t0075> a skos:Concept;
  dct:identifier "t0075"^^xsd:token;
  dct:source "https://nrc-publications.canada.ca/eng/view/object/?id=69fb8993-1baa-4225-b33a-6a02341d383d"^^xsd:anyURI,
    "https://nrc-publications.canada.ca/fra/voir/objet/?id=549123c3-092c-4fca-8dea-99d53eac06dd"^^xsd:anyURI;
  skos:definition "The distance from the ground surface downward to the level beneath which there is practically no annual fluctuation in ground temperature (see Figure 2)."@en;
  skos:hiddenLabel "zone of minimum annual amplitude"@en, "zone of zero annual amplitude"@en;
  skos:inScheme <https://w3id.org/permafrost/v/nrcglossary/scheme>;
  skos:prefLabel "depth of zero annual amplitude"@en, "profondeur de l'amplitude annuelle nulle"@fr;
  skos:scopeNote "A change of no more than 0.1?C throughout the year is arbitrarily considered as \"practically no annual fluctuation\". The temperature at the depth (or level) of zero annual amplitude ranges from about -0.1?C at the southern limit of the permafrost region to about -15?C in the extreme polar reaches of the zone of continuous permafrost. The depth of zero annual amplitude varies widely but generally lies between 10 and 20 m below the ground surface, depending on climatic and terrain conditions such as amplitude of annual surface temperature variation, vegetation, snowcover and characteristics of the soils and rocks including thermal diffusivity (see thermal properties of frozen ground)."@en;
  skos:topConceptOf <https://w3id.org/permafrost/v/nrcglossary/scheme> .

<https://w3id.org/permafrost/v/nrcglossary/t0076> a skos:Concept;
  dct:identifier "t0076"^^xsd:token;
  dct:source "https://nrc-publications.canada.ca/eng/view/object/?id=69fb8993-1baa-4225-b33a-6a02341d383d"^^xsd:anyURI,
    "https://nrc-publications.canada.ca/fra/voir/objet/?id=549123c3-092c-4fca-8dea-99d53eac06dd"^^xsd:anyURI;
  skos:definition "Crack or fissure developed in fine-grained soil material as a result of shrinkage during drying."@en;
  skos:inScheme <https://w3id.org/permafrost/v/nrcglossary/scheme>;
  skos:prefLabel "desiccation crack"@en;
  skos:topConceptOf <https://w3id.org/permafrost/v/nrcglossary/scheme> .

<https://w3id.org/permafrost/v/nrcglossary/t0077> a skos:Concept;
  dct:identifier "t0077"^^xsd:token;
  dct:source "https://nrc-publications.canada.ca/eng/view/object/?id=69fb8993-1baa-4225-b33a-6a02341d383d"^^xsd:anyURI,
    "https://nrc-publications.canada.ca/fra/voir/objet/?id=549123c3-092c-4fca-8dea-99d53eac06dd"^^xsd:anyURI;
  skos:definition "Closed, multi-sided patterned-ground feature formed by desiccation cracks"@en;
  skos:inScheme <https://w3id.org/permafrost/v/nrcglossary/scheme>;
  skos:prefLabel "desiccation polygon"@en;
  skos:topConceptOf <https://w3id.org/permafrost/v/nrcglossary/scheme> .

<https://w3id.org/permafrost/v/nrcglossary/t0078> a skos:Concept;
  dct:identifier "t0078"^^xsd:token;
  dct:source "https://nrc-publications.canada.ca/eng/view/object/?id=69fb8993-1baa-4225-b33a-6a02341d383d"^^xsd:anyURI,
    "https://nrc-publications.canada.ca/fra/voir/objet/?id=549123c3-092c-4fca-8dea-99d53eac06dd"^^xsd:anyURI;
  skos:definition "1. (North-American usage) The mean of the three largest depths of seasonal frost penetration measured during the past thirty years, or the largest depth of seasonal frost penetration beneath a snow-free soil surface measured during the past ten years. 2. (Russian usage) The mean of the depths of seasonal frost penetration measured during at least the last ten years with the ground surface free of snow and the groundwater level below the depth of seasonal frost penetration."@en;
  skos:inScheme <https://w3id.org/permafrost/v/nrcglossary/scheme>;
  skos:prefLabel "design depth of frost penetration"@en;
  skos:topConceptOf <https://w3id.org/permafrost/v/nrcglossary/scheme> .

<https://w3id.org/permafrost/v/nrcglossary/t0079> a skos:Concept;
  dct:identifier "t0079"^^xsd:token;
  dct:source "https://nrc-publications.canada.ca/eng/view/object/?id=69fb8993-1baa-4225-b33a-6a02341d383d"^^xsd:anyURI,
    "https://nrc-publications.canada.ca/fra/voir/objet/?id=549123c3-092c-4fca-8dea-99d53eac06dd"^^xsd:anyURI;
  skos:definition "The cumulative number of degree-days below 0°C, calculated by taking the average of the seasonal freezing indices for the three coldest winters in the most recent 30 years of record."@en;
  skos:inScheme <https://w3id.org/permafrost/v/nrcglossary/scheme>;
  skos:prefLabel "design freezing index"@en;
  skos:scopeNote "If data for 30 years are not available, then the index is based on the coldest winter in the latest 10-year period of record."@en;
  skos:topConceptOf <https://w3id.org/permafrost/v/nrcglossary/scheme> .

<https://w3id.org/permafrost/v/nrcglossary/t0080> a skos:Concept;
  dct:identifier "t0080"^^xsd:token;
  dct:source "https://nrc-publications.canada.ca/eng/view/object/?id=69fb8993-1baa-4225-b33a-6a02341d383d"^^xsd:anyURI,
    "https://nrc-publications.canada.ca/fra/voir/objet/?id=549123c3-092c-4fca-8dea-99d53eac06dd"^^xsd:anyURI;
  skos:definition "The cumulative number of degree-days above 0°C, calculated by taking the average of the seasonal thawing indices for the three warmest summers in the most recent 30 years of record."@en;
  skos:inScheme <https://w3id.org/permafrost/v/nrcglossary/scheme>;
  skos:prefLabel "design thawing index"@en;
  skos:scopeNote "If data for 30 years are not available, then the index is based on the warmest summer in the latest 10-year period of record."@en;
  skos:topConceptOf <https://w3id.org/permafrost/v/nrcglossary/scheme> .

<https://w3id.org/permafrost/v/nrcglossary/t0081> a skos:Concept;
  dct:identifier "t0081"^^xsd:token;
  dct:source "https://nrc-publications.canada.ca/eng/view/object/?id=69fb8993-1baa-4225-b33a-6a02341d383d"^^xsd:anyURI,
    "https://nrc-publications.canada.ca/fra/voir/objet/?id=549123c3-092c-4fca-8dea-99d53eac06dd"^^xsd:anyURI;
  skos:definition "A slope failure in which the thawed or thawing portion of the active layer detaches from the underlying frozen material (see Figure 21b)."@en;
  skos:hiddenLabel "active-layer glide"@en, "skin flow"@en;
  skos:inScheme <https://w3id.org/permafrost/v/nrcglossary/scheme>;
  skos:prefLabel "detachment failure"@en, "rupture par décollement"@fr;
  skos:scopeNote "Detachment failures are common on colluvial slopes in areas of fine-grained, ice-rich deposits. They occur more frequently during warm summers or following disturbance of the vegetation or ground surface by, for example, tundra or forest fires or engineering activity, when the depth of thaw is greater than normal. Detachment failures that expose massive ice or icy sediments can develop into retrogressive thaw slumps."@en;
  skos:topConceptOf <https://w3id.org/permafrost/v/nrcglossary/scheme> .

<https://w3id.org/permafrost/v/nrcglossary/t0082> a skos:Concept;
  dct:identifier "t0082"^^xsd:token;
  dct:source "https://nrc-publications.canada.ca/eng/view/object/?id=69fb8993-1baa-4225-b33a-6a02341d383d"^^xsd:anyURI,
    "https://nrc-publications.canada.ca/fra/voir/objet/?id=549123c3-092c-4fca-8dea-99d53eac06dd"^^xsd:anyURI;
  skos:altLabel "relative permittivity"@en;
  skos:definition "The dielectric constant of a soil is a measure of the ability of the soil to store electrical energy in the presence of an electrostatic field."@en;
  skos:inScheme <https://w3id.org/permafrost/v/nrcglossary/scheme>;
  skos:prefLabel "dielectric constant"@en;
  skos:scopeNote "The dielectric constant is calculated as the ratio of the permittivity of the soil to the permittivity of a vacuum. It varies with soil type, temperature, unfrozen water content, and the dissolved-solids content of the pore water."@en;
  skos:topConceptOf <https://w3id.org/permafrost/v/nrcglossary/scheme> .

<https://w3id.org/permafrost/v/nrcglossary/t0083> a skos:Concept;
  dct:identifier "t0083"^^xsd:token;
  dct:source "https://nrc-publications.canada.ca/eng/view/object/?id=69fb8993-1baa-4225-b33a-6a02341d383d"^^xsd:anyURI,
    "https://nrc-publications.canada.ca/fra/voir/objet/?id=549123c3-092c-4fca-8dea-99d53eac06dd"^^xsd:anyURI;
  skos:definition "A tensile fracture in a frozen material due to surface extension caused by doming."@en;
  skos:inScheme <https://w3id.org/permafrost/v/nrcglossary/scheme>;
  skos:prefLabel "dilation crack"@en, "fissure de dilatation"@fr;
  skos:scopeNote "This usually occurs during the growth of frost mounds."@en;
  skos:topConceptOf <https://w3id.org/permafrost/v/nrcglossary/scheme> .

<https://w3id.org/permafrost/v/nrcglossary/t0084> a skos:Concept;
  dct:identifier "t0084"^^xsd:token;
  dct:source "https://nrc-publications.canada.ca/eng/view/object/?id=69fb8993-1baa-4225-b33a-6a02341d383d"^^xsd:anyURI,
    "https://nrc-publications.canada.ca/fra/voir/objet/?id=549123c3-092c-4fca-8dea-99d53eac06dd"^^xsd:anyURI;
  skos:definition "Ice that forms in dilation cracks (see Figure 10b)."@en;
  skos:inScheme <https://w3id.org/permafrost/v/nrcglossary/scheme>;
  skos:prefLabel "dilation crack ice"@en;
  skos:scopeNote "Dilation crack ice may form a significant component of the total ice content of features such as pingos. The ice is vertically banded and may be discoloured by inclusions of mineral soil and organic matter. Individual bands may be up to 20 cm wide."@en;
  skos:topConceptOf <https://w3id.org/permafrost/v/nrcglossary/scheme> .

<https://w3id.org/permafrost/v/nrcglossary/t0085> a skos:Concept;
  dct:identifier "t0085"^^xsd:token;
  dct:source "https://nrc-publications.canada.ca/eng/view/object/?id=69fb8993-1baa-4225-b33a-6a02341d383d"^^xsd:anyURI,
    "https://nrc-publications.canada.ca/fra/voir/objet/?id=549123c3-092c-4fca-8dea-99d53eac06dd"^^xsd:anyURI;
  skos:definition "Permafrost occurring in some areas beneath the exposed land surface throughout a geographic region where other areas are free of permafrost (see Figure 1)."@en;
  skos:hiddenLabel "insular permafrost"@en, "island permafrost"@en, "scattered permafrost"@en;
  skos:inScheme <https://w3id.org/permafrost/v/nrcglossary/scheme>;
  skos:prefLabel "discontinuous permafrost"@en;
  skos:scopeNote "Discontinuous permafrost occurs between the continuous permafrost zone and the southern latitudinal limit of permafrost in lowlands. Depending on the scale of mapping, several subzones can often be distinguished, based on the percentage of the land surface underlain by permafrost, as shown in the following table. [Table not included in Excel spreadsheet]"@en;
  skos:topConceptOf <https://w3id.org/permafrost/v/nrcglossary/scheme> .

<https://w3id.org/permafrost/v/nrcglossary/t0086> a skos:Concept;
  dct:identifier "t0086"^^xsd:token;
  dct:source "https://nrc-publications.canada.ca/eng/view/object/?id=69fb8993-1baa-4225-b33a-6a02341d383d"^^xsd:anyURI,
    "https://nrc-publications.canada.ca/fra/voir/objet/?id=549123c3-092c-4fca-8dea-99d53eac06dd"^^xsd:anyURI;
  skos:definition "The major subdivision of a permafrost region in which permafrost occurs in some areas beneath the exposed land surface, whereas other areas are free of permafrost."@en;
  skos:inScheme <https://w3id.org/permafrost/v/nrcglossary/scheme>;
  skos:prefLabel "discontinuous permafrost zone"@en;
  skos:scopeNote "The zone of discontinuous permafrost lies between the continuous permafrost zone and the southern latitudinal limit of permafrost in lowlands. Near its northern boundary, discontinuous permafrost is extensive, whereas near its southern boundary it occurs as isolated patches of permafrost, and sporadic permafrost. There is no sharp distinction, or boundary, between the continuous and discontinuous permafrost zones."@en;
  skos:topConceptOf <https://w3id.org/permafrost/v/nrcglossary/scheme> .

<https://w3id.org/permafrost/v/nrcglossary/t0087> a skos:Concept;
  dct:identifier "t0087"^^xsd:token;
  dct:source "https://nrc-publications.canada.ca/eng/view/object/?id=69fb8993-1baa-4225-b33a-6a02341d383d"^^xsd:anyURI,
    "https://nrc-publications.canada.ca/fra/voir/objet/?id=549123c3-092c-4fca-8dea-99d53eac06dd"^^xsd:anyURI;
  skos:definition "Permafrost that is not in thermal equilibrium with the existing mean annual surface or sea-bottom temperature and the geothermal heat flux."@en;
  skos:inScheme <https://w3id.org/permafrost/v/nrcglossary/scheme>;
  skos:prefLabel "disequilibrium permafrost"@en;
  skos:topConceptOf <https://w3id.org/permafrost/v/nrcglossary/scheme> .

<https://w3id.org/permafrost/v/nrcglossary/t0088> a skos:Concept;
  dct:identifier "t0088"^^xsd:token;
  dct:source "https://nrc-publications.canada.ca/eng/view/object/?id=69fb8993-1baa-4225-b33a-6a02341d383d"^^xsd:anyURI,
    "https://nrc-publications.canada.ca/fra/voir/objet/?id=549123c3-092c-4fca-8dea-99d53eac06dd"^^xsd:anyURI;
  skos:definition "Trees leaning in random directions."@en;
  skos:inScheme <https://w3id.org/permafrost/v/nrcglossary/scheme>;
  skos:prefLabel "drunken forest"@en, "forêt ivre"@fr;
  skos:scopeNote "A descriptive term for trees usually growing on ice-rich terrain and subject to repeated differential frost heave or thermokarst subsidence. Active, forested rock glaciers may also exhibit this phenomenon due to differential movements."@en;
  skos:topConceptOf <https://w3id.org/permafrost/v/nrcglossary/scheme> .

<https://w3id.org/permafrost/v/nrcglossary/t0089> a skos:Concept;
  dct:identifier "t0089"^^xsd:token;
  dct:source "https://nrc-publications.canada.ca/eng/view/object/?id=69fb8993-1baa-4225-b33a-6a02341d383d"^^xsd:anyURI,
    "https://nrc-publications.canada.ca/fra/voir/objet/?id=549123c3-092c-4fca-8dea-99d53eac06dd"^^xsd:anyURI;
  skos:definition "The mass of a unit volume of dried material (e.g. soil)."@en;
  skos:inScheme <https://w3id.org/permafrost/v/nrcglossary/scheme>;
  skos:prefLabel "dry density"@en;
  skos:scopeNote "To determine the dry density of frozen ground, a measured volume of the material has to be thawed and then dried and weighed."@en;
  skos:topConceptOf <https://w3id.org/permafrost/v/nrcglossary/scheme> .

<https://w3id.org/permafrost/v/nrcglossary/t0090> a skos:Concept;
  dct:identifier "t0090"^^xsd:token;
  dct:source "https://nrc-publications.canada.ca/eng/view/object/?id=69fb8993-1baa-4225-b33a-6a02341d383d"^^xsd:anyURI,
    "https://nrc-publications.canada.ca/fra/voir/objet/?id=549123c3-092c-4fca-8dea-99d53eac06dd"^^xsd:anyURI;
  skos:definition "Frozen ground with a very low total water content consisting almost completely of interfacial water, and not cemented by ice."@en;
  skos:inScheme <https://w3id.org/permafrost/v/nrcglossary/scheme>;
  skos:prefLabel "dry frozen ground"@en;
  skos:scopeNote "The compressibility of dry frozen ground is the same as that of unfrozen ground of the same composition, total water content, and density."@en;
  skos:topConceptOf <https://w3id.org/permafrost/v/nrcglossary/scheme> .

<https://w3id.org/permafrost/v/nrcglossary/t0091> a skos:Concept;
  dct:identifier "t0091"^^xsd:token;
  dct:source "https://nrc-publications.canada.ca/eng/view/object/?id=69fb8993-1baa-4225-b33a-6a02341d383d"^^xsd:anyURI,
    "https://nrc-publications.canada.ca/fra/voir/objet/?id=549123c3-092c-4fca-8dea-99d53eac06dd"^^xsd:anyURI;
  skos:definition "Permafrost containing neither free water nor ice."@en;
  skos:inScheme <https://w3id.org/permafrost/v/nrcglossary/scheme>;
  skos:prefLabel "dry permafrost"@en;
  skos:scopeNote "A negligible quantity of moisture in the form of interfacial water may be present. Dry permafrost is thaw-stable."@en;
  skos:topConceptOf <https://w3id.org/permafrost/v/nrcglossary/scheme> .

<https://w3id.org/permafrost/v/nrcglossary/t0092> a skos:Concept;
  dct:identifier "t0092"^^xsd:token;
  dct:source "https://nrc-publications.canada.ca/eng/view/object/?id=69fb8993-1baa-4225-b33a-6a02341d383d"^^xsd:anyURI,
    "https://nrc-publications.canada.ca/fra/voir/objet/?id=549123c3-092c-4fca-8dea-99d53eac06dd"^^xsd:anyURI;
  skos:definition "The ratio of stress to strain for a material under dynamic loading conditions."@en;
  skos:inScheme <https://w3id.org/permafrost/v/nrcglossary/scheme>;
  skos:prefLabel "dynamic modulus of elasticity"@en;
  skos:topConceptOf <https://w3id.org/permafrost/v/nrcglossary/scheme> .

<https://w3id.org/permafrost/v/nrcglossary/t0093> a skos:Concept;
  dct:identifier "t0093"^^xsd:token;
  dct:source "https://nrc-publications.canada.ca/eng/view/object/?id=69fb8993-1baa-4225-b33a-6a02341d383d"^^xsd:anyURI,
    "https://nrc-publications.canada.ca/fra/voir/objet/?id=549123c3-092c-4fca-8dea-99d53eac06dd"^^xsd:anyURI;
  skos:definition "The absolute value of the ratio between the linear strain changes, perpendicular to and in the direction of a given uniaxial stress change, respectively, under dynamic loading conditions."@en;
  skos:inScheme <https://w3id.org/permafrost/v/nrcglossary/scheme>;
  skos:prefLabel "dynamic Poisson's ratio"@en;
  skos:topConceptOf <https://w3id.org/permafrost/v/nrcglossary/scheme> .

<https://w3id.org/permafrost/v/nrcglossary/t0094> a skos:Concept;
  dct:identifier "t0094"^^xsd:token;
  dct:source "https://nrc-publications.canada.ca/eng/view/object/?id=69fb8993-1baa-4225-b33a-6a02341d383d"^^xsd:anyURI,
    "https://nrc-publications.canada.ca/fra/voir/objet/?id=549123c3-092c-4fca-8dea-99d53eac06dd"^^xsd:anyURI;
  skos:altLabel "mud hummock"@en;
  skos:definition "A hummock having a core of silty and clayey mineral soil which may show evidence of cryoturbation (see Figure 20a, b)."@en;
  skos:hiddenLabel "earth mound"@en, "tundra hummock"@en;
  skos:inScheme <https://w3id.org/permafrost/v/nrcglossary/scheme>;
  skos:prefLabel "earth hummock"@en;
  skos:scopeNote "Earth hummocks are a type of nonsorted circle (see also patterned ground) commonly found in the zone of continuous permafrost. They develop in materials of a high silt and clay content and/or of high ice content. Earth hummocks found outside the southern limit of present-day permafrost are believed to have formed during a previous period of cooler climate when the area was underlain by permafrost."@en;
  skos:topConceptOf <https://w3id.org/permafrost/v/nrcglossary/scheme> .

<https://w3id.org/permafrost/v/nrcglossary/t0095> a skos:Concept;
  dct:identifier "t0095"^^xsd:token;
  dct:source "https://nrc-publications.canada.ca/eng/view/object/?id=69fb8993-1baa-4225-b33a-6a02341d383d"^^xsd:anyURI,
    "https://nrc-publications.canada.ca/fra/voir/objet/?id=549123c3-092c-4fca-8dea-99d53eac06dd"^^xsd:anyURI;
  skos:definition "The inverse of electrical resistivity."@en;
  skos:inScheme <https://w3id.org/permafrost/v/nrcglossary/scheme>;
  skos:prefLabel "electrical conductivity"@en;
  skos:scopeNote "The electrical conductivity of unfrozen soils decreases slightly with a decrease in temperature. A significant decrease in conductivity occurs when a soil freezes, but this change is directly related to the decreasing unfrozen water content of the frozen ground, and it may be affected by cryostructure. Available data show that the conductivities of frozen ground may be from 1 to more than 2 orders of magnitude smaller than those of the same material when unfrozen. The conductivity of frozen soils decreases further with further decreases in temperature."@en;
  skos:topConceptOf <https://w3id.org/permafrost/v/nrcglossary/scheme> .

<https://w3id.org/permafrost/v/nrcglossary/t0096> a skos:Concept;
  dct:identifier "t0096"^^xsd:token;
  dct:source "https://nrc-publications.canada.ca/eng/view/object/?id=69fb8993-1baa-4225-b33a-6a02341d383d"^^xsd:anyURI,
    "https://nrc-publications.canada.ca/fra/voir/objet/?id=549123c3-092c-4fca-8dea-99d53eac06dd"^^xsd:anyURI;
  skos:definition "The dielectric constant (or relative permittivity), electrical conductivity and electrical resistivity are the major electrical properties governing the flow of electric current through frozen ground."@en;
  skos:inScheme <https://w3id.org/permafrost/v/nrcglossary/scheme>;
  skos:prefLabel "electrical properties of frozen ground"@en, "propriétés électriques du gélisol"@fr;
  skos:scopeNote "The dielectric constant of a soil is a measure of the ability of the soil to store electrical energy in the presence of an electrostatic field; it is the ratio of the soil's permittivity to the permittivity of a vacuum. The electrical conductance of a soil is the inverse of the resistance offered by a soil to current flow. Current flow under an electrical gradient in a frozen soil occurs almost entirely through the unfrozen water films. Electrical conduction is related to the thickness of these water films and their degree of interconnection; it decreases with decreasing temperature and increases with increasing pressure. As a consequence, all these electrical properties are influenced by soil type, density, salinity, temperature and, in particular, the unfrozen water content. For example, the resistivity of unfrozen soils increases slightly with decrease in temperature. A significant increase in resistivity occurs when the soil freezes; this change is directly related to the decreasing unfrozen water content of the frozen ground. Available data show that the resistivities of frozen soils and rocks may be from 10 to more than 100 times larger than those of the same materials when unfrozen. Electromagnetic geophysical techniques for mapping permafrost, and the electrical grounding of various types of machines and electrical equipment, power transmission systems and radio transmitting antennae in permafrost areas, require a knowledge of the electrical properties of frozen ground."@en;
  skos:topConceptOf <https://w3id.org/permafrost/v/nrcglossary/scheme> .

<https://w3id.org/permafrost/v/nrcglossary/t0097> a skos:Concept;
  dct:identifier "t0097"^^xsd:token;
  dct:source "https://nrc-publications.canada.ca/eng/view/object/?id=69fb8993-1baa-4225-b33a-6a02341d383d"^^xsd:anyURI,
    "https://nrc-publications.canada.ca/fra/voir/objet/?id=549123c3-092c-4fca-8dea-99d53eac06dd"^^xsd:anyURI;
  skos:definition "The property of a material that determines the electrical current flowing through a centimetre cube of the material when an electrical potential is applied to opposite faces of the cube."@en;
  skos:inScheme <https://w3id.org/permafrost/v/nrcglossary/scheme>;
  skos:prefLabel "electrical resistivity"@en;
  skos:scopeNote "The electrical resistivity of unfrozen soils increases slightly with a decrease in temperature. A significant increase in resistivity occurs when a soil freezes, but this change is directly related to the decreasing unfrozen water content of the frozen ground, and it may be affected by cryostructure. Available data show that the resistivities of frozen ground may be from 10 to more than 100 times larger than those of the same material when unfrozen. The resistivity of frozen soils increases further with further decreases in temperature."@en;
  skos:topConceptOf <https://w3id.org/permafrost/v/nrcglossary/scheme> .

<https://w3id.org/permafrost/v/nrcglossary/t0098> a skos:Concept;
  dct:identifier "t0098"^^xsd:token;
  dct:source "https://nrc-publications.canada.ca/eng/view/object/?id=69fb8993-1baa-4225-b33a-6a02341d383d"^^xsd:anyURI,
    "https://nrc-publications.canada.ca/fra/voir/objet/?id=549123c3-092c-4fca-8dea-99d53eac06dd"^^xsd:anyURI;
  skos:definition "Ground ice developed in epigenetic permafrost, or in previously formed syngenetic permafrost ."@en;
  skos:inScheme <https://w3id.org/permafrost/v/nrcglossary/scheme>;
  skos:prefLabel "epigenetic ice"@en;
  skos:scopeNote "If epigenetic ice occurs in the form of ice lenses in which the volume of ice to soil is large, the more descriptive term segregated ice is preferred. Examples of epigenetic ice also include wedge ice and intrusive ice."@en;
  skos:topConceptOf <https://w3id.org/permafrost/v/nrcglossary/scheme> .

<https://w3id.org/permafrost/v/nrcglossary/t0099> a skos:Concept;
  dct:identifier "t0099"^^xsd:token;
  dct:source "https://nrc-publications.canada.ca/eng/view/object/?id=69fb8993-1baa-4225-b33a-6a02341d383d"^^xsd:anyURI,
    "https://nrc-publications.canada.ca/fra/voir/objet/?id=549123c3-092c-4fca-8dea-99d53eac06dd"^^xsd:anyURI;
  skos:definition "An ice wedge developed in epigenetic permafrost, or in previously formed syngenetic permafrost (see Figure 17i)."@en;
  skos:inScheme <https://w3id.org/permafrost/v/nrcglossary/scheme>;
  skos:prefLabel "epigenetic ice wedge"@en;
  skos:scopeNote "Epigenetic ice wedges grow progressively wider, rather than deeper, and are characteristically wedge-shaped. The ice of an epigenetic ice wedge is oldest on the outside edges."@en;
  skos:topConceptOf <https://w3id.org/permafrost/v/nrcglossary/scheme> .

<https://w3id.org/permafrost/v/nrcglossary/t0100> a skos:Concept;
  dct:identifier "t0100"^^xsd:token;
  dct:source "https://nrc-publications.canada.ca/eng/view/object/?id=69fb8993-1baa-4225-b33a-6a02341d383d"^^xsd:anyURI,
    "https://nrc-publications.canada.ca/fra/voir/objet/?id=549123c3-092c-4fca-8dea-99d53eac06dd"^^xsd:anyURI;
  skos:definition "Permafrost that formed through lowering of the permafrost base in previously deposited sediment or other earth material."@en;
  skos:inScheme <https://w3id.org/permafrost/v/nrcglossary/scheme>;
  skos:prefLabel "epigenetic permafrost"@en;
  skos:topConceptOf <https://w3id.org/permafrost/v/nrcglossary/scheme> .

<https://w3id.org/permafrost/v/nrcglossary/t0101> a skos:Concept;
  dct:identifier "t0101"^^xsd:token;
  dct:source "https://nrc-publications.canada.ca/eng/view/object/?id=69fb8993-1baa-4225-b33a-6a02341d383d"^^xsd:anyURI,
    "https://nrc-publications.canada.ca/fra/voir/objet/?id=549123c3-092c-4fca-8dea-99d53eac06dd"^^xsd:anyURI;
  skos:altLabel "contemporary permafrost"@en;
  skos:definition "Permafrost that is in thermal equilibrium with the existing mean annual surface or sea-bottom temperature and with the geothermal heat flux."@en;
  skos:inScheme <https://w3id.org/permafrost/v/nrcglossary/scheme>;
  skos:prefLabel "equilibrium permafrost"@en;
  skos:topConceptOf <https://w3id.org/permafrost/v/nrcglossary/scheme> .

<https://w3id.org/permafrost/v/nrcglossary/t0102> a skos:Concept;
  dct:identifier "t0102"^^xsd:token;
  dct:source "https://nrc-publications.canada.ca/eng/view/object/?id=69fb8993-1baa-4225-b33a-6a02341d383d"^^xsd:anyURI,
    "https://nrc-publications.canada.ca/fra/voir/objet/?id=549123c3-092c-4fca-8dea-99d53eac06dd"^^xsd:anyURI;
  skos:definition "The volume of ice in the ground which exceeds the total pore volume that the ground would have under natural unfrozen conditions (see Figure 7)."@en;
  skos:inScheme <https://w3id.org/permafrost/v/nrcglossary/scheme>;
  skos:prefLabel "excess ice"@en;
  skos:scopeNote "In standard geotechnical terminology, a soil is considered normally consolidated when its total pore volume or its total water content is in equilibrium with the acting gravity stresses. Due to the presence of ground ice, the total water content of a frozen soil may exceed that corresponding to its normally consolidated state when unfrozen. As a result, upon thawing, a soil containing excess ice will settle under its own weight until it attains its consolidated state."@en;
  skos:topConceptOf <https://w3id.org/permafrost/v/nrcglossary/scheme> .

<https://w3id.org/permafrost/v/nrcglossary/t0103> a skos:Concept;
  dct:identifier "t0103"^^xsd:token;
  dct:source "https://nrc-publications.canada.ca/eng/view/object/?id=69fb8993-1baa-4225-b33a-6a02341d383d"^^xsd:anyURI,
    "https://nrc-publications.canada.ca/fra/voir/objet/?id=549123c3-092c-4fca-8dea-99d53eac06dd"^^xsd:anyURI;
  skos:altLabel "widespread discontinuous permafrost"@en;
  skos:definition "1. (North-American usage) Permafrost underlying 65 to 90 percent of the area of exposed land surface. 2. (Russian usage) Permafrost underlying 70 to 80 percent of the area of exposed land surface."@en;
  skos:inScheme <https://w3id.org/permafrost/v/nrcglossary/scheme>;
  skos:prefLabel "extensive discontinuous permafrost"@en;
  skos:scopeNote "It is suggested that this term be used as a replacement for \"widespread\" discontinuous permafrost, because the word \"widespread\" can mean either \"extensively distributed\" or \"widely spaced\"."@en;
  skos:topConceptOf <https://w3id.org/permafrost/v/nrcglossary/scheme> .

<https://w3id.org/permafrost/v/nrcglossary/t0104> a skos:Concept;
  dct:identifier "t0104"^^xsd:token;
  dct:source "https://nrc-publications.canada.ca/eng/view/object/?id=69fb8993-1baa-4225-b33a-6a02341d383d"^^xsd:anyURI,
    "https://nrc-publications.canada.ca/fra/voir/objet/?id=549123c3-092c-4fca-8dea-99d53eac06dd"^^xsd:anyURI;
  skos:definition "Soil micromorphology."@en;
  skos:inScheme <https://w3id.org/permafrost/v/nrcglossary/scheme>;
  skos:prefLabel "fabric"@en;
  skos:topConceptOf <https://w3id.org/permafrost/v/nrcglossary/scheme> .

<https://w3id.org/permafrost/v/nrcglossary/t0105> a skos:Concept;
  dct:identifier "t0105"^^xsd:token;
  dct:source "https://nrc-publications.canada.ca/eng/view/object/?id=69fb8993-1baa-4225-b33a-6a02341d383d"^^xsd:anyURI,
    "https://nrc-publications.canada.ca/fra/voir/objet/?id=549123c3-092c-4fca-8dea-99d53eac06dd"^^xsd:anyURI;
  skos:definition "A distinct soil micromorphology, resulting from the effects of freezing and thawing processes, in which soil particles form discrete units that are densely packed."@en;
  skos:inScheme <https://w3id.org/permafrost/v/nrcglossary/scheme>;
  skos:prefLabel "fragmic cryogenic fabric"@en;
  skos:scopeNote "This fabric, found in cryosols, commonly occurs in soil horizons close to the"@en;
  skos:topConceptOf <https://w3id.org/permafrost/v/nrcglossary/scheme> .

<https://w3id.org/permafrost/v/nrcglossary/t0106> a skos:Concept;
  dct:identifier "t0106"^^xsd:token;
  dct:source "https://nrc-publications.canada.ca/eng/view/object/?id=69fb8993-1baa-4225-b33a-6a02341d383d"^^xsd:anyURI,
    "https://nrc-publications.canada.ca/fra/voir/objet/?id=549123c3-092c-4fca-8dea-99d53eac06dd"^^xsd:anyURI;
  skos:definition "A distinct soil micromorphology, resulting from the effects of freezing and thawing processes, in which soil particles form discrete units that are coalescing (see Figure 8b)."@en;
  skos:inScheme <https://w3id.org/permafrost/v/nrcglossary/scheme>;
  skos:prefLabel "fragmoidal cryogenic fabric"@en;
  skos:scopeNote "This fabric, found in cryosols, commonly occurs in soil horizons close to the freezing front, where soil material is subject to ice lense formation."@en;
  skos:topConceptOf <https://w3id.org/permafrost/v/nrcglossary/scheme> .

<https://w3id.org/permafrost/v/nrcglossary/t0107> a skos:Concept;
  dct:identifier "t0107"^^xsd:token;
  dct:source "https://nrc-publications.canada.ca/eng/view/object/?id=69fb8993-1baa-4225-b33a-6a02341d383d"^^xsd:anyURI,
    "https://nrc-publications.canada.ca/fra/voir/objet/?id=549123c3-092c-4fca-8dea-99d53eac06dd"^^xsd:anyURI;
  skos:definition "Free water is that portion of the pore water that is free to move between interconnected pores under the influence of gravity."@en;
  skos:inScheme <https://w3id.org/permafrost/v/nrcglossary/scheme>;
  skos:prefLabel "free water"@en;
  skos:scopeNote "The term free water also covers water in fissures, solution channels, and other openings in soils or rocks. The temperature at which free water will change phase depends primarily on its dissolved-solids content, which determines the freezing- point depression."@en;
  skos:topConceptOf <https://w3id.org/permafrost/v/nrcglossary/scheme> .

<https://w3id.org/permafrost/v/nrcglossary/t0108> a skos:Concept;
  dct:identifier "t0108"^^xsd:token;
  dct:source "https://nrc-publications.canada.ca/eng/view/object/?id=69fb8993-1baa-4225-b33a-6a02341d383d"^^xsd:anyURI,
    "https://nrc-publications.canada.ca/fra/voir/objet/?id=549123c3-092c-4fca-8dea-99d53eac06dd"^^xsd:anyURI;
  skos:definition "Freezing of a material followed by thawing."@en;
  skos:inScheme <https://w3id.org/permafrost/v/nrcglossary/scheme>;
  skos:prefLabel "freeze-thaw cycle"@en;
  skos:scopeNote "Natural freeze-thaw cycles consist of the freezing and subsequent thawing during a freezing season and the following thawing season. In laboratory experiments and geotechnical testing, freeze-thaw cycles are usually much shorter (several days to a few months)."@en;
  skos:topConceptOf <https://w3id.org/permafrost/v/nrcglossary/scheme> .

<https://w3id.org/permafrost/v/nrcglossary/t0109> a skos:Concept;
  dct:identifier "t0109"^^xsd:token;
  dct:source "https://nrc-publications.canada.ca/eng/view/object/?id=69fb8993-1baa-4225-b33a-6a02341d383d"^^xsd:anyURI,
    "https://nrc-publications.canada.ca/fra/voir/objet/?id=549123c3-092c-4fca-8dea-99d53eac06dd"^^xsd:anyURI;
  skos:definition "Refreezing of thawed materials."@en;
  skos:inScheme <https://w3id.org/permafrost/v/nrcglossary/scheme>;
  skos:prefLabel "freezeback"@en, "regel"@fr;
  skos:scopeNote "This term is used to describe: 1. seasonal refreezing of the thawed active layer (see Figure 4), or 2. refreezing of soil thawed as a result of construction activity or drilling of a well in permafrost, and of soil placed as backfill or a slurry around foundations or engineering facilities buried or embedded in frozen ground, e.g., pipelines, piles or shallow foundations in permafrost."@en;
  skos:topConceptOf <https://w3id.org/permafrost/v/nrcglossary/scheme> .

<https://w3id.org/permafrost/v/nrcglossary/t0110> a skos:Concept;
  dct:identifier "t0110"^^xsd:token;
  dct:source "https://nrc-publications.canada.ca/eng/view/object/?id=69fb8993-1baa-4225-b33a-6a02341d383d"^^xsd:anyURI,
    "https://nrc-publications.canada.ca/fra/voir/objet/?id=549123c3-092c-4fca-8dea-99d53eac06dd"^^xsd:anyURI;
  skos:definition "The changing of phase from water to ice in soil or rock."@en;
  skos:inScheme <https://w3id.org/permafrost/v/nrcglossary/scheme>;
  skos:prefLabel "engel"@fr, "freezing (of ground)"@en;
  skos:scopeNote "The temperature at which ground freezing starts may be lower than 0°C as a result of freezing-point depression."@en;
  skos:topConceptOf <https://w3id.org/permafrost/v/nrcglossary/scheme> .

<https://w3id.org/permafrost/v/nrcglossary/t0111> a skos:Concept;
  dct:identifier "t0111"^^xsd:token;
  dct:source "https://nrc-publications.canada.ca/eng/view/object/?id=69fb8993-1baa-4225-b33a-6a02341d383d"^^xsd:anyURI,
    "https://nrc-publications.canada.ca/fra/voir/objet/?id=549123c3-092c-4fca-8dea-99d53eac06dd"^^xsd:anyURI;
  skos:definition "The advancing boundary between frozen (or partially frozen) ground and unfrozen ground (see Figures 4 and 5)."@en;
  skos:hiddenLabel "freezing plane"@en, "frost front"@en;
  skos:inScheme <https://w3id.org/permafrost/v/nrcglossary/scheme>;
  skos:prefLabel "freezing front"@en, "front de gel"@fr;
  skos:scopeNote "In the usual case, where the active layer extends to the permafrost table, two freezing fronts will be present during annual freezing of the ground, one moving downward from the ground surface, the other moving upward from the permafrost table. The freezing front may not coincide with the 0°C isotherm (cryofront)."@en;
  skos:topConceptOf <https://w3id.org/permafrost/v/nrcglossary/scheme> .

<https://w3id.org/permafrost/v/nrcglossary/t0112> a skos:Concept;
  dct:identifier "t0112"^^xsd:token;
  dct:source "https://nrc-publications.canada.ca/eng/view/object/?id=69fb8993-1baa-4225-b33a-6a02341d383d"^^xsd:anyURI,
    "https://nrc-publications.canada.ca/fra/voir/objet/?id=549123c3-092c-4fca-8dea-99d53eac06dd"^^xsd:anyURI;
  skos:definition "The cumulative number of degree-days below 0°C for a given time period."@en;
  skos:inScheme <https://w3id.org/permafrost/v/nrcglossary/scheme>;
  skos:prefLabel "freezing index"@en, "indice de gel"@fr;
  skos:scopeNote "Four main types of air freezing indices have been used: 1. approximate freezing index - calculated from the mean monthly air temperatures for a specific station without making corrections for positive degree-days (T > 0°C) in spring and fall (Boyd, 1973, 1979); 2. total annual freezing index - calculated by adding all the negative mean daily air temperatures (°C) for a specific station during a calendar year (Harris, 1981); 3. seasonal freezing index - calculated as the arithmetic sum of all the negative and positive mean daily air temperatures (°C) for a specific station during the time period between the highest point in the fall and the lowest point the next spring on the cumulative degree-day time curve (Huschke, 1959); 4. design freezing index - calculated by taking the average of the seasonal freezing indices for the three coldest winters in the most recent 30 years of record. If data for 30 years are not available, then the index is based on the coldest winter in the latest 10-year period of record (U.S. Army/Air Force, 1966). The total annual freezing index has been used to predict permafrost distribution, and the design freezing index is commonly used in engineering to estimate the maximum thickness of lake ice and the maximum depth of frost penetration in the ground. A surface (ground, pavement, etc.) freezing index differs from the air freezing index (see n-factor)."@en;
  skos:topConceptOf <https://w3id.org/permafrost/v/nrcglossary/scheme> .

<https://w3id.org/permafrost/v/nrcglossary/t0113> a skos:Concept;
  dct:identifier "t0113"^^xsd:token;
  dct:source "https://nrc-publications.canada.ca/eng/view/object/?id=69fb8993-1baa-4225-b33a-6a02341d383d"^^xsd:anyURI,
    "https://nrc-publications.canada.ca/fra/voir/objet/?id=549123c3-092c-4fca-8dea-99d53eac06dd"^^xsd:anyURI;
  skos:definition "1. The temperature at which a pure liquid solidifies under atmospheric pressure. 2. The temperature at which a ground material starts to freeze."@en;
  skos:inScheme <https://w3id.org/permafrost/v/nrcglossary/scheme>;
  skos:prefLabel "freezing point"@en;
  skos:scopeNote "See also freezing-point depression."@en;
  skos:topConceptOf <https://w3id.org/permafrost/v/nrcglossary/scheme> .

<https://w3id.org/permafrost/v/nrcglossary/t0114> a skos:Concept;
  dct:identifier "t0114"^^xsd:token;
  dct:source "https://nrc-publications.canada.ca/eng/view/object/?id=69fb8993-1baa-4225-b33a-6a02341d383d"^^xsd:anyURI,
    "https://nrc-publications.canada.ca/fra/voir/objet/?id=549123c3-092c-4fca-8dea-99d53eac06dd"^^xsd:anyURI;
  skos:definition "The number of degrees by which the freezing point of an earth material is depressed below 0°C (see Figures 2 and 3)."@en;
  skos:inScheme <https://w3id.org/permafrost/v/nrcglossary/scheme>;
  skos:prefLabel "abaissement du point de congélation"@fr, "freezing-point depression"@en;
  skos:scopeNote "The highest temperature at which soil, water, ice and air can coexist at equilibrium. In soils, the freezing-point depression is due mainly to capillarity and surface adsorption. It depends on soil particle effects (curvature and nature of soil particle surfaces), pressure, and the effects of dissolved solids in the pore water. The freezing-point depression can often be determined from the ground temperature profile where it is the difference between the temperature at the base of the ice-bearing permafrost and 0°C."@en;
  skos:topConceptOf <https://w3id.org/permafrost/v/nrcglossary/scheme> .

<https://w3id.org/permafrost/v/nrcglossary/t0115> a skos:Concept;
  dct:identifier "t0115"^^xsd:token;
  dct:source "https://nrc-publications.canada.ca/eng/view/object/?id=69fb8993-1baa-4225-b33a-6a02341d383d"^^xsd:anyURI,
    "https://nrc-publications.canada.ca/fra/voir/objet/?id=549123c3-092c-4fca-8dea-99d53eac06dd"^^xsd:anyURI;
  skos:definition "The positive pressure developed at ice-water interfaces in a soil as it freezes."@en;
  skos:inScheme <https://w3id.org/permafrost/v/nrcglossary/scheme>;
  skos:prefLabel "freezing pressure"@en, "pression de gel"@fr;
  skos:scopeNote "It is also known to result in a heaving pressure or frost-heave pressure that is responsible for the heaving of utilities, foundations and pavements. Ice-water interfaces occur at the contact between ice lenses and the frozen fringe."@en;
  skos:topConceptOf <https://w3id.org/permafrost/v/nrcglossary/scheme> .

<https://w3id.org/permafrost/v/nrcglossary/t0116> a skos:Concept;
  dct:identifier "t0116"^^xsd:token;
  dct:source "https://nrc-publications.canada.ca/eng/view/object/?id=69fb8993-1baa-4225-b33a-6a02341d383d"^^xsd:anyURI,
    "https://nrc-publications.canada.ca/fra/voir/objet/?id=549123c3-092c-4fca-8dea-99d53eac06dd"^^xsd:anyURI;
  skos:definition "Permafrost in which the soil particles are not held together by ice."@en;
  skos:inScheme <https://w3id.org/permafrost/v/nrcglossary/scheme>;
  skos:prefLabel "friable permafrost"@en;
  skos:topConceptOf <https://w3id.org/permafrost/v/nrcglossary/scheme> .

<https://w3id.org/permafrost/v/nrcglossary/t0117> a skos:Concept;
  dct:identifier "t0117"^^xsd:token;
  dct:source "https://nrc-publications.canada.ca/eng/view/object/?id=69fb8993-1baa-4225-b33a-6a02341d383d"^^xsd:anyURI,
    "https://nrc-publications.canada.ca/fra/voir/objet/?id=549123c3-092c-4fca-8dea-99d53eac06dd"^^xsd:anyURI;
  skos:definition "The occurrence of air temperatures below 0°C."@en;
  skos:inScheme <https://w3id.org/permafrost/v/nrcglossary/scheme>;
  skos:prefLabel "frost"@en;
  skos:scopeNote "An alternative definition states that \"frost is the condition existing when the surface temperature falls below freezing (0°C)\". In British usage, \"ground frost\" is recorded when a minimum thermometer just above a grass surface reads less than 30.4?F."@en;
  skos:topConceptOf <https://w3id.org/permafrost/v/nrcglossary/scheme> .

<https://w3id.org/permafrost/v/nrcglossary/t0118> a skos:Concept;
  dct:identifier "t0118"^^xsd:token;
  dct:source "https://nrc-publications.canada.ca/eng/view/object/?id=69fb8993-1baa-4225-b33a-6a02341d383d"^^xsd:anyURI,
    "https://nrc-publications.canada.ca/fra/voir/objet/?id=549123c3-092c-4fca-8dea-99d53eac06dd"^^xsd:anyURI;
  skos:definition "The process of alternate freezing and thawing of moisture in soil, rock and other materials, and the resulting effects on materials and on structures placed on, or in, the ground."@en;
  skos:inScheme <https://w3id.org/permafrost/v/nrcglossary/scheme>;
  skos:prefLabel "frost action"@en, "gélivation"@fr;
  skos:scopeNote "Frost action in soils describes the detrimental processes of frost heave that occurs in the ground during the freezing period, and thaw weakening (followed by thaw settlement) that occurs as the seasonally frozen ground thaws. Although it normally refers to seasonal freezing and thawing processes and effects, the term \"frost action\" has also been used to describe the long-term heaving that occurs when soils are subjected continuously to a freezing temperature over a long period of time (years), e.g., under cold storage plants and buried chilled pipelines. Frost action contributes to the mechanical weathering (i.e., disintegration or breakdown) of soil and rock materials, by frost wedging, cryoturbation activity, and to the development of cryotexture and cryogenic fabric in soils."@en;
  skos:topConceptOf <https://w3id.org/permafrost/v/nrcglossary/scheme> .

<https://w3id.org/permafrost/v/nrcglossary/t0119> a skos:Concept;
  dct:identifier "t0119"^^xsd:token;
  dct:source "https://nrc-publications.canada.ca/eng/view/object/?id=69fb8993-1baa-4225-b33a-6a02341d383d"^^xsd:anyURI,
    "https://nrc-publications.canada.ca/fra/voir/objet/?id=549123c3-092c-4fca-8dea-99d53eac06dd"^^xsd:anyURI;
  skos:definition "A seasonal frost mound produced through doming of seasonally frozen ground by a subsurface accumulation of water under elevated hydraulic potential during progressive freezing of the active layer (see Figures 12 and 13)."@en;
  skos:hiddenLabel "cryolaccolith"@en, "hydrolaccolith"@en, "seasonal pingo"@en, "winter pingo"@en;
  skos:inScheme <https://w3id.org/permafrost/v/nrcglossary/scheme>;
  skos:prefLabel "butte saisonnière à noyau de glace"@fr, "frost blister"@en;
  skos:scopeNote "Freezing of the accumulated subsurface water produces a domed layer of clear ice beneath the overlying frozen ground. Frost blisters are formed in a single winter; their decay may take more than a year. They are distinguished from icing blisters by the layer of seasonally frozen ground overlying the ice layer."@en;
  skos:topConceptOf <https://w3id.org/permafrost/v/nrcglossary/scheme> .

<https://w3id.org/permafrost/v/nrcglossary/t0120> a skos:Concept;
  dct:identifier "t0120"^^xsd:token;
  dct:source "https://nrc-publications.canada.ca/eng/view/object/?id=69fb8993-1baa-4225-b33a-6a02341d383d"^^xsd:anyURI,
    "https://nrc-publications.canada.ca/fra/voir/objet/?id=549123c3-092c-4fca-8dea-99d53eac06dd"^^xsd:anyURI;
  skos:altLabel "mud boil"@en;
  skos:definition "A small mound of soil material, presumed to have been formed by frost action (see Figure 16c, d)."@en;
  skos:inScheme <https://w3id.org/permafrost/v/nrcglossary/scheme>;
  skos:prefLabel "frost boil"@en;
  skos:scopeNote "A type of nonsorted circle; they are commonly found in fine-grained sediments underlain by permafrost, but also occur in non-permafrost areas. ."@en;
  skos:topConceptOf <https://w3id.org/permafrost/v/nrcglossary/scheme> .

<https://w3id.org/permafrost/v/nrcglossary/t0121> a skos:Concept;
  dct:identifier "t0121"^^xsd:token;
  dct:source "https://nrc-publications.canada.ca/eng/view/object/?id=69fb8993-1baa-4225-b33a-6a02341d383d"^^xsd:anyURI,
    "https://nrc-publications.canada.ca/fra/voir/objet/?id=549123c3-092c-4fca-8dea-99d53eac06dd"^^xsd:anyURI;
  skos:definition "A more or less symmetrical zone of frozen ground formed around a buried chilled pipeline or beneath or around a structure maintained at temperatures below 0°C (see Figure 23)."@en;
  skos:inScheme <https://w3id.org/permafrost/v/nrcglossary/scheme>;
  skos:prefLabel "bulbe de gel"@fr, "frost bulb"@en;
  skos:scopeNote "Heaving of the ground and/or of a structure or facility may occur as the frost bulb forms."@en;
  skos:topConceptOf <https://w3id.org/permafrost/v/nrcglossary/scheme> .

<https://w3id.org/permafrost/v/nrcglossary/t0122> a skos:Concept;
  dct:identifier "t0122"^^xsd:token;
  dct:source "https://nrc-publications.canada.ca/eng/view/object/?id=69fb8993-1baa-4225-b33a-6a02341d383d"^^xsd:anyURI,
    "https://nrc-publications.canada.ca/fra/voir/objet/?id=549123c3-092c-4fca-8dea-99d53eac06dd"^^xsd:anyURI;
  skos:definition "The net downslope displacement that occurs when a soil, during a freeze- thaw cycle, expands normal to the ground surface and settles in a nearly vertical direction."@en;
  skos:inScheme <https://w3id.org/permafrost/v/nrcglossary/scheme>;
  skos:prefLabel "frost creep"@en, "reptation due au gel"@fr;
  skos:topConceptOf <https://w3id.org/permafrost/v/nrcglossary/scheme> .

<https://w3id.org/permafrost/v/nrcglossary/t0123> a skos:Concept;
  dct:identifier "t0123"^^xsd:token;
  dct:source "https://nrc-publications.canada.ca/eng/view/object/?id=69fb8993-1baa-4225-b33a-6a02341d383d"^^xsd:anyURI,
    "https://nrc-publications.canada.ca/fra/voir/objet/?id=549123c3-092c-4fca-8dea-99d53eac06dd"^^xsd:anyURI;
  skos:definition "The upward or outward movement of the ground surface (or objects on, or in, the ground) caused by the formation of ice in the soil (see Figure 7)."@en;
  skos:inScheme <https://w3id.org/permafrost/v/nrcglossary/scheme>;
  skos:prefLabel "frost heave"@en, "soulèvement dû au gel"@fr;
  skos:scopeNote "Frost action in fine-grained soils increases the volume of the soil not only by freezing of in situ pore water (? 9% expansion) but also by drawing water to the freezing front where ice lenses form. Soils that have undergone substantial heaving may consist of alternate layers of ice-saturated soil and relatively clear ice lenses. The lenses are formed normal to the direction of heat flow and when freezing penetrates from the ground surface (which may be horizontal, sloping or vertical), they form parallel to that surface. When unrestrained, the amount of surface heave may be almost as much as the total thickness of the ice lenses. Frost heave can occur seasonally or continuously if freezing of the ground proceeds without interruption over a period of years. Differential, or non-uniform, frost heaving is one of the main detrimental aspects of the frost action process and reflects the heterogeneous nature of most soils, or variations in heat removal rate and groundwater supply over short distances. Depending on the degree of restraint, large freezing pressures (up to 1 MPa) can be developed as the ground freezes. These can be transmitted to a foundation, structure or other object placed on the ground surface, or embedded or buried in the ground, as basal (i.e., vertical) forces acting on their underside, or through adfreezing of the soil to the sides of the foundation, structure or object."@en;
  skos:topConceptOf <https://w3id.org/permafrost/v/nrcglossary/scheme> .

<https://w3id.org/permafrost/v/nrcglossary/t0124> a skos:Concept;
  dct:identifier "t0124"^^xsd:token;
  dct:source "https://nrc-publications.canada.ca/eng/view/object/?id=69fb8993-1baa-4225-b33a-6a02341d383d"^^xsd:anyURI,
    "https://nrc-publications.canada.ca/fra/voir/objet/?id=549123c3-092c-4fca-8dea-99d53eac06dd"^^xsd:anyURI;
  skos:definition "The difference between the elevations of the ground surface before and after the occurrence of frost heave."@en;
  skos:inScheme <https://w3id.org/permafrost/v/nrcglossary/scheme>;
  skos:prefLabel "frost-heave extent"@en;
  skos:topConceptOf <https://w3id.org/permafrost/v/nrcglossary/scheme> .

<https://w3id.org/permafrost/v/nrcglossary/t0125> a skos:Concept;
  dct:identifier "t0125"^^xsd:token;
  dct:source "https://nrc-publications.canada.ca/eng/view/object/?id=69fb8993-1baa-4225-b33a-6a02341d383d"^^xsd:anyURI,
    "https://nrc-publications.canada.ca/fra/voir/objet/?id=549123c3-092c-4fca-8dea-99d53eac06dd"^^xsd:anyURI;
  skos:definition "Cumulative upward displacement of objects embedded in the ground, caused by frost action."@en;
  skos:hiddenLabel "upfreezing"@en;
  skos:inScheme <https://w3id.org/permafrost/v/nrcglossary/scheme>;
  skos:prefLabel "frost jacking"@en, "éjection gélivale"@fr;
  skos:scopeNote "Frost jacking results from basal or vertical freezing pressures acting on the underside of a foundation, structure or object, or from adfreezing of soil to the sides of these objects. The cumulative upward movement over a period of time (one or several freeze-thaw cycles) may result in the foundation unit or object being ejected from the ground. Fence posts and utility poles or towers are commonly affected, and both deep (pile) and shallow (post) foundations (e.g., used for bridges, wharves, unheated or lightweight buildings) have been seriously affected by frost jacking. Blocks of jointed or fractured bedrock have also been displaced upward by frost jacking."@en;
  skos:topConceptOf <https://w3id.org/permafrost/v/nrcglossary/scheme> .

<https://w3id.org/permafrost/v/nrcglossary/t0126> a skos:Concept;
  dct:identifier "t0126"^^xsd:token;
  dct:source "https://nrc-publications.canada.ca/eng/view/object/?id=69fb8993-1baa-4225-b33a-6a02341d383d"^^xsd:anyURI,
    "https://nrc-publications.canada.ca/fra/voir/objet/?id=549123c3-092c-4fca-8dea-99d53eac06dd"^^xsd:anyURI;
  skos:definition "Any mound-shaped landform produced by ground freezing combined with accumulation of ground ice due to groundwater movement or the migration of soil moisture."@en;
  skos:hiddenLabel "bugor"@en, "bulgunniakh"@en, "cryogenic mound"@en, "earth mound"@en,
    "frost hummock"@en, "ground-ice mound"@en, "tundra hummock"@en;
  skos:inScheme <https://w3id.org/permafrost/v/nrcglossary/scheme>;
  skos:prefLabel "butte cryogène"@fr, "frost mound"@en;
  skos:scopeNote "Various types of frost mounds, (e.g., frost blisters, icing blisters, palsas and pingos) can be distinguished on the basis of their structure and duration, and the character of the ice contained in them."@en;
  skos:topConceptOf <https://w3id.org/permafrost/v/nrcglossary/scheme> .

<https://w3id.org/permafrost/v/nrcglossary/t0127> a skos:Concept;
  dct:identifier "t0127"^^xsd:token;
  dct:source "https://nrc-publications.canada.ca/eng/view/object/?id=69fb8993-1baa-4225-b33a-6a02341d383d"^^xsd:anyURI,
    "https://nrc-publications.canada.ca/fra/voir/objet/?id=549123c3-092c-4fca-8dea-99d53eac06dd"^^xsd:anyURI;
  skos:definition "The movement of the freezing front into the ground during freezing."@en;
  skos:inScheme <https://w3id.org/permafrost/v/nrcglossary/scheme>;
  skos:prefLabel "frost penetration"@en, "pénétration du gel"@fr;
  skos:topConceptOf <https://w3id.org/permafrost/v/nrcglossary/scheme> .

<https://w3id.org/permafrost/v/nrcglossary/t0128> a skos:Concept;
  dct:identifier "t0128"^^xsd:token;
  dct:source "https://nrc-publications.canada.ca/eng/view/object/?id=69fb8993-1baa-4225-b33a-6a02341d383d"^^xsd:anyURI,
    "https://nrc-publications.canada.ca/fra/voir/objet/?id=549123c3-092c-4fca-8dea-99d53eac06dd"^^xsd:anyURI;
  skos:definition "Effects on earth materials and on structures placed in or on the ground, resulting from frost action."@en;
  skos:inScheme <https://w3id.org/permafrost/v/nrcglossary/scheme>;
  skos:prefLabel "frost phenomena"@en;
  skos:topConceptOf <https://w3id.org/permafrost/v/nrcglossary/scheme> .

<https://w3id.org/permafrost/v/nrcglossary/t0129> a skos:Concept;
  dct:identifier "t0129"^^xsd:token;
  dct:source "https://nrc-publications.canada.ca/eng/view/object/?id=69fb8993-1baa-4225-b33a-6a02341d383d"^^xsd:anyURI,
    "https://nrc-publications.canada.ca/fra/voir/objet/?id=549123c3-092c-4fca-8dea-99d53eac06dd"^^xsd:anyURI;
  skos:definition "The mechanical disintegration of rock by the pressure of the freezing of water in pores and along grain boundaries."@en;
  skos:inScheme <https://w3id.org/permafrost/v/nrcglossary/scheme>;
  skos:prefLabel "frost shattering"@en;
  skos:scopeNote "Frost shattering is the process of grain loosening and rock disintegration by the freezing pressure of water in films of varying thickness on the surfaces of individual mineral grains. Freezing of the water drawn between the grains by various particle surface forces exerts sufficient differential pressure to loosen and separate the grains."@en;
  skos:topConceptOf <https://w3id.org/permafrost/v/nrcglossary/scheme> .

<https://w3id.org/permafrost/v/nrcglossary/t0130> a skos:Concept;
  dct:identifier "t0130"^^xsd:token;
  dct:source "https://nrc-publications.canada.ca/eng/view/object/?id=69fb8993-1baa-4225-b33a-6a02341d383d"^^xsd:anyURI,
    "https://nrc-publications.canada.ca/fra/voir/objet/?id=549123c3-092c-4fca-8dea-99d53eac06dd"^^xsd:anyURI;
  skos:definition "The differential movement of soil particles of different size ranges as a result of frost action."@en;
  skos:inScheme <https://w3id.org/permafrost/v/nrcglossary/scheme>;
  skos:prefLabel "frost sorting"@en, "triage gélival"@fr;
  skos:scopeNote "Frost sorting often accompanies cryoturbation."@en;
  skos:topConceptOf <https://w3id.org/permafrost/v/nrcglossary/scheme> .

<https://w3id.org/permafrost/v/nrcglossary/t0131> a skos:Concept;
  dct:identifier "t0131"^^xsd:token;
  dct:source "https://nrc-publications.canada.ca/eng/view/object/?id=69fb8993-1baa-4225-b33a-6a02341d383d"^^xsd:anyURI,
    "https://nrc-publications.canada.ca/fra/voir/objet/?id=549123c3-092c-4fca-8dea-99d53eac06dd"^^xsd:anyURI;
  skos:definition "Ground (soil or rock) in which little or no segregated ice forms during seasonal freezing."@en;
  skos:hiddenLabel "non-frost-susceptible ground"@en;
  skos:inScheme <https://w3id.org/permafrost/v/nrcglossary/scheme>;
  skos:prefLabel "frost-stable ground"@en, "sol non gélif"@fr;
  skos:scopeNote "Significant cumulative ice segregation and frost heave may occur even in seasonally frost-stable ground (e.g., gravels and rock) under conditions of continuous freezing and plentiful water supply."@en;
  skos:topConceptOf <https://w3id.org/permafrost/v/nrcglossary/scheme> .

<https://w3id.org/permafrost/v/nrcglossary/t0132> a skos:Concept;
  dct:identifier "t0132"^^xsd:token;
  dct:source "https://nrc-publications.canada.ca/eng/view/object/?id=69fb8993-1baa-4225-b33a-6a02341d383d"^^xsd:anyURI,
    "https://nrc-publications.canada.ca/fra/voir/objet/?id=549123c3-092c-4fca-8dea-99d53eac06dd"^^xsd:anyURI;
  skos:definition "Soil in which little or no segregated ice forms during seasonal freezing."@en;
  skos:hiddenLabel "non-frost-susceptible soil"@en;
  skos:inScheme <https://w3id.org/permafrost/v/nrcglossary/scheme>;
  skos:prefLabel "frost-stable soil"@en;
  skos:topConceptOf <https://w3id.org/permafrost/v/nrcglossary/scheme> .

<https://w3id.org/permafrost/v/nrcglossary/t0133> a skos:Concept;
  dct:identifier "t0133"^^xsd:token;
  dct:source "https://nrc-publications.canada.ca/eng/view/object/?id=69fb8993-1baa-4225-b33a-6a02341d383d"^^xsd:anyURI,
    "https://nrc-publications.canada.ca/fra/voir/objet/?id=549123c3-092c-4fca-8dea-99d53eac06dd"^^xsd:anyURI;
  skos:definition "Ground (soil or rock) in which segregated ice will form (causing frost heave) under the required conditions of moisture supply and temperature."@en;
  skos:hiddenLabel "frost-sensitive ground"@en;
  skos:inScheme <https://w3id.org/permafrost/v/nrcglossary/scheme>;
  skos:prefLabel "frost-susceptible ground"@en, "sol gélif"@fr;
  skos:scopeNote "Frost-susceptible ground will eventually become ice-rich, regardless of its initial total water content, if the appropriate moisture supply and temperature conditions persist. By implication, frost-susceptible ground may also be susceptible to thaw weakening effects when it thaws."@en;
  skos:topConceptOf <https://w3id.org/permafrost/v/nrcglossary/scheme> .

<https://w3id.org/permafrost/v/nrcglossary/t0134> a skos:Concept;
  dct:identifier "t0134"^^xsd:token;
  dct:source "https://nrc-publications.canada.ca/eng/view/object/?id=69fb8993-1baa-4225-b33a-6a02341d383d"^^xsd:anyURI,
    "https://nrc-publications.canada.ca/fra/voir/objet/?id=549123c3-092c-4fca-8dea-99d53eac06dd"^^xsd:anyURI;
  skos:definition "Soil in which segregated ice will form (causing frost heave) under the required conditions of moisture supply and temperature."@en;
  skos:hiddenLabel "frost-sensitive soil"@en;
  skos:inScheme <https://w3id.org/permafrost/v/nrcglossary/scheme>;
  skos:prefLabel "frost-susceptible soil"@en;
  skos:topConceptOf <https://w3id.org/permafrost/v/nrcglossary/scheme> .

<https://w3id.org/permafrost/v/nrcglossary/t0135> a skos:Concept;
  dct:identifier "t0135"^^xsd:token;
  dct:source "https://nrc-publications.canada.ca/eng/view/object/?id=69fb8993-1baa-4225-b33a-6a02341d383d"^^xsd:anyURI,
    "https://nrc-publications.canada.ca/fra/voir/objet/?id=549123c3-092c-4fca-8dea-99d53eac06dd"^^xsd:anyURI;
  skos:definition "The disintegration and break-up of soil or rock by the combined action of frost shattering, frost wedging and hydration shattering."@en;
  skos:hiddenLabel "rock shattering"@en;
  skos:inScheme <https://w3id.org/permafrost/v/nrcglossary/scheme>;
  skos:prefLabel "altération due au gel"@fr, "frost weathering"@en;
  skos:scopeNote "Hydration shattering is the process of grain loosening and soil or rock disintegration by the wedging pressure of water in films of varying thickness on the surfaces of silicate minerals. Water is drawn between the grains by various particle surface forces and exerts sufficient differential pressure to loosen and separate the grains. The process can act in all climates without the aid of freezing and thawing. When combined with freezing and thawing (frost shattering and frost wedging), however, the resulting process of frost weathering can be a very efficient mechanism for the break-up of soil or rock."@en;
  skos:topConceptOf <https://w3id.org/permafrost/v/nrcglossary/scheme> .

<https://w3id.org/permafrost/v/nrcglossary/t0136> a skos:Concept;
  dct:identifier "t0136"^^xsd:token;
  dct:source "https://nrc-publications.canada.ca/eng/view/object/?id=69fb8993-1baa-4225-b33a-6a02341d383d"^^xsd:anyURI,
    "https://nrc-publications.canada.ca/fra/voir/objet/?id=549123c3-092c-4fca-8dea-99d53eac06dd"^^xsd:anyURI;
  skos:altLabel "congelifraction"@en, "frost bursting"@en, "frost prying"@en, "frost riving"@en,
    "frost splitting"@en, "gelifraction"@en;
  skos:definition "The mechanical disintegration, splitting or break-up of rock by the pressure of the freezing of water in cracks, crevices, pores, joints or bedding planes."@en;
  skos:inScheme <https://w3id.org/permafrost/v/nrcglossary/scheme>;
  skos:prefLabel "frost wedging"@en, "gélifraction"@fr;
  skos:scopeNote "A wide variety of terms has been used to describe what appears to be a single process."@en;
  skos:topConceptOf <https://w3id.org/permafrost/v/nrcglossary/scheme> .

<https://w3id.org/permafrost/v/nrcglossary/t0137> a skos:Concept;
  dct:identifier "t0137"^^xsd:token;
  dct:source "https://nrc-publications.canada.ca/eng/view/object/?id=69fb8993-1baa-4225-b33a-6a02341d383d"^^xsd:anyURI,
    "https://nrc-publications.canada.ca/fra/voir/objet/?id=549123c3-092c-4fca-8dea-99d53eac06dd"^^xsd:anyURI;
  skos:definition "The zone in a freezing, frost-susceptible soil between the warmest isotherm at which ice exists in pores and the isotherm at which the warmest ice lens is growing (see Figure 5)."@en;
  skos:inScheme <https://w3id.org/permafrost/v/nrcglossary/scheme>;
  skos:prefLabel "frange gelée"@fr, "frozen fringe"@en;
  skos:scopeNote "The temperature at the growing ice lens is slightly below 0°C."@en;
  skos:topConceptOf <https://w3id.org/permafrost/v/nrcglossary/scheme> .

<https://w3id.org/permafrost/v/nrcglossary/t0138> a skos:Concept;
  dct:identifier "t0138"^^xsd:token;
  dct:source "https://nrc-publications.canada.ca/eng/view/object/?id=69fb8993-1baa-4225-b33a-6a02341d383d"^^xsd:anyURI,
    "https://nrc-publications.canada.ca/fra/voir/objet/?id=549123c3-092c-4fca-8dea-99d53eac06dd"^^xsd:anyURI;
  skos:definition "Soil or rock in which part or all of the pore water has turned into ice."@en;
  skos:inScheme <https://w3id.org/permafrost/v/nrcglossary/scheme>;
  skos:prefLabel "frozen ground"@en, "gélisol"@fr;
  skos:scopeNote "Perennially and seasonally frozen ground can vary from being partially to extensively frozen depending on the extent of the phase change. It may be described as hard frozen ground, plastic frozen ground, or dry frozen ground, depending on the pore ice and unfrozen water contents and its compressibility under load. Hard-frozen soils are firmly cemented by ice, are subject to brittle failure, and exhibit practically no consolidation under load. Plastic-frozen soils are cemented by ice but have viscous properties due to their high unfrozen water content and therefore will compress under load. Dry-, or friable-frozen, soils have a very low total water content and are not cemented by ice; their compressibility is the same as for unfrozen soils having the same composition, total water content and density."@en;
  skos:topConceptOf <https://w3id.org/permafrost/v/nrcglossary/scheme> .

<https://w3id.org/permafrost/v/nrcglossary/t0139> a skos:Concept;
  dct:identifier "t0139"^^xsd:token;
  dct:source "https://nrc-publications.canada.ca/eng/view/object/?id=69fb8993-1baa-4225-b33a-6a02341d383d"^^xsd:anyURI,
    "https://nrc-publications.canada.ca/fra/voir/objet/?id=549123c3-092c-4fca-8dea-99d53eac06dd"^^xsd:anyURI;
  skos:definition "A special form of solid clathrate compound in which crystal lattice cages or chambers, consisting of host molecules, enclose guest molecules."@en;
  skos:inScheme <https://w3id.org/permafrost/v/nrcglossary/scheme>;
  skos:prefLabel "gas hydrate"@en, "hydrate de gaz"@fr;
  skos:scopeNote "Gas hydrates are formed under special temperature and pressure conditions. The host molecules are water, and the guest molecules may be a variety of gases, including argon, nitrogen, carbon dioxide, hydrogen sulfide, methane, ethane, halogens and other small molecules. In permafrost regions, gas hydrates are commonly found near the permafrost base and may lead to unexpected problems during drilling for hydrocarbons."@en;
  skos:topConceptOf <https://w3id.org/permafrost/v/nrcglossary/scheme> .

<https://w3id.org/permafrost/v/nrcglossary/t0140> a skos:Concept;
  dct:identifier "t0140"^^xsd:token;
  dct:source "https://nrc-publications.canada.ca/eng/view/object/?id=69fb8993-1baa-4225-b33a-6a02341d383d"^^xsd:anyURI,
    "https://nrc-publications.canada.ca/fra/voir/objet/?id=549123c3-092c-4fca-8dea-99d53eac06dd"^^xsd:anyURI;
  skos:definition "The slow downslope flow of unfrozen earth materials on a frozen substrate."@en;
  skos:inScheme <https://w3id.org/permafrost/v/nrcglossary/scheme>;
  skos:prefLabel "gelifluction"@en, "gélijluxion"@fr;
  skos:scopeNote "Gelifluction is a type of solifluction implying the presence of either seasonal frost or permafrost."@en;
  skos:topConceptOf <https://w3id.org/permafrost/v/nrcglossary/scheme> .

<https://w3id.org/permafrost/v/nrcglossary/t0141> a skos:Concept;
  dct:identifier "t0141"^^xsd:token;
  dct:source "https://nrc-publications.canada.ca/eng/view/object/?id=69fb8993-1baa-4225-b33a-6a02341d383d"^^xsd:anyURI,
    "https://nrc-publications.canada.ca/fra/voir/objet/?id=549123c3-092c-4fca-8dea-99d53eac06dd"^^xsd:anyURI;
  skos:definition "The study of earth materials having a temperature below 0°C."@en;
  skos:inScheme <https://w3id.org/permafrost/v/nrcglossary/scheme>;
  skos:prefLabel "geocryology"@en, "géocryotogie"@fr;
  skos:scopeNote "The term is derived from the Russian word \"geokriologiya\". Although glaciers are not excluded, the term is usually applied to the study of frozen ground, including seasonally frozen ground as well as permafrost."@en;
  skos:topConceptOf <https://w3id.org/permafrost/v/nrcglossary/scheme> .

<https://w3id.org/permafrost/v/nrcglossary/t0142> a skos:Concept;
  dct:identifier "t0142"^^xsd:token;
  dct:source "https://nrc-publications.canada.ca/eng/view/object/?id=69fb8993-1baa-4225-b33a-6a02341d383d"^^xsd:anyURI,
    "https://nrc-publications.canada.ca/fra/voir/objet/?id=549123c3-092c-4fca-8dea-99d53eac06dd"^^xsd:anyURI;
  skos:definition "The rate of temperature increase with depth in the subsurface (see Figure 2)."@en;
  skos:inScheme <https://w3id.org/permafrost/v/nrcglossary/scheme>;
  skos:prefLabel "geothermal gradient"@en;
  skos:scopeNote "Commonly expressed as °C per metre depth."@en;
  skos:topConceptOf <https://w3id.org/permafrost/v/nrcglossary/scheme> .

<https://w3id.org/permafrost/v/nrcglossary/t0143> a skos:Concept;
  dct:identifier "t0143"^^xsd:token;
  dct:source "https://nrc-publications.canada.ca/eng/view/object/?id=69fb8993-1baa-4225-b33a-6a02341d383d"^^xsd:anyURI,
    "https://nrc-publications.canada.ca/fra/voir/objet/?id=549123c3-092c-4fca-8dea-99d53eac06dd"^^xsd:anyURI;
  skos:definition "The amount of heat moving steadily outward from the interior of the earth through a unit area in unit time."@en;
  skos:inScheme <https://w3id.org/permafrost/v/nrcglossary/scheme>;
  skos:prefLabel "geothermal heat flux"@en;
  skos:scopeNote "Commonly expressed as joules per square metre per second."@en;
  skos:topConceptOf <https://w3id.org/permafrost/v/nrcglossary/scheme> .

<https://w3id.org/permafrost/v/nrcglossary/t0144> a skos:Concept;
  dct:identifier "t0144"^^xsd:token;
  dct:source "https://nrc-publications.canada.ca/eng/view/object/?id=69fb8993-1baa-4225-b33a-6a02341d383d"^^xsd:anyURI,
    "https://nrc-publications.canada.ca/fra/voir/objet/?id=549123c3-092c-4fca-8dea-99d53eac06dd"^^xsd:anyURI;
  skos:definition "A distinct soil micromorphology, resulting from the effects of freezing and thawing processes, in which soil particles form discrete loosely packed units (see Figure 8a)."@en;
  skos:inScheme <https://w3id.org/permafrost/v/nrcglossary/scheme>;
  skos:prefLabel "granic cryogenic fabric"@en;
  skos:scopeNote "This fabric, found in cryosols, is generally attributed to freeze-thaw processes and the formation of needle ice near the ground surface."@en;
  skos:topConceptOf <https://w3id.org/permafrost/v/nrcglossary/scheme> .

<https://w3id.org/permafrost/v/nrcglossary/t0145> a skos:Concept;
  dct:identifier "t0145"^^xsd:token;
  dct:source "https://nrc-publications.canada.ca/eng/view/object/?id=69fb8993-1baa-4225-b33a-6a02341d383d"^^xsd:anyURI,
    "https://nrc-publications.canada.ca/fra/voir/objet/?id=549123c3-092c-4fca-8dea-99d53eac06dd"^^xsd:anyURI;
  skos:definition "A distinct soil micromorphology, resulting from the effects of freezing and thawing processes, in which soil particles form more or less discrete loosely packed units."@en;
  skos:inScheme <https://w3id.org/permafrost/v/nrcglossary/scheme>;
  skos:prefLabel "granoidic cryogenic fabric"@en;
  skos:scopeNote "This fabric, found in cryosols, is generally attributed to freeze-thaw processes and the formation of needle ice near the ground surface."@en;
  skos:topConceptOf <https://w3id.org/permafrost/v/nrcglossary/scheme> .

<https://w3id.org/permafrost/v/nrcglossary/t0146> a skos:Concept;
  dct:identifier "t0146"^^xsd:token;
  dct:source "https://nrc-publications.canada.ca/eng/view/object/?id=69fb8993-1baa-4225-b33a-6a02341d383d"^^xsd:anyURI,
    "https://nrc-publications.canada.ca/fra/voir/objet/?id=549123c3-092c-4fca-8dea-99d53eac06dd"^^xsd:anyURI;
  skos:definition "The ratio of the mass of the water and ice in a sample to the dry mass of the sample, commonly expressed as a percentage."@en;
  skos:inScheme <https://w3id.org/permafrost/v/nrcglossary/scheme>;
  skos:prefLabel "gravimetric (total) water content"@en;
  skos:scopeNote "Because of the way it is defined, the gravimetric total water content can greatly exceed 100 percent. During thawing of a sample of frozen ground the gravimetric total water content remains constant, unless excess water is allowed to drain out of the sample."@en;
  skos:topConceptOf <https://w3id.org/permafrost/v/nrcglossary/scheme> .

<https://w3id.org/permafrost/v/nrcglossary/t0147> a skos:Concept;
  dct:identifier "t0147"^^xsd:token;
  dct:references <https://doi.org/10.1002/ppp.1912>;
  dct:source "https://nrc-publications.canada.ca/eng/view/object/?id=69fb8993-1baa-4225-b33a-6a02341d383d"^^xsd:anyURI,
    "https://nrc-publications.canada.ca/fra/voir/objet/?id=549123c3-092c-4fca-8dea-99d53eac06dd"^^xsd:anyURI;
  skos:definition "A general term referring to all types of ice contained in freezing and frozen ground (see Figure 10)."@en;
  skos:inScheme <https://w3id.org/permafrost/v/nrcglossary/scheme>;
  skos:prefLabel "ground ice"@en;
  skos:scopeNote "Ground ice occurs in pores, cavities, voids or other openings in soil or rock and includes massive ice. It generally excludes buried ice, except in Russian usage. Ground ice may be epigenetic or syngenetic, contemporaneous or relict, aggrading or degrading, perennial or seasonal. It may occur as lenses, wedges, veins, sheets, seams, irregular masses, or as individual crystals or coatings on mineral or organic particles. Perennial ground ice can only occur within permafrost bodies."@en;
  skos:topConceptOf <https://w3id.org/permafrost/v/nrcglossary/scheme>;
  foaf:depiction "https://upload.wikimedia.org/wikipedia/commons/thumb/9/94/Permafrost_in_Herschel_Island_015.jpg/1280px-Permafrost_in_Herschel_Island_015.jpg"^^rdf:resource;
  foaf:img "https://upload.wikimedia.org/wikipedia/commons/5/56/Permafrost_-_Massive_buried_ice_%28blue%29.png"^^rdf:resource .

<https://w3id.org/permafrost/v/nrcglossary/t0148> a skos:Concept;
  dct:identifier "t0148"^^xsd:token;
  dct:source "https://nrc-publications.canada.ca/eng/view/object/?id=69fb8993-1baa-4225-b33a-6a02341d383d"^^xsd:anyURI,
    "https://nrc-publications.canada.ca/fra/voir/objet/?id=549123c3-092c-4fca-8dea-99d53eac06dd"^^xsd:anyURI;
  skos:definition "Frozen ground (soil or rock) which is firmly cemented by ice."@en;
  skos:inScheme <https://w3id.org/permafrost/v/nrcglossary/scheme>;
  skos:prefLabel "hard frozen ground"@en;
  skos:scopeNote "Hard frozen ground is subject to brittle failure, and exhibits practically no consolidation under load."@en;
  skos:topConceptOf <https://w3id.org/permafrost/v/nrcglossary/scheme> .

<https://w3id.org/permafrost/v/nrcglossary/t0149> a skos:Concept;
  dct:identifier "t0149"^^xsd:token;
  dct:source "https://nrc-publications.canada.ca/eng/view/object/?id=69fb8993-1baa-4225-b33a-6a02341d383d"^^xsd:anyURI,
    "https://nrc-publications.canada.ca/fra/voir/objet/?id=549123c3-092c-4fca-8dea-99d53eac06dd"^^xsd:anyURI;
  skos:definition "The amount of heat required to raise the temperature of a unit mass of a substance by one degree."@en;
  skos:inScheme <https://w3id.org/permafrost/v/nrcglossary/scheme>;
  skos:prefLabel "heat capacity"@en;
  skos:scopeNote "This term is a commonly used abbreviation of specific heat capacity, which does not include the effects of changes in latent heat due to the melting of ice or the freezing of water with changes in temperature. Because the phase change in a frozen soil often occurs gradually over a range of temperatures, the apparent heat capacity (covering both sensible and latent heat contents) may vary significantly with temperature. Heat capacity is commonly expressed in Joules per kg per degree K."@en;
  skos:topConceptOf <https://w3id.org/permafrost/v/nrcglossary/scheme> .

<https://w3id.org/permafrost/v/nrcglossary/t0150> a skos:Concept;
  dct:identifier "t0150"^^xsd:token;
  dct:source "https://nrc-publications.canada.ca/eng/view/object/?id=69fb8993-1baa-4225-b33a-6a02341d383d"^^xsd:anyURI,
    "https://nrc-publications.canada.ca/fra/voir/objet/?id=549123c3-092c-4fca-8dea-99d53eac06dd"^^xsd:anyURI;
  skos:definition "Upward pressure developed during freezing of the ground."@en;
  skos:inScheme <https://w3id.org/permafrost/v/nrcglossary/scheme>;
  skos:prefLabel "heaving pressure"@en;
  skos:scopeNote "Heaving pressure develops during the formation of both pore ice and ice lenses. It is responsible for the heaving of utilities, foundations, pavements etc."@en;
  skos:topConceptOf <https://w3id.org/permafrost/v/nrcglossary/scheme> .

<https://w3id.org/permafrost/v/nrcglossary/t0151> a skos:Concept;
  dct:identifier "t0151"^^xsd:token;
  dct:source "https://nrc-publications.canada.ca/eng/view/object/?id=69fb8993-1baa-4225-b33a-6a02341d383d"^^xsd:anyURI,
    "https://nrc-publications.canada.ca/fra/voir/objet/?id=549123c3-092c-4fca-8dea-99d53eac06dd"^^xsd:anyURI;
  skos:definition "An ice-wedge polygon in which melting of the surrounding ice wedges has left the central area in a relatively elevated position."@en;
  skos:inScheme <https://w3id.org/permafrost/v/nrcglossary/scheme>;
  skos:prefLabel "high-centre polygon"@en;
  skos:topConceptOf <https://w3id.org/permafrost/v/nrcglossary/scheme> .

<https://w3id.org/permafrost/v/nrcglossary/t0152> a skos:Concept;
  dct:identifier "t0152"^^xsd:token;
  dct:source "https://nrc-publications.canada.ca/eng/view/object/?id=69fb8993-1baa-4225-b33a-6a02341d383d"^^xsd:anyURI,
    "https://nrc-publications.canada.ca/fra/voir/objet/?id=549123c3-092c-4fca-8dea-99d53eac06dd"^^xsd:anyURI;
  skos:definition "The volume of fluid passing through a unit cross section in unit time under the action of a unit hydraulic potential gradient."@en;
  skos:inScheme <https://w3id.org/permafrost/v/nrcglossary/scheme>;
  skos:prefLabel "hydraulic conductivity"@en;
  skos:scopeNote "The hydraulic conductivity is a function of the viscosity and density of the fluid, which in turn depend on the fluid temperature. In practice it is commonly expressed in cm per second or m per day."@en;
  skos:topConceptOf <https://w3id.org/permafrost/v/nrcglossary/scheme> .

<https://w3id.org/permafrost/v/nrcglossary/t0153> a skos:Concept;
  dct:identifier "t0153"^^xsd:token;
  dct:source "https://nrc-publications.canada.ca/eng/view/object/?id=69fb8993-1baa-4225-b33a-6a02341d383d"^^xsd:anyURI,
    "https://nrc-publications.canada.ca/fra/voir/objet/?id=549123c3-092c-4fca-8dea-99d53eac06dd"^^xsd:anyURI;
  skos:definition "The ratio of the hydraulic conductivity and the storage capacity of a groundwater aquifer."@en;
  skos:inScheme <https://w3id.org/permafrost/v/nrcglossary/scheme>;
  skos:prefLabel "hydraulic diffusivity"@en;
  skos:scopeNote "The hydraulic diffusivity expresses the facility with which an aquifer will undergo a pressure change."@en;
  skos:topConceptOf <https://w3id.org/permafrost/v/nrcglossary/scheme> .

<https://w3id.org/permafrost/v/nrcglossary/t0154> a skos:Concept;
  dct:identifier "t0154"^^xsd:token;
  dct:source "https://nrc-publications.canada.ca/eng/view/object/?id=69fb8993-1baa-4225-b33a-6a02341d383d"^^xsd:anyURI,
    "https://nrc-publications.canada.ca/fra/voir/objet/?id=549123c3-092c-4fca-8dea-99d53eac06dd"^^xsd:anyURI;
  skos:definition "Artificial thawing (and removal) of frozen ground by the use of a stream or jet of water under high pressure."@en;
  skos:inScheme <https://w3id.org/permafrost/v/nrcglossary/scheme>;
  skos:prefLabel "dégel hydraulique"@fr, "hydraulic thawing"@en;
  skos:scopeNote "Hydraulic thawing (hydraulicking) is a common method of working frozen placer deposits in North America."@en;
  skos:topConceptOf <https://w3id.org/permafrost/v/nrcglossary/scheme> .

<https://w3id.org/permafrost/v/nrcglossary/t0155> a skos:Concept;
  dct:identifier "t0155"^^xsd:token;
  dct:source "https://nrc-publications.canada.ca/eng/view/object/?id=69fb8993-1baa-4225-b33a-6a02341d383d"^^xsd:anyURI,
    "https://nrc-publications.canada.ca/fra/voir/objet/?id=549123c3-092c-4fca-8dea-99d53eac06dd"^^xsd:anyURI;
  skos:definition "A layer or body of cryotic (but unfrozen) ground in a permafrost area, maintained by moving mineralized groundwater (see Figure 11)."@en;
  skos:inScheme <https://w3id.org/permafrost/v/nrcglossary/scheme>;
  skos:prefLabel "hydrochemical talik"@en;
  skos:scopeNote "In a hydrochemical talik, freezing is prevented by freezing-point depression due to the dissolved-solids content of mineralized groundwater moving through the talik."@en;
  skos:topConceptOf <https://w3id.org/permafrost/v/nrcglossary/scheme> .

<https://w3id.org/permafrost/v/nrcglossary/t0156> a skos:Concept;
  dct:identifier "t0156"^^xsd:token;
  dct:source "https://nrc-publications.canada.ca/eng/view/object/?id=69fb8993-1baa-4225-b33a-6a02341d383d"^^xsd:anyURI,
    "https://nrc-publications.canada.ca/fra/voir/objet/?id=549123c3-092c-4fca-8dea-99d53eac06dd"^^xsd:anyURI;
  skos:definition "A layer or body of noncryotic unfrozen ground in a permafrost area, maintained by moving groundwater (see Figure 11)."@en;
  skos:inScheme <https://w3id.org/permafrost/v/nrcglossary/scheme>;
  skos:prefLabel "hydrothermal talik"@en;
  skos:scopeNote "In a hydrothermal talik, the temperature is maintained above 0?C by the heat supplied by moving groundwater."@en;
  skos:topConceptOf <https://w3id.org/permafrost/v/nrcglossary/scheme> .

<https://w3id.org/permafrost/v/nrcglossary/t0157> a skos:Concept;
  dct:identifier "t0157"^^xsd:token;
  dct:source "https://nrc-publications.canada.ca/eng/view/object/?id=69fb8993-1baa-4225-b33a-6a02341d383d"^^xsd:anyURI,
    "https://nrc-publications.canada.ca/fra/voir/objet/?id=549123c3-092c-4fca-8dea-99d53eac06dd"^^xsd:anyURI;
  skos:definition "Water in the solid state."@en;
  skos:inScheme <https://w3id.org/permafrost/v/nrcglossary/scheme>;
  skos:prefLabel "glace"@fr, "ice"@en;
  skos:scopeNote "Ice commonly occurs as hexagonal crystals. In permafrost regions, ice may occupy voids in soils and rocks and may develop in a variety of forms. Ice may be colourless to pale blue or greenish-blue. It may appear white due to included gas bubbles; in exposures, ground ice may also appear black. Various types of ground ice are defined elsewhere in this Glossary."@en;
  skos:topConceptOf <https://w3id.org/permafrost/v/nrcglossary/scheme> .

<https://w3id.org/permafrost/v/nrcglossary/t0158> a skos:Concept;
  dct:identifier "t0158"^^xsd:token;
  dct:source "https://nrc-publications.canada.ca/eng/view/object/?id=69fb8993-1baa-4225-b33a-6a02341d383d"^^xsd:anyURI,
    "https://nrc-publications.canada.ca/fra/voir/objet/?id=549123c3-092c-4fca-8dea-99d53eac06dd"^^xsd:anyURI;
  skos:definition "Permafrost that contains ice."@en;
  skos:inScheme <https://w3id.org/permafrost/v/nrcglossary/scheme>;
  skos:prefLabel "ice-bearing permafrost"@en;
  skos:topConceptOf <https://w3id.org/permafrost/v/nrcglossary/scheme> .

<https://w3id.org/permafrost/v/nrcglossary/t0159> a skos:Concept;
  dct:identifier "t0159"^^xsd:token;
  dct:source "https://nrc-publications.canada.ca/eng/view/object/?id=69fb8993-1baa-4225-b33a-6a02341d383d"^^xsd:anyURI,
    "https://nrc-publications.canada.ca/fra/voir/objet/?id=549123c3-092c-4fca-8dea-99d53eac06dd"^^xsd:anyURI;
  skos:definition "Ice-bearing permafrost in which the soil particles are cemented together by ice."@en;
  skos:inScheme <https://w3id.org/permafrost/v/nrcglossary/scheme>;
  skos:prefLabel "ice-bonded permafrost"@en;
  skos:scopeNote "Frozen soils may be partially-bonded, poorly-bonded or friable, if the soil particles are held together (cemented) weakly by the ice. If ice bonding is strong, the soil is said to be well-bonded. The distinction between ice-bonded permafrost and permafrost that contains ice but in which the ice does not act as a cement, is particularly important in subsea permafrost, where the dissolved-solids content of the pore water affects the ability of ice to act as a cement. Acoustic geophysical methods can be used to delineate ice-bonded permafrost, but use of the term \"acoustically-defined permafrost\" is not recommended except as a modifier to describe the method used to determine the permafrost conditions."@en;
  skos:topConceptOf <https://w3id.org/permafrost/v/nrcglossary/scheme> .

<https://w3id.org/permafrost/v/nrcglossary/t0160> a skos:Concept;
  dct:identifier "t0160"^^xsd:token;
  dct:source "https://nrc-publications.canada.ca/eng/view/object/?id=69fb8993-1baa-4225-b33a-6a02341d383d"^^xsd:anyURI,
    "https://nrc-publications.canada.ca/fra/voir/objet/?id=549123c3-092c-4fca-8dea-99d53eac06dd"^^xsd:anyURI;
  skos:definition "The amount of ice contained in frozen or partially frozen soil or rock."@en;
  skos:inScheme <https://w3id.org/permafrost/v/nrcglossary/scheme>;
  skos:prefLabel "ice content"@en, "teneur en glace"@fr;
  skos:scopeNote "Ice content is normally expressed in one of two ways: 1. on a dry-weight basis (gravimetric), as the ratio of the mass of the ice in a sample to the mass of the dry sample, expressed as a percentage, or 2. on a volume basis (volumetric), as the ratio of the volume of ice in a sample to the volume of the whole sample, expressed as a fraction. The volumetric ice content cannot exceed unity whereas the gravimetric ice content can greatly exceed 100 percent."@en;
  skos:topConceptOf <https://w3id.org/permafrost/v/nrcglossary/scheme> .

<https://w3id.org/permafrost/v/nrcglossary/t0161> a skos:Concept;
  dct:identifier "t0161"^^xsd:token;
  dct:source "https://nrc-publications.canada.ca/eng/view/object/?id=69fb8993-1baa-4225-b33a-6a02341d383d"^^xsd:anyURI,
    "https://nrc-publications.canada.ca/fra/voir/objet/?id=549123c3-092c-4fca-8dea-99d53eac06dd"^^xsd:anyURI;
  skos:definition "Topography that is due almost solely to differences in the amount of excess ice underlying its surface."@en;
  skos:inScheme <https://w3id.org/permafrost/v/nrcglossary/scheme>;
  skos:prefLabel "ice-cored topography"@en, "relief à noyaux de glace"@fr;
  skos:scopeNote "The relief may be totally or partially due to thermokarst, or to irregular development of ground ice, primarily segregated ice, or to buried glacier ice. An example is the \"involuted hill\" near Tuktoyaktuk, N.W.T."@en;
  skos:topConceptOf <https://w3id.org/permafrost/v/nrcglossary/scheme> .

<https://w3id.org/permafrost/v/nrcglossary/t0162> a skos:Concept;
  dct:identifier "t0162"^^xsd:token;
  dct:source "https://nrc-publications.canada.ca/eng/view/object/?id=69fb8993-1baa-4225-b33a-6a02341d383d"^^xsd:anyURI,
    "https://nrc-publications.canada.ca/fra/voir/objet/?id=549123c3-092c-4fca-8dea-99d53eac06dd"^^xsd:anyURI;
  skos:definition "A dominantly horizontal, lens-shaped body of ice of any dimension."@en;
  skos:inScheme <https://w3id.org/permafrost/v/nrcglossary/scheme>;
  skos:prefLabel "ice lens"@en;
  skos:scopeNote "The term is commonly used for layers of segregated ice. Ice lenses may range in thickness from hairline to more than 10 m. Very thick and extensive ice lenses are better termed massive ice beds."@en;
  skos:topConceptOf <https://w3id.org/permafrost/v/nrcglossary/scheme> .

<https://w3id.org/permafrost/v/nrcglossary/t0163> a skos:Concept;
  dct:identifier "t0163"^^xsd:token;
  dct:source "https://nrc-publications.canada.ca/eng/view/object/?id=69fb8993-1baa-4225-b33a-6a02341d383d"^^xsd:anyURI,
    "https://nrc-publications.canada.ca/fra/voir/objet/?id=549123c3-092c-4fca-8dea-99d53eac06dd"^^xsd:anyURI;
  skos:definition "The temperature at which ice first forms during freezing of a soil/water system that does not initially contain ice."@en;
  skos:inScheme <https://w3id.org/permafrost/v/nrcglossary/scheme>;
  skos:prefLabel "ice-nucleation temperature"@en, "températurede nucléation de la glace"@fr;
  skos:scopeNote "The ice-nucleation temperature may be lower than 0°C due to freezing-point depression caused by the dissolved-solids content of the pore water."@en;
  skos:topConceptOf <https://w3id.org/permafrost/v/nrcglossary/scheme> .

<https://w3id.org/permafrost/v/nrcglossary/t0164> a skos:Concept;
  dct:identifier "t0164"^^xsd:token;
  dct:source "https://nrc-publications.canada.ca/eng/view/object/?id=69fb8993-1baa-4225-b33a-6a02341d383d"^^xsd:anyURI,
    "https://nrc-publications.canada.ca/fra/voir/objet/?id=549123c3-092c-4fca-8dea-99d53eac06dd"^^xsd:anyURI;
  skos:definition "Permafrost containing excess ice."@en;
  skos:inScheme <https://w3id.org/permafrost/v/nrcglossary/scheme>;
  skos:prefLabel "ice-rich permafrost"@en;
  skos:scopeNote "A qualitative term. Ice-rich permafrost is thaw-sensitive."@en;
  skos:topConceptOf <https://w3id.org/permafrost/v/nrcglossary/scheme> .

<https://w3id.org/permafrost/v/nrcglossary/t0165> a skos:Concept;
  dct:identifier "t0165"^^xsd:token;
  dct:source "https://nrc-publications.canada.ca/eng/view/object/?id=69fb8993-1baa-4225-b33a-6a02341d383d"^^xsd:anyURI,
    "https://nrc-publications.canada.ca/fra/voir/objet/?id=549123c3-092c-4fca-8dea-99d53eac06dd"^^xsd:anyURI;
  skos:definition "The formation of discrete layers or lenses of segregated ice in freezing mineral or organic soils, as a result of the migration (and subsequent freezing) of pore water."@en;
  skos:inScheme <https://w3id.org/permafrost/v/nrcglossary/scheme>;
  skos:prefLabel "ice segregation"@en;
  skos:scopeNote "The migration of pore water to the frozen fringe is caused by cryosuction."@en;
  skos:topConceptOf <https://w3id.org/permafrost/v/nrcglossary/scheme> .

<https://w3id.org/permafrost/v/nrcglossary/t0166> a skos:Concept;
  dct:identifier "t0166"^^xsd:token;
  dct:source "https://nrc-publications.canada.ca/eng/view/object/?id=69fb8993-1baa-4225-b33a-6a02341d383d"^^xsd:anyURI,
    "https://nrc-publications.canada.ca/fra/voir/objet/?id=549123c3-092c-4fca-8dea-99d53eac06dd"^^xsd:anyURI;
  skos:definition "An ice-filled crack or fissure in the ground."@en;
  skos:inScheme <https://w3id.org/permafrost/v/nrcglossary/scheme>;
  skos:prefLabel "ice vein"@en, "veine de glace"@fr;
  skos:topConceptOf <https://w3id.org/permafrost/v/nrcglossary/scheme> .

<https://w3id.org/permafrost/v/nrcglossary/t0167> a skos:Concept;
  dct:identifier "t0167"^^xsd:token;
  dct:references "J. Ross Mackay. The frequency of ice-wedge cracking (19671987) at Garry Island, western Arctic coast, Canada. Canadian Journal of Earth Sciences. 29(2): 236-248. https://doi.org/10.1139/e92-022",
    <https://doi.org/10.1002/ppp.523>;
  dct:source "https://nrc-publications.canada.ca/eng/view/object/?id=69fb8993-1baa-4225-b33a-6a02341d383d"^^xsd:anyURI,
    "https://nrc-publications.canada.ca/fra/voir/objet/?id=549123c3-092c-4fca-8dea-99d53eac06dd"^^xsd:anyURI;
  skos:definition "A massive, generally wedge-shaped body with its apex pointing downward, composed of foliated or vertically banded, commonly white, ice (see Figure 17)."@en;
  skos:inScheme <https://w3id.org/permafrost/v/nrcglossary/scheme>;
  skos:prefLabel "coin de glace"@fr, "ice wedge"@en;
  skos:scopeNote "The size of ice wedges varies from less than 10 cm to more than 3 m in width at the top, commonly tapering to a feather edge at a depth of 1 to more than 10 m. Some ice wedges may extend downward as much as 25 m and may have shapes dissimilar to wedges. Epigenetic ice wedges are characteristically wedge-shaped, whereas syngenetic ice wedges and anti-syngenetic ice wedges are generally wedge-shaped but with more irregular sides (see also epigenetic permafrost, syngenetic permafrost). Ice wedges are formed in thermal contraction cracks in which hoar frost (see open-cavity ice) forms and into which water from melting snow penetrates in the spring. Repeated annual contraction cracking of the ice in the wedge, followed by freezing of water in the crack, gradually increases the width (and possibly the depth) of the wedge and causes vertical banding of the ice mass. The surface expression of ice wedges is generally a network of polygons. Ice wedges growing as a result of repeated (but not necessarily annual) winter cracking are called active ice wedges. They occur primarily in areas of continuous permafrost when developed in mineral soil. Inactive ice wedges can be stable and remain for many centuries without changing."@en;
  skos:topConceptOf <https://w3id.org/permafrost/v/nrcglossary/scheme>;
  foaf:depiction "https://media.springernature.com/full/springer-static/image/chp%3A10.1007%2F978-1-4614-9213-9_193-1/MediaObjects/214584_0_En_193-1_Fig3_HTML.jpg?as=webp"^^rdf:resource,
    "https://upload.wikimedia.org/wikipedia/commons/7/7c/Ice_wedge_iceland.jpg"^^rdf:resource;
  foaf:img "https://upload.wikimedia.org/wikipedia/commons/c/c6/Ice_wedge.jpg"^^rdf:resource .

<https://w3id.org/permafrost/v/nrcglossary/t0168> a skos:Concept;
  dct:identifier "t0168"^^xsd:token;
  dct:source "https://nrc-publications.canada.ca/eng/view/object/?id=69fb8993-1baa-4225-b33a-6a02341d383d"^^xsd:anyURI,
    "https://nrc-publications.canada.ca/fra/voir/objet/?id=549123c3-092c-4fca-8dea-99d53eac06dd"^^xsd:anyURI;
  skos:definition "A filling of sediment in the space formerly occupied by an ice wedge."@en;
  skos:hiddenLabel "ice-wedge pseudomorph"@en;
  skos:inScheme <https://w3id.org/permafrost/v/nrcglossary/scheme>;
  skos:prefLabel "fente en coin fossile"@fr, "ice-wedge cast"@en;
  skos:scopeNote "An ice-wedge cast is a wedge of secondary filling. When the permafrost thawed, the ice wedge melted and the enclosing and overlying sediments collapsed into the resulting trough. An ice-wedge cast is one of the few acceptable criteria indicating the earlier presence of permafrost. The term \"fossil ice wedge\" is not recommended because ice is no longer present."@en;
  skos:topConceptOf <https://w3id.org/permafrost/v/nrcglossary/scheme> .

<https://w3id.org/permafrost/v/nrcglossary/t0169> a skos:Concept;
  dct:identifier "t0169"^^xsd:token;
  dct:source "https://nrc-publications.canada.ca/eng/view/object/?id=69fb8993-1baa-4225-b33a-6a02341d383d"^^xsd:anyURI,
    "https://nrc-publications.canada.ca/fra/voir/objet/?id=549123c3-092c-4fca-8dea-99d53eac06dd"^^xsd:anyURI;
  skos:definition "A polygon outlined by ice wedges underlying its boundaries."@en;
  skos:inScheme <https://w3id.org/permafrost/v/nrcglossary/scheme>;
  skos:prefLabel "ice-wedge polygon"@en;
  skos:scopeNote "Ice-wedge polygons occur in both mineral terrain and peatland, commonly in poorly drained permafrost areas."@en;
  skos:topConceptOf <https://w3id.org/permafrost/v/nrcglossary/scheme> .

<https://w3id.org/permafrost/v/nrcglossary/t0170> a skos:Concept;
  dct:identifier "t0170"^^xsd:token;
  dct:source "https://nrc-publications.canada.ca/eng/view/object/?id=69fb8993-1baa-4225-b33a-6a02341d383d"^^xsd:anyURI,
    "https://nrc-publications.canada.ca/fra/voir/objet/?id=549123c3-092c-4fca-8dea-99d53eac06dd"^^xsd:anyURI;
  skos:definition "A qualitative term describing the quantity of ice in frozen ground."@en;
  skos:inScheme <https://w3id.org/permafrost/v/nrcglossary/scheme>;
  skos:prefLabel "iciness"@en;
  skos:scopeNote "In Russian literature, the equivalent term is used to describe volumetric ice content of frozen, or partially frozen, soil or rock. The \"relative iciness\" is expressed as the ratio of the mass of ice to the total mass of water (ice and unfrozen water) present."@en;
  skos:topConceptOf <https://w3id.org/permafrost/v/nrcglossary/scheme> .

<https://w3id.org/permafrost/v/nrcglossary/t0171> a skos:Concept;
  dct:identifier "t0171"^^xsd:token;
  dct:source "https://nrc-publications.canada.ca/eng/view/object/?id=69fb8993-1baa-4225-b33a-6a02341d383d"^^xsd:anyURI,
    "https://nrc-publications.canada.ca/fra/voir/objet/?id=549123c3-092c-4fca-8dea-99d53eac06dd"^^xsd:anyURI;
  skos:definition "A sheetlike mass of layered ice formed on the ground surface, or on river or lake ice, by freezing of successive flows of water that may seep from the ground, flow from a spring or emerge from below river or lake ice through fractures."@en;
  skos:inScheme <https://w3id.org/permafrost/v/nrcglossary/scheme>;
  skos:prefLabel "glaçage"@fr, "icing"@en;
  skos:scopeNote "Icings also occur in non-permafrost areas. Many icings incorporate snow. In North America the term \"icing\" is gradually replacing a variety of terms used in the past. Aufeis (German), flood ice, flood-plain icing, ice field, naled (Russian) and overflow ice usually indicated icings formed on river ice and floodplains. Chrystocrene (or crystocrene), ground icing, groundwater icing and spring icing usually indicated icings formed by freezing of ground-water discharge. Use of the term \"glacier\" to describe icings, which is common in Alaska and the Yukon, is inappropriate and should be avoided."@en;
  skos:topConceptOf <https://w3id.org/permafrost/v/nrcglossary/scheme> .

<https://w3id.org/permafrost/v/nrcglossary/t0172> a skos:Concept;
  dct:identifier "t0172"^^xsd:token;
  dct:source "https://nrc-publications.canada.ca/eng/view/object/?id=69fb8993-1baa-4225-b33a-6a02341d383d"^^xsd:anyURI,
    "https://nrc-publications.canada.ca/fra/voir/objet/?id=549123c3-092c-4fca-8dea-99d53eac06dd"^^xsd:anyURI;
  skos:definition "A seasonal frost mound consisting of ice only and formed at least in part through lifting of one or more layers of an icing by injected water (see Figures 12 and 13)."@en;
  skos:inScheme <https://w3id.org/permafrost/v/nrcglossary/scheme>;
  skos:prefLabel "dôme de glaçage"@fr, "icing blister"@en;
  skos:scopeNote "Freezing of the injected water will produce a layer of clear ice, contrasting with the overlying thinly layered ice of the icing. Rupture and draining of an icing blister may leave an empty cavity. Icing blisters are distinguished from frost blisters by the absence of a covering layer of seasonally frozen ground; they are distinguished from icing mounds by the layer of clear ice, and in some cases by the presence of an empty cavity. They have also been termed \"ice blisters\" (not recommended)."@en;
  skos:topConceptOf <https://w3id.org/permafrost/v/nrcglossary/scheme> .

<https://w3id.org/permafrost/v/nrcglossary/t0173> a skos:Concept;
  dct:identifier "t0173"^^xsd:token;
  dct:source "https://nrc-publications.canada.ca/eng/view/object/?id=69fb8993-1baa-4225-b33a-6a02341d383d"^^xsd:anyURI,
    "https://nrc-publications.canada.ca/fra/voir/objet/?id=549123c3-092c-4fca-8dea-99d53eac06dd"^^xsd:anyURI;
  skos:definition "An area kept clear of trees and shrubs by the annual occurrence of icings."@en;
  skos:inScheme <https://w3id.org/permafrost/v/nrcglossary/scheme>;
  skos:prefLabel "icing glade"@en;
  skos:scopeNote "Icing glades along streams may also show the effects of lateral erosion occurring along the edges of the icings during and after the snowmelt."@en;
  skos:topConceptOf <https://w3id.org/permafrost/v/nrcglossary/scheme> .

<https://w3id.org/permafrost/v/nrcglossary/t0174> a skos:Concept;
  dct:identifier "t0174"^^xsd:token;
  dct:source "https://nrc-publications.canada.ca/eng/view/object/?id=69fb8993-1baa-4225-b33a-6a02341d383d"^^xsd:anyURI,
    "https://nrc-publications.canada.ca/fra/voir/objet/?id=549123c3-092c-4fca-8dea-99d53eac06dd"^^xsd:anyURI;
  skos:definition "A seasonal frost mound consisting exclusively of thinly layered ice, formed by freezing of successive flows of water issuing from the ground or from below river ice."@en;
  skos:hiddenLabel "ice mound"@en;
  skos:inScheme <https://w3id.org/permafrost/v/nrcglossary/scheme>;
  skos:prefLabel "butte de glaçage"@fr, "icing mound"@en;
  skos:scopeNote "Icing mounds may incorporate snow."@en;
  skos:topConceptOf <https://w3id.org/permafrost/v/nrcglossary/scheme> .

<https://w3id.org/permafrost/v/nrcglossary/t0175> a skos:Concept;
  dct:identifier "t0175"^^xsd:token;
  dct:source "https://nrc-publications.canada.ca/eng/view/object/?id=69fb8993-1baa-4225-b33a-6a02341d383d"^^xsd:anyURI,
    "https://nrc-publications.canada.ca/fra/voir/objet/?id=549123c3-092c-4fca-8dea-99d53eac06dd"^^xsd:anyURI;
  skos:definition "An ice wedge that is no longer growing."@en;
  skos:inScheme <https://w3id.org/permafrost/v/nrcglossary/scheme>;
  skos:prefLabel "inactive ice wedge"@en;
  skos:scopeNote "Inactive ice wedges can be stable and remain unchanged for decades or centuries."@en;
  skos:topConceptOf <https://w3id.org/permafrost/v/nrcglossary/scheme> .

<https://w3id.org/permafrost/v/nrcglossary/t0176> a skos:Concept;
  dct:identifier "t0176"^^xsd:token;
  dct:source "https://nrc-publications.canada.ca/eng/view/object/?id=69fb8993-1baa-4225-b33a-6a02341d383d"^^xsd:anyURI,
    "https://nrc-publications.canada.ca/fra/voir/objet/?id=549123c3-092c-4fca-8dea-99d53eac06dd"^^xsd:anyURI;
  skos:definition "A mass of rock fragments and finer material, on a slope, that contains either an ice core or interstitial ice, and shows evidence of past, but not present, movement."@en;
  skos:inScheme <https://w3id.org/permafrost/v/nrcglossary/scheme>;
  skos:prefLabel "inactive rock glacier"@en;
  skos:scopeNote "Rock glaciers are said to be inactive when their main body ceases to move, and they show no evidence of very recent movement."@en;
  skos:topConceptOf <https://w3id.org/permafrost/v/nrcglossary/scheme> .

<https://w3id.org/permafrost/v/nrcglossary/t0177> a skos:Concept;
  dct:identifier "t0177"^^xsd:token;
  dct:source "https://nrc-publications.canada.ca/eng/view/object/?id=69fb8993-1baa-4225-b33a-6a02341d383d"^^xsd:anyURI,
    "https://nrc-publications.canada.ca/fra/voir/objet/?id=549123c3-092c-4fca-8dea-99d53eac06dd"^^xsd:anyURI;
  skos:definition "Interfacial water forms transition layers at mineral/water and mineral/water/ice interfaces in frozen ground."@en;
  skos:inScheme <https://w3id.org/permafrost/v/nrcglossary/scheme>;
  skos:prefLabel "interfacial water"@en;
  skos:scopeNote "The intermolecular forces involved are such that interfacial water does not move under the influence of gravity. The temperature at which any portion of the interfacial water will change phase depends on the total energy of the various adsorption forces, which in turn depends on the distance from the mineral surface, the type of mineral, and the solute content of the water."@en;
  skos:topConceptOf <https://w3id.org/permafrost/v/nrcglossary/scheme> .

<https://w3id.org/permafrost/v/nrcglossary/t0178> a skos:Concept;
  dct:identifier "t0178"^^xsd:token;
  dct:source "https://nrc-publications.canada.ca/eng/view/object/?id=69fb8993-1baa-4225-b33a-6a02341d383d"^^xsd:anyURI,
    "https://nrc-publications.canada.ca/fra/voir/objet/?id=549123c3-092c-4fca-8dea-99d53eac06dd"^^xsd:anyURI;
  skos:definition "1. (North-American usage) Permafrost underlying 35 to 65 percent of the area of exposed land surface. 2. (Russian usage) Permafrost underlying 40 to 60 percent of the area of exposed land surface."@en;
  skos:inScheme <https://w3id.org/permafrost/v/nrcglossary/scheme>;
  skos:prefLabel "intermediate discontinuous permafrost"@en;
  skos:topConceptOf <https://w3id.org/permafrost/v/nrcglossary/scheme> .

<https://w3id.org/permafrost/v/nrcglossary/t0179> a skos:Concept;
  dct:identifier "t0179"^^xsd:token;
  dct:source "https://nrc-publications.canada.ca/eng/view/object/?id=69fb8993-1baa-4225-b33a-6a02341d383d"^^xsd:anyURI,
    "https://nrc-publications.canada.ca/fra/voir/objet/?id=549123c3-092c-4fca-8dea-99d53eac06dd"^^xsd:anyURI;
  skos:definition "Water occurring in unfrozen zones (taliks and cryopegs) within permafrost(see Figure 11)."@en;
  skos:inScheme <https://w3id.org/permafrost/v/nrcglossary/scheme>;
  skos:prefLabel "eau d'intrapergéliso!"@fr, "intrapermafrost water"@en;
  skos:scopeNote "Intrapermafrost water includes water in open, lateral and transient taliks and in basal, isolated and marine cryopegs. Sometimes erroneously called interpermafrost water."@en;
  skos:topConceptOf <https://w3id.org/permafrost/v/nrcglossary/scheme> .

<https://w3id.org/permafrost/v/nrcglossary/t0180> a skos:Concept;
  dct:identifier "t0180"^^xsd:token;
  dct:source "https://nrc-publications.canada.ca/eng/view/object/?id=69fb8993-1baa-4225-b33a-6a02341d383d"^^xsd:anyURI,
    "https://nrc-publications.canada.ca/fra/voir/objet/?id=549123c3-092c-4fca-8dea-99d53eac06dd"^^xsd:anyURI;
  skos:definition "Ice formed from water injected into soils or rocks (see Figure 10c)."@en;
  skos:hiddenLabel "injection ice"@en;
  skos:inScheme <https://w3id.org/permafrost/v/nrcglossary/scheme>;
  skos:prefLabel "intrusive ice"@en;
  skos:scopeNote "Freezing of injected water will normally lift the ground above it, thereby producing topographic forms somewhat resembling those of igneous intrusions in rocks. Thus, a tabular mass of intrusive ice is analogous to a sill or a dyke (see ice vein) whereas the domed form is analogous to a laccolith (see frost blister, pingo). Use of terms such as \"sill ice\" or \"hydrolaccolith,\" however, is not recommended. Intrusive ice may develop in porous unconsolidated sediments and in jointed or fractured bedrock. Fractures may become enlarged by hydraulic fracturing or frost wedging processes. For the greatest effect, water must become trapped in the joints or fractures and be subjected to relatively rapid freezing."@en;
  skos:topConceptOf <https://w3id.org/permafrost/v/nrcglossary/scheme> .

<https://w3id.org/permafrost/v/nrcglossary/t0181> a skos:Concept;
  dct:identifier "t0181"^^xsd:token;
  dct:source "https://nrc-publications.canada.ca/eng/view/object/?id=69fb8993-1baa-4225-b33a-6a02341d383d"^^xsd:anyURI,
    "https://nrc-publications.canada.ca/fra/voir/objet/?id=549123c3-092c-4fca-8dea-99d53eac06dd"^^xsd:anyURI;
  skos:definition "A distinct soil micromorphology, resulting from the effects of freezing and thawing processes, in which soil particles form subhorizontal layers of similar thickness."@en;
  skos:inScheme <https://w3id.org/permafrost/v/nrcglossary/scheme>;
  skos:prefLabel "isoband cryogenic fabric"@en;
  skos:scopeNote "This fabric, found in cryosols, results from freeze-thaw processes accompanied by eluviation."@en;
  skos:topConceptOf <https://w3id.org/permafrost/v/nrcglossary/scheme> .

<https://w3id.org/permafrost/v/nrcglossary/t0182> a skos:Concept;
  dct:identifier "t0182"^^xsd:token;
  dct:source "https://nrc-publications.canada.ca/eng/view/object/?id=69fb8993-1baa-4225-b33a-6a02341d383d"^^xsd:anyURI,
    "https://nrc-publications.canada.ca/fra/voir/objet/?id=549123c3-092c-4fca-8dea-99d53eac06dd"^^xsd:anyURI;
  skos:definition "A body of unfrozen ground, that is perennially cryotic (T < 0°C) and entirely surrounded by perennially frozen ground (see Figure 11)."@en;
  skos:inScheme <https://w3id.org/permafrost/v/nrcglossary/scheme>;
  skos:prefLabel "isolated cryopeg"@en;
  skos:scopeNote "In an isolated cryopeg, freezing is prevented by freezing-point depression due to the dissolved-solids content of its pore water."@en;
  skos:topConceptOf <https://w3id.org/permafrost/v/nrcglossary/scheme> .

<https://w3id.org/permafrost/v/nrcglossary/t0183> a skos:Concept;
  dct:identifier "t0183"^^xsd:token;
  dct:source "https://nrc-publications.canada.ca/eng/view/object/?id=69fb8993-1baa-4225-b33a-6a02341d383d"^^xsd:anyURI,
    "https://nrc-publications.canada.ca/fra/voir/objet/?id=549123c3-092c-4fca-8dea-99d53eac06dd"^^xsd:anyURI;
  skos:definition "Permafrost underlying less than 10 percent of the exposed land surface."@en;
  skos:hiddenLabel "insular permafrost"@en, "island permafrost"@en, "scattered permafrost"@en;
  skos:inScheme <https://w3id.org/permafrost/v/nrcglossary/scheme>;
  skos:prefLabel "isolated patches of permafrost"@en;
  skos:scopeNote "Individual areas of permafrost are of limited areal extent, widely separated, and are completely surrounded by unfrozen ground."@en;
  skos:topConceptOf <https://w3id.org/permafrost/v/nrcglossary/scheme> .

<https://w3id.org/permafrost/v/nrcglossary/t0184> a skos:Concept;
  dct:identifier "t0184"^^xsd:token;
  dct:source "https://nrc-publications.canada.ca/eng/view/object/?id=69fb8993-1baa-4225-b33a-6a02341d383d"^^xsd:anyURI,
    "https://nrc-publications.canada.ca/fra/voir/objet/?id=549123c3-092c-4fca-8dea-99d53eac06dd"^^xsd:anyURI;
  skos:definition "A layer or body of unfrozen ground entirely surrounded by perennially frozen ground (see Figure 11)."@en;
  skos:inScheme <https://w3id.org/permafrost/v/nrcglossary/scheme>;
  skos:prefLabel "isolated talik"@en;
  skos:scopeNote "Isolated taliks are commonly cryotic (see isolated cryopeg), but they may be noncryotic (see transient talik)."@en;
  skos:topConceptOf <https://w3id.org/permafrost/v/nrcglossary/scheme> .

<https://w3id.org/permafrost/v/nrcglossary/t0185> a skos:Concept;
  dct:identifier "t0185"^^xsd:token;
  dct:source "https://nrc-publications.canada.ca/eng/view/object/?id=69fb8993-1baa-4225-b33a-6a02341d383d"^^xsd:anyURI,
    "https://nrc-publications.canada.ca/fra/voir/objet/?id=549123c3-092c-4fca-8dea-99d53eac06dd"^^xsd:anyURI;
  skos:definition "A general term for all types of coarse clastic formations on slopes of 2-3 to 40 degrees, moving downslope mainly due to creep."@en;
  skos:inScheme <https://w3id.org/permafrost/v/nrcglossary/scheme>;
  skos:prefLabel "kurum"@en;
  skos:scopeNote "This Russian term, used extensively in Siberia, covers \"stone streams\", \"rock streams\", \"rock covers\", and \"rock fields\"."@en;
  skos:topConceptOf <https://w3id.org/permafrost/v/nrcglossary/scheme> .

<https://w3id.org/permafrost/v/nrcglossary/t0186> a skos:Concept;
  dct:identifier "t0186"^^xsd:token;
  dct:source "https://nrc-publications.canada.ca/eng/view/object/?id=69fb8993-1baa-4225-b33a-6a02341d383d"^^xsd:anyURI,
    "https://nrc-publications.canada.ca/fra/voir/objet/?id=549123c3-092c-4fca-8dea-99d53eac06dd"^^xsd:anyURI;
  skos:definition "A layer or body of unfrozen ground occupying a depression in the permafrost table beneath a lake."@en;
  skos:inScheme <https://w3id.org/permafrost/v/nrcglossary/scheme>;
  skos:prefLabel "lake talik"@en;
  skos:scopeNote "The temperature of a lake talik remains above 0°C due to the heat storage effect of the lake water. Depending on the permafrost thickness and the size of the lake, such taliks may be either open or closed."@en;
  skos:topConceptOf <https://w3id.org/permafrost/v/nrcglossary/scheme> .

<https://w3id.org/permafrost/v/nrcglossary/t0187> a skos:Concept;
  dct:identifier "t0187"^^xsd:token;
  dct:source "https://nrc-publications.canada.ca/eng/view/object/?id=69fb8993-1baa-4225-b33a-6a02341d383d"^^xsd:anyURI,
    "https://nrc-publications.canada.ca/fra/voir/objet/?id=549123c3-092c-4fca-8dea-99d53eac06dd"^^xsd:anyURI;
  skos:definition "The amount of heat required to melt all the ice (or freeze all the pore water) in a unit mass of soil or rock."@en;
  skos:inScheme <https://w3id.org/permafrost/v/nrcglossary/scheme>;
  skos:prefLabel "latent heat (of fusion)"@en;
  skos:topConceptOf <https://w3id.org/permafrost/v/nrcglossary/scheme> .

<https://w3id.org/permafrost/v/nrcglossary/t0188> a skos:Concept;
  dct:identifier "t0188"^^xsd:token;
  dct:source "https://nrc-publications.canada.ca/eng/view/object/?id=69fb8993-1baa-4225-b33a-6a02341d383d"^^xsd:anyURI,
    "https://nrc-publications.canada.ca/fra/voir/objet/?id=549123c3-092c-4fca-8dea-99d53eac06dd"^^xsd:anyURI;
  skos:definition "A layer or body of unfrozen ground, overlain and underlain by perennially frozen ground (see Figure 11)."@en;
  skos:inScheme <https://w3id.org/permafrost/v/nrcglossary/scheme>;
  skos:prefLabel "lateral talik"@en;
  skos:scopeNote "Lateral taliks may be cryotic (see hydrochemical talik) or noncryotic (see hydrothermal talik)."@en;
  skos:topConceptOf <https://w3id.org/permafrost/v/nrcglossary/scheme> .

<https://w3id.org/permafrost/v/nrcglossary/t0189> a skos:Concept;
  dct:identifier "t0189"^^xsd:token;
  dct:source "https://nrc-publications.canada.ca/eng/view/object/?id=69fb8993-1baa-4225-b33a-6a02341d383d"^^xsd:anyURI,
    "https://nrc-publications.canada.ca/fra/voir/objet/?id=549123c3-092c-4fca-8dea-99d53eac06dd"^^xsd:anyURI;
  skos:definition "The southernmost (northernmost) latitude at which permafrost occurs in a lowland region in the northern (southern) hemisphere."@en;
  skos:inScheme <https://w3id.org/permafrost/v/nrcglossary/scheme>;
  skos:prefLabel "latitudinal limit of permafrost"@en;
  skos:topConceptOf <https://w3id.org/permafrost/v/nrcglossary/scheme> .

<https://w3id.org/permafrost/v/nrcglossary/t0190> a skos:Concept;
  dct:identifier "t0190"^^xsd:token;
  dct:source "https://nrc-publications.canada.ca/eng/view/object/?id=69fb8993-1baa-4225-b33a-6a02341d383d"^^xsd:anyURI,
    "https://nrc-publications.canada.ca/fra/voir/objet/?id=549123c3-092c-4fca-8dea-99d53eac06dd"^^xsd:anyURI;
  skos:definition "The subdivision of a permafrost region into permafrost zones, based on the percentage of the area that is underlain by permafrost."@en;
  skos:inScheme <https://w3id.org/permafrost/v/nrcglossary/scheme>;
  skos:prefLabel "latitudinal zonation of permafrost"@en;
  skos:topConceptOf <https://w3id.org/permafrost/v/nrcglossary/scheme> .

<https://w3id.org/permafrost/v/nrcglossary/t0191> a skos:Concept;
  dct:identifier "t0191"^^xsd:token;
  dct:source "https://nrc-publications.canada.ca/eng/view/object/?id=69fb8993-1baa-4225-b33a-6a02341d383d"^^xsd:anyURI,
    "https://nrc-publications.canada.ca/fra/voir/objet/?id=549123c3-092c-4fca-8dea-99d53eac06dd"^^xsd:anyURI;
  skos:definition "The cryostructure of frozen silt or loam in which ice layers alternate with mineral layers that have a massive cryostructure (see Figure 9e)."@en;
  skos:inScheme <https://w3id.org/permafrost/v/nrcglossary/scheme>;
  skos:prefLabel "layered cryostructure"@en;
  skos:scopeNote "Silt or loam with a layered cryostructure has a relatively high ice content."@en;
  skos:topConceptOf <https://w3id.org/permafrost/v/nrcglossary/scheme> .

<https://w3id.org/permafrost/v/nrcglossary/t0192> a skos:Concept;
  dct:identifier "t0192"^^xsd:token;
  dct:source "https://nrc-publications.canada.ca/eng/view/object/?id=69fb8993-1baa-4225-b33a-6a02341d383d"^^xsd:anyURI,
    "https://nrc-publications.canada.ca/fra/voir/objet/?id=549123c3-092c-4fca-8dea-99d53eac06dd"^^xsd:anyURI;
  skos:definition "Ground ice occurring as ice lenses."@en;
  skos:inScheme <https://w3id.org/permafrost/v/nrcglossary/scheme>;
  skos:prefLabel "lens ice"@en;
  skos:topConceptOf <https://w3id.org/permafrost/v/nrcglossary/scheme> .

<https://w3id.org/permafrost/v/nrcglossary/t0193> a skos:Concept;
  dct:identifier "t0193"^^xsd:token;
  dct:source "https://nrc-publications.canada.ca/eng/view/object/?id=69fb8993-1baa-4225-b33a-6a02341d383d"^^xsd:anyURI,
    "https://nrc-publications.canada.ca/fra/voir/objet/?id=549123c3-092c-4fca-8dea-99d53eac06dd"^^xsd:anyURI;
  skos:definition "The cryostructure of frozen silt or loam containing numerous ice lenses (see Figure 9e)."@en;
  skos:inScheme <https://w3id.org/permafrost/v/nrcglossary/scheme>;
  skos:prefLabel "lens-type cryostructure"@en;
  skos:scopeNote "Silt or loam with a lens-type cryostructure has a relatively high ice content."@en;
  skos:topConceptOf <https://w3id.org/permafrost/v/nrcglossary/scheme> .

<https://w3id.org/permafrost/v/nrcglossary/t0194> a skos:Concept;
  dct:identifier "t0194"^^xsd:token;
  dct:source "https://nrc-publications.canada.ca/eng/view/object/?id=69fb8993-1baa-4225-b33a-6a02341d383d"^^xsd:anyURI,
    "https://nrc-publications.canada.ca/fra/voir/objet/?id=549123c3-092c-4fca-8dea-99d53eac06dd"^^xsd:anyURI;
  skos:definition "The failure strength of a material after a long period of creep deformation."@en;
  skos:inScheme <https://w3id.org/permafrost/v/nrcglossary/scheme>;
  skos:prefLabel "long-term strength"@en;
  skos:scopeNote "It is sometimes defined in practice as the creep strength (or the delayed strength) related to the service life of a structure, but its general definition is the failure strength attained when the strain rate tends to zero or time tends to infinity."@en;
  skos:topConceptOf <https://w3id.org/permafrost/v/nrcglossary/scheme> .

<https://w3id.org/permafrost/v/nrcglossary/t0195> a skos:Concept;
  dct:identifier "t0195"^^xsd:token;
  dct:source "https://nrc-publications.canada.ca/eng/view/object/?id=69fb8993-1baa-4225-b33a-6a02341d383d"^^xsd:anyURI,
    "https://nrc-publications.canada.ca/fra/voir/objet/?id=549123c3-092c-4fca-8dea-99d53eac06dd"^^xsd:anyURI;
  skos:definition "An ice-wedge polygon in which thawing of ice-rich permafrost has left the central area in a relatively depressed position."@en;
  skos:inScheme <https://w3id.org/permafrost/v/nrcglossary/scheme>;
  skos:prefLabel "low-centre polygon"@en;
  skos:topConceptOf <https://w3id.org/permafrost/v/nrcglossary/scheme> .

<https://w3id.org/permafrost/v/nrcglossary/t0196> a skos:Concept;
  dct:identifier "t0196"^^xsd:token;
  dct:source "https://nrc-publications.canada.ca/eng/view/object/?id=69fb8993-1baa-4225-b33a-6a02341d383d"^^xsd:anyURI,
    "https://nrc-publications.canada.ca/fra/voir/objet/?id=549123c3-092c-4fca-8dea-99d53eac06dd"^^xsd:anyURI;
  skos:definition "Macro-scale polygons are closed, multi-sided, roughly equidimensional patterned-ground features, typically 15 to 30 m across, commonly resulting from thermal contraction cracking of the ground."@en;
  skos:inScheme <https://w3id.org/permafrost/v/nrcglossary/scheme>;
  skos:prefLabel "macro-scale polygons"@en;
  skos:scopeNote "Macro-scale polygons form random or oriented polygonal patterns in both mineral terrain and peatland in permafrost areas."@en;
  skos:topConceptOf <https://w3id.org/permafrost/v/nrcglossary/scheme> .

<https://w3id.org/permafrost/v/nrcglossary/t0197> a skos:Concept;
  dct:identifier "t0197"^^xsd:token;
  dct:source "https://nrc-publications.canada.ca/eng/view/object/?id=69fb8993-1baa-4225-b33a-6a02341d383d"^^xsd:anyURI,
    "https://nrc-publications.canada.ca/fra/voir/objet/?id=549123c3-092c-4fca-8dea-99d53eac06dd"^^xsd:anyURI;
  skos:definition "A layer or body of unfrozen ground, that is perennially cryotic (T < 0°C), forming part of coastal or subsea permafrost (see Figure 11)."@en;
  skos:inScheme <https://w3id.org/permafrost/v/nrcglossary/scheme>;
  skos:prefLabel "marine cryopeg"@en;
  skos:scopeNote "Freezing of a marine cryopeg is prevented by freezing-point depression due to the high dissolved-solids content of its pore water."@en;
  skos:topConceptOf <https://w3id.org/permafrost/v/nrcglossary/scheme> .

<https://w3id.org/permafrost/v/nrcglossary/t0198> a skos:Concept;
  dct:identifier "t0198"^^xsd:token;
  dct:source "https://nrc-publications.canada.ca/eng/view/object/?id=69fb8993-1baa-4225-b33a-6a02341d383d"^^xsd:anyURI,
    "https://nrc-publications.canada.ca/fra/voir/objet/?id=549123c3-092c-4fca-8dea-99d53eac06dd"^^xsd:anyURI;
  skos:definition "Downslope movement of soil or rock on, or near, the earth's surface under the influence of gravity (see Figure 21)."@en;
  skos:inScheme <https://w3id.org/permafrost/v/nrcglossary/scheme>;
  skos:prefLabel "mass wasting"@en, "mouvement de masse"@fr;
  skos:scopeNote "Mass wasting includes slow displacements such as frost creep, gelifluction or solifluction, and more rapid movements such as earthflows or active-layer failures. It does not include crustal displacements resulting from tectonic activity or those movements where material is carried directly by an active transporting medium, such as glacial ice, snow, water or air. In permafrost areas, mass wasting is not limited to the active layer; it can include displacements caused by the formation and creep of ground ice within permafrost. When frost heave is a component of frost creep, it is a mass wasting process."@en;
  skos:topConceptOf <https://w3id.org/permafrost/v/nrcglossary/scheme> .

<https://w3id.org/permafrost/v/nrcglossary/t0199> a skos:Concept;
  dct:identifier "t0199"^^xsd:token;
  dct:source "https://nrc-publications.canada.ca/eng/view/object/?id=69fb8993-1baa-4225-b33a-6a02341d383d"^^xsd:anyURI,
    "https://nrc-publications.canada.ca/fra/voir/objet/?id=549123c3-092c-4fca-8dea-99d53eac06dd"^^xsd:anyURI;
  skos:definition "The cryostructure of frozen silt or loam in which ice veins form an irregular three-dimensional network (see Figure 9e)."@en;
  skos:inScheme <https://w3id.org/permafrost/v/nrcglossary/scheme>;
  skos:prefLabel "massive-agglomerate cryostructure"@en;
  skos:scopeNote "Massive-agglomerate cryostructure is characterized by a relative high ice content."@en;
  skos:topConceptOf <https://w3id.org/permafrost/v/nrcglossary/scheme> .

<https://w3id.org/permafrost/v/nrcglossary/t0200> a skos:Concept;
  dct:identifier "t0200"^^xsd:token;
  dct:source "https://nrc-publications.canada.ca/eng/view/object/?id=69fb8993-1baa-4225-b33a-6a02341d383d"^^xsd:anyURI,
    "https://nrc-publications.canada.ca/fra/voir/objet/?id=549123c3-092c-4fca-8dea-99d53eac06dd"^^xsd:anyURI;
  skos:definition "The cryostructure of frozen sand in which all mineral particles are bonded together by ice, and all pore spaces completely filled with ice (see Figure 9e)."@en;
  skos:inScheme <https://w3id.org/permafrost/v/nrcglossary/scheme>;
  skos:prefLabel "massive cryostructure"@en;
  skos:scopeNote "Massive cryostructure is characterized by the predominance of pore ice."@en;
  skos:topConceptOf <https://w3id.org/permafrost/v/nrcglossary/scheme> .

<https://w3id.org/permafrost/v/nrcglossary/t0201> a skos:Concept;
  dct:identifier "t0201"^^xsd:token;
  dct:source "https://nrc-publications.canada.ca/eng/view/object/?id=69fb8993-1baa-4225-b33a-6a02341d383d"^^xsd:anyURI,
    "https://nrc-publications.canada.ca/fra/voir/objet/?id=549123c3-092c-4fca-8dea-99d53eac06dd"^^xsd:anyURI;
  skos:definition "A comprehensive term used to describe large masses of ground ice, including ice wedges, pingo ice, buried ice and large ice lenses (see Figure 10d, e, f)."@en;
  skos:inScheme <https://w3id.org/permafrost/v/nrcglossary/scheme>;
  skos:prefLabel "massive ice"@en;
  skos:scopeNote "Massive ice beds typically have an ice content of at least 250 percent (on an ice-to-dry-soil weight basis). If the ice content is less than 250 percent, the beds are better termed \"massive icy beds\". Some massive ice beds are more than 40 m thick and 2 km in horizontal extent, and some are responsible for prominent topographic rises."@en;
  skos:topConceptOf <https://w3id.org/permafrost/v/nrcglossary/scheme> .

<https://w3id.org/permafrost/v/nrcglossary/t0202> a skos:Concept;
  dct:identifier "t0202"^^xsd:token;
  dct:source "https://nrc-publications.canada.ca/eng/view/object/?id=69fb8993-1baa-4225-b33a-6a02341d383d"^^xsd:anyURI,
    "https://nrc-publications.canada.ca/fra/voir/objet/?id=549123c3-092c-4fca-8dea-99d53eac06dd"^^xsd:anyURI;
  skos:definition "The cryostructure of frozen sand and gravel in which all mineral particles are bonded together with ice, but larger pore spaces are not completely filled with ice (see Figure 9e)."@en;
  skos:inScheme <https://w3id.org/permafrost/v/nrcglossary/scheme>;
  skos:prefLabel "massive-porous cryostructure"@en;
  skos:scopeNote "Massive-porous cryostructure is characterized by the predominance of pore ice and a relatively low ice content."@en;
  skos:topConceptOf <https://w3id.org/permafrost/v/nrcglossary/scheme> .

<https://w3id.org/permafrost/v/nrcglossary/t0203> a skos:Concept;
  dct:identifier "t0203"^^xsd:token;
  dct:source "https://nrc-publications.canada.ca/eng/view/object/?id=69fb8993-1baa-4225-b33a-6a02341d383d"^^xsd:anyURI,
    "https://nrc-publications.canada.ca/fra/voir/objet/?id=549123c3-092c-4fca-8dea-99d53eac06dd"^^xsd:anyURI;
  skos:definition "Mean annual temperature of the surface of the ground."@en;
  skos:inScheme <https://w3id.org/permafrost/v/nrcglossary/scheme>;
  skos:prefLabel "mean annual ground-surface temperature (MAGST)"@en;
  skos:scopeNote "Permafrost exists if the mean annual ground-surface temperature is perennially below 0°C. Although the mean annual surface temperature may be below 0°C, the surface temperature will fluctuate during the year, causing a layer of ground immediately beneath the surface to thaw in the summer and freeze in the winter (the active layer). Small changes in the annual range of surface temperature and in the mean annual surface temperature from year to year, or over a period of a few years, may cause a layer of ground between the bottom of the active layer and the permafrost table to remain at a temperature above 0°C, creating a talik or residual thaw layer."@en;
  skos:topConceptOf <https://w3id.org/permafrost/v/nrcglossary/scheme> .

<https://w3id.org/permafrost/v/nrcglossary/t0204> a skos:Concept;
  dct:identifier "t0204"^^xsd:token;
  dct:source "https://nrc-publications.canada.ca/eng/view/object/?id=69fb8993-1baa-4225-b33a-6a02341d383d"^^xsd:anyURI,
    "https://nrc-publications.canada.ca/fra/voir/objet/?id=549123c3-092c-4fca-8dea-99d53eac06dd"^^xsd:anyURI;
  skos:definition "Mean annual temperature of the ground at a particular depth."@en;
  skos:inScheme <https://w3id.org/permafrost/v/nrcglossary/scheme>;
  skos:prefLabel "mean annual ground temperature (MAGT)"@en;
  skos:scopeNote "The mean annual temperature of the ground usually increases with depth below the surface. In some northern areas, however, it is not uncommon to find that the mean annual ground temperature decreases in the upper 50 to 100 metres below the ground surface as a result of past changes in surface and climate conditions. Below that depth, it will increase as a result of the geothermal heat flux from the interior of the earth. The mean annual ground temperature at the depth of zero annual amplitude is often used to assess the thermal regime of the ground at various locations."@en;
  skos:topConceptOf <https://w3id.org/permafrost/v/nrcglossary/scheme> .

<https://w3id.org/permafrost/v/nrcglossary/t0205> a skos:Concept;
  dct:identifier "t0205"^^xsd:token;
  dct:source "https://nrc-publications.canada.ca/eng/view/object/?id=69fb8993-1baa-4225-b33a-6a02341d383d"^^xsd:anyURI,
    "https://nrc-publications.canada.ca/fra/voir/objet/?id=549123c3-092c-4fca-8dea-99d53eac06dd"^^xsd:anyURI;
  skos:definition "The properties of frozen ground governing its deformability and strength."@en;
  skos:inScheme <https://w3id.org/permafrost/v/nrcglossary/scheme>;
  skos:prefLabel "mechanical properties of frozen ground"@en, "propriétés mécaniques du gélisol"@fr;
  skos:scopeNote "1. Properties under quasi-static loading: The behaviour of frozen soils under quasi-static loading is usually different from that of unfrozen soils because of the presence of ice and unfrozen water films. In particular, frozen soils are more susceptible to creep and relaxation effects, and their behaviour is strongly affected by temperature change. In addition to creep, volumetric consolidation may also develop in frozen soils with large unfrozen water contents. As with unfrozen soils, the strength of frozen soils depends on interparticle friction, particle interlocking and cohesion. In frozen soil, however, bonding of particles by ice is the dominant strength factor. This is complicated by the unfrozen water films surrounding the soil particles, which reduce interparticle bonding. The strength of ice in frozen soil is dependent on many factors, such as temperature, pressure, strain rate, grain size, crystal orientation and density. At very high ice contents, frozen soil behaviour under load is similar to that of ice. At low ice contents, however, when interparticle forces begin to contribute, the unfrozen water films play an important role, especially in fine-grained frozen soils. (a) Deformability and strength: The deformability and strength of a frozen soil can be studied by specially designed tests either in a cold room or in situ. Quasi-static elastic parameters usually determined in such tests are: Young's modulus and Poisson's ratio for short- term response, and creep parameters (used in a creep equation) for long-term response. In addition, the variation of strength with time or with strain rate is also determined from the tests. The strength is usually found to vary from a high short- term value to a much smaller long-term value, which is considered to govern the behaviour of frozen soil under sustained loading. Under high confining stresses and at relatively high freezing temperatures, most frozen soils creep and eventually fail in a plastic manner. On the other hand, under compression at low confining stresses, or at tensile stresses combined with low temperatures, many frozen soils fail in a brittle manner by tensile crack propagation. (b) Compressibility of frozen soils: Although frozen soils are usually considered to be practically incompressible, and volume change deformations can therefore be neglected, investigations show, however, that the compressibility of frozen soils can be significant and should not be neglected in some cases, especially when large areas are loaded. Compressibility and its time dependence in frozen soils are due to several causes, such as instantaneous compression of the gaseous phase, creep of the pore ice due to shear stresses at the grain contacts, and hydrodynamic consolidation due to the expulsion of unfrozen water under stress, the amount of which varies with the applied pressure. 2. Dynamic properties of frozen ground: Information on the dynamic properties of frozen soils is important with regard to the behaviour of structures subjected to seismic or vibratory loads, and the evaluation of results of seismic field surveys in permafrost areas. Dynamic properties are expressed either in terms of two dynamic elastic parameters: the dynamic modulus of elasticity and the dynamic Poisson's ratio, or in terms of the propagation velocities of compressional waves and shear waves in the material. The two sets of dynamic parameters are uniquely related by the theory of elasticity. The dynamic elastic parameters deduced from wave propagation velocities are different from those obtained from any type of static loading tests because the latter contain the additional effects of elastic relaxation and creep. Parameters that influence the compressional and shear wave velocities in soils and rocks include grain size, lithology, total water content, porosity and pore structure, the nature, temperature and degree of freezing of the interstitial water, degree of cementation, and confining pressure. Due to the ice content, seismic velocities are generally higher in frozen soils or rocks than in the same unfrozen materials. The change in velocity can occur gradually as temperatures decrease below 0°C, if freezing point depression conditions exist in the soil."@en;
  skos:topConceptOf <https://w3id.org/permafrost/v/nrcglossary/scheme> .

<https://w3id.org/permafrost/v/nrcglossary/t0206> a skos:Concept;
  dct:identifier "t0206"^^xsd:token;
  dct:source "https://nrc-publications.canada.ca/eng/view/object/?id=69fb8993-1baa-4225-b33a-6a02341d383d"^^xsd:anyURI,
    "https://nrc-publications.canada.ca/fra/voir/objet/?id=549123c3-092c-4fca-8dea-99d53eac06dd"^^xsd:anyURI;
  skos:definition "The failure strength of a material under given loading conditions."@en;
  skos:inScheme <https://w3id.org/permafrost/v/nrcglossary/scheme>;
  skos:prefLabel "mechanical strength"@en;
  skos:topConceptOf <https://w3id.org/permafrost/v/nrcglossary/scheme> .

<https://w3id.org/permafrost/v/nrcglossary/t0207> a skos:Concept;
  dct:identifier "t0207"^^xsd:token;
  dct:source "https://nrc-publications.canada.ca/eng/view/object/?id=69fb8993-1baa-4225-b33a-6a02341d383d"^^xsd:anyURI,
    "https://nrc-publications.canada.ca/fra/voir/objet/?id=549123c3-092c-4fca-8dea-99d53eac06dd"^^xsd:anyURI;
  skos:definition "Micro-scale polygons are closed, multi-sided, roughly equidimensional patterned-ground features, less than 2 m in diameter, usually caused by desiccation cracking of fine-grained soil materials."@en;
  skos:inScheme <https://w3id.org/permafrost/v/nrcglossary/scheme>;
  skos:prefLabel "micro-scale polygon"@en;
  skos:topConceptOf <https://w3id.org/permafrost/v/nrcglossary/scheme> .

<https://w3id.org/permafrost/v/nrcglossary/t0208> a skos:Concept;
  dct:identifier "t0208"^^xsd:token;
  dct:source "https://nrc-publications.canada.ca/eng/view/object/?id=69fb8993-1baa-4225-b33a-6a02341d383d"^^xsd:anyURI,
    "https://nrc-publications.canada.ca/fra/voir/objet/?id=549123c3-092c-4fca-8dea-99d53eac06dd"^^xsd:anyURI;
  skos:definition "A palsa in which the frozen core extends below the peat into underlying mineral material."@en;
  skos:inScheme <https://w3id.org/permafrost/v/nrcglossary/scheme>;
  skos:prefLabel "minerogenic palsa"@en;
  skos:scopeNote "Palsas were originally regarded as having developed completely in peat (Fries and Bergström, 1910). Later it was found that such true palsas are relatively rare, and that the frozen core in most palsa-like landforms extends down into mineral layers (Lundqvist, 1962; Lundqvist and Mattsson, 1965; Wramner, 1965). Fosgren (1966) and Åhman (1977) also reported \"palsas\" developed entirely in mineral soil, and they called both types \"minerogenic palsas\". Harris (1993) described a sequence of stages in the development of palsa-like mounds developed entirely in mineral soils in the Fox Lake area (Yukon), for which he proposed the name \"lithalsa\". He suggested a new name was needed, because the heat- and moisture-transport processes in mineral soils differ from those in peat (Brown, 1970a)."@en;
  skos:topConceptOf <https://w3id.org/permafrost/v/nrcglossary/scheme> .

<https://w3id.org/permafrost/v/nrcglossary/t0209> a skos:Concept;
  dct:identifier "t0209"^^xsd:token;
  dct:source "https://nrc-publications.canada.ca/eng/view/object/?id=69fb8993-1baa-4225-b33a-6a02341d383d"^^xsd:anyURI,
    "https://nrc-publications.canada.ca/fra/voir/objet/?id=549123c3-092c-4fca-8dea-99d53eac06dd"^^xsd:anyURI;
  skos:definition "Permafrost existing at high altitudes in high, middle, and low latitudes (see Figure 1)."@en;
  skos:hiddenLabel "alpine permafrost"@en, "high-altitude permafrost"@en;
  skos:inScheme <https://w3id.org/permafrost/v/nrcglossary/scheme>;
  skos:prefLabel "mountain permafrost"@en;
  skos:scopeNote "Mountain permafrost may show some degree of altitudinal zonation. Mountain permafrost grades into the permafrost of high latitudes in areas such as the North American Cordillera. Plateau permafrost is a subdivision of mountain permafrost but use of this term is not recommended."@en;
  skos:topConceptOf <https://w3id.org/permafrost/v/nrcglossary/scheme> .

<https://w3id.org/permafrost/v/nrcglossary/t0210> a skos:Concept;
  dct:identifier "t0210"^^xsd:token;
  dct:source "https://nrc-publications.canada.ca/eng/view/object/?id=69fb8993-1baa-4225-b33a-6a02341d383d"^^xsd:anyURI,
    "https://nrc-publications.canada.ca/fra/voir/objet/?id=549123c3-092c-4fca-8dea-99d53eac06dd"^^xsd:anyURI;
  skos:altLabel "mud boil"@en;
  skos:definition "A type of nonsorted circle developed in fine-grained materials."@en;
  skos:inScheme <https://w3id.org/permafrost/v/nrcglossary/scheme>;
  skos:prefLabel "mud circle"@en;
  skos:topConceptOf <https://w3id.org/permafrost/v/nrcglossary/scheme> .

<https://w3id.org/permafrost/v/nrcglossary/t0211> a skos:Concept;
  dct:identifier "t0211"^^xsd:token;
  dct:source "https://nrc-publications.canada.ca/eng/view/object/?id=69fb8993-1baa-4225-b33a-6a02341d383d"^^xsd:anyURI,
    "https://nrc-publications.canada.ca/fra/voir/objet/?id=549123c3-092c-4fca-8dea-99d53eac06dd"^^xsd:anyURI;
  skos:definition "A type of mass movement associated with shear failure in unfrozen sediments underlying permafrost, leading to detachment of blocks of frozen ground that move downslope."@en;
  skos:inScheme <https://w3id.org/permafrost/v/nrcglossary/scheme>;
  skos:prefLabel "glissement régressifmultiple"@fr, "multiple retrogressive slide"@en;
  skos:scopeNote "A degree of back-tilting or rotation of the failure components may be involved."@en;
  skos:topConceptOf <https://w3id.org/permafrost/v/nrcglossary/scheme> .

<https://w3id.org/permafrost/v/nrcglossary/t0212> a skos:Concept;
  dct:identifier "t0212"^^xsd:token;
  dct:source "https://nrc-publications.canada.ca/eng/view/object/?id=69fb8993-1baa-4225-b33a-6a02341d383d"^^xsd:anyURI,
    "https://nrc-publications.canada.ca/fra/voir/objet/?id=549123c3-092c-4fca-8dea-99d53eac06dd"^^xsd:anyURI;
  skos:definition "The ratio of the surface freezing or thawing index to the air freezing or thawing index."@en;
  skos:inScheme <https://w3id.org/permafrost/v/nrcglossary/scheme>;
  skos:prefLabel "facteur n"@fr, "n-factor"@en;
  skos:scopeNote "At any site, (standard) air temperatures are seldom the same as surface (air/substrate boundary) temperatures. Because air temperatures (measured at weather stations) are usually available and surface temperatures are not, the n- factor (an empirically determined coefficient) is used to relate air temperatures to surface temperatures in order to establish the thermal boundary condition at the surface, particularly for engineering purposes. The difference between air and surface temperatures at any specific time and location is greatly influenced by climatic, surface and subsurface conditions (e.g., latitude, cloud cover, time of day or year, relative humidity, wind speed, type of surface--wet, dry, moss, snow, natural vegetated terrain, mineral soil, pavements-- and thermal properties of the ground). The average surface temperature and n- factor may vary significantly from year to year, even for a given surface and location, as well as for different sites, surfaces and soil systems. Values of the freezing and thawing n-factors have been determined for a large number of sites and surfaces and are widely used for predicting surface temperatures and the thermal regime of the ground. The data vary widely, however, and indicate that a rigorous value of n for a given site cannot simply be chosen from these data. Direct determination of the n-factor for a specific location is much better and requires concurrent observations of air and surface temperatures throughout at least one and preferably several complete freezing and thawing seasons."@en;
  skos:topConceptOf <https://w3id.org/permafrost/v/nrcglossary/scheme> .

<https://w3id.org/permafrost/v/nrcglossary/t0213> a skos:Concept;
  dct:identifier "t0213"^^xsd:token;
  dct:source "https://nrc-publications.canada.ca/eng/view/object/?id=69fb8993-1baa-4225-b33a-6a02341d383d"^^xsd:anyURI,
    "https://nrc-publications.canada.ca/fra/voir/objet/?id=549123c3-092c-4fca-8dea-99d53eac06dd"^^xsd:anyURI;
  skos:definition "Thin, elongated ice crystals that form perpendicular to the ground surface (see Figure 10g)."@en;
  skos:inScheme <https://w3id.org/permafrost/v/nrcglossary/scheme>;
  skos:prefLabel "needle ice"@en;
  skos:scopeNote "Needle ice forms during nights when there is extensive radiative cooling, causing ice segregation in the surface layer of the soil. The needles can form under stones, soil peds, moss or other surface vegetation and are best developed in alpine areas with maritime temperate climates where silty or organic soils are present. They can also form on coarse-grained, porous volcanic ejectamenta (e.g., in British Columbia and Iceland). The Swedish term \"pipkrake\" is sometimes used to describe needle ice."@en;
  skos:topConceptOf <https://w3id.org/permafrost/v/nrcglossary/scheme> .

<https://w3id.org/permafrost/v/nrcglossary/t0214> a skos:Concept;
  dct:identifier "t0214"^^xsd:token;
  dct:source "https://nrc-publications.canada.ca/eng/view/object/?id=69fb8993-1baa-4225-b33a-6a02341d383d"^^xsd:anyURI,
    "https://nrc-publications.canada.ca/fra/voir/objet/?id=549123c3-092c-4fca-8dea-99d53eac06dd"^^xsd:anyURI;
  skos:definition "Soil or rock at temperatures above 0°C (see Figures 2 and 3)."@en;
  skos:inScheme <https://w3id.org/permafrost/v/nrcglossary/scheme>;
  skos:prefLabel "noncryotic ground"@en, "sol non cryotique"@fr;
  skos:scopeNote "Noncryotic ground is not synonymous with thawed ground (which implies an earlier frozen state), nor with unfrozen ground (the temperature of which may be below 0°C)."@en;
  skos:topConceptOf <https://w3id.org/permafrost/v/nrcglossary/scheme> .

<https://w3id.org/permafrost/v/nrcglossary/t0215> a skos:Concept;
  dct:identifier "t0215"^^xsd:token;
  dct:source "https://nrc-publications.canada.ca/eng/view/object/?id=69fb8993-1baa-4225-b33a-6a02341d383d"^^xsd:anyURI,
    "https://nrc-publications.canada.ca/fra/voir/objet/?id=549123c3-092c-4fca-8dea-99d53eac06dd"^^xsd:anyURI;
  skos:definition "A nonsorted circle is a patterned ground form that is equidimensional in several directions, with a dominantly circular outline which lacks a border of stones."@en;
  skos:inScheme <https://w3id.org/permafrost/v/nrcglossary/scheme>;
  skos:prefLabel "nonsorted circle"@en;
  skos:scopeNote "Nonsorted circles characteristically have margins of vegetation; they occur singly or in groups; their diameter is commonly between 0.5 and 3.0 m. Their central areas tend to be slightly dome-shaped and may be cracked into small nonsorted polygons. In places, the long axes of stones and sand particles tend toward vertical. The term covers both mud circles, developed in fine-grained materials, and stony earth circles, developed in gravelly materials."@en;
  skos:topConceptOf <https://w3id.org/permafrost/v/nrcglossary/scheme> .

<https://w3id.org/permafrost/v/nrcglossary/t0216> a skos:Concept;
  dct:identifier "t0216"^^xsd:token;
  dct:source "https://nrc-publications.canada.ca/eng/view/object/?id=69fb8993-1baa-4225-b33a-6a02341d383d"^^xsd:anyURI,
    "https://nrc-publications.canada.ca/fra/voir/objet/?id=549123c3-092c-4fca-8dea-99d53eac06dd"^^xsd:anyURI;
  skos:definition "A nonsorted net is a type of patterned ground with cells that are equidimensional in several directions, neither dominantly circular nor polygonal, and lacking borders of stones."@en;
  skos:inScheme <https://w3id.org/permafrost/v/nrcglossary/scheme>;
  skos:prefLabel "nonsorted net"@en;
  skos:scopeNote "Nonsorted nets occur on nearly horizontal surfaces. Diameters of individual cells range from 0.5 to as much as 10 m. Where vegetation is sparse, it is generally concentrated in furrows bordering the individual cells of the net, emphasizing the pattern."@en;
  skos:topConceptOf <https://w3id.org/permafrost/v/nrcglossary/scheme> .

<https://w3id.org/permafrost/v/nrcglossary/t0217> a skos:Concept;
  dct:identifier "t0217"^^xsd:token;
  dct:source "https://nrc-publications.canada.ca/eng/view/object/?id=69fb8993-1baa-4225-b33a-6a02341d383d"^^xsd:anyURI,
    "https://nrc-publications.canada.ca/fra/voir/objet/?id=549123c3-092c-4fca-8dea-99d53eac06dd"^^xsd:anyURI;
  skos:definition "A nonsorted polygon is a patterned ground form that is equidimensional in several directions, with a dominantly polygonal outline which lacks a border of stones."@en;
  skos:inScheme <https://w3id.org/permafrost/v/nrcglossary/scheme>;
  skos:prefLabel "nonsorted polygon"@en;
  skos:scopeNote "Nonsorted polygons commonly occur in extensive patterns, most frequently on nearly horizontal surfaces (although small forms have been found on slopes up to 27?; large ones have been found on slopes as steep as 31? in polar regions). Micro- scale polygons range in size from 5 cm to about 1 m; macro-scale polygons may be more than 100 m in diameter. Where vegetation is sparse, it is generally concentrated in furrows along the borders between the polygons, emphasizing the pattern. The mineral soil can be well-sorted fines, sand, gravel, or a mixture."@en;
  skos:topConceptOf <https://w3id.org/permafrost/v/nrcglossary/scheme> .

<https://w3id.org/permafrost/v/nrcglossary/t0218> a skos:Concept;
  dct:identifier "t0218"^^xsd:token;
  dct:source "https://nrc-publications.canada.ca/eng/view/object/?id=69fb8993-1baa-4225-b33a-6a02341d383d"^^xsd:anyURI,
    "https://nrc-publications.canada.ca/fra/voir/objet/?id=549123c3-092c-4fca-8dea-99d53eac06dd"^^xsd:anyURI;
  skos:definition "A nonsorted step is a patterned ground feature with a step-like form and a downslope border of vegetation embanking an area of relatively bare ground upslope."@en;
  skos:inScheme <https://w3id.org/permafrost/v/nrcglossary/scheme>;
  skos:prefLabel "nonsorted step"@en;
  skos:scopeNote "Nonsorted steps are only found on slopes, commonly ranging from 5? to 15?; their downslope border forms a low riser fronting a tread whose slope is less than the general slope. Nonsorted steps are assumed to be derived from nonsorted nets or hummocks or nonsorted polygons, rather than to develop independently."@en;
  skos:topConceptOf <https://w3id.org/permafrost/v/nrcglossary/scheme> .

<https://w3id.org/permafrost/v/nrcglossary/t0219> a skos:Concept;
  dct:identifier "t0219"^^xsd:token;
  dct:source "https://nrc-publications.canada.ca/eng/view/object/?id=69fb8993-1baa-4225-b33a-6a02341d383d"^^xsd:anyURI,
    "https://nrc-publications.canada.ca/fra/voir/objet/?id=549123c3-092c-4fca-8dea-99d53eac06dd"^^xsd:anyURI;
  skos:definition "Nonsorted stripes form patterned ground with a striped and nonsorted appearance, due to parallel strips of vegetation-covered ground and intervening strips of relatively bare ground, oriented down the steepest available slope."@en;
  skos:inScheme <https://w3id.org/permafrost/v/nrcglossary/scheme>;
  skos:prefLabel "nonsorted stripe"@en;
  skos:scopeNote "Nonsorted stripes, both large and small, occur on slopes of 5-6?, downslope from nonsorted polygons or nonsorted nets. In some places the vegetated and non- vegetated strips are equally wide; in other places vegetated strips of 0.3-0.6 m are spaced from 3 to 4.5 m apart. They can be several hundred metres long."@en;
  skos:topConceptOf <https://w3id.org/permafrost/v/nrcglossary/scheme> .

<https://w3id.org/permafrost/v/nrcglossary/t0220> a skos:Concept;
  dct:identifier "t0220"^^xsd:token;
  dct:source "https://nrc-publications.canada.ca/eng/view/object/?id=69fb8993-1baa-4225-b33a-6a02341d383d"^^xsd:anyURI,
    "https://nrc-publications.canada.ca/fra/voir/objet/?id=549123c3-092c-4fca-8dea-99d53eac06dd"^^xsd:anyURI;
  skos:altLabel "continental permafrost"@en;
  skos:definition "Permafrost occurring beneath exposed land surfaces."@en;
  skos:inScheme <https://w3id.org/permafrost/v/nrcglossary/scheme>;
  skos:prefLabel "onshore permafrost"@en;
  skos:scopeNote "Often used to indicate permafrost in coastal land areas, as contrasted with subsea permafrost."@en;
  skos:topConceptOf <https://w3id.org/permafrost/v/nrcglossary/scheme> .

<https://w3id.org/permafrost/v/nrcglossary/t0221> a skos:Concept;
  dct:identifier "t0221"^^xsd:token;
  dct:source "https://nrc-publications.canada.ca/eng/view/object/?id=69fb8993-1baa-4225-b33a-6a02341d383d"^^xsd:anyURI,
    "https://nrc-publications.canada.ca/fra/voir/objet/?id=549123c3-092c-4fca-8dea-99d53eac06dd"^^xsd:anyURI;
  skos:altLabel "sublimation ice"@en;
  skos:definition "Ice formed in an open cavity or crack in the ground by reverse sublimation of water vapour."@en;
  skos:inScheme <https://w3id.org/permafrost/v/nrcglossary/scheme>;
  skos:prefLabel "open-cavity ice"@en;
  skos:scopeNote "Open-cavity ice is similar to hoar frost, except that the ice crystals grow in cavities rather than on the surface. It is common in thermal contraction cracks, mine workings, ice caves and ice cellars in permafrost."@en;
  skos:topConceptOf <https://w3id.org/permafrost/v/nrcglossary/scheme> .

<https://w3id.org/permafrost/v/nrcglossary/t0222> a skos:Concept;
  dct:identifier "t0222"^^xsd:token;
  dct:source "https://nrc-publications.canada.ca/eng/view/object/?id=69fb8993-1baa-4225-b33a-6a02341d383d"^^xsd:anyURI,
    "https://nrc-publications.canada.ca/fra/voir/objet/?id=549123c3-092c-4fca-8dea-99d53eac06dd"^^xsd:anyURI;
  skos:definition "Freezing that occurs under conditions that allow gain or loss of water by the system (see Figure 7)."@en;
  skos:inScheme <https://w3id.org/permafrost/v/nrcglossary/scheme>;
  skos:prefLabel "open-system freezing"@en;
  skos:scopeNote "The effects of open-system freezing can be quite different for different soil materials. During freezing of clean, medium- to coarse-grained materials, some pore water may be expelled ahead of the freezing front (compensating for the volume increase during phase change) thus reducing frost heave. During freezing of fine-grained materials, however, water often migrates to the freezing front, contributing to the formation of segregated ice, thus causing increased frost heave."@en;
  skos:topConceptOf <https://w3id.org/permafrost/v/nrcglossary/scheme> .

<https://w3id.org/permafrost/v/nrcglossary/t0223> a skos:Concept;
  dct:identifier "t0223"^^xsd:token;
  dct:source "https://nrc-publications.canada.ca/eng/view/object/?id=69fb8993-1baa-4225-b33a-6a02341d383d"^^xsd:anyURI,
    "https://nrc-publications.canada.ca/fra/voir/objet/?id=549123c3-092c-4fca-8dea-99d53eac06dd"^^xsd:anyURI;
  skos:altLabel "hydraulic pingo"@en;
  skos:definition "A pingo formed by doming of frozen ground due to freezing of injected water supplied by groundwater moving downslope through taliks to the site of the pingo, where it moves towards the surface (see Figure 19b)."@en;
  skos:hiddenLabel "East Greenland pingo"@en;
  skos:inScheme <https://w3id.org/permafrost/v/nrcglossary/scheme>;
  skos:prefLabel "open-system pingo"@en;
  skos:scopeNote "Most open-system pingos are found in or near areas of marked relief, mainly in the discontinuous permafrost zone. High hydraulic potential, due to water originating in elevated areas, causes repeated injection of water into the weakest portion of the permafrost, followed by freezing. This leads to the development of the massive ice forming the core of the pingo."@en;
  skos:topConceptOf <https://w3id.org/permafrost/v/nrcglossary/scheme> .

<https://w3id.org/permafrost/v/nrcglossary/t0224> a skos:Concept;
  dct:identifier "t0224"^^xsd:token;
  dct:source "https://nrc-publications.canada.ca/eng/view/object/?id=69fb8993-1baa-4225-b33a-6a02341d383d"^^xsd:anyURI,
    "https://nrc-publications.canada.ca/fra/voir/objet/?id=549123c3-092c-4fca-8dea-99d53eac06dd"^^xsd:anyURI;
  skos:definition "A body of unfrozen ground that penetrates the permafrost completely, connecting suprapermafrost and subpermafrost water (see Figure 11)."@en;
  skos:hiddenLabel "penetrating talik"@en, "perforating talik"@en, "piercing talik"@en,
    "through talik"@en;
  skos:inScheme <https://w3id.org/permafrost/v/nrcglossary/scheme>;
  skos:prefLabel "open talik"@en;
  skos:scopeNote "Open taliks can be found below large rivers (see river talik) and lakes (see lake talik). They may be noncryotic (see hydrothermal talik) or cryotic (see hydrochemical talik)."@en;
  skos:topConceptOf <https://w3id.org/permafrost/v/nrcglossary/scheme> .

<https://w3id.org/permafrost/v/nrcglossary/t0225> a skos:Concept;
  dct:identifier "t0225"^^xsd:token;
  dct:source "https://nrc-publications.canada.ca/eng/view/object/?id=69fb8993-1baa-4225-b33a-6a02341d383d"^^xsd:anyURI,
    "https://nrc-publications.canada.ca/fra/voir/objet/?id=549123c3-092c-4fca-8dea-99d53eac06dd"^^xsd:anyURI;
  skos:definition "A distinct soil micromorphology, resulting from the effects of freezing and thawing processes, in which coarser soil particles form circular to ellipsoidal patterns (see Figure 8d)."@en;
  skos:inScheme <https://w3id.org/permafrost/v/nrcglossary/scheme>;
  skos:prefLabel "orbiculic cryogenic fabric"@en;
  skos:scopeNote "This fabric, found in cryosols, results from freeze-thaw processes probably accompanied by cryoturbation."@en;
  skos:topConceptOf <https://w3id.org/permafrost/v/nrcglossary/scheme> .

<https://w3id.org/permafrost/v/nrcglossary/t0226> a skos:Concept;
  dct:identifier "t0226"^^xsd:token;
  dct:source "https://nrc-publications.canada.ca/eng/view/object/?id=69fb8993-1baa-4225-b33a-6a02341d383d"^^xsd:anyURI,
    "https://nrc-publications.canada.ca/fra/voir/objet/?id=549123c3-092c-4fca-8dea-99d53eac06dd"^^xsd:anyURI;
  skos:definition "An organic soil having a surface layer containing more than 17% organic carbon by weight, with permafrost within 1 m below the surface.."@en;
  skos:inScheme <https://w3id.org/permafrost/v/nrcglossary/scheme>;
  skos:prefLabel "organic cryosol"@en;
  skos:scopeNote "Organic cryosol is more than 40°Cm thick, or more than 10°Cm thick over a lithic contact, or more than 10°Cm thick over an ice layer that is at least 30°Cm thick. Organic cryosols have mean annual ground temperatures below 0°C. ."@en;
  skos:topConceptOf <https://w3id.org/permafrost/v/nrcglossary/scheme> .

<https://w3id.org/permafrost/v/nrcglossary/t0227> a skos:Concept;
  dct:identifier "t0227"^^xsd:token;
  dct:source "https://nrc-publications.canada.ca/eng/view/object/?id=69fb8993-1baa-4225-b33a-6a02341d383d"^^xsd:anyURI,
    "https://nrc-publications.canada.ca/fra/voir/objet/?id=549123c3-092c-4fca-8dea-99d53eac06dd"^^xsd:anyURI;
  skos:definition "One of a group of lakes possessing a common, preferred, long-axis orientation (see Figure 22b)."@en;
  skos:inScheme <https://w3id.org/permafrost/v/nrcglossary/scheme>;
  skos:prefLabel "lac orienté"@fr, "oriented lake"@en;
  skos:scopeNote "Oriented lakes appear to develop by differential erosion of permafrost shorelines formed in fine-grained, homogeneous sediments under the influence of predominant winds. In some cases, bedrock structural control may also determine lake orientation. Oriented lakes also occur in non-permafrost environments."@en;
  skos:topConceptOf <https://w3id.org/permafrost/v/nrcglossary/scheme> .

<https://w3id.org/permafrost/v/nrcglossary/t0228> a skos:Concept;
  dct:identifier "t0228"^^xsd:token;
  dct:source "https://nrc-publications.canada.ca/eng/view/object/?id=69fb8993-1baa-4225-b33a-6a02341d383d"^^xsd:anyURI,
    "https://nrc-publications.canada.ca/fra/voir/objet/?id=549123c3-092c-4fca-8dea-99d53eac06dd"^^xsd:anyURI;
  skos:definition "A peaty permafrost mound possessing a core of alternating layers of segregated ice and peat or mineral soil material (see Figures 14 and 15a)."@en;
  skos:hiddenLabel "peat hummock"@en, "peat mound"@en;
  skos:inScheme <https://w3id.org/permafrost/v/nrcglossary/scheme>;
  skos:prefLabel "palsa"@en, "palse"@fr;
  skos:scopeNote "Palsas are typically between 1 and 7 m in height and a few metres to 100 m in diameter. The term is of Fennoscandian origin, originally meaning \". a hummock rising out of a bog with a core of ice\" (Seppälä, 1972). Implicit in this definition are their constructional nature, their origin in wetlands (fens or peat bogs), and that ice segregation in mineral soil beneath peat is the process responsible for growth. Most, but not all, palsas occur in the discontinuous permafrost zone. A more general definition has been proposed by Washburn (1983) in which the term is applied in a descriptive sense to a broader range of permafrost mounds that may include intrusive as well as segregated ice: \"Palsas are peaty permafrost mounds, ranging from about 0.5 to about 10 m in height and exceeding about 2 m in average diameter, comprising (1) aggradation forms due to permafrost aggradation at an active-layer/permafrost contact zone, and (2) similar-appearing degradation forms due to disintegration of an extensive peaty deposit\". The disadvantage of this broader definition is that mounds of entirely different origins (e.g., those including intrusive ice) are grouped under one term. It is proposed, therefore, that the term \"palsa\" be restricted to those features where the internal structure shows the presence of segregated ice and where the environment lacks high hydraulic potentials, provided that other parameters (size, shape, location in wetlands) are also satisfied. The term \"frost mound\" should be used as a non- genetic term to describe the range of morphologically similar, but genetically different, features that occur in permafrost terrain."@en;
  skos:topConceptOf <https://w3id.org/permafrost/v/nrcglossary/scheme> .

<https://w3id.org/permafrost/v/nrcglossary/t0229> a skos:Concept;
  dct:identifier "t0229"^^xsd:token;
  dct:source "https://nrc-publications.canada.ca/eng/view/object/?id=69fb8993-1baa-4225-b33a-6a02341d383d"^^xsd:anyURI,
    "https://nrc-publications.canada.ca/fra/voir/objet/?id=549123c3-092c-4fca-8dea-99d53eac06dd"^^xsd:anyURI;
  skos:altLabel "palsa mire"@en;
  skos:definition "A poorly-drained lowland underlain by organic-rich sediments, which contains perennially frozen peat bodies (peat plateaux) and occasionally palsas."@en;
  skos:inScheme <https://w3id.org/permafrost/v/nrcglossary/scheme>;
  skos:prefLabel "palsa bog"@en;
  skos:scopeNote "Palsa bogs occur in subarctic lowlands and are characteristic of the zone of discontinuous permafrost."@en;
  skos:topConceptOf <https://w3id.org/permafrost/v/nrcglossary/scheme> .

<https://w3id.org/permafrost/v/nrcglossary/t0230> a skos:Concept;
  dct:identifier "t0230"^^xsd:token;
  dct:source "https://nrc-publications.canada.ca/eng/view/object/?id=69fb8993-1baa-4225-b33a-6a02341d383d"^^xsd:anyURI,
    "https://nrc-publications.canada.ca/fra/voir/objet/?id=549123c3-092c-4fca-8dea-99d53eac06dd"^^xsd:anyURI;
  skos:definition "Ice-bearing permafrost in which some of the soil particles are not held together by ice."@en;
  skos:inScheme <https://w3id.org/permafrost/v/nrcglossary/scheme>;
  skos:prefLabel "partially-bonded permafrost"@en;
  skos:topConceptOf <https://w3id.org/permafrost/v/nrcglossary/scheme> .

<https://w3id.org/permafrost/v/nrcglossary/t0231> a skos:Concept;
  dct:identifier "t0231"^^xsd:token;
  dct:source "https://nrc-publications.canada.ca/eng/view/object/?id=69fb8993-1baa-4225-b33a-6a02341d383d"^^xsd:anyURI,
    "https://nrc-publications.canada.ca/fra/voir/objet/?id=549123c3-092c-4fca-8dea-99d53eac06dd"^^xsd:anyURI;
  skos:definition "Special design and construction methods used for engineering works in permafrost areas where preservation of the frozen condition is feasible."@en;
  skos:inScheme <https://w3id.org/permafrost/v/nrcglossary/scheme>;
  skos:prefLabel "passive construction methods in permafrost"@en;
  skos:scopeNote "Passive methods should maintain the foundation materials in a frozen state. Preservation of the frozen condition or permafrost aggradation can be accomplished using thermal piles or thermosyphons, or by using either a ventilation or an insulation construction technique; often a combination of these techniques is used. The ventilation technique requires that there is a clear space left between the bottom of the structure and the ground surface, or that the structure is placed on a fill pad with ventilation ducts incorporated in the pad or the floor system.Movement of cold air through the air space or ducts dissipates heat from the structure above and removes heat from the ground below. Using the insulation technique, a relatively thick fill (sometimes containing a layer of insulation) is placed on the ground surface to prevent thawing or to reduce or control the depth of thaw below the original ground surface."@en;
  skos:topConceptOf <https://w3id.org/permafrost/v/nrcglossary/scheme> .

<https://w3id.org/permafrost/v/nrcglossary/t0232> a skos:Concept;
  dct:identifier "t0232"^^xsd:token;
  dct:source "https://nrc-publications.canada.ca/eng/view/object/?id=69fb8993-1baa-4225-b33a-6a02341d383d"^^xsd:anyURI,
    "https://nrc-publications.canada.ca/fra/voir/objet/?id=549123c3-092c-4fca-8dea-99d53eac06dd"^^xsd:anyURI;
  skos:definition "A foundation pile provided with a single-phase natural convection cooling system to remove heat from the ground."@en;
  skos:inScheme <https://w3id.org/permafrost/v/nrcglossary/scheme>;
  skos:prefLabel "passive single-phase thermal pile"@en;
  skos:scopeNote "Natural convection cooling systems consist of self-powered devices, commonly referred to as thermosyphons, or heat pipes, which operate only when air temperatures are lower than the ground temperature. Passive single-phase thermal piles usually contain a sealed tube with a small radiator above the ground surface, and are filled with a liquid or gas which does not change phase. During the winter, heat from the soil surrounding the embedded portion of the pipe is absorbed by and thus warms the working fluid, which rises to the above-ground radiator section of the pipe exposed to the cooler air and loses its heat by conduction and natural convection."@en;
  skos:topConceptOf <https://w3id.org/permafrost/v/nrcglossary/scheme> .

<https://w3id.org/permafrost/v/nrcglossary/t0233> a skos:Concept;
  dct:identifier "t0233"^^xsd:token;
  dct:source "https://nrc-publications.canada.ca/eng/view/object/?id=69fb8993-1baa-4225-b33a-6a02341d383d"^^xsd:anyURI,
    "https://nrc-publications.canada.ca/fra/voir/objet/?id=549123c3-092c-4fca-8dea-99d53eac06dd"^^xsd:anyURI;
  skos:definition "A foundation pile provided with a two-phase natural convection cooling system to remove heat from the ground."@en;
  skos:inScheme <https://w3id.org/permafrost/v/nrcglossary/scheme>;
  skos:prefLabel "passive two-phase thermal pile"@en;
  skos:scopeNote "Natural convection cooling systems consist of self-powered devices, commonly referred to as thermosyphons, or heat pipes, which operate only when air temperatures are lower than the ground temperature. Passive two-phase thermal piles usually contain a sealed tube with a small radiator above the ground surface, and are filled with a substance which can be in the liquid or vapour phase, depending on its temperature. When the air temperature falls below the ground temperature, the vapour condenses in the radiator section of the tube, the pressure in the tube is reduced and the liquid in the lower section starts to boil. The resulting cycle of boiling, vapour movement up the tube, condensation, and return of the condensate by gravity flow is an effective way of transferring heat up the tube, thus cooling the ground."@en;
  skos:topConceptOf <https://w3id.org/permafrost/v/nrcglossary/scheme> .

<https://w3id.org/permafrost/v/nrcglossary/t0234> a skos:Concept;
  dct:identifier "t0234"^^xsd:token;
  dct:source "https://nrc-publications.canada.ca/eng/view/object/?id=69fb8993-1baa-4225-b33a-6a02341d383d"^^xsd:anyURI,
    "https://nrc-publications.canada.ca/fra/voir/objet/?id=549123c3-092c-4fca-8dea-99d53eac06dd"^^xsd:anyURI;
  skos:definition "A general term for any ground surface exhibiting a discernibly ordered, more or less symmetrical, morphological pattern of ground and, where present, vegetation (see Figure 16)."@en;
  skos:inScheme <https://w3id.org/permafrost/v/nrcglossary/scheme>;
  skos:prefLabel "patterned ground"@en;
  skos:scopeNote "Some patterned ground features are not confined to permafrost regions but they are best developed in regions of present or past intensive frost action. A descriptive classification of patterned ground includes such features as nonsorted and sorted circles, nets, polygons, steps and stripes, and solifluction features. In permafrost regions, the most ubiquitous macro-form is the ice-wedge polygon, and a common micro-form is the nonsorted circle. The latter includes mud boils, mud hummocks, frost boils, stony earth circles, earth hummocks, turf hummocks, thufa and (not recommended) tundra hummocks. Nonsorted circles are not all of the same origin. Some, such as mud and earth hummocks and frost boils, involve cryoturbation activity and differential heave of frost-susceptible materials. Others, such as mud boils, involve hydraulic pressures and diapiric displacements of water- saturated sediments. The genesis of many types of patterned ground phenomena is not clearly understood. Patterned ground also occurs in peatland in the form of string fens and other peatland features (see Stanek, 1977 and Stanek and Worley, 1983)."@en;
  skos:topConceptOf <https://w3id.org/permafrost/v/nrcglossary/scheme> .

<https://w3id.org/permafrost/v/nrcglossary/t0235> a skos:Concept;
  dct:identifier "t0235"^^xsd:token;
  dct:source "https://nrc-publications.canada.ca/eng/view/object/?id=69fb8993-1baa-4225-b33a-6a02341d383d"^^xsd:anyURI,
    "https://nrc-publications.canada.ca/fra/voir/objet/?id=549123c3-092c-4fca-8dea-99d53eac06dd"^^xsd:anyURI;
  skos:definition "A deposit consisting of decayed or partially decayed humified plant remains."@en;
  skos:inScheme <https://w3id.org/permafrost/v/nrcglossary/scheme>;
  skos:prefLabel "peat"@en;
  skos:scopeNote "Peat is commonly formed by the slow decay of successive layers of aquatic and semi-aquatic plants in swampy or water-logged areas, where oxygen is absent."@en;
  skos:topConceptOf <https://w3id.org/permafrost/v/nrcglossary/scheme> .

<https://w3id.org/permafrost/v/nrcglossary/t0236> a skos:Concept;
  dct:identifier "t0236"^^xsd:token;
  dct:source "https://nrc-publications.canada.ca/eng/view/object/?id=69fb8993-1baa-4225-b33a-6a02341d383d"^^xsd:anyURI,
    "https://nrc-publications.canada.ca/fra/voir/objet/?id=549123c3-092c-4fca-8dea-99d53eac06dd"^^xsd:anyURI;
  skos:definition "A hummock consisting of peat."@en;
  skos:inScheme <https://w3id.org/permafrost/v/nrcglossary/scheme>;
  skos:prefLabel "peat hummock"@en;
  skos:topConceptOf <https://w3id.org/permafrost/v/nrcglossary/scheme> .

<https://w3id.org/permafrost/v/nrcglossary/t0237> a skos:Concept;
  dct:identifier "t0237"^^xsd:token;
  dct:source "https://nrc-publications.canada.ca/eng/view/object/?id=69fb8993-1baa-4225-b33a-6a02341d383d"^^xsd:anyURI,
    "https://nrc-publications.canada.ca/fra/voir/objet/?id=549123c3-092c-4fca-8dea-99d53eac06dd"^^xsd:anyURI;
  skos:altLabel "palsa plateau"@en;
  skos:definition "A generally flat-topped expanse of peat, elevated above the general surface of a peatland, and containing segregated ice that may or may not extend downward into the underlying mineral soil (see Figures 14 and 15b)."@en;
  skos:inScheme <https://w3id.org/permafrost/v/nrcglossary/scheme>;
  skos:prefLabel "peat plateau"@en;
  skos:scopeNote "Some controversy exists as to whether peat plateaus and palsas are morphological variations of the same features, or genetically different. Layers or lenses of segregated ice occur especially in the mineral soil but they are thinner and less extensive in peat plateaus than in palsas. Flat-topped, somewhat raised peatlands without an icy core occur in non-permafrost environments but are not peat plateaus."@en;
  skos:topConceptOf <https://w3id.org/permafrost/v/nrcglossary/scheme> .

<https://w3id.org/permafrost/v/nrcglossary/t0238> a skos:Concept;
  dct:identifier "t0238"^^xsd:token;
  dct:source "https://nrc-publications.canada.ca/eng/view/object/?id=69fb8993-1baa-4225-b33a-6a02341d383d"^^xsd:anyURI,
    "https://nrc-publications.canada.ca/fra/voir/objet/?id=549123c3-092c-4fca-8dea-99d53eac06dd"^^xsd:anyURI;
  skos:definition "Peat-covered terrain."@en;
  skos:hiddenLabel "muskeg"@en, "organic terrain"@en;
  skos:inScheme <https://w3id.org/permafrost/v/nrcglossary/scheme>;
  skos:prefLabel "peatland"@en, "tourbière"@fr;
  skos:scopeNote "Stanek (1977) and Stanek and Worley (1983) should be consulted for definitions and information on peat and peatland and associated features. There is no international agreement on the minimum thickness of peat required for the terrain to be classified as \"peatland\". In Canada, peatland is defined as a type of wetland formed by the accumulation of plant remains with negligible decomposition. In the discontinuous permafrost zone, especially near the southern limit, peatland is often underlain by permafrost, reflecting the thermal insulating qualities of peat. Palsas, peat plateaus and polygonal peat plateaus are permafrost-related peatland features (see Figure 15)."@en;
  skos:topConceptOf <https://w3id.org/permafrost/v/nrcglossary/scheme> .

<https://w3id.org/permafrost/v/nrcglossary/t0239> a skos:Concept;
  dct:identifier "t0239"^^xsd:token;
  dct:source "https://nrc-publications.canada.ca/eng/view/object/?id=69fb8993-1baa-4225-b33a-6a02341d383d"^^xsd:anyURI,
    "https://nrc-publications.canada.ca/fra/voir/objet/?id=549123c3-092c-4fca-8dea-99d53eac06dd"^^xsd:anyURI;
  skos:definition "A layer of frozen ground which forms as part of the seasonally frozen ground (in areas free of permafrost or with a lowered permafrost table), remains frozen throughout one or several summers, and then thaws."@en;
  skos:inScheme <https://w3id.org/permafrost/v/nrcglossary/scheme>;
  skos:prefLabel "pereletok"@en, "pérélétok"@fr;
  skos:scopeNote "Use of this Russian term is not recommended. It presupposes arbitrarily that pereletok is not permafrost although the definition assigns a sufficient duration of time for it to be considered as permafrost. Furthermore, the definition implies a basic difference in characteristics between pereletok, on the one hand, and permafrost of only a few years' duration, on the other hand, where in fact no difference exists. It is preferable to regard frozen ground as permafrost if it lasts at least from one winter through the succeeding thawing season to the next winter, and as seasonally frozen ground if it lasts only through part of a year. For the same reason, the use of the term \"climafrost\" as a synonym for pereletok is not recommended."@en;
  skos:topConceptOf <https://w3id.org/permafrost/v/nrcglossary/scheme> .

<https://w3id.org/permafrost/v/nrcglossary/t0240> a skos:Concept;
  dct:identifier "t0240"^^xsd:token;
  dct:source "https://nrc-publications.canada.ca/eng/view/object/?id=69fb8993-1baa-4225-b33a-6a02341d383d"^^xsd:anyURI,
    "https://nrc-publications.canada.ca/fra/voir/objet/?id=549123c3-092c-4fca-8dea-99d53eac06dd"^^xsd:anyURI;
  skos:definition "The conditions, processes and landforms associated with cold, nonglacial environments."@en;
  skos:inScheme <https://w3id.org/permafrost/v/nrcglossary/scheme>;
  skos:prefLabel "periglacial"@en, "périglaciaire"@fr;
  skos:scopeNote "The term was originally used to describe the climatic and geomorphic conditions of areas peripheral to Pleistocene ice sheets and glaciers. Modern usage refers, however, to a wider range of cold climatic conditions regardless of their proximity to a glacier, either in space or time. Many, but not all, periglacial environments possess permafrost; all are dominated by frost action processes."@en;
  skos:topConceptOf <https://w3id.org/permafrost/v/nrcglossary/scheme> .

<https://w3id.org/permafrost/v/nrcglossary/t0241> a skos:Concept;
  dct:identifier "t0241"^^xsd:token;
  dct:source "https://nrc-publications.canada.ca/eng/view/object/?id=69fb8993-1baa-4225-b33a-6a02341d383d"^^xsd:anyURI,
    "https://nrc-publications.canada.ca/fra/voir/objet/?id=549123c3-092c-4fca-8dea-99d53eac06dd"^^xsd:anyURI;
  skos:definition "Landforms and soil characteristics produced by periglacial processes."@en;
  skos:inScheme <https://w3id.org/permafrost/v/nrcglossary/scheme>;
  skos:prefLabel "periglacial phenomena"@en;
  skos:scopeNote "Periglacial phenomena include landforms like seasonal and perennial frost mounds, as well as the cryotextures, cryostructures and cryogenic fabrics found in soils."@en;
  skos:topConceptOf <https://w3id.org/permafrost/v/nrcglossary/scheme> .

<https://w3id.org/permafrost/v/nrcglossary/t0242> a skos:Concept;
  dct:identifier "t0242"^^xsd:token;
  dct:source "https://nrc-publications.canada.ca/eng/view/object/?id=69fb8993-1baa-4225-b33a-6a02341d383d"^^xsd:anyURI,
    "https://nrc-publications.canada.ca/fra/voir/objet/?id=549123c3-092c-4fca-8dea-99d53eac06dd"^^xsd:anyURI;
  skos:definition "Processes associated with frost action in cold, nonglacial environments."@en;
  skos:inScheme <https://w3id.org/permafrost/v/nrcglossary/scheme>;
  skos:prefLabel "periglacial processes"@en;
  skos:scopeNote "Periglacial processes include frost jacking, frost sorting, frost wedging, cryoturbation, and the development of cryotextures, cryostructures and cryogenic fabrics in soils."@en;
  skos:topConceptOf <https://w3id.org/permafrost/v/nrcglossary/scheme> .

<https://w3id.org/permafrost/v/nrcglossary/t0243> a skos:Concept;
  dct:identifier "t0243"^^xsd:token;
  dct:source "https://nrc-publications.canada.ca/eng/view/object/?id=69fb8993-1baa-4225-b33a-6a02341d383d"^^xsd:anyURI,
    "https://nrc-publications.canada.ca/fra/voir/objet/?id=549123c3-092c-4fca-8dea-99d53eac06dd"^^xsd:anyURI;
  skos:definition "An artificial mixture of frozen soil materials cemented by pore ice, which forms a concrete-like construction material used in cold regions."@en;
  skos:inScheme <https://w3id.org/permafrost/v/nrcglossary/scheme>;
  skos:prefLabel "géliciment"@fr, "permacrete"@en;
  skos:scopeNote "When soils of appropriate gradation are brought to their saturation moisture content, mixed and compacted to maximum density and then frozen, a material of relatively high strength is obtained so long as it is kept frozen. Permacrete has been moulded in brick or block form or placed in forms and used for construction (e.g., of walls and columns, both underground in tunnels, mines, etc., and on the ground surface in a freezing environment)."@en;
  skos:topConceptOf <https://w3id.org/permafrost/v/nrcglossary/scheme> .

<https://w3id.org/permafrost/v/nrcglossary/t0244> a skos:Concept;
  dct:identifier "t0244"^^xsd:token;
  dct:source "https://nrc-publications.canada.ca/eng/view/object/?id=69fb8993-1baa-4225-b33a-6a02341d383d"^^xsd:anyURI,
    "https://nrc-publications.canada.ca/fra/voir/objet/?id=549123c3-092c-4fca-8dea-99d53eac06dd"^^xsd:anyURI;
  skos:altLabel "perennially cryotic ground"@en, "perennially frozen ground"@en;
  skos:definition "Ground (soil or rock and included ice and organic material) that remains at or below 0°C for at least two consecutive years (see Figure 2)."@en;
  skos:hiddenLabel "biennially frozen ground"@en, "climafrost"@en, "cryic layer"@en,
    "permanently frozen ground"@en;
  skos:inScheme <https://w3id.org/permafrost/v/nrcglossary/scheme>;
  skos:prefLabel "pergélisol"@fr, "permafrost"@en;
  skos:scopeNote "Permafrost is synonymous with perennially cryotic ground: it is defined on the basis of temperature. It is not necessarily frozen, because the freezing point of the included water may be depressed several degrees below 0°C; moisture in the form of water or ice may or may not be present. In other words, whereas all perennially frozen ground is permafrost, not all permafrost is perennially frozen. Permafrost should not be regarded as permanent, because natural or man-made changes in the climate or terrain may cause the temperature of the ground to rise above 0°C. Permafrost includes perennial ground ice, but not glacier ice or icings, or bodies of surface water with temperatures perennially below 0°C; it does include man-made perennially frozen ground around or below chilled pipelines, hockey arenas, etc. Russian usage requires the continuous existence of temperatures below 0°C for at least three years, and also the presence of at least some ice. (see pereletok)."@en;
  skos:topConceptOf <https://w3id.org/permafrost/v/nrcglossary/scheme> .

<https://w3id.org/permafrost/v/nrcglossary/t0245> a skos:Concept;
  dct:identifier "t0245"^^xsd:token;
  dct:source "https://nrc-publications.canada.ca/eng/view/object/?id=69fb8993-1baa-4225-b33a-6a02341d383d"^^xsd:anyURI,
    "https://nrc-publications.canada.ca/fra/voir/objet/?id=549123c3-092c-4fca-8dea-99d53eac06dd"^^xsd:anyURI;
  skos:definition "A naturally or artificially caused increase in the thickness and/or areal extent of permafrost."@en;
  skos:inScheme <https://w3id.org/permafrost/v/nrcglossary/scheme>;
  skos:prefLabel "permafrost aggradation"@en;
  skos:scopeNote "Permafrost aggradation may be caused by climatic cooling or by changes in terrain conditions, including vegetation succession, infilling of lake basins and a decrease in snowcover. It can also occur under ice arenas, road and airfield embankments, etc. It may be expressed as a thinning of the active layer and a thickening of the permafrost, as well as an increase in the areal extent of permafrost."@en;
  skos:topConceptOf <https://w3id.org/permafrost/v/nrcglossary/scheme> .

<https://w3id.org/permafrost/v/nrcglossary/t0246> a skos:Concept;
  dct:identifier "t0246"^^xsd:token;
  dct:source "https://nrc-publications.canada.ca/eng/view/object/?id=69fb8993-1baa-4225-b33a-6a02341d383d"^^xsd:anyURI,
    "https://nrc-publications.canada.ca/fra/voir/objet/?id=549123c3-092c-4fca-8dea-99d53eac06dd"^^xsd:anyURI;
  skos:definition "The lower boundary surface of permafrost, above which temperatures are perennially below 0°C (cryotic) and below which temperatures are perennially above 0°C (noncryotic) (see Figures 2, 4 and 11)."@en;
  skos:inScheme <https://w3id.org/permafrost/v/nrcglossary/scheme>;
  skos:prefLabel "base du pergélisol"@fr, "permafrost base"@en;
  skos:topConceptOf <https://w3id.org/permafrost/v/nrcglossary/scheme> .

<https://w3id.org/permafrost/v/nrcglossary/t0247> a skos:Concept;
  dct:identifier "t0247"^^xsd:token;
  dct:source "https://nrc-publications.canada.ca/eng/view/object/?id=69fb8993-1baa-4225-b33a-6a02341d383d"^^xsd:anyURI,
    "https://nrc-publications.canada.ca/fra/voir/objet/?id=549123c3-092c-4fca-8dea-99d53eac06dd"^^xsd:anyURI;
  skos:definition "1. The geographical boundary between the continuous and discontinuous permafrost zones. 2. The margin of a discrete body of permafrost."@en;
  skos:inScheme <https://w3id.org/permafrost/v/nrcglossary/scheme>;
  skos:prefLabel "limite du pergélisol"@fr, "permafrost boundary"@en;
  skos:topConceptOf <https://w3id.org/permafrost/v/nrcglossary/scheme> .

<https://w3id.org/permafrost/v/nrcglossary/t0248> a skos:Concept;
  dct:identifier "t0248"^^xsd:token;
  dct:source "https://nrc-publications.canada.ca/eng/view/object/?id=69fb8993-1baa-4225-b33a-6a02341d383d"^^xsd:anyURI,
    "https://nrc-publications.canada.ca/fra/voir/objet/?id=549123c3-092c-4fca-8dea-99d53eac06dd"^^xsd:anyURI;
  skos:definition "A naturally or artificially caused decrease in the thickness and/or areal extent of permafrost."@en;
  skos:inScheme <https://w3id.org/permafrost/v/nrcglossary/scheme>;
  skos:prefLabel "permafrost degradation"@en, "régression du pergélisol"@fr;
  skos:scopeNote "Permafrost degradation may be caused by climatic warming or by changes in terrain conditions, such as disturbance or removal of an insulating vegetation layer by fire, or by flooding caused by a landslide-blocked stream, or by human activity. It may be expressed as a thickening of the active layer, a lowering of the permafrost table, a raising of the permafrost base, or a reduction in the areal extent or the complete disappearance of permafrost."@en;
  skos:topConceptOf <https://w3id.org/permafrost/v/nrcglossary/scheme> .

<https://w3id.org/permafrost/v/nrcglossary/t0249> a skos:Concept;
  dct:identifier "t0249"^^xsd:token;
  dct:source "https://nrc-publications.canada.ca/eng/view/object/?id=69fb8993-1baa-4225-b33a-6a02341d383d"^^xsd:anyURI,
    "https://nrc-publications.canada.ca/fra/voir/objet/?id=549123c3-092c-4fca-8dea-99d53eac06dd"^^xsd:anyURI;
  skos:definition "Outermost (latitudinal) or lowest (altitudinal) limit of the occurrence of permafrost (see Figure 1)."@en;
  skos:inScheme <https://w3id.org/permafrost/v/nrcglossary/scheme>;
  skos:prefLabel "permafrost limit"@en;
  skos:topConceptOf <https://w3id.org/permafrost/v/nrcglossary/scheme> .

<https://w3id.org/permafrost/v/nrcglossary/t0250> a skos:Concept;
  dct:identifier "t0250"^^xsd:token;
  dct:source "https://nrc-publications.canada.ca/eng/view/object/?id=69fb8993-1baa-4225-b33a-6a02341d383d"^^xsd:anyURI,
    "https://nrc-publications.canada.ca/fra/voir/objet/?id=549123c3-092c-4fca-8dea-99d53eac06dd"^^xsd:anyURI;
  skos:definition "A region in which the temperature of some or all of the ground below the seasonally freezing and thawing layer remains continuously at or below 0°C for at least two consecutive years."@en;
  skos:inScheme <https://w3id.org/permafrost/v/nrcglossary/scheme>;
  skos:prefLabel "permafrost region"@en, "région pergélisolée"@fr;
  skos:scopeNote "The permafrost region is commonly subdivided into permafrost zones (see Figure 1)."@en;
  skos:topConceptOf <https://w3id.org/permafrost/v/nrcglossary/scheme> .

<https://w3id.org/permafrost/v/nrcglossary/t0251> a skos:Concept;
  dct:identifier "t0251"^^xsd:token;
  dct:source "https://nrc-publications.canada.ca/eng/view/object/?id=69fb8993-1baa-4225-b33a-6a02341d383d"^^xsd:anyURI,
    "https://nrc-publications.canada.ca/fra/voir/objet/?id=549123c3-092c-4fca-8dea-99d53eac06dd"^^xsd:anyURI;
  skos:definition "The upper boundary surface of permafrost (see Figures 2, 4 and 11)."@en;
  skos:inScheme <https://w3id.org/permafrost/v/nrcglossary/scheme>;
  skos:prefLabel "permafrost table"@en, "plafond du pergélisol"@fr;
  skos:scopeNote "The depth of this boundary below the land surface, whether exposed or covered by a water body or glacier ice, is variable depending on such local factors as topography, exposure to the sun, insulating cover of vegetation and snow, drainage, grain size and degree of sorting of the soil, and thermal properties of soil and rock."@en;
  skos:topConceptOf <https://w3id.org/permafrost/v/nrcglossary/scheme> .

<https://w3id.org/permafrost/v/nrcglossary/t0252> a skos:Concept;
  dct:identifier "t0252"^^xsd:token;
  dct:source "https://nrc-publications.canada.ca/eng/view/object/?id=69fb8993-1baa-4225-b33a-6a02341d383d"^^xsd:anyURI,
    "https://nrc-publications.canada.ca/fra/voir/objet/?id=549123c3-092c-4fca-8dea-99d53eac06dd"^^xsd:anyURI;
  skos:definition "The vertical distance between the permafrost table and the permafrost base(see Figures 2 and 4)."@en;
  skos:inScheme <https://w3id.org/permafrost/v/nrcglossary/scheme>;
  skos:prefLabel "permafrost thickness"@en, "épaisseur du pergélisol"@fr;
  skos:scopeNote "The thickness of permafrost may range from less than 1 m to more than 1000 metres."@en;
  skos:topConceptOf <https://w3id.org/permafrost/v/nrcglossary/scheme> .

<https://w3id.org/permafrost/v/nrcglossary/t0253> a skos:Concept;
  dct:identifier "t0253"^^xsd:token;
  dct:source "https://nrc-publications.canada.ca/eng/view/object/?id=69fb8993-1baa-4225-b33a-6a02341d383d"^^xsd:anyURI,
    "https://nrc-publications.canada.ca/fra/voir/objet/?id=549123c3-092c-4fca-8dea-99d53eac06dd"^^xsd:anyURI;
  skos:definition "A major subdivision of a permafrost region (see Figure 1)."@en;
  skos:inScheme <https://w3id.org/permafrost/v/nrcglossary/scheme>;
  skos:prefLabel "permafrost zone"@en, "zone de pergélisol"@fr;
  skos:scopeNote "A permafrost region is commonly subdivided into permafrost zones based on the proportion of the ground that is perennially cryotic. The basic subdivision in high latitudes is into zones of continuous permafrost and discontinuous permafrost."@en;
  skos:topConceptOf <https://w3id.org/permafrost/v/nrcglossary/scheme> .

<https://w3id.org/permafrost/v/nrcglossary/t0254> a skos:Concept;
  dct:identifier "t0254"^^xsd:token;
  dct:source "https://nrc-publications.canada.ca/eng/view/object/?id=69fb8993-1baa-4225-b33a-6a02341d383d"^^xsd:anyURI,
    "https://nrc-publications.canada.ca/fra/voir/objet/?id=549123c3-092c-4fca-8dea-99d53eac06dd"^^xsd:anyURI;
  skos:definition "A perennial frost mound consisting of a core of massive ice, produced primarily by injection of water, and covered with soil and vegetation."@en;
  skos:hiddenLabel "bulgunniakh"@en, "hydrolaccolith"@en;
  skos:inScheme <https://w3id.org/permafrost/v/nrcglossary/scheme>;
  skos:prefLabel "pingo"@en, "pingo"@fr;
  skos:scopeNote "Pingos occur in both the continuous and discontinuous permafrost zones. The term \"pingo,\" a local Inuktitut term used in the Mackenzie Delta, Canada, was applied to relatively large features with heights of 10 m or more and horizontal dimensions of more than 100 m. Most pingos are conical, somewhat asymmetric, and have a circular or oval base and a fissured top that may be cratered. The fissures and craters are the result of rupturing of the soil and vegetation cover during doming due to progressive development of the ice core (see dilation crack). Seasonal frost mounds (e.g., frost blisters), should not be called pingos."@en;
  skos:topConceptOf <https://w3id.org/permafrost/v/nrcglossary/scheme> .

<https://w3id.org/permafrost/v/nrcglossary/t0255> a skos:Concept;
  dct:identifier "t0255"^^xsd:token;
  dct:source "https://nrc-publications.canada.ca/eng/view/object/?id=69fb8993-1baa-4225-b33a-6a02341d383d"^^xsd:anyURI,
    "https://nrc-publications.canada.ca/fra/voir/objet/?id=549123c3-092c-4fca-8dea-99d53eac06dd"^^xsd:anyURI;
  skos:definition "Massive ice forming the core of a pingo (see Figure 10h)."@en;
  skos:inScheme <https://w3id.org/permafrost/v/nrcglossary/scheme>;
  skos:prefLabel "pingo ice"@en;
  skos:scopeNote "The ice in a pingo may be nearly pure or mixed with sediment. It includes intrusive ice, segregated ice and dilation crack ice."@en;
  skos:topConceptOf <https://w3id.org/permafrost/v/nrcglossary/scheme> .

<https://w3id.org/permafrost/v/nrcglossary/t0256> a skos:Concept;
  dct:identifier "t0256"^^xsd:token;
  dct:source "https://nrc-publications.canada.ca/eng/view/object/?id=69fb8993-1baa-4225-b33a-6a02341d383d"^^xsd:anyURI,
    "https://nrc-publications.canada.ca/fra/voir/objet/?id=549123c3-092c-4fca-8dea-99d53eac06dd"^^xsd:anyURI;
  skos:altLabel "fossil pingo"@en;
  skos:definition "A collapsed pingo (see Figure 19c)."@en;
  skos:inScheme <https://w3id.org/permafrost/v/nrcglossary/scheme>;
  skos:prefLabel "pingo remnant"@en;
  skos:scopeNote "In contemporary permafrost environments, a pingo remnant is commonly represented by a low, circular or arcuate ridge of material resulting from the slumping of the sides of the pingo during thawing. The former centre is marked by a depression which may be filled with water."@en;
  skos:topConceptOf <https://w3id.org/permafrost/v/nrcglossary/scheme> .

<https://w3id.org/permafrost/v/nrcglossary/t0257> a skos:Concept;
  dct:identifier "t0257"^^xsd:token;
  dct:source "https://nrc-publications.canada.ca/eng/view/object/?id=69fb8993-1baa-4225-b33a-6a02341d383d"^^xsd:anyURI,
    "https://nrc-publications.canada.ca/fra/voir/objet/?id=549123c3-092c-4fca-8dea-99d53eac06dd"^^xsd:anyURI;
  skos:definition "A pingo remnant in a contemporary non-permafrost environment."@en;
  skos:inScheme <https://w3id.org/permafrost/v/nrcglossary/scheme>;
  skos:prefLabel "pingo fossile"@fr, "pingo scar"@en;
  skos:scopeNote "Their occurrence provides evidence of former permafrost conditions."@en;
  skos:topConceptOf <https://w3id.org/permafrost/v/nrcglossary/scheme> .

<https://w3id.org/permafrost/v/nrcglossary/t0258> a skos:Concept;
  dct:identifier "t0258"^^xsd:token;
  dct:source "https://nrc-publications.canada.ca/eng/view/object/?id=69fb8993-1baa-4225-b33a-6a02341d383d"^^xsd:anyURI,
    "https://nrc-publications.canada.ca/fra/voir/objet/?id=549123c3-092c-4fca-8dea-99d53eac06dd"^^xsd:anyURI;
  skos:definition "Permafrost occurring on other planetary bodies (planets, moons, asteroids)."@en;
  skos:inScheme <https://w3id.org/permafrost/v/nrcglossary/scheme>;
  skos:prefLabel "planetary permafrost"@en;
  skos:scopeNote "The most extensive suite of permafrost-related features known is from Mars, where large volumes of water and/or ice are believed to exist beneath the planet's surface. Water ice, alone or in combination with methane ice and/or gas hydrates, is also believed to occur on moons of Jupiter (Callisto, Ganymede and Europa) and Saturn (Titan). Most of the moons and asteroids of the solar system are characterized by permafrost (temperature perennially below 0°C), but in the absence of any water they are all unfrozen, although cryotic. All the planetary bodies noted above include some frozen material."@en;
  skos:topConceptOf <https://w3id.org/permafrost/v/nrcglossary/scheme> .

<https://w3id.org/permafrost/v/nrcglossary/t0259> a skos:Concept;
  dct:identifier "t0259"^^xsd:token;
  dct:source "https://nrc-publications.canada.ca/eng/view/object/?id=69fb8993-1baa-4225-b33a-6a02341d383d"^^xsd:anyURI,
    "https://nrc-publications.canada.ca/fra/voir/objet/?id=549123c3-092c-4fca-8dea-99d53eac06dd"^^xsd:anyURI;
  skos:definition "Fine-grained soil in which only a portion of the pore water has turned into ice."@en;
  skos:inScheme <https://w3id.org/permafrost/v/nrcglossary/scheme>;
  skos:prefLabel "plastic frozen ground"@en;
  skos:scopeNote "Plastic frozen ground is cemented by ice, but it has viscous properties due to its high unfrozen water content and will therefore indergo plastic deformation under load, rather than brittle failure."@en;
  skos:topConceptOf <https://w3id.org/permafrost/v/nrcglossary/scheme> .

<https://w3id.org/permafrost/v/nrcglossary/t0260> a skos:Concept;
  dct:identifier "t0260"^^xsd:token;
  dct:source "https://nrc-publications.canada.ca/eng/view/object/?id=69fb8993-1baa-4225-b33a-6a02341d383d"^^xsd:anyURI,
    "https://nrc-publications.canada.ca/fra/voir/objet/?id=549123c3-092c-4fca-8dea-99d53eac06dd"^^xsd:anyURI;
  skos:definition "The absolute value of the ratio between linear strain changes, perpendicular to and in the direction of a given uniaxial stress change, respectively."@en;
  skos:inScheme <https://w3id.org/permafrost/v/nrcglossary/scheme>;
  skos:prefLabel "Poisson's ratio"@en;
  skos:topConceptOf <https://w3id.org/permafrost/v/nrcglossary/scheme> .

<https://w3id.org/permafrost/v/nrcglossary/t0261> a skos:Concept;
  dct:identifier "t0261"^^xsd:token;
  dct:source "https://nrc-publications.canada.ca/eng/view/object/?id=69fb8993-1baa-4225-b33a-6a02341d383d"^^xsd:anyURI,
    "https://nrc-publications.canada.ca/fra/voir/objet/?id=549123c3-092c-4fca-8dea-99d53eac06dd"^^xsd:anyURI;
  skos:altLabel "frost polygon"@en, "frost-crack polygon"@en;
  skos:definition "Polygons are closed, multi-sided, roughly equidimensional patterned- ground features, bounded by more or less straight sides; some of the sides may be irregular (see Figure 16a, b)."@en;
  skos:hiddenLabel "Taimyr polygon"@en, "depressed-centre polygon"@en, "fissure polygon"@en,
    "raised-centre polygon"@en, "tundra polygon"@en;
  skos:inScheme <https://w3id.org/permafrost/v/nrcglossary/scheme>;
  skos:prefLabel "polygon"@en, "polygone"@fr;
  skos:scopeNote "Macro-scale polygons, typically 15 to 30 m across, result from thermal contraction cracking of the ground and form random or oriented polygonal patterns. They occur in both mineral terrain and peatland (see polygonal peat plateau). Ice- wedge polygons are common in poorly drained areas and may be either high- centred or low-centred. Sand-wedge polygons occur where wedges of primary mineral infill underly the polygon boundaries. Some polygons may be formed by seasonal frost cracking in areas of deep seasonal frost. Micro-scale polygonal patterns, usually less than 2 m in diameter, are normally caused by desiccation cracking."@en;
  skos:topConceptOf <https://w3id.org/permafrost/v/nrcglossary/scheme> .

<https://w3id.org/permafrost/v/nrcglossary/t0262> a skos:Concept;
  dct:identifier "t0262"^^xsd:token;
  dct:source "https://nrc-publications.canada.ca/eng/view/object/?id=69fb8993-1baa-4225-b33a-6a02341d383d"^^xsd:anyURI,
    "https://nrc-publications.canada.ca/fra/voir/objet/?id=549123c3-092c-4fca-8dea-99d53eac06dd"^^xsd:anyURI;
  skos:definition "The narrow depression surrounding a high-centre polygon."@en;
  skos:inScheme <https://w3id.org/permafrost/v/nrcglossary/scheme>;
  skos:prefLabel "polygon trough"@en;
  skos:scopeNote "A polygon trough develops as a result of thawing of the ice wedges surrounding an ice-wedge polygon."@en;
  skos:topConceptOf <https://w3id.org/permafrost/v/nrcglossary/scheme> .

<https://w3id.org/permafrost/v/nrcglossary/t0263> a skos:Concept;
  dct:identifier "t0263"^^xsd:token;
  dct:source "https://nrc-publications.canada.ca/eng/view/object/?id=69fb8993-1baa-4225-b33a-6a02341d383d"^^xsd:anyURI,
    "https://nrc-publications.canada.ca/fra/voir/objet/?id=549123c3-092c-4fca-8dea-99d53eac06dd"^^xsd:anyURI;
  skos:definition "A pattern consisting of numerous multi-sided, roughly equidimensional figures bounded by more or less straight sides."@en;
  skos:inScheme <https://w3id.org/permafrost/v/nrcglossary/scheme>;
  skos:prefLabel "polygonal pattern"@en;
  skos:topConceptOf <https://w3id.org/permafrost/v/nrcglossary/scheme> .

<https://w3id.org/permafrost/v/nrcglossary/t0264> a skos:Concept;
  dct:identifier "t0264"^^xsd:token;
  dct:source "https://nrc-publications.canada.ca/eng/view/object/?id=69fb8993-1baa-4225-b33a-6a02341d383d"^^xsd:anyURI,
    "https://nrc-publications.canada.ca/fra/voir/objet/?id=549123c3-092c-4fca-8dea-99d53eac06dd"^^xsd:anyURI;
  skos:definition "A peat plateau with ice-wedge polygons (see Figure 15c)."@en;
  skos:inScheme <https://w3id.org/permafrost/v/nrcglossary/scheme>;
  skos:prefLabel "plateau palsique à polygones"@fr, "polygonal peat plateau"@en;
  skos:scopeNote "Polygonal peat plateaus are commonly found near the boundary between the zones of discontinuous and continuous permafrost."@en;
  skos:topConceptOf <https://w3id.org/permafrost/v/nrcglossary/scheme> .

<https://w3id.org/permafrost/v/nrcglossary/t0265> a skos:Concept;
  dct:identifier "t0265"^^xsd:token;
  dct:source "https://nrc-publications.canada.ca/eng/view/object/?id=69fb8993-1baa-4225-b33a-6a02341d383d"^^xsd:anyURI,
    "https://nrc-publications.canada.ca/fra/voir/objet/?id=549123c3-092c-4fca-8dea-99d53eac06dd"^^xsd:anyURI;
  skos:definition "Ice-bearing permafrost in which few of the soil particles are held together by ice."@en;
  skos:inScheme <https://w3id.org/permafrost/v/nrcglossary/scheme>;
  skos:prefLabel "poorly-bonded permafrost"@en;
  skos:topConceptOf <https://w3id.org/permafrost/v/nrcglossary/scheme> .

<https://w3id.org/permafrost/v/nrcglossary/t0266> a skos:Concept;
  dct:identifier "t0266"^^xsd:token;
  dct:source "https://nrc-publications.canada.ca/eng/view/object/?id=69fb8993-1baa-4225-b33a-6a02341d383d"^^xsd:anyURI,
    "https://nrc-publications.canada.ca/fra/voir/objet/?id=549123c3-092c-4fca-8dea-99d53eac06dd"^^xsd:anyURI;
  skos:altLabel "ice cement"@en, "interstitial ice"@en;
  skos:definition "Ice occurring in the pores of soils and rocks."@en;
  skos:inScheme <https://w3id.org/permafrost/v/nrcglossary/scheme>;
  skos:prefLabel "pore ice"@en;
  skos:scopeNote "Pore ice does not include segregated ice. On melting, pore ice does not yield water in excess of the pore volume of the same soil when unfrozen."@en;
  skos:topConceptOf <https://w3id.org/permafrost/v/nrcglossary/scheme> .

<https://w3id.org/permafrost/v/nrcglossary/t0267> a skos:Concept;
  dct:identifier "t0267"^^xsd:token;
  dct:source "https://nrc-publications.canada.ca/eng/view/object/?id=69fb8993-1baa-4225-b33a-6a02341d383d"^^xsd:anyURI,
    "https://nrc-publications.canada.ca/fra/voir/objet/?id=549123c3-092c-4fca-8dea-99d53eac06dd"^^xsd:anyURI;
  skos:definition "Water occurring in the pores of soils and rocks."@en;
  skos:inScheme <https://w3id.org/permafrost/v/nrcglossary/scheme>;
  skos:prefLabel "pore water"@en;
  skos:scopeNote "Pore water includes free water and interfacial (adsorbed) water. Free water is that portion of the pore water that is free to move between interconnected pores under the influence of gravity. The temperature at which free water will change phase depends primarily on its dissolved-solids content, which determines freezing-point depression. It should be noted that the term \"free water\" also covers water in fissures, solution channels and other openings in soils or rocks. Interfacial water forms transition layers at mineral/water and mineral/water/ice interfaces. The intermolecular forces involved are such that this water does not move under the influence of gravity. The temperature at which any portion of the interfacial water will change phase depends on the total energy of the various adsorption forces, which in turn depend on distance from the mineral surface, type of mineral and solute content of the water."@en;
  skos:topConceptOf <https://w3id.org/permafrost/v/nrcglossary/scheme> .

<https://w3id.org/permafrost/v/nrcglossary/t0268> a skos:Concept;
  dct:identifier "t0268"^^xsd:token;
  dct:source "https://nrc-publications.canada.ca/eng/view/object/?id=69fb8993-1baa-4225-b33a-6a02341d383d"^^xsd:anyURI,
    "https://nrc-publications.canada.ca/fra/voir/objet/?id=549123c3-092c-4fca-8dea-99d53eac06dd"^^xsd:anyURI;
  skos:definition "Lowering the melting point of ice by applying pressure."@en;
  skos:inScheme <https://w3id.org/permafrost/v/nrcglossary/scheme>;
  skos:prefLabel "fonte sous pression"@fr, "pressure-melting"@en;
  skos:scopeNote "Application of pressure increases the unfrozen water content by a small amount in frozen soils at a given temperature. Ice in soils is more easily melted by this process than bulk ice, because of stress concentrations at the soil intergranular contacts."@en;
  skos:topConceptOf <https://w3id.org/permafrost/v/nrcglossary/scheme> .

<https://w3id.org/permafrost/v/nrcglossary/t0269> a skos:Concept;
  dct:identifier "t0269"^^xsd:token;
  dct:source "https://nrc-publications.canada.ca/eng/view/object/?id=69fb8993-1baa-4225-b33a-6a02341d383d"^^xsd:anyURI,
    "https://nrc-publications.canada.ca/fra/voir/objet/?id=549123c3-092c-4fca-8dea-99d53eac06dd"^^xsd:anyURI;
  skos:altLabel "dielectric constant"@en;
  skos:definition "The relative permittivity of a soil is the ratio of the permittivity of the soil to the permittivity of a vacuum."@en;
  skos:inScheme <https://w3id.org/permafrost/v/nrcglossary/scheme>;
  skos:prefLabel "relative permittivity"@en;
  skos:scopeNote "The relative permittivity varies with soil type, temperature, unfrozen water content, and the dissolved-solids content of the pore water."@en;
  skos:topConceptOf <https://w3id.org/permafrost/v/nrcglossary/scheme> .

<https://w3id.org/permafrost/v/nrcglossary/t0270> a skos:Concept;
  dct:identifier "t0270"^^xsd:token;
  dct:source "https://nrc-publications.canada.ca/eng/view/object/?id=69fb8993-1baa-4225-b33a-6a02341d383d"^^xsd:anyURI,
    "https://nrc-publications.canada.ca/fra/voir/objet/?id=549123c3-092c-4fca-8dea-99d53eac06dd"^^xsd:anyURI;
  skos:definition "A layer of ground, now perennially frozen, lying immediately below the modern active layer. Its thickness indicates the greater annual depth of thaw that occurred during a previous period."@en;
  skos:inScheme <https://w3id.org/permafrost/v/nrcglossary/scheme>;
  skos:prefLabel "relict active layer"@en;
  skos:scopeNote "The base of the relict active layer is a thaw unconformity, which may be recognized by differences in ice contents, stable isotope contents, and heavy mineral and pollen assemblages above and below the unconformity, and by the truncation of ice bodies."@en;
  skos:topConceptOf <https://w3id.org/permafrost/v/nrcglossary/scheme> .

<https://w3id.org/permafrost/v/nrcglossary/t0271> a skos:Concept;
  dct:identifier "t0271"^^xsd:token;
  dct:source "https://nrc-publications.canada.ca/eng/view/object/?id=69fb8993-1baa-4225-b33a-6a02341d383d"^^xsd:anyURI,
    "https://nrc-publications.canada.ca/fra/voir/objet/?id=549123c3-092c-4fca-8dea-99d53eac06dd"^^xsd:anyURI;
  skos:altLabel "fossil ice"@en;
  skos:definition "Ice formed in, and remaining from, the geologically recent past."@en;
  skos:inScheme <https://w3id.org/permafrost/v/nrcglossary/scheme>;
  skos:prefLabel "relict ice"@en;
  skos:scopeNote "Relict ice may include ground ice preserved in cold regions such as the coastal plains of western Arctic Canada and northern Siberia, where relict permafrost of Pleistocene age has been preserved. In Russian literature the term is usually associated with buried ice."@en;
  skos:topConceptOf <https://w3id.org/permafrost/v/nrcglossary/scheme> .

<https://w3id.org/permafrost/v/nrcglossary/t0272> a skos:Concept;
  dct:identifier "t0272"^^xsd:token;
  dct:source "https://nrc-publications.canada.ca/eng/view/object/?id=69fb8993-1baa-4225-b33a-6a02341d383d"^^xsd:anyURI,
    "https://nrc-publications.canada.ca/fra/voir/objet/?id=549123c3-092c-4fca-8dea-99d53eac06dd"^^xsd:anyURI;
  skos:altLabel "fossil permafrost"@en;
  skos:definition "Permafrost existing in areas where permafrost can not form under present climatic conditions."@en;
  skos:inScheme <https://w3id.org/permafrost/v/nrcglossary/scheme>;
  skos:prefLabel "relict permafrost"@en;
  skos:scopeNote "Relict permafrost (including relict ice) formed when the mean annual surface temperature was lower than at present; it is in disequilibrium with the present mean annual surface temperature. This permafrost persists in places where it could not form today."@en;
  skos:topConceptOf <https://w3id.org/permafrost/v/nrcglossary/scheme> .

<https://w3id.org/permafrost/v/nrcglossary/t0273> a skos:Concept;
  dct:identifier "t0273"^^xsd:token;
  dct:source "https://nrc-publications.canada.ca/eng/view/object/?id=69fb8993-1baa-4225-b33a-6a02341d383d"^^xsd:anyURI,
    "https://nrc-publications.canada.ca/fra/voir/objet/?id=549123c3-092c-4fca-8dea-99d53eac06dd"^^xsd:anyURI;
  skos:definition "The effective stress generated in a thawing soil if no volume change is permitted during thaw."@en;
  skos:inScheme <https://w3id.org/permafrost/v/nrcglossary/scheme>;
  skos:prefLabel "contrainte résiduelle"@fr, "residual stress"@en;
  skos:topConceptOf <https://w3id.org/permafrost/v/nrcglossary/scheme> .

<https://w3id.org/permafrost/v/nrcglossary/t0274> a skos:Concept;
  dct:identifier "t0274"^^xsd:token;
  dct:source "https://nrc-publications.canada.ca/eng/view/object/?id=69fb8993-1baa-4225-b33a-6a02341d383d"^^xsd:anyURI,
    "https://nrc-publications.canada.ca/fra/voir/objet/?id=549123c3-092c-4fca-8dea-99d53eac06dd"^^xsd:anyURI;
  skos:definition "A layer of thawed ground between the seasonally frozen ground and the permafrost table (see Figure 4)."@en;
  skos:inScheme <https://w3id.org/permafrost/v/nrcglossary/scheme>;
  skos:prefLabel "couche dégelée résiduelle"@fr, "residual thaw layer"@en;
  skos:scopeNote "This layer may result from thawing of the permafrost which causes a lowering of the permafrost table, or from incomplete freezing of the active layer during a mild winter after a very warm summer, or during a winter in which an unusually heavy snowfall (providing a thick insulating cover on the ground surface) occurs before extreme cold sets in. It may exist for one year or for several years, or it may be permanent if permafrost is degrading due to climatic warming or changes in terrain conditions resulting from natural or human disturbance or activity. This layer does not exist where the seasonal frost extends to the permafrost table."@en;
  skos:topConceptOf <https://w3id.org/permafrost/v/nrcglossary/scheme> .

<https://w3id.org/permafrost/v/nrcglossary/t0275> a skos:Concept;
  dct:identifier "t0275"^^xsd:token;
  dct:source "https://nrc-publications.canada.ca/eng/view/object/?id=69fb8993-1baa-4225-b33a-6a02341d383d"^^xsd:anyURI,
    "https://nrc-publications.canada.ca/fra/voir/objet/?id=549123c3-092c-4fca-8dea-99d53eac06dd"^^xsd:anyURI;
  skos:definition "The cryostructure in which horizontal and vertical ice veins form a three- dimensional, irregular rectangular lattice (see Figure 9e)."@en;
  skos:inScheme <https://w3id.org/permafrost/v/nrcglossary/scheme>;
  skos:prefLabel "reticulate-blocky cryostructure"@en;
  skos:scopeNote "The mesh size in reticulate-blocky cryostructure is larger and more irregular than that in reticulate cryostructure. It is found in frozen loam, silt and clay deposits with a high ice content."@en;
  skos:topConceptOf <https://w3id.org/permafrost/v/nrcglossary/scheme> .

<https://w3id.org/permafrost/v/nrcglossary/t0276> a skos:Concept;
  dct:identifier "t0276"^^xsd:token;
  dct:source "https://nrc-publications.canada.ca/eng/view/object/?id=69fb8993-1baa-4225-b33a-6a02341d383d"^^xsd:anyURI,
    "https://nrc-publications.canada.ca/fra/voir/objet/?id=549123c3-092c-4fca-8dea-99d53eac06dd"^^xsd:anyURI;
  skos:definition "The cryostructure in which horizontal and vertical ice veins form a three- dimensional, rectangular or square lattice (see Figure 9e)."@en;
  skos:inScheme <https://w3id.org/permafrost/v/nrcglossary/scheme>;
  skos:prefLabel "reticulate cryostructure"@en;
  skos:scopeNote "Reticulate cryostructure is often found in frozen glaciolacustrine sediments with a high ice content."@en;
  skos:topConceptOf <https://w3id.org/permafrost/v/nrcglossary/scheme> .

<https://w3id.org/permafrost/v/nrcglossary/t0277> a skos:Concept;
  dct:identifier "t0277"^^xsd:token;
  dct:source "https://nrc-publications.canada.ca/eng/view/object/?id=69fb8993-1baa-4225-b33a-6a02341d383d"^^xsd:anyURI,
    "https://nrc-publications.canada.ca/fra/voir/objet/?id=549123c3-092c-4fca-8dea-99d53eac06dd"^^xsd:anyURI;
  skos:definition "A network of horizontal and vertical ice veins forming a three- dimensional, often rectangular or square lattice (see Figure 9c, d)."@en;
  skos:inScheme <https://w3id.org/permafrost/v/nrcglossary/scheme>;
  skos:prefLabel "reticulate ice"@en;
  skos:scopeNote "Field observations suggest that reticulate ice veins grow in horizontal and vertical shrinkage cracks with much of the water coming from the adjacent material in a semi-closed freezing system, rather than from migration of water in an open system. It is commonly found in frozen glaciolacustrine sediments."@en;
  skos:topConceptOf <https://w3id.org/permafrost/v/nrcglossary/scheme> .

<https://w3id.org/permafrost/v/nrcglossary/t0278> a skos:Concept;
  dct:identifier "t0278"^^xsd:token;
  dct:source "https://nrc-publications.canada.ca/eng/view/object/?id=69fb8993-1baa-4225-b33a-6a02341d383d"^^xsd:anyURI,
    "https://nrc-publications.canada.ca/fra/voir/objet/?id=549123c3-092c-4fca-8dea-99d53eac06dd"^^xsd:anyURI;
  skos:altLabel "bi-modal flow"@en, "ground-ice slump"@en, "ice slump"@en, "retrogressive-thaw flow slide"@en,
    "thermo-erosional cirque"@en, "thermocirque"@en;
  skos:definition "A slope failure resulting from thawing of ice-rich permafrost (see Figure 21c, d)."@en;
  skos:inScheme <https://w3id.org/permafrost/v/nrcglossary/scheme>;
  skos:prefLabel "glissement régressif dû au dégel"@fr, "retrogressive thaw slump"@en;
  skos:scopeNote "Retrogressive thaw slumps consist of a steep headwall that retreats in a retrogressive fashion due to thawing, and a debris flow formed by the mixture of thawed sediment and meltwater that slides down the face of the headwall and flows away. Such slumps are common in ice-rich glaciolacustrine sediments and fine- grained diamictons."@en;
  skos:topConceptOf <https://w3id.org/permafrost/v/nrcglossary/scheme> .

<https://w3id.org/permafrost/v/nrcglossary/t0279> a skos:Concept;
  dct:identifier "t0279"^^xsd:token;
  dct:source "https://nrc-publications.canada.ca/eng/view/object/?id=69fb8993-1baa-4225-b33a-6a02341d383d"^^xsd:anyURI,
    "https://nrc-publications.canada.ca/fra/voir/objet/?id=549123c3-092c-4fca-8dea-99d53eac06dd"^^xsd:anyURI;
  skos:definition "A layer or body of unfrozen ground occupying a depression in the permafrost table beneath a river."@en;
  skos:inScheme <https://w3id.org/permafrost/v/nrcglossary/scheme>;
  skos:prefLabel "river talik"@en;
  skos:scopeNote "The temperature of a river talik remains above 0°C due to the heat storage effect of the river water. Depending on the permafrost thickness and the size of the river, such taliks may be either open or closed."@en;
  skos:topConceptOf <https://w3id.org/permafrost/v/nrcglossary/scheme> .

<https://w3id.org/permafrost/v/nrcglossary/t0280> a skos:Concept;
  dct:identifier "t0280"^^xsd:token;
  dct:source "https://nrc-publications.canada.ca/eng/view/object/?id=69fb8993-1baa-4225-b33a-6a02341d383d"^^xsd:anyURI,
    "https://nrc-publications.canada.ca/fra/voir/objet/?id=549123c3-092c-4fca-8dea-99d53eac06dd"^^xsd:anyURI;
  skos:definition "A mass of rock fragments and finer material, on a slope, that contains either interstitial ice or an ice core and shows evidence of past or present movement."@en;
  skos:inScheme <https://w3id.org/permafrost/v/nrcglossary/scheme>;
  skos:prefLabel "rock glacier"@en;
  skos:scopeNote "Rock glaciers do not form where there is insufficient moisture to form the interstitial ice that permits movement of the mass. Some are believed to have been formed, at least partly, by burial of glacier ice. Active rock glaciers move at speeds up to 50 m per year and possess steep fronts with slope angles greater than the angle of repose. Rock glaciers are said to be inactive when the main body ceases to move. Most rock glaciers have transverse ridges and furrows on their surface."@en;
  skos:topConceptOf <https://w3id.org/permafrost/v/nrcglossary/scheme> .

<https://w3id.org/permafrost/v/nrcglossary/t0281> a skos:Concept;
  dct:identifier "t0281"^^xsd:token;
  dct:source "https://nrc-publications.canada.ca/eng/view/object/?id=69fb8993-1baa-4225-b33a-6a02341d383d"^^xsd:anyURI,
    "https://nrc-publications.canada.ca/fra/voir/objet/?id=549123c3-092c-4fca-8dea-99d53eac06dd"^^xsd:anyURI;
  skos:definition "Permafrost in which part or all of the total water content is unfrozen because of freezing-point depression due to the dissolved-solids content of the pore water."@en;
  skos:inScheme <https://w3id.org/permafrost/v/nrcglossary/scheme>;
  skos:prefLabel "saline permafrost"@en;
  skos:scopeNote "Saline permafrost is found in cryopegs. At temperatures below the ice- nucleation temperature, a higher than normal unfrozen water content will persist due to increased dissolved-solids content of the remaining pore water."@en;
  skos:topConceptOf <https://w3id.org/permafrost/v/nrcglossary/scheme> .

<https://w3id.org/permafrost/v/nrcglossary/t0282> a skos:Concept;
  dct:identifier "t0282"^^xsd:token;
  dct:source "https://nrc-publications.canada.ca/eng/view/object/?id=69fb8993-1baa-4225-b33a-6a02341d383d"^^xsd:anyURI,
    "https://nrc-publications.canada.ca/fra/voir/objet/?id=549123c3-092c-4fca-8dea-99d53eac06dd"^^xsd:anyURI;
  skos:definition "1. A general property of aqueous solutions caused by the alkali, alkaline earth, and metal salts of strong acids (Cl, SO4 and NO3) that are not hydrolyzed. 2. In soil science, the ratio of the weight of salt in a soil sample to the total weight of the sample."@en;
  skos:inScheme <https://w3id.org/permafrost/v/nrcglossary/scheme>;
  skos:prefLabel "salinity"@en;
  skos:scopeNote "Often used, inappropriately, as a synonym for the dissolved-solids content of aqueous solutions."@en;
  skos:topConceptOf <https://w3id.org/permafrost/v/nrcglossary/scheme> .

<https://w3id.org/permafrost/v/nrcglossary/t0283> a skos:Concept;
  dct:identifier "t0283"^^xsd:token;
  dct:source "https://nrc-publications.canada.ca/eng/view/object/?id=69fb8993-1baa-4225-b33a-6a02341d383d"^^xsd:anyURI,
    "https://nrc-publications.canada.ca/fra/voir/objet/?id=549123c3-092c-4fca-8dea-99d53eac06dd"^^xsd:anyURI;
  skos:definition "A wedge-shaped body of sand produced by filling of a thermal contraction crack with sand either blown in from above or washed down the walls of the crack (see Figure 17h)."@en;
  skos:hiddenLabel "tesselation"@en;
  skos:inScheme <https://w3id.org/permafrost/v/nrcglossary/scheme>;
  skos:prefLabel "sand wedge"@en;
  skos:scopeNote "Sand wedges are wedges of primary filling since, at the time of their formation, they are filled with mineral soil. Upon thawing of the permafrost, there is little or no void space left, and any subsequent downward movement of material into the wedge is negligible. A sand wedge is not a replacement feature (or ice-wedge cast) associated with the melting of an ice wedge. It is a type of soil wedge showing marked vertical fabric and laminations."@en;
  skos:topConceptOf <https://w3id.org/permafrost/v/nrcglossary/scheme> .

<https://w3id.org/permafrost/v/nrcglossary/t0284> a skos:Concept;
  dct:identifier "t0284"^^xsd:token;
  dct:source "https://nrc-publications.canada.ca/eng/view/object/?id=69fb8993-1baa-4225-b33a-6a02341d383d"^^xsd:anyURI,
    "https://nrc-publications.canada.ca/fra/voir/objet/?id=549123c3-092c-4fca-8dea-99d53eac06dd"^^xsd:anyURI;
  skos:definition "A polygon outlined by sand wedges underlying its boundaries."@en;
  skos:inScheme <https://w3id.org/permafrost/v/nrcglossary/scheme>;
  skos:prefLabel "sand-wedge polygon"@en;
  skos:scopeNote "Sand-wedge polygons may be formed by seasonal thermal contraction cracking in areas of deep seasonal frost."@en;
  skos:topConceptOf <https://w3id.org/permafrost/v/nrcglossary/scheme> .

<https://w3id.org/permafrost/v/nrcglossary/t0285> a skos:Concept;
  dct:identifier "t0285"^^xsd:token;
  dct:source "https://nrc-publications.canada.ca/eng/view/object/?id=69fb8993-1baa-4225-b33a-6a02341d383d"^^xsd:anyURI,
    "https://nrc-publications.canada.ca/fra/voir/objet/?id=549123c3-092c-4fca-8dea-99d53eac06dd"^^xsd:anyURI;
  skos:definition "The cumulative number of degree-days below 0°C, calculated as the arithmetic sum of all the negative and positive mean daily air temperatures (°C) for a specific station during the time period between the highest point in the fall and the lowest point the next spring on the cumulative degree-day time curve."@en;
  skos:inScheme <https://w3id.org/permafrost/v/nrcglossary/scheme>;
  skos:prefLabel "seasonal freezing index"@en;
  skos:topConceptOf <https://w3id.org/permafrost/v/nrcglossary/scheme> .

<https://w3id.org/permafrost/v/nrcglossary/t0286> a skos:Concept;
  dct:identifier "t0286"^^xsd:token;
  dct:source "https://nrc-publications.canada.ca/eng/view/object/?id=69fb8993-1baa-4225-b33a-6a02341d383d"^^xsd:anyURI,
    "https://nrc-publications.canada.ca/fra/voir/objet/?id=549123c3-092c-4fca-8dea-99d53eac06dd"^^xsd:anyURI;
  skos:definition "The occurrence of ground temperatures below 0°C for only part of the year."@en;
  skos:hiddenLabel "active frost"@en, "winter frost"@en;
  skos:inScheme <https://w3id.org/permafrost/v/nrcglossary/scheme>;
  skos:prefLabel "seasonal frost"@en;
  skos:topConceptOf <https://w3id.org/permafrost/v/nrcglossary/scheme> .

<https://w3id.org/permafrost/v/nrcglossary/t0287> a skos:Concept;
  dct:identifier "t0287"^^xsd:token;
  dct:source "https://nrc-publications.canada.ca/eng/view/object/?id=69fb8993-1baa-4225-b33a-6a02341d383d"^^xsd:anyURI,
    "https://nrc-publications.canada.ca/fra/voir/objet/?id=549123c3-092c-4fca-8dea-99d53eac06dd"^^xsd:anyURI;
  skos:definition "The cumulative number of degree-days above 0°C, calculated as the arithmetic sum of all the positive and negative mean daily air temperatures (°C) for a specific station during the time period between the lowest point in the spring and the highest point the next fall on the cumulative degree-day time curve."@en;
  skos:inScheme <https://w3id.org/permafrost/v/nrcglossary/scheme>;
  skos:prefLabel "seasonal thawing index"@en;
  skos:topConceptOf <https://w3id.org/permafrost/v/nrcglossary/scheme> .

<https://w3id.org/permafrost/v/nrcglossary/t0288> a skos:Concept;
  dct:identifier "t0288"^^xsd:token;
  dct:source "https://nrc-publications.canada.ca/eng/view/object/?id=69fb8993-1baa-4225-b33a-6a02341d383d"^^xsd:anyURI,
    "https://nrc-publications.canada.ca/fra/voir/objet/?id=549123c3-092c-4fca-8dea-99d53eac06dd"^^xsd:anyURI;
  skos:definition "The uppermost layer of the permafrost which undergoes seasonal phase changes due to a lowered thawing temperature (see Figures 2 and 4)."@en;
  skos:inScheme <https://w3id.org/permafrost/v/nrcglossary/scheme>;
  skos:prefLabel "seasonally-active permafrost"@en;
  skos:scopeNote "Seasonally-active permafrost can occur wherever its salinity or clay content allows it to thaw and refreeze annually, even though the materials remains cryotic (T < 0°C). It forms part of the active layer."@en;
  skos:topConceptOf <https://w3id.org/permafrost/v/nrcglossary/scheme> .

<https://w3id.org/permafrost/v/nrcglossary/t0289> a skos:Concept;
  dct:identifier "t0289"^^xsd:token;
  dct:source "https://nrc-publications.canada.ca/eng/view/object/?id=69fb8993-1baa-4225-b33a-6a02341d383d"^^xsd:anyURI,
    "https://nrc-publications.canada.ca/fra/voir/objet/?id=549123c3-092c-4fca-8dea-99d53eac06dd"^^xsd:anyURI;
  skos:definition "Ground that freezes and thaws annually (see Figures 2 and 4)."@en;
  skos:inScheme <https://w3id.org/permafrost/v/nrcglossary/scheme>;
  skos:prefLabel "gélisol saisonnier"@fr, "seasonally frozen ground"@en;
  skos:scopeNote "In Russian and Chinese literature, seasonally frozen ground forms the \"active layer\" in areas without permafrost or with a deep permafrost table."@en;
  skos:topConceptOf <https://w3id.org/permafrost/v/nrcglossary/scheme> .

<https://w3id.org/permafrost/v/nrcglossary/t0290> a skos:Concept;
  dct:identifier "t0290"^^xsd:token;
  dct:source "https://nrc-publications.canada.ca/eng/view/object/?id=69fb8993-1baa-4225-b33a-6a02341d383d"^^xsd:anyURI,
    "https://nrc-publications.canada.ca/fra/voir/objet/?id=549123c3-092c-4fca-8dea-99d53eac06dd"^^xsd:anyURI;
  skos:definition "Active layer in areas without permafrost."@en;
  skos:inScheme <https://w3id.org/permafrost/v/nrcglossary/scheme>;
  skos:prefLabel "seasonally frozen layer (SFL)"@en;
  skos:scopeNote "In Chinese and Russian literature, the seasonally frozen layer is synonymous with the \"active layer\" in areas without permafrost or with a deep permafrost table. It is underlain by unfrozen ground and usually has a positive mean annual ground temperature. Freezing progresses from the surface downward, whereas thawing progresses both downward from the surface, and upward from the bottom of the seasonally frozen layer."@en;
  skos:topConceptOf <https://w3id.org/permafrost/v/nrcglossary/scheme> .

<https://w3id.org/permafrost/v/nrcglossary/t0291> a skos:Concept;
  dct:identifier "t0291"^^xsd:token;
  dct:source "https://nrc-publications.canada.ca/eng/view/object/?id=69fb8993-1baa-4225-b33a-6a02341d383d"^^xsd:anyURI,
    "https://nrc-publications.canada.ca/fra/voir/objet/?id=549123c3-092c-4fca-8dea-99d53eac06dd"^^xsd:anyURI;
  skos:definition "Ground that thaws and refreezes annually (see Figures 2 and 4)."@en;
  skos:inScheme <https://w3id.org/permafrost/v/nrcglossary/scheme>;
  skos:prefLabel "seasonally thawed ground"@en;
  skos:scopeNote "In areas with permafrost, seasonally thawed ground forms the active layer; it can include the uppermost portion of the permafrost in places where annual thawing takes place at temperatures slightly below 0°C, due to high salinity or a high clay content."@en;
  skos:topConceptOf <https://w3id.org/permafrost/v/nrcglossary/scheme> .

<https://w3id.org/permafrost/v/nrcglossary/t0292> a skos:Concept;
  dct:identifier "t0292"^^xsd:token;
  dct:source "https://nrc-publications.canada.ca/eng/view/object/?id=69fb8993-1baa-4225-b33a-6a02341d383d"^^xsd:anyURI,
    "https://nrc-publications.canada.ca/fra/voir/objet/?id=549123c3-092c-4fca-8dea-99d53eac06dd"^^xsd:anyURI;
  skos:definition "The active layer in permafrost areas."@en;
  skos:inScheme <https://w3id.org/permafrost/v/nrcglossary/scheme>;
  skos:prefLabel "seasonally thawed layer (STL)"@en;
  skos:scopeNote "The seasonally thawed layer is synonymous with the active layer in areas with permafrost where seasonal freezing commonly reaches the permafrost table. Thawing progresses from the surface downward, whereas freezing progresses both downward from the surface and upward from the permafrost table. The seasonally thawed layer usually has a negative mean annual ground temperature."@en;
  skos:topConceptOf <https://w3id.org/permafrost/v/nrcglossary/scheme> .

<https://w3id.org/permafrost/v/nrcglossary/t0293> a skos:Concept;
  dct:identifier "t0293"^^xsd:token;
  dct:source "https://nrc-publications.canada.ca/eng/view/object/?id=69fb8993-1baa-4225-b33a-6a02341d383d"^^xsd:anyURI,
    "https://nrc-publications.canada.ca/fra/voir/objet/?id=549123c3-092c-4fca-8dea-99d53eac06dd"^^xsd:anyURI;
  skos:definition "Ice in discrete layers or ice lenses, formed by ice segregation (Figure 9a)."@en;
  skos:hiddenLabel "Taber ice"@en, "ice gneiss"@en, "sirloin ice"@en;
  skos:inScheme <https://w3id.org/permafrost/v/nrcglossary/scheme>;
  skos:prefLabel "segregated ice"@en;
  skos:scopeNote "Segregated ice can range in thickness from hairline to more than 10 m. It commonly occurs in alternating layers of ice and soil (see ice lens)."@en;
  skos:topConceptOf <https://w3id.org/permafrost/v/nrcglossary/scheme> .

<https://w3id.org/permafrost/v/nrcglossary/t0294> a skos:Concept;
  dct:identifier "t0294"^^xsd:token;
  dct:source "https://nrc-publications.canada.ca/eng/view/object/?id=69fb8993-1baa-4225-b33a-6a02341d383d"^^xsd:anyURI,
    "https://nrc-publications.canada.ca/fra/voir/objet/?id=549123c3-092c-4fca-8dea-99d53eac06dd"^^xsd:anyURI;
  skos:definition "The ratio of the rate of moisture migration to the temperature gradient in a frozen soil near the 0°C isotherm."@en;
  skos:inScheme <https://w3id.org/permafrost/v/nrcglossary/scheme>;
  skos:prefLabel "potentiel de ségrégation"@fr, "segregation potential"@en;
  skos:scopeNote "An engineering parameter that couples mass (water) flow and heat flow in a freezing soil. It is used by some workers to predict amounts of frost heave."@en;
  skos:topConceptOf <https://w3id.org/permafrost/v/nrcglossary/scheme> .

<https://w3id.org/permafrost/v/nrcglossary/t0295> a skos:Concept;
  dct:identifier "t0295"^^xsd:token;
  dct:source "https://nrc-publications.canada.ca/eng/view/object/?id=69fb8993-1baa-4225-b33a-6a02341d383d"^^xsd:anyURI,
    "https://nrc-publications.canada.ca/fra/voir/objet/?id=549123c3-092c-4fca-8dea-99d53eac06dd"^^xsd:anyURI;
  skos:definition "The failure strength of a material under a short-term loading (e.g. up to about 10 minutes in a uniaxial compression test)."@en;
  skos:inScheme <https://w3id.org/permafrost/v/nrcglossary/scheme>;
  skos:prefLabel "short-term strength"@en;
  skos:topConceptOf <https://w3id.org/permafrost/v/nrcglossary/scheme> .

<https://w3id.org/permafrost/v/nrcglossary/t0296> a skos:Concept;
  dct:identifier "t0296"^^xsd:token;
  dct:source "https://nrc-publications.canada.ca/eng/view/object/?id=69fb8993-1baa-4225-b33a-6a02341d383d"^^xsd:anyURI,
    "https://nrc-publications.canada.ca/fra/voir/objet/?id=549123c3-092c-4fca-8dea-99d53eac06dd"^^xsd:anyURI;
  skos:definition "A passive heat transfer device, filled with either a liquid or a gas, installed to remove heat from the ground (see Figure 24)."@en;
  skos:inScheme <https://w3id.org/permafrost/v/nrcglossary/scheme>;
  skos:prefLabel "single-phase thermosyphon"@en;
  skos:scopeNote "A single-phase thermosyphon usually consists of a sealed tube, with a small radiator above the ground surface, containing a fluid (liquid or gas) which does not change phase. These devices have no moving parts, and they require no external power for operation. During the winter, heat from the soil surrounding the embedded portion of the pipe is absorbed by and thus warms the working fluid, which rises to the above- ground radiator section of the pipe exposed to the cooler air and loses its heat by conduction and natural convection."@en;
  skos:topConceptOf <https://w3id.org/permafrost/v/nrcglossary/scheme> .

<https://w3id.org/permafrost/v/nrcglossary/t0297> a skos:Concept;
  dct:identifier "t0297"^^xsd:token;
  dct:source "https://nrc-publications.canada.ca/eng/view/object/?id=69fb8993-1baa-4225-b33a-6a02341d383d"^^xsd:anyURI,
    "https://nrc-publications.canada.ca/fra/voir/objet/?id=549123c3-092c-4fca-8dea-99d53eac06dd"^^xsd:anyURI;
  skos:definition "Ice crystals precipitated from the atmosphere, mainly in complex hexagon (plate, column or needle) form, often agglomerated into snowflakes."@en;
  skos:inScheme <https://w3id.org/permafrost/v/nrcglossary/scheme>;
  skos:prefLabel "snow"@en;
  skos:scopeNote "Meteorologically, snow also includes snow grains (opaque granular ice particles). Snow pellets are aggregations of supercooled water droplets collected on an initial ice crystal."@en;
  skos:topConceptOf <https://w3id.org/permafrost/v/nrcglossary/scheme> .

<https://w3id.org/permafrost/v/nrcglossary/t0298> a skos:Concept;
  dct:identifier "t0298"^^xsd:token;
  dct:source "https://nrc-publications.canada.ca/eng/view/object/?id=69fb8993-1baa-4225-b33a-6a02341d383d"^^xsd:anyURI,
    "https://nrc-publications.canada.ca/fra/voir/objet/?id=549123c3-092c-4fca-8dea-99d53eac06dd"^^xsd:anyURI;
  skos:definition "The accumulation of fallen snow covering the ground."@en;
  skos:inScheme <https://w3id.org/permafrost/v/nrcglossary/scheme>;
  skos:prefLabel "snowcover"@en;
  skos:topConceptOf <https://w3id.org/permafrost/v/nrcglossary/scheme> .

<https://w3id.org/permafrost/v/nrcglossary/t0299> a skos:Concept;
  dct:identifier "t0299"^^xsd:token;
  dct:source "https://nrc-publications.canada.ca/eng/view/object/?id=69fb8993-1baa-4225-b33a-6a02341d383d"^^xsd:anyURI,
    "https://nrc-publications.canada.ca/fra/voir/objet/?id=549123c3-092c-4fca-8dea-99d53eac06dd"^^xsd:anyURI;
  skos:definition "An accumulation of wind-blown snow, commonly considerably thicker than the surrounding snowcover."@en;
  skos:inScheme <https://w3id.org/permafrost/v/nrcglossary/scheme>;
  skos:prefLabel "snowdrift"@en;
  skos:topConceptOf <https://w3id.org/permafrost/v/nrcglossary/scheme> .

<https://w3id.org/permafrost/v/nrcglossary/t0300> a skos:Concept;
  dct:identifier "t0300"^^xsd:token;
  dct:source "https://nrc-publications.canada.ca/eng/view/object/?id=69fb8993-1baa-4225-b33a-6a02341d383d"^^xsd:anyURI,
    "https://nrc-publications.canada.ca/fra/voir/objet/?id=549123c3-092c-4fca-8dea-99d53eac06dd"^^xsd:anyURI;
  skos:definition "The lower boundary of a highland region in which snow never melts."@en;
  skos:inScheme <https://w3id.org/permafrost/v/nrcglossary/scheme>;
  skos:prefLabel "snowline"@en;
  skos:topConceptOf <https://w3id.org/permafrost/v/nrcglossary/scheme> .

<https://w3id.org/permafrost/v/nrcglossary/t0301> a skos:Concept;
  dct:identifier "t0301"^^xsd:token;
  dct:source "https://nrc-publications.canada.ca/eng/view/object/?id=69fb8993-1baa-4225-b33a-6a02341d383d"^^xsd:anyURI,
    "https://nrc-publications.canada.ca/fra/voir/objet/?id=549123c3-092c-4fca-8dea-99d53eac06dd"^^xsd:anyURI;
  skos:definition "Melting of the snowcover, and also the period during which melting of the snowcover occurs at the end of the winter."@en;
  skos:inScheme <https://w3id.org/permafrost/v/nrcglossary/scheme>;
  skos:prefLabel "snowmelt"@en;
  skos:topConceptOf <https://w3id.org/permafrost/v/nrcglossary/scheme> .

<https://w3id.org/permafrost/v/nrcglossary/t0302> a skos:Concept;
  dct:identifier "t0302"^^xsd:token;
  dct:source "https://nrc-publications.canada.ca/eng/view/object/?id=69fb8993-1baa-4225-b33a-6a02341d383d"^^xsd:anyURI,
    "https://nrc-publications.canada.ca/fra/voir/objet/?id=549123c3-092c-4fca-8dea-99d53eac06dd"^^xsd:anyURI;
  skos:definition "Relatively small area of snowcover remaining after the main snowmelt period."@en;
  skos:inScheme <https://w3id.org/permafrost/v/nrcglossary/scheme>;
  skos:prefLabel "snowpatch"@en;
  skos:scopeNote "Such areas commonly represent remnants of snowdrifts."@en;
  skos:topConceptOf <https://w3id.org/permafrost/v/nrcglossary/scheme> .

<https://w3id.org/permafrost/v/nrcglossary/t0303> a skos:Concept;
  dct:identifier "t0303"^^xsd:token;
  dct:source "https://nrc-publications.canada.ca/eng/view/object/?id=69fb8993-1baa-4225-b33a-6a02341d383d"^^xsd:anyURI,
    "https://nrc-publications.canada.ca/fra/voir/objet/?id=549123c3-092c-4fca-8dea-99d53eac06dd"^^xsd:anyURI;
  skos:definition "A wedge-shaped body of soil that is different in structure and texture from the surrounding soil (see Figure 17g)."@en;
  skos:inScheme <https://w3id.org/permafrost/v/nrcglossary/scheme>;
  skos:prefLabel "coin de sol"@fr, "soil wedge"@en;
  skos:scopeNote "A soil wedge may be an ice-wedge cast (i.e., a feature of secondary filling), or a sand wedge (i.e., a feature of primary filling), or it may be produced by repeated formation of thermal contraction cracks in seasonally frozen ground followed by filling of the crack with soil. It is usually difficult to distinguish between soil wedges in the active layer, soil occupying cracks in seasonally frozen ground (i.e., in a non-permafrost environment), soil as original fillings in cracks in permafrost, and soil replacing ice wedges."@en;
  skos:topConceptOf <https://w3id.org/permafrost/v/nrcglossary/scheme> .

<https://w3id.org/permafrost/v/nrcglossary/t0304> a skos:Concept;
  dct:identifier "t0304"^^xsd:token;
  dct:source "https://nrc-publications.canada.ca/eng/view/object/?id=69fb8993-1baa-4225-b33a-6a02341d383d"^^xsd:anyURI,
    "https://nrc-publications.canada.ca/fra/voir/objet/?id=549123c3-092c-4fca-8dea-99d53eac06dd"^^xsd:anyURI;
  skos:definition "Slow downslope flow of saturated unfrozen earth materials (see Figure 16d)."@en;
  skos:inScheme <https://w3id.org/permafrost/v/nrcglossary/scheme>;
  skos:prefLabel "solifluction"@en, "solifluxion"@fr;
  skos:scopeNote "The presence of a frozen substrate, or even freezing and thawing is not implied in the original definition (Andersson, 1906). However, one component of solifluction can be the creep of frozen ground. Rates of flow vary widely. The term is commonly applied to processes operating in both seasonal frost and permafrost areas."@en;
  skos:topConceptOf <https://w3id.org/permafrost/v/nrcglossary/scheme> .

<https://w3id.org/permafrost/v/nrcglossary/t0305> a skos:Concept;
  dct:identifier "t0305"^^xsd:token;
  dct:source "https://nrc-publications.canada.ca/eng/view/object/?id=69fb8993-1baa-4225-b33a-6a02341d383d"^^xsd:anyURI,
    "https://nrc-publications.canada.ca/fra/voir/objet/?id=549123c3-092c-4fca-8dea-99d53eac06dd"^^xsd:anyURI;
  skos:definition "A fan-like deposit at the base of a slope, produced by solifluction."@en;
  skos:inScheme <https://w3id.org/permafrost/v/nrcglossary/scheme>;
  skos:prefLabel "solifluction apron"@en;
  skos:topConceptOf <https://w3id.org/permafrost/v/nrcglossary/scheme> .

<https://w3id.org/permafrost/v/nrcglossary/t0306> a skos:Concept;
  dct:identifier "t0306"^^xsd:token;
  dct:source "https://nrc-publications.canada.ca/eng/view/object/?id=69fb8993-1baa-4225-b33a-6a02341d383d"^^xsd:anyURI,
    "https://nrc-publications.canada.ca/fra/voir/objet/?id=549123c3-092c-4fca-8dea-99d53eac06dd"^^xsd:anyURI;
  skos:altLabel "solifluction bench"@en, "solifluction step"@en;
  skos:definition "Geomorphological features of varying scale produced by the process of solifluction (see Figure 16d)."@en;
  skos:hiddenLabel "soliflual garland terrace"@en;
  skos:inScheme <https://w3id.org/permafrost/v/nrcglossary/scheme>;
  skos:prefLabel "formes dues à la solifluxion"@fr, "solifluction features"@en;
  skos:scopeNote "Typical solifluction features include: 1. solifluction apron - a fan-like deposit at the base of a slope; 2. solifluction lobe - an isolated, tongue-shaped feature, up to 25 m wide and 150 m or more long, formed by more rapid solifluction on certain sections of a slope showing variations in gradient; commonly has a steep (15?-60?) front and a relatively smooth upper surface. Fronts covered by a vegetation mat are called \"turf-banked lobes\" whereas those that are stony are called \"stone- banked lobes\". SYNONYM: (not recommended) mud-debris tongue. 3. solifluction sheet - a broad deposit of nonsorted, water-saturated, locally derived materials that is moving or has moved downslope. Sorted and/or nonsorted stripes are commonly associated with solifluction sheets. SYNONYM: solifluction mantle. 4. solifluction terrace - a low step, or bench, with a straight or lobate front, the latter reflecting local differences in rate of flow. A solifluction terrace may have bare mineral soil on the upslope part and 'folded-under' organic matter in both the seasonally thawed ground and the frozen ground. Those covered with a vegetation mat are called \"turf-banked terraces\"; those that are stony are called \"stone-banked terraces\"."@en;
  skos:topConceptOf <https://w3id.org/permafrost/v/nrcglossary/scheme> .

<https://w3id.org/permafrost/v/nrcglossary/t0307> a skos:Concept;
  dct:identifier "t0307"^^xsd:token;
  dct:source "https://nrc-publications.canada.ca/eng/view/object/?id=69fb8993-1baa-4225-b33a-6a02341d383d"^^xsd:anyURI,
    "https://nrc-publications.canada.ca/fra/voir/objet/?id=549123c3-092c-4fca-8dea-99d53eac06dd"^^xsd:anyURI;
  skos:definition "An isolated, tongue-shaped solifluction feature, up to 25 m wide and 150 m or more long, formed by more rapid solifluction on certain sections of a slope showing variations in gradient."@en;
  skos:hiddenLabel "mud-debris tongue"@en;
  skos:inScheme <https://w3id.org/permafrost/v/nrcglossary/scheme>;
  skos:prefLabel "solifluction lobe"@en;
  skos:scopeNote "Commonly has a steep (15?-60?) front and a relatively smooth upper surface. Solifluction lobes with fronts covered by a vegetation mat are called \"turf-banked lobes\" whereas those that are stony are called \"stone-banked lobes\"."@en;
  skos:topConceptOf <https://w3id.org/permafrost/v/nrcglossary/scheme> .

<https://w3id.org/permafrost/v/nrcglossary/t0308> a skos:Concept;
  dct:identifier "t0308"^^xsd:token;
  dct:source "https://nrc-publications.canada.ca/eng/view/object/?id=69fb8993-1baa-4225-b33a-6a02341d383d"^^xsd:anyURI,
    "https://nrc-publications.canada.ca/fra/voir/objet/?id=549123c3-092c-4fca-8dea-99d53eac06dd"^^xsd:anyURI;
  skos:altLabel "solifluction mantle"@en;
  skos:definition "A broad deposit of nonsorted, water-saturated, locally derived materials that is moving or has moved downslope."@en;
  skos:inScheme <https://w3id.org/permafrost/v/nrcglossary/scheme>;
  skos:prefLabel "solifluction sheet"@en;
  skos:scopeNote "Sorted and/or nonsorted stripes are commonly associated with solifluction sheets."@en;
  skos:topConceptOf <https://w3id.org/permafrost/v/nrcglossary/scheme> .

<https://w3id.org/permafrost/v/nrcglossary/t0309> a skos:Concept;
  dct:identifier "t0309"^^xsd:token;
  dct:source "https://nrc-publications.canada.ca/eng/view/object/?id=69fb8993-1baa-4225-b33a-6a02341d383d"^^xsd:anyURI,
    "https://nrc-publications.canada.ca/fra/voir/objet/?id=549123c3-092c-4fca-8dea-99d53eac06dd"^^xsd:anyURI;
  skos:altLabel "solifluction bench"@en, "solifluction step"@en;
  skos:definition "A low step, or bench, with a straight or lobate front, the latter reflecting local differences in the rate of solifluction movement."@en;
  skos:hiddenLabel "soliflual garland terrace"@en;
  skos:inScheme <https://w3id.org/permafrost/v/nrcglossary/scheme>;
  skos:prefLabel "solifluction terrace"@en;
  skos:scopeNote "A solifluction terrace may have bare mineral soil on the upslope part and 'folded-under' organic matter in both the seasonally thawed ground and the frozen ground. Those covered with a vegetation mat are called \"turf-banked (solifluction) terraces\"; those that are stony are called \"stone-banked (solifluction) terraces\"."@en;
  skos:topConceptOf <https://w3id.org/permafrost/v/nrcglossary/scheme> .

<https://w3id.org/permafrost/v/nrcglossary/t0310> a skos:Concept;
  dct:identifier "t0310"^^xsd:token;
  dct:source "https://nrc-publications.canada.ca/eng/view/object/?id=69fb8993-1baa-4225-b33a-6a02341d383d"^^xsd:anyURI,
    "https://nrc-publications.canada.ca/fra/voir/objet/?id=549123c3-092c-4fca-8dea-99d53eac06dd"^^xsd:anyURI;
  skos:definition "A sorted circle is a patterned ground form that is equidimensional in several directions, with a dominantly circular outline, and a sorted appearance commonly due to a border of stones surrounding a central area of finer material."@en;
  skos:inScheme <https://w3id.org/permafrost/v/nrcglossary/scheme>;
  skos:prefLabel "sorted circle"@en;
  skos:scopeNote "Sorted circles occur singly or in groups; their diameter is commonly between 0.5 and 3.0 m. Their central areas have a concentration of fines, with or without stones. The stones of the borders surrounding the central areas tend to increase in size with the size of the circles. Tabular stones tend to stand on edge, with their long axes in the vertical plane parallel to the border."@en;
  skos:topConceptOf <https://w3id.org/permafrost/v/nrcglossary/scheme> .

<https://w3id.org/permafrost/v/nrcglossary/t0311> a skos:Concept;
  dct:identifier "t0311"^^xsd:token;
  dct:source "https://nrc-publications.canada.ca/eng/view/object/?id=69fb8993-1baa-4225-b33a-6a02341d383d"^^xsd:anyURI,
    "https://nrc-publications.canada.ca/fra/voir/objet/?id=549123c3-092c-4fca-8dea-99d53eac06dd"^^xsd:anyURI;
  skos:definition "A sorted net is a type of patterned ground with cells that are equidimensional in several directions, neither dominantly circular nor polygonal, with a sorted appearance commonly due to borders of stones surrounding central areas of finer material."@en;
  skos:inScheme <https://w3id.org/permafrost/v/nrcglossary/scheme>;
  skos:prefLabel "sorted net"@en;
  skos:scopeNote "Sorted nets occur most frequently on nearly horizontal surfaces. Diameters of individual cells range from 0.5 to as much as 10 m. Central areas have a concentration of fines, with or without stones. The bordering stones tend to increase in size with the size of the net."@en;
  skos:topConceptOf <https://w3id.org/permafrost/v/nrcglossary/scheme> .

<https://w3id.org/permafrost/v/nrcglossary/t0312> a skos:Concept;
  dct:identifier "t0312"^^xsd:token;
  dct:source "https://nrc-publications.canada.ca/eng/view/object/?id=69fb8993-1baa-4225-b33a-6a02341d383d"^^xsd:anyURI,
    "https://nrc-publications.canada.ca/fra/voir/objet/?id=549123c3-092c-4fca-8dea-99d53eac06dd"^^xsd:anyURI;
  skos:definition "A sorted polygon is a patterned ground form that is equidimensional in several directions, with a dominantly polygonal outline, and a sorted appearance commonly due to a border of stones surrounding a central area of finer material."@en;
  skos:inScheme <https://w3id.org/permafrost/v/nrcglossary/scheme>;
  skos:prefLabel "sorted polygon"@en;
  skos:scopeNote "Sorted polygons commonly occur in extensive patterns, most frequently on nearly horizontal surfaces, and on slopes of less then 20°. They range in size from 10 cm to about 10 m. In places, small sorted polygons occur in the central areas of larger polygons. Central areas have a concentration of fines, with or without stones. The bordering stones tend to increase in size with the size of the polygons, but to decrease with depth, regardless of the size of the polygons."@en;
  skos:topConceptOf <https://w3id.org/permafrost/v/nrcglossary/scheme> .

<https://w3id.org/permafrost/v/nrcglossary/t0313> a skos:Concept;
  dct:identifier "t0313"^^xsd:token;
  dct:source "https://nrc-publications.canada.ca/eng/view/object/?id=69fb8993-1baa-4225-b33a-6a02341d383d"^^xsd:anyURI,
    "https://nrc-publications.canada.ca/fra/voir/objet/?id=549123c3-092c-4fca-8dea-99d53eac06dd"^^xsd:anyURI;
  skos:altLabel "stone garland"@en;
  skos:definition "A sorted step is a patterned ground feature with a step-like form and a downslope border of stones embanking an area of relatively fine-grained bare ground upslope."@en;
  skos:inScheme <https://w3id.org/permafrost/v/nrcglossary/scheme>;
  skos:prefLabel "sorted step"@en;
  skos:scopeNote "Sorted steps are only found on slopes ranging from 5? to 15?; their downslope border forms a low riser fronting a tread whose slope is less than the general slope. Sorted steps are presumed to be derived either from sorted circles or from sorted polygons, rather than to develop independently. Some sorted steps clearly form an intermediate stage between sorted polygons and sorted stripes."@en;
  skos:topConceptOf <https://w3id.org/permafrost/v/nrcglossary/scheme> .

<https://w3id.org/permafrost/v/nrcglossary/t0314> a skos:Concept;
  dct:identifier "t0314"^^xsd:token;
  dct:source "https://nrc-publications.canada.ca/eng/view/object/?id=69fb8993-1baa-4225-b33a-6a02341d383d"^^xsd:anyURI,
    "https://nrc-publications.canada.ca/fra/voir/objet/?id=549123c3-092c-4fca-8dea-99d53eac06dd"^^xsd:anyURI;
  skos:definition "Sorted stripes form patterned ground with a striped and sorted appearance, due to parallel strips of stones and intervening strips of finer material, oriented down the steepest available slope."@en;
  skos:inScheme <https://w3id.org/permafrost/v/nrcglossary/scheme>;
  skos:prefLabel "sorted stripe"@en;
  skos:scopeNote "Sorted stripes, both large and small, occur on slopes of more than 3?, downslope from sorted polygons or sorted nets; they are derived by downslope extension of sorted polygons or sorted nets. They can be several hundred metres long. The stones of the coarse stripes can range from pebbles to boulders, depending on the size of the stripes. The intervening finer material can be stone- free or contain stones and be a diamicton."@en;
  skos:topConceptOf <https://w3id.org/permafrost/v/nrcglossary/scheme> .

<https://w3id.org/permafrost/v/nrcglossary/t0315> a skos:Concept;
  dct:identifier "t0315"^^xsd:token;
  dct:source "https://nrc-publications.canada.ca/eng/view/object/?id=69fb8993-1baa-4225-b33a-6a02341d383d"^^xsd:anyURI,
    "https://nrc-publications.canada.ca/fra/voir/objet/?id=549123c3-092c-4fca-8dea-99d53eac06dd"^^xsd:anyURI;
  skos:definition "The amount of heat required to raise the temperature of a unit mass of a substance by one degree."@en;
  skos:inScheme <https://w3id.org/permafrost/v/nrcglossary/scheme>;
  skos:prefLabel "specific heat capacity"@en;
  skos:scopeNote "Specific heat capacity is commonly expressed in Joules per kg per degree K."@en;
  skos:topConceptOf <https://w3id.org/permafrost/v/nrcglossary/scheme> .

<https://w3id.org/permafrost/v/nrcglossary/t0316> a skos:Concept;
  dct:identifier "t0316"^^xsd:token;
  dct:source "https://nrc-publications.canada.ca/eng/view/object/?id=69fb8993-1baa-4225-b33a-6a02341d383d"^^xsd:anyURI,
    "https://nrc-publications.canada.ca/fra/voir/objet/?id=549123c3-092c-4fca-8dea-99d53eac06dd"^^xsd:anyURI;
  skos:definition "1. (North-American usage) Permafrost underlying 10 to 35 percent of the exposed land surface. 2. (Russian usage) Permafrost underlying 5 to 30 percent of the exposed land surface."@en;
  skos:hiddenLabel "insular permafrost"@en, "island permafrost"@en, "scattered permafrost"@en;
  skos:inScheme <https://w3id.org/permafrost/v/nrcglossary/scheme>;
  skos:prefLabel "sporadic discontinuous permafrost"@en;
  skos:scopeNote "Individual areas of permafrost are completely surrounded by unfrozen ground."@en;
  skos:topConceptOf <https://w3id.org/permafrost/v/nrcglossary/scheme> .

<https://w3id.org/permafrost/v/nrcglossary/t0317> a skos:Concept;
  dct:identifier "t0317"^^xsd:token;
  dct:source "https://nrc-publications.canada.ca/eng/view/object/?id=69fb8993-1baa-4225-b33a-6a02341d383d"^^xsd:anyURI,
    "https://nrc-publications.canada.ca/fra/voir/objet/?id=549123c3-092c-4fca-8dea-99d53eac06dd"^^xsd:anyURI;
  skos:definition "A mineral soil showing little or no evidence of cryoturbation, with permafrost within 1 m below the surface ."@en;
  skos:inScheme <https://w3id.org/permafrost/v/nrcglossary/scheme>;
  skos:prefLabel "static cryosol"@en;
  skos:scopeNote "Static cryosols occur most commonly in coarse-textured materials, and patterned ground features may or may not be present. They have mean annual ground temperatures below 0°C."@en;
  skos:topConceptOf <https://w3id.org/permafrost/v/nrcglossary/scheme> .

<https://w3id.org/permafrost/v/nrcglossary/t0318> a skos:Concept;
  dct:identifier "t0318"^^xsd:token;
  dct:source "https://nrc-publications.canada.ca/eng/view/object/?id=69fb8993-1baa-4225-b33a-6a02341d383d"^^xsd:anyURI,
    "https://nrc-publications.canada.ca/fra/voir/objet/?id=549123c3-092c-4fca-8dea-99d53eac06dd"^^xsd:anyURI;
  skos:definition "A solifluction lobe with a stony front."@en;
  skos:inScheme <https://w3id.org/permafrost/v/nrcglossary/scheme>;
  skos:prefLabel "stone-banked (solifluction) lobe"@en;
  skos:topConceptOf <https://w3id.org/permafrost/v/nrcglossary/scheme> .

<https://w3id.org/permafrost/v/nrcglossary/t0319> a skos:Concept;
  dct:identifier "t0319"^^xsd:token;
  dct:source "https://nrc-publications.canada.ca/eng/view/object/?id=69fb8993-1baa-4225-b33a-6a02341d383d"^^xsd:anyURI,
    "https://nrc-publications.canada.ca/fra/voir/objet/?id=549123c3-092c-4fca-8dea-99d53eac06dd"^^xsd:anyURI;
  skos:definition "A solifluction terrace with a stony front."@en;
  skos:inScheme <https://w3id.org/permafrost/v/nrcglossary/scheme>;
  skos:prefLabel "stone-banked (solifluction) terrace"@en;
  skos:topConceptOf <https://w3id.org/permafrost/v/nrcglossary/scheme> .

<https://w3id.org/permafrost/v/nrcglossary/t0320> a skos:Concept;
  dct:identifier "t0320"^^xsd:token;
  dct:source "https://nrc-publications.canada.ca/eng/view/object/?id=69fb8993-1baa-4225-b33a-6a02341d383d"^^xsd:anyURI,
    "https://nrc-publications.canada.ca/fra/voir/objet/?id=549123c3-092c-4fca-8dea-99d53eac06dd"^^xsd:anyURI;
  skos:definition "A stone garland is the downslope border of stones along a sorted step, embanking an area of relatively fine-grained bare ground upslope."@en;
  skos:inScheme <https://w3id.org/permafrost/v/nrcglossary/scheme>;
  skos:prefLabel "stone garland"@en;
  skos:topConceptOf <https://w3id.org/permafrost/v/nrcglossary/scheme> .

<https://w3id.org/permafrost/v/nrcglossary/t0321> a skos:Concept;
  dct:identifier "t0321"^^xsd:token;
  dct:source "https://nrc-publications.canada.ca/eng/view/object/?id=69fb8993-1baa-4225-b33a-6a02341d383d"^^xsd:anyURI,
    "https://nrc-publications.canada.ca/fra/voir/objet/?id=549123c3-092c-4fca-8dea-99d53eac06dd"^^xsd:anyURI;
  skos:definition "A type of nonsorted circle developed in gravelly materials."@en;
  skos:inScheme <https://w3id.org/permafrost/v/nrcglossary/scheme>;
  skos:prefLabel "stony earth circle"@en;
  skos:topConceptOf <https://w3id.org/permafrost/v/nrcglossary/scheme> .

<https://w3id.org/permafrost/v/nrcglossary/t0322> a skos:Concept;
  dct:identifier "t0322"^^xsd:token;
  dct:source "https://nrc-publications.canada.ca/eng/view/object/?id=69fb8993-1baa-4225-b33a-6a02341d383d"^^xsd:anyURI,
    "https://nrc-publications.canada.ca/fra/voir/objet/?id=549123c3-092c-4fca-8dea-99d53eac06dd"^^xsd:anyURI;
  skos:altLabel "ribbed fen"@en, "string bog"@en;
  skos:definition "A peatland with roughly parallel narrow ridges of peat dominated by fenland vegetation interspersed with slight depressions, many of which contain shallow pools (see Figure 15d)."@en;
  skos:inScheme <https://w3id.org/permafrost/v/nrcglossary/scheme>;
  skos:prefLabel "string fen"@en, "tourbièreréticulée"@fr;
  skos:scopeNote "The ridges or strings are arranged at right angles to the slope, which is usually less than 2?. They are typically 1 to 3 m wide, up to 1 m high and may be over 1 km long. Although the ridges are usually parallel to one another, they may interconnect at acute angles. On nearly level fens the ridges are farther apart but shorter; and they interconnect frequently, giving a roughly polygonal appearance. Since the strings are elevated, they are better drained and allow shrubs and trees to grow on them. String fens are composed of sedge-fen peat with some woody shrub remains. The ridges are composed of moss-sedge or moss peat. They are best developed in the zone of discontinuous permafrost and immediately to the south of the permafrost region. In the central and northern parts of the zone of discontinuous permafrost, the ridges are often perennially frozen. Permafrost conditions may extend into the underlying soil."@en;
  skos:topConceptOf <https://w3id.org/permafrost/v/nrcglossary/scheme> .

<https://w3id.org/permafrost/v/nrcglossary/t0323> a skos:Concept;
  dct:identifier "t0323"^^xsd:token;
  dct:source "https://nrc-publications.canada.ca/eng/view/object/?id=69fb8993-1baa-4225-b33a-6a02341d383d"^^xsd:anyURI,
    "https://nrc-publications.canada.ca/fra/voir/objet/?id=549123c3-092c-4fca-8dea-99d53eac06dd"^^xsd:anyURI;
  skos:definition "Permafrost beneath a glacier."@en;
  skos:inScheme <https://w3id.org/permafrost/v/nrcglossary/scheme>;
  skos:prefLabel "subglacial permafrost"@en;
  skos:topConceptOf <https://w3id.org/permafrost/v/nrcglossary/scheme> .

<https://w3id.org/permafrost/v/nrcglossary/t0324> a skos:Concept;
  dct:identifier "t0324"^^xsd:token;
  dct:source "https://nrc-publications.canada.ca/eng/view/object/?id=69fb8993-1baa-4225-b33a-6a02341d383d"^^xsd:anyURI,
    "https://nrc-publications.canada.ca/fra/voir/objet/?id=549123c3-092c-4fca-8dea-99d53eac06dd"^^xsd:anyURI;
  skos:definition "A layer or body of unfrozen ground beneath a glacier in an area with permafrost."@en;
  skos:inScheme <https://w3id.org/permafrost/v/nrcglossary/scheme>;
  skos:prefLabel "subglacial talik"@en;
  skos:topConceptOf <https://w3id.org/permafrost/v/nrcglossary/scheme> .

<https://w3id.org/permafrost/v/nrcglossary/t0325> a skos:Concept;
  dct:identifier "t0325"^^xsd:token;
  dct:source "https://nrc-publications.canada.ca/eng/view/object/?id=69fb8993-1baa-4225-b33a-6a02341d383d"^^xsd:anyURI,
    "https://nrc-publications.canada.ca/fra/voir/objet/?id=549123c3-092c-4fca-8dea-99d53eac06dd"^^xsd:anyURI;
  skos:definition "Ice formed by reverse sublimation of water vapour onto cold surfaces."@en;
  skos:inScheme <https://w3id.org/permafrost/v/nrcglossary/scheme>;
  skos:prefLabel "sublimation ice"@en;
  skos:scopeNote "Hoar frost and open-cavity ice are examples of sublimation ice."@en;
  skos:topConceptOf <https://w3id.org/permafrost/v/nrcglossary/scheme> .

<https://w3id.org/permafrost/v/nrcglossary/t0326> a skos:Concept;
  dct:identifier "t0326"^^xsd:token;
  dct:source "https://nrc-publications.canada.ca/eng/view/object/?id=69fb8993-1baa-4225-b33a-6a02341d383d"^^xsd:anyURI,
    "https://nrc-publications.canada.ca/fra/voir/objet/?id=549123c3-092c-4fca-8dea-99d53eac06dd"^^xsd:anyURI;
  skos:definition "Water occurring in the noncryotic ground below the permafrost (see Figure 11)."@en;
  skos:inScheme <https://w3id.org/permafrost/v/nrcglossary/scheme>;
  skos:prefLabel "eau de subpergélisol"@fr, "subpermafrost water"@en;
  skos:scopeNote "This term does not include the water in basal cryopegs, i.e., the unfrozen zones that may occur in the basal portion of the permafrost (see intrapermafrost water)."@en;
  skos:topConceptOf <https://w3id.org/permafrost/v/nrcglossary/scheme> .

<https://w3id.org/permafrost/v/nrcglossary/t0327> a skos:Concept;
  dct:identifier "t0327"^^xsd:token;
  dct:source "https://nrc-publications.canada.ca/eng/view/object/?id=69fb8993-1baa-4225-b33a-6a02341d383d"^^xsd:anyURI,
    "https://nrc-publications.canada.ca/fra/voir/objet/?id=549123c3-092c-4fca-8dea-99d53eac06dd"^^xsd:anyURI;
  skos:altLabel "offshore permafrost"@en;
  skos:definition "Permafrost occurring beneath the sea bottom (see Figures 1 and 11)."@en;
  skos:hiddenLabel "sea-bed permafrost"@en, "sub-seabed permafrost"@en, "submarine permafrost"@en;
  skos:inScheme <https://w3id.org/permafrost/v/nrcglossary/scheme>;
  skos:prefLabel "subsea permafrost"@en;
  skos:scopeNote "Subsea permafrost either occurs in response to negative sea-bottom water temperatures, or it formed in now submerged coastal areas that were exposed previously to air temperatures below 0°C (relict permafrost). Much of the ice-bonded permafrost that has been found beneath the sea bottom has been inferred from acoustic geophysical surveys, and the term \"acoustically- defined permafrost\" has been used to describe such permafrost found in areas where temperature records or visual confirmation of ice bonding are not available."@en;
  skos:topConceptOf <https://w3id.org/permafrost/v/nrcglossary/scheme> .

<https://w3id.org/permafrost/v/nrcglossary/t0328> a skos:Concept;
  dct:identifier "t0328"^^xsd:token;
  dct:source "https://nrc-publications.canada.ca/eng/view/object/?id=69fb8993-1baa-4225-b33a-6a02341d383d"^^xsd:anyURI,
    "https://nrc-publications.canada.ca/fra/voir/objet/?id=549123c3-092c-4fca-8dea-99d53eac06dd"^^xsd:anyURI;
  skos:definition "A layer or body of unfrozen ground beneath the seabottom, and forming part of the subsea permafrost."@en;
  skos:inScheme <https://w3id.org/permafrost/v/nrcglossary/scheme>;
  skos:prefLabel "subsea talik"@en;
  skos:scopeNote "Subsea taliks are usually cryotic (T < 0°C). See also marine cryopeg."@en;
  skos:topConceptOf <https://w3id.org/permafrost/v/nrcglossary/scheme> .

<https://w3id.org/permafrost/v/nrcglossary/t0329> a skos:Concept;
  dct:identifier "t0329"^^xsd:token;
  dct:source "https://nrc-publications.canada.ca/eng/view/object/?id=69fb8993-1baa-4225-b33a-6a02341d383d"^^xsd:anyURI,
    "https://nrc-publications.canada.ca/fra/voir/objet/?id=549123c3-092c-4fca-8dea-99d53eac06dd"^^xsd:anyURI;
  skos:definition "Cooling of a liquid to a temperature below its freezing point, without causing solidification."@en;
  skos:inScheme <https://w3id.org/permafrost/v/nrcglossary/scheme>;
  skos:prefLabel "supercooling"@en;
  skos:topConceptOf <https://w3id.org/permafrost/v/nrcglossary/scheme> .

<https://w3id.org/permafrost/v/nrcglossary/t0330> a skos:Concept;
  dct:identifier "t0330"^^xsd:token;
  dct:source "https://nrc-publications.canada.ca/eng/view/object/?id=69fb8993-1baa-4225-b33a-6a02341d383d"^^xsd:anyURI,
    "https://nrc-publications.canada.ca/fra/voir/objet/?id=549123c3-092c-4fca-8dea-99d53eac06dd"^^xsd:anyURI;
  skos:definition "Water occurring in unfrozen ground above perennially frozen ground (see Figure 11)."@en;
  skos:inScheme <https://w3id.org/permafrost/v/nrcglossary/scheme>;
  skos:prefLabel "eau de suprapergélisol"@fr, "suprapermafrost water"@en;
  skos:scopeNote "Suprapermafrost water occurs in the active layer, between the active layer and the permafrost table, and in taliks below rivers and lakes. It is replenished by infiltration of rain, snowmelt or surface waters, or from intra- or subpermafrost water via open taliks. Much of the suprapermafrost water in the active layer may freeze in the winter; the remainder can temporarily become confined and subjected to increasing pressure during progressive freezing of the active layer (see cryogenic aquiclude)."@en;
  skos:topConceptOf <https://w3id.org/permafrost/v/nrcglossary/scheme> .

<https://w3id.org/permafrost/v/nrcglossary/t0331> a skos:Concept;
  dct:identifier "t0331"^^xsd:token;
  dct:source "https://nrc-publications.canada.ca/eng/view/object/?id=69fb8993-1baa-4225-b33a-6a02341d383d"^^xsd:anyURI,
    "https://nrc-publications.canada.ca/fra/voir/objet/?id=549123c3-092c-4fca-8dea-99d53eac06dd"^^xsd:anyURI;
  skos:definition "The cumulative number of degree-days below 0°C for the surface temperature (of the ground, pavement, etc.) during a given time period."@en;
  skos:inScheme <https://w3id.org/permafrost/v/nrcglossary/scheme>;
  skos:prefLabel "surface freezing index"@en;
  skos:scopeNote "The surface freezing index differs from the corresponding air freezing index (see n-factor)."@en;
  skos:topConceptOf <https://w3id.org/permafrost/v/nrcglossary/scheme> .

<https://w3id.org/permafrost/v/nrcglossary/t0332> a skos:Concept;
  dct:identifier "t0332"^^xsd:token;
  dct:source "https://nrc-publications.canada.ca/eng/view/object/?id=69fb8993-1baa-4225-b33a-6a02341d383d"^^xsd:anyURI,
    "https://nrc-publications.canada.ca/fra/voir/objet/?id=549123c3-092c-4fca-8dea-99d53eac06dd"^^xsd:anyURI;
  skos:definition "The cumulative number of degree-days above 0°C for the surface temperature (of the ground, pavement, etc.) during a given period."@en;
  skos:inScheme <https://w3id.org/permafrost/v/nrcglossary/scheme>;
  skos:prefLabel "surface thawing index"@en;
  skos:scopeNote "The surface thawing index differs from the corresponding air thawing index (see n-factor)."@en;
  skos:topConceptOf <https://w3id.org/permafrost/v/nrcglossary/scheme> .

<https://w3id.org/permafrost/v/nrcglossary/t0333> a skos:Concept;
  dct:identifier "t0333"^^xsd:token;
  dct:source "https://nrc-publications.canada.ca/eng/view/object/?id=69fb8993-1baa-4225-b33a-6a02341d383d"^^xsd:anyURI,
    "https://nrc-publications.canada.ca/fra/voir/objet/?id=549123c3-092c-4fca-8dea-99d53eac06dd"^^xsd:anyURI;
  skos:definition "A distinct soil micromorphology, resulting from the effects of freezing and thawing processes, in which coarser soil particles have vertical or near- vertical orientation (see Figure 8e)."@en;
  skos:inScheme <https://w3id.org/permafrost/v/nrcglossary/scheme>;
  skos:prefLabel "suscitic cryogenic fabric"@en;
  skos:scopeNote "This fabric, found in cryosols, results from freeze-thaw processes probably accompanied by cryoturbation."@en;
  skos:topConceptOf <https://w3id.org/permafrost/v/nrcglossary/scheme> .

<https://w3id.org/permafrost/v/nrcglossary/t0334> a skos:Concept;
  dct:identifier "t0334"^^xsd:token;
  dct:source "https://nrc-publications.canada.ca/eng/view/object/?id=69fb8993-1baa-4225-b33a-6a02341d383d"^^xsd:anyURI,
    "https://nrc-publications.canada.ca/fra/voir/objet/?id=549123c3-092c-4fca-8dea-99d53eac06dd"^^xsd:anyURI;
  skos:definition "Ground ice developed during the formation of syngenetic permafrost."@en;
  skos:hiddenLabel "penecontemporaneous ice"@en;
  skos:inScheme <https://w3id.org/permafrost/v/nrcglossary/scheme>;
  skos:prefLabel "syngenetic ice"@en;
  skos:topConceptOf <https://w3id.org/permafrost/v/nrcglossary/scheme> .

<https://w3id.org/permafrost/v/nrcglossary/t0335> a skos:Concept;
  dct:identifier "t0335"^^xsd:token;
  dct:source "https://nrc-publications.canada.ca/eng/view/object/?id=69fb8993-1baa-4225-b33a-6a02341d383d"^^xsd:anyURI,
    "https://nrc-publications.canada.ca/fra/voir/objet/?id=549123c3-092c-4fca-8dea-99d53eac06dd"^^xsd:anyURI;
  skos:definition "An ice wedge developed during the formation of syngenetic permafrost (see Figure 17i)."@en;
  skos:inScheme <https://w3id.org/permafrost/v/nrcglossary/scheme>;
  skos:prefLabel "syngenetic ice wedge"@en;
  skos:scopeNote "Syngenetic ice wedges grow both wider and higher, more or less simultaneously with the deposition of additional sediment or other earth material on the ground surafce. Hence the ice on the outside edges decreases in age from bottom to top. Syngenetic ice wedges are generally wedge-shaped but with more irregular sides than epigenetic ice wedges."@en;
  skos:topConceptOf <https://w3id.org/permafrost/v/nrcglossary/scheme> .

<https://w3id.org/permafrost/v/nrcglossary/t0336> a skos:Concept;
  dct:identifier "t0336"^^xsd:token;
  dct:source "https://nrc-publications.canada.ca/eng/view/object/?id=69fb8993-1baa-4225-b33a-6a02341d383d"^^xsd:anyURI,
    "https://nrc-publications.canada.ca/fra/voir/objet/?id=549123c3-092c-4fca-8dea-99d53eac06dd"^^xsd:anyURI;
  skos:definition "Permafrost that formed through a rise of the permafrost table during the deposition of additional sediment or other earth material on the ground surface."@en;
  skos:inScheme <https://w3id.org/permafrost/v/nrcglossary/scheme>;
  skos:prefLabel "syngenetic permafrost"@en;
  skos:topConceptOf <https://w3id.org/permafrost/v/nrcglossary/scheme> .

<https://w3id.org/permafrost/v/nrcglossary/t0337> a skos:Concept;
  dct:identifier "t0337"^^xsd:token;
  dct:source "https://nrc-publications.canada.ca/eng/view/object/?id=69fb8993-1baa-4225-b33a-6a02341d383d"^^xsd:anyURI,
    "https://nrc-publications.canada.ca/fra/voir/objet/?id=549123c3-092c-4fca-8dea-99d53eac06dd"^^xsd:anyURI;
  skos:definition "A layer or body of unfrozen ground occurring in a permafrost area due to a local anomaly in thermal, hydrological, hydrogeological, or hydrochemical conditions (see Figure 11)."@en;
  skos:inScheme <https://w3id.org/permafrost/v/nrcglossary/scheme>;
  skos:prefLabel "talik"@en, "talik"@fr;
  skos:scopeNote "Taliks may have temperatures above 0°C (noncryotic) or below 0°C (cryotic, forming part of the permafrost). Some taliks may be affected by seasonal freezing. Several types of taliks can be distinguished on the basis of their relationship to the permafrost (closed, open, lateral, isolated and transient taliks), and on the basis of the mechanism responsible for their unfrozen condition (hydrochemical, hydrothermal and thermal taliks): 1. closed talik - a noncryotic talik occupying a depression in the permafrost table below a lake or river (also called \"lake talik\" and \"river talik\"); its temperature remains above 0°C because of the heat storage effect of the surface water; 2. hydrochemical talik - a cryotic talik in which freezing is prevented by mineralized groundwater flowing through the talik. 3. hydrothermal talik - a noncryotic talik, the temperature of which is maintained above 0°C by the heat supplied by groundwater flowing through the talik; 4. isolated talik - a talik entirely surrounded by perennially frozen ground; usually cryotic (see isolated cryopeg), but may be noncryotic (see transient talik); 5. lateral talik - a talik overlain and underlain by perennially frozen ground; can be noncryotic or cryotic; 6. open talik - a talik that penetrates the permafrost completely, connecting suprapermafrost and subpermafrost water, (e.g., below large rivers and lakes). It may be noncryotic (see hydrothermal talik) or cryotic (see hydrochemical talik). SYNONYMS: (not recommended) through talik, penetrating talik, perforating talik, piercing talik; 7. thermal talik - a noncryotic talik, the temperature of which is above 0°C due to the local thermal regime of the ground; 8. transient talik - a talik that is gradually being eliminated by freezing, e.g., the initially noncryotic closed talik below a small lake which, upon draining of the lake, is turned into a transient isolated talik by permafrost aggradation (see also closed-system pingo)."@en;
  skos:topConceptOf <https://w3id.org/permafrost/v/nrcglossary/scheme> .

<https://w3id.org/permafrost/v/nrcglossary/t0338> a skos:Concept;
  dct:identifier "t0338"^^xsd:token;
  dct:source "https://nrc-publications.canada.ca/eng/view/object/?id=69fb8993-1baa-4225-b33a-6a02341d383d"^^xsd:anyURI,
    "https://nrc-publications.canada.ca/fra/voir/objet/?id=549123c3-092c-4fca-8dea-99d53eac06dd"^^xsd:anyURI;
  skos:definition "The graphic or analytical expression of the variation in ground temperature with depth."@en;
  skos:inScheme <https://w3id.org/permafrost/v/nrcglossary/scheme>;
  skos:prefLabel "temperature profile"@en;
  skos:topConceptOf <https://w3id.org/permafrost/v/nrcglossary/scheme> .

<https://w3id.org/permafrost/v/nrcglossary/t0339> a skos:Concept;
  dct:identifier "t0339"^^xsd:token;
  dct:source "https://nrc-publications.canada.ca/eng/view/object/?id=69fb8993-1baa-4225-b33a-6a02341d383d"^^xsd:anyURI,
    "https://nrc-publications.canada.ca/fra/voir/objet/?id=549123c3-092c-4fca-8dea-99d53eac06dd"^^xsd:anyURI;
  skos:altLabel "closed talik"@en;
  skos:definition "A depression of the permafrost table created by naturally induced thawing."@en;
  skos:hiddenLabel "thaw depression"@en;
  skos:inScheme <https://w3id.org/permafrost/v/nrcglossary/scheme>;
  skos:prefLabel "cuvette de dégel"@fr, "thaw basin"@en;
  skos:scopeNote "In permafrost regions, thaw basins exist beneath bodies of water such as lakes or rivers that do not freeze to the bottom in winter. They may be quite extensive both in depth (from a few metres to more than a 100 m) and in areal extent (from several tens of metres to more than 2 km) and they may be irregular in shape. Their depth, areal extent and shape depend on the size of the water body, the type and properties of earth material underlying it, and the presence of ground ice and groundwater."@en;
  skos:topConceptOf <https://w3id.org/permafrost/v/nrcglossary/scheme> .

<https://w3id.org/permafrost/v/nrcglossary/t0340> a skos:Concept;
  dct:identifier "t0340"^^xsd:token;
  dct:source "https://nrc-publications.canada.ca/eng/view/object/?id=69fb8993-1baa-4225-b33a-6a02341d383d"^^xsd:anyURI,
    "https://nrc-publications.canada.ca/fra/voir/objet/?id=549123c3-092c-4fca-8dea-99d53eac06dd"^^xsd:anyURI;
  skos:definition "A zone of thawed ground below or surrounding a man-made structure placed on or in permafrost and maintained at temperatures above 0°C (see Figure 23)."@en;
  skos:inScheme <https://w3id.org/permafrost/v/nrcglossary/scheme>;
  skos:prefLabel "bulbe de dégel"@fr, "thaw bulb"@en;
  skos:scopeNote "Construction and operation of structures usually lead to alteration of the thermal regime of the ground. Where permitted, the development of a thaw bulb under a structure is taken into account and controlled as part of the engineering design. It is frequently nearly symmetrical in form and limited in size under structures such as buildings. Beneath linear structures or facilities built in permafrost areas, such as road embankments or buried warm pipelines, the thaw bulb may extend for the full length of the structure. Settlement of the ground and the structure or facility may occur as the thaw bulb forms. A thaw bulb may also form when a structure or facility, around which a frost bulb has developed, is abandoned and the ground is no longer maintained at a temperature below 0°C."@en;
  skos:topConceptOf <https://w3id.org/permafrost/v/nrcglossary/scheme> .

<https://w3id.org/permafrost/v/nrcglossary/t0341> a skos:Concept;
  dct:identifier "t0341"^^xsd:token;
  dct:source "https://nrc-publications.canada.ca/eng/view/object/?id=69fb8993-1baa-4225-b33a-6a02341d383d"^^xsd:anyURI,
    "https://nrc-publications.canada.ca/fra/voir/objet/?id=549123c3-092c-4fca-8dea-99d53eac06dd"^^xsd:anyURI;
  skos:definition "Time-dependent compression resulting from thawing of frozen ground and subsequent draining of excess water."@en;
  skos:inScheme <https://w3id.org/permafrost/v/nrcglossary/scheme>;
  skos:prefLabel "consolidation due au dégel"@fr, "thaw consolidation"@en;
  skos:scopeNote "If during thaw, the flow of water from the thawed ground is unimpeded, then the variation of thaw settlement with time is controlled solely by the position of the thawing front. If the thawed ground is not sufficiently permeable, and flow is impeded, however, the rate of settlement with time is also controlled by the compressibility and permeability of the thawed ground. In the case of thawing fine-grained soils, if the rate of thaw is sufficiently fast, water is released at a rate exceeding that at which it can flow from the soil, and pore pressures in excess of hydrostatic will be generated. These excess pore pressures may cause severe instability problems in slopes and foundation soils. It has been found that excess pore pressures and the degree of consolidation in thawing soils depend principally on the thaw consolidation ratio."@en;
  skos:topConceptOf <https://w3id.org/permafrost/v/nrcglossary/scheme> .

<https://w3id.org/permafrost/v/nrcglossary/t0342> a skos:Concept;
  dct:identifier "t0342"^^xsd:token;
  dct:source "https://nrc-publications.canada.ca/eng/view/object/?id=69fb8993-1baa-4225-b33a-6a02341d383d"^^xsd:anyURI,
    "https://nrc-publications.canada.ca/fra/voir/objet/?id=549123c3-092c-4fca-8dea-99d53eac06dd"^^xsd:anyURI;
  skos:definition "A dimensionless ratio describing the relationship between the rate of thaw and the rate of consolidation of a thawing soil, which is considered to be a measure of the relative rates of generation and expulsion of excess water during thaw."@en;
  skos:inScheme <https://w3id.org/permafrost/v/nrcglossary/scheme>;
  skos:prefLabel "coefficient de consolidation au dégel"@fr, "thaw consolidation ratio"@en;
  skos:scopeNote "According to Morgenstern and Nixon (1971), a value of the ratio greater than unity would predict the danger of sustained substantial pore pressures at the thawing front and hence the possibility of instability due to the reduction of shear strength at that plane."@en;
  skos:topConceptOf <https://w3id.org/permafrost/v/nrcglossary/scheme> .

<https://w3id.org/permafrost/v/nrcglossary/t0343> a skos:Concept;
  dct:identifier "t0343"^^xsd:token;
  dct:source "https://nrc-publications.canada.ca/eng/view/object/?id=69fb8993-1baa-4225-b33a-6a02341d383d"^^xsd:anyURI,
    "https://nrc-publications.canada.ca/fra/voir/objet/?id=549123c3-092c-4fca-8dea-99d53eac06dd"^^xsd:anyURI;
  skos:definition "The downward movement of the thawing front during thawing of frozen ground."@en;
  skos:inScheme <https://w3id.org/permafrost/v/nrcglossary/scheme>;
  skos:prefLabel "thaw penetration"@en;
  skos:scopeNote "The rate of thaw penetration depends on the rate of heat conduction and on the ice content of the ground."@en;
  skos:topConceptOf <https://w3id.org/permafrost/v/nrcglossary/scheme> .

<https://w3id.org/permafrost/v/nrcglossary/t0344> a skos:Concept;
  dct:identifier "t0344"^^xsd:token;
  dct:source "https://nrc-publications.canada.ca/eng/view/object/?id=69fb8993-1baa-4225-b33a-6a02341d383d"^^xsd:anyURI,
    "https://nrc-publications.canada.ca/fra/voir/objet/?id=549123c3-092c-4fca-8dea-99d53eac06dd"^^xsd:anyURI;
  skos:definition "Perennially frozen ground which, upon thawing, will experience significant thaw settlement and suffer loss of strength to a value significantly lower than that for similar material in an unfrozen condition."@en;
  skos:hiddenLabel "thaw-unstable permafrost"@en;
  skos:inScheme <https://w3id.org/permafrost/v/nrcglossary/scheme>;
  skos:prefLabel "thaw-sensitive permafrost"@en;
  skos:scopeNote "Ice-rich permafrost is thaw-sensitive."@en;
  skos:topConceptOf <https://w3id.org/permafrost/v/nrcglossary/scheme> .

<https://w3id.org/permafrost/v/nrcglossary/t0345> a skos:Concept;
  dct:identifier "t0345"^^xsd:token;
  dct:source "https://nrc-publications.canada.ca/eng/view/object/?id=69fb8993-1baa-4225-b33a-6a02341d383d"^^xsd:anyURI,
    "https://nrc-publications.canada.ca/fra/voir/objet/?id=549123c3-092c-4fca-8dea-99d53eac06dd"^^xsd:anyURI;
  skos:definition "Compression of the ground due to thaw consolidation (see Figure 7)."@en;
  skos:inScheme <https://w3id.org/permafrost/v/nrcglossary/scheme>;
  skos:prefLabel "tassement dû au dégel"@fr, "thaw settlement"@en;
  skos:scopeNote "In coarse-grained and dense soils, the amount of thaw settlement is usually small because it is governed mainly by the melting of pore ice. In ice-rich permafrost, and seasonally frozen ground containing excess ice, however, the amount of thaw settlement may be quite substantial. In general, on thawing, any frozen ground will settle both under its own weight and under applied stresses. The settlement will continue as long as the thawing front advances and until the pore pressures generated during thawing are dissipated. In relatively permeable coarse-grained soils, where draining of pore water is rapid, the thaw settlement rate will usually follow closely the rate of thaw, and development of pore pressures will be negligible during the thaw period. On the other hand, if a relatively impermeable fine-grained soil is thawed rapidly, then excess pore pressures will be generated. If these excess pore pressures are sustained for any length of time, then severe problems may develop (e.g., slopes may become unstable, dam foundations may fail, and differential settlements may be aggravated)."@en;
  skos:topConceptOf <https://w3id.org/permafrost/v/nrcglossary/scheme> .

<https://w3id.org/permafrost/v/nrcglossary/t0346> a skos:Concept;
  dct:identifier "t0346"^^xsd:token;
  dct:source "https://nrc-publications.canada.ca/eng/view/object/?id=69fb8993-1baa-4225-b33a-6a02341d383d"^^xsd:anyURI,
    "https://nrc-publications.canada.ca/fra/voir/objet/?id=549123c3-092c-4fca-8dea-99d53eac06dd"^^xsd:anyURI;
  skos:definition "A closed thaw basin with subterranean drainage."@en;
  skos:hiddenLabel "thaw hole"@en, "thaw pit"@en;
  skos:inScheme <https://w3id.org/permafrost/v/nrcglossary/scheme>;
  skos:prefLabel "doline de dégel"@fr, "thaw sink"@en;
  skos:topConceptOf <https://w3id.org/permafrost/v/nrcglossary/scheme> .

<https://w3id.org/permafrost/v/nrcglossary/t0347> a skos:Concept;
  dct:identifier "t0347"^^xsd:token;
  dct:source "https://nrc-publications.canada.ca/eng/view/object/?id=69fb8993-1baa-4225-b33a-6a02341d383d"^^xsd:anyURI,
    "https://nrc-publications.canada.ca/fra/voir/objet/?id=549123c3-092c-4fca-8dea-99d53eac06dd"^^xsd:anyURI;
  skos:definition "A slope failure mechanism characterized by the melting of ground ice, and downslope sliding and flowing of the resulting debris."@en;
  skos:hiddenLabel "ice slump"@en;
  skos:inScheme <https://w3id.org/permafrost/v/nrcglossary/scheme>;
  skos:prefLabel "thaw slumping"@en;
  skos:scopeNote "The resulting landform is a retrogressive thaw slump."@en;
  skos:topConceptOf <https://w3id.org/permafrost/v/nrcglossary/scheme> .

<https://w3id.org/permafrost/v/nrcglossary/t0348> a skos:Concept;
  dct:identifier "t0348"^^xsd:token;
  dct:source "https://nrc-publications.canada.ca/eng/view/object/?id=69fb8993-1baa-4225-b33a-6a02341d383d"^^xsd:anyURI,
    "https://nrc-publications.canada.ca/fra/voir/objet/?id=549123c3-092c-4fca-8dea-99d53eac06dd"^^xsd:anyURI;
  skos:definition "Perennially frozen ground which, upon thawing, will not experience either significant thaw settlement or loss of strength."@en;
  skos:inScheme <https://w3id.org/permafrost/v/nrcglossary/scheme>;
  skos:prefLabel "thaw-stable permafrost"@en;
  skos:scopeNote "Thaw-stable permafrost may have the same mineral and particle-size compositions as thaw-sensitive permafrost. It may be frost-susceptible. Dry permafrost is thaw-stable."@en;
  skos:topConceptOf <https://w3id.org/permafrost/v/nrcglossary/scheme> .

<https://w3id.org/permafrost/v/nrcglossary/t0349> a skos:Concept;
  dct:identifier "t0349"^^xsd:token;
  dct:source "https://nrc-publications.canada.ca/eng/view/object/?id=69fb8993-1baa-4225-b33a-6a02341d383d"^^xsd:anyURI,
    "https://nrc-publications.canada.ca/fra/voir/objet/?id=549123c3-092c-4fca-8dea-99d53eac06dd"^^xsd:anyURI;
  skos:definition "The amount that frozen ground compresses upon thawing."@en;
  skos:inScheme <https://w3id.org/permafrost/v/nrcglossary/scheme>;
  skos:prefLabel "déformation due au dégel"@fr, "thaw strain"@en;
  skos:scopeNote "The thaw strain is equal to the thaw settlement divided by the original thickness of the frozen ground before thawing. When freezing of the ground occurred in a closed system, the thaw strain is due only to the 9 percent volume contraction associated with the melting of pore ice."@en;
  skos:topConceptOf <https://w3id.org/permafrost/v/nrcglossary/scheme> .

<https://w3id.org/permafrost/v/nrcglossary/t0350> a skos:Concept;
  dct:identifier "t0350"^^xsd:token;
  dct:source "https://nrc-publications.canada.ca/eng/view/object/?id=69fb8993-1baa-4225-b33a-6a02341d383d"^^xsd:anyURI,
    "https://nrc-publications.canada.ca/fra/voir/objet/?id=549123c3-092c-4fca-8dea-99d53eac06dd"^^xsd:anyURI;
  skos:definition "A boundary sometimes identified in perennially frozen ground, representing the base of a relict active layer, as well as the corresponding earlier permafrost table."@en;
  skos:inScheme <https://w3id.org/permafrost/v/nrcglossary/scheme>;
  skos:prefLabel "thaw unconformity"@en;
  skos:scopeNote "A thaw unconformity may be recognized by differences in ice contents, stable isotope contents, and heavy mineral and pollen assemblages above and below the unconformity, and by the truncation of ice bodies."@en;
  skos:topConceptOf <https://w3id.org/permafrost/v/nrcglossary/scheme> .

<https://w3id.org/permafrost/v/nrcglossary/t0351> a skos:Concept;
  dct:identifier "t0351"^^xsd:token;
  dct:source "https://nrc-publications.canada.ca/eng/view/object/?id=69fb8993-1baa-4225-b33a-6a02341d383d"^^xsd:anyURI,
    "https://nrc-publications.canada.ca/fra/voir/objet/?id=549123c3-092c-4fca-8dea-99d53eac06dd"^^xsd:anyURI;
  skos:altLabel "thaw softening"@en;
  skos:definition "The reduction in shear strength due to the decrease in effective stresses resulting from the generation and slow dissipation of excess pore pressures when frozen soils containing ice are thawing."@en;
  skos:inScheme <https://w3id.org/permafrost/v/nrcglossary/scheme>;
  skos:prefLabel "affaiblissement dû au dégel"@fr, "thaw weakening"@en;
  skos:scopeNote "Thaw weakening, although generally used with respect to the thawing of seasonally frozen ground when melting of ice lenses and pore ice occurs, is equally applicable to thawing of ice-bearing and ice-rich permafrost. The usual effects of thaw weakening are a significant decrease in bearing capacity and an increase in stability problems (e.g., on road embankments, natural slopes, etc.)."@en;
  skos:topConceptOf <https://w3id.org/permafrost/v/nrcglossary/scheme> .

<https://w3id.org/permafrost/v/nrcglossary/t0352> a skos:Concept;
  dct:identifier "t0352"^^xsd:token;
  dct:source "https://nrc-publications.canada.ca/eng/view/object/?id=69fb8993-1baa-4225-b33a-6a02341d383d"^^xsd:anyURI,
    "https://nrc-publications.canada.ca/fra/voir/objet/?id=549123c3-092c-4fca-8dea-99d53eac06dd"^^xsd:anyURI;
  skos:definition "Previously frozen ground in which all ice has melted."@en;
  skos:inScheme <https://w3id.org/permafrost/v/nrcglossary/scheme>;
  skos:prefLabel "sol dégelé"@fr, "thawed ground"@en;
  skos:scopeNote "Unfrozen ground is thawed ground only if it were previously frozen. Thawed ground is commonly noncryotic, but it may be cryotic."@en;
  skos:topConceptOf <https://w3id.org/permafrost/v/nrcglossary/scheme> .

<https://w3id.org/permafrost/v/nrcglossary/t0353> a skos:Concept;
  dct:identifier "t0353"^^xsd:token;
  dct:source "https://nrc-publications.canada.ca/eng/view/object/?id=69fb8993-1baa-4225-b33a-6a02341d383d"^^xsd:anyURI,
    "https://nrc-publications.canada.ca/fra/voir/objet/?id=549123c3-092c-4fca-8dea-99d53eac06dd"^^xsd:anyURI;
  skos:definition "Melting of the ice in frozen ground, usually as a result of a rise in temperature."@en;
  skos:inScheme <https://w3id.org/permafrost/v/nrcglossary/scheme>;
  skos:prefLabel "dégel"@fr, "thawing (of frozen ground)"@en;
  skos:topConceptOf <https://w3id.org/permafrost/v/nrcglossary/scheme> .

<https://w3id.org/permafrost/v/nrcglossary/t0354> a skos:Concept;
  dct:identifier "t0354"^^xsd:token;
  dct:source "https://nrc-publications.canada.ca/eng/view/object/?id=69fb8993-1baa-4225-b33a-6a02341d383d"^^xsd:anyURI,
    "https://nrc-publications.canada.ca/fra/voir/objet/?id=549123c3-092c-4fca-8dea-99d53eac06dd"^^xsd:anyURI;
  skos:altLabel "frost table"@en;
  skos:definition "The advancing boundary between thawed ground and frozen ground (see Figure 4)."@en;
  skos:inScheme <https://w3id.org/permafrost/v/nrcglossary/scheme>;
  skos:prefLabel "thawing front"@en;
  skos:scopeNote "The thawing front may be advancing into either seasonally or perennially frozen ground during progressive thawing. In non-permafrost areas there will be two thawing fronts during the annual thawing period, one moving downward from the surface, the other moving upward from the bottom of the seasonally frozen ground. The thawing front usually coincides more closely with the position of the 0°C isotherm than the freezing front, except in saline permafrost."@en;
  skos:topConceptOf <https://w3id.org/permafrost/v/nrcglossary/scheme> .

<https://w3id.org/permafrost/v/nrcglossary/t0355> a skos:Concept;
  dct:identifier "t0355"^^xsd:token;
  dct:source "https://nrc-publications.canada.ca/eng/view/object/?id=69fb8993-1baa-4225-b33a-6a02341d383d"^^xsd:anyURI,
    "https://nrc-publications.canada.ca/fra/voir/objet/?id=549123c3-092c-4fca-8dea-99d53eac06dd"^^xsd:anyURI;
  skos:definition "The cumulative number of degree-days above 0°C for a given time period."@en;
  skos:inScheme <https://w3id.org/permafrost/v/nrcglossary/scheme>;
  skos:prefLabel "indice de dégel"@fr, "thawing index"@en;
  skos:scopeNote "Four main types of air thawing indices have been used: 1. approximate thawing index - calculated from the mean monthly air temperatures for a specific station without making corrections for negative degree-days (T < 0°C) in spring and fall (Boyd, 1973, 1979); 2. total annual thawing index - calculated by adding all the positive mean daily temperatures (°C) for a specific station during a calendar year (Harris, 1981); 3. seasonal thawing index - calculated as the arithmetic sum of all the positive and negative mean daily air temperatures (°C) for a specific station during the time period between the lowest point in the spring and the highest point the next fall on the cumulative degree-day time curve (Huschke, 1959); 4. design thawing index - calculated by taking the average of the seasonal thawing indices for the three warmest summers in the most recent 30 years of record. If data for 30 years are not available, then the index is based on the warmest summer in the latest 10-year period of record (U.S. Army/Air Force, 1966). The total annual thawing index has been used to predict permafrost distribution, and the design thawing index is commonly used in engineering design to estimate the maximum depth of thaw in frozen ground. A surface (ground, pavement, etc.) thawing index differs from the air thawing index (see n-factor)."@en;
  skos:topConceptOf <https://w3id.org/permafrost/v/nrcglossary/scheme> .

<https://w3id.org/permafrost/v/nrcglossary/t0356> a skos:Concept;
  dct:identifier "t0356"^^xsd:token;
  dct:source "https://nrc-publications.canada.ca/eng/view/object/?id=69fb8993-1baa-4225-b33a-6a02341d383d"^^xsd:anyURI,
    "https://nrc-publications.canada.ca/fra/voir/objet/?id=549123c3-092c-4fca-8dea-99d53eac06dd"^^xsd:anyURI;
  skos:definition "The quantity of heat that will flow through a unit area of a substance in unit time under a unit temperature gradient."@en;
  skos:inScheme <https://w3id.org/permafrost/v/nrcglossary/scheme>;
  skos:prefLabel "thermal conductivity"@en;
  skos:scopeNote "Commonly expressed in joules per second per metre per degree K."@en;
  skos:topConceptOf <https://w3id.org/permafrost/v/nrcglossary/scheme> .

<https://w3id.org/permafrost/v/nrcglossary/t0357> a skos:Concept;
  dct:identifier "t0357"^^xsd:token;
  dct:source "https://nrc-publications.canada.ca/eng/view/object/?id=69fb8993-1baa-4225-b33a-6a02341d383d"^^xsd:anyURI,
    "https://nrc-publications.canada.ca/fra/voir/objet/?id=549123c3-092c-4fca-8dea-99d53eac06dd"^^xsd:anyURI;
  skos:altLabel "frost crack"@en, "frost fissure"@en;
  skos:definition "A tensile fracture resulting from thermal stresses in frozen ground."@en;
  skos:hiddenLabel "contraction crack"@en, "frost wedge"@en;
  skos:inScheme <https://w3id.org/permafrost/v/nrcglossary/scheme>;
  skos:prefLabel "thermal-contraction crack"@en;
  skos:scopeNote "Tensile stresses caused by a reduction in ground temperature are probably a major factor in thermal contraction cracking, but it is usually difficult to prove that desiccation is not also involved. Ice wedges, sand wedges, soil wedges and ice veins form in thermal contraction cracks."@en;
  skos:topConceptOf <https://w3id.org/permafrost/v/nrcglossary/scheme> .

<https://w3id.org/permafrost/v/nrcglossary/t0358> a skos:Concept;
  dct:identifier "t0358"^^xsd:token;
  dct:source "https://nrc-publications.canada.ca/eng/view/object/?id=69fb8993-1baa-4225-b33a-6a02341d383d"^^xsd:anyURI,
    "https://nrc-publications.canada.ca/fra/voir/objet/?id=549123c3-092c-4fca-8dea-99d53eac06dd"^^xsd:anyURI;
  skos:definition "Ice formed in thermal contraction cracks in the ground (see Figure 17)."@en;
  skos:inScheme <https://w3id.org/permafrost/v/nrcglossary/scheme>;
  skos:prefLabel "thermal-contraction-crack ice"@en;
  skos:scopeNote "Both wedge ice and some kinds of vein ice are types of thermal contraction crack ice. Open-cavity ice may be a constitutent of thermal contraction crack ice."@en;
  skos:topConceptOf <https://w3id.org/permafrost/v/nrcglossary/scheme> .

<https://w3id.org/permafrost/v/nrcglossary/t0359> a skos:Concept;
  dct:identifier "t0359"^^xsd:token;
  dct:source "https://nrc-publications.canada.ca/eng/view/object/?id=69fb8993-1baa-4225-b33a-6a02341d383d"^^xsd:anyURI,
    "https://nrc-publications.canada.ca/fra/voir/objet/?id=549123c3-092c-4fca-8dea-99d53eac06dd"^^xsd:anyURI;
  skos:definition "The ratio of the thermal conductivity to the volumetric heat capacity."@en;
  skos:inScheme <https://w3id.org/permafrost/v/nrcglossary/scheme>;
  skos:prefLabel "thermal diffusivity"@en;
  skos:scopeNote "The thermal diffusivity expresses the facility with which a material will ondergo a temperature change."@en;
  skos:topConceptOf <https://w3id.org/permafrost/v/nrcglossary/scheme> .

<https://w3id.org/permafrost/v/nrcglossary/t0360> a skos:Concept;
  dct:identifier "t0360"^^xsd:token;
  dct:source "https://nrc-publications.canada.ca/eng/view/object/?id=69fb8993-1baa-4225-b33a-6a02341d383d"^^xsd:anyURI,
    "https://nrc-publications.canada.ca/fra/voir/objet/?id=549123c3-092c-4fca-8dea-99d53eac06dd"^^xsd:anyURI;
  skos:definition "The erosion of ice-bearing permafrost by the combined thermal and mechanical action of moving water."@en;
  skos:inScheme <https://w3id.org/permafrost/v/nrcglossary/scheme>;
  skos:prefLabel "thermal erosion"@en, "érosion thermique"@fr;
  skos:scopeNote "Thermal erosion is a dynamic process involving the wearing away by thermal means (i.e., the melting of ice), and by mechanical means (i.e., hydraulic transport). Thermal erosion is distinct from the development of thermokarst terrain, which results from thermal melting followed by subsidence of the ground but without hydraulic transport of earth materials. An example of the combined thermal and mechanical effects of moving water is the formation of a thermo-erosional niche."@en;
  skos:topConceptOf <https://w3id.org/permafrost/v/nrcglossary/scheme> .

<https://w3id.org/permafrost/v/nrcglossary/t0361> a skos:Concept;
  dct:identifier "t0361"^^xsd:token;
  dct:source "https://nrc-publications.canada.ca/eng/view/object/?id=69fb8993-1baa-4225-b33a-6a02341d383d"^^xsd:anyURI,
    "https://nrc-publications.canada.ca/fra/voir/objet/?id=549123c3-092c-4fca-8dea-99d53eac06dd"^^xsd:anyURI;
  skos:definition "The volume change per unit volume of a substance due to a one degree change in its temperature."@en;
  skos:inScheme <https://w3id.org/permafrost/v/nrcglossary/scheme>;
  skos:prefLabel "thermal expansion (or contraction) coefficient"@en;
  skos:topConceptOf <https://w3id.org/permafrost/v/nrcglossary/scheme> .

<https://w3id.org/permafrost/v/nrcglossary/t0362> a skos:Concept;
  dct:identifier "t0362"^^xsd:token;
  dct:source "https://nrc-publications.canada.ca/eng/view/object/?id=69fb8993-1baa-4225-b33a-6a02341d383d"^^xsd:anyURI,
    "https://nrc-publications.canada.ca/fra/voir/objet/?id=549123c3-092c-4fca-8dea-99d53eac06dd"^^xsd:anyURI;
  skos:definition "A foundation pile on which natural convection or forced circulation cooling systems or devices have been installed to remove heat from the ground (see Figure 24)."@en;
  skos:inScheme <https://w3id.org/permafrost/v/nrcglossary/scheme>;
  skos:prefLabel "pieu thermique"@fr, "thermal pile"@en;
  skos:scopeNote "There are two basic types of thermal piles. Passive or natural convection systems use self-powered devices, commonly referred to as thermosyphons, or heat pipes, which operate only when air temperatures are lower than the ground temperature. Forced circulation refrigeration systems require external power and mechanical equipment to circulate refrigerants, such as antifreeze liquids, chilled gases or cool air, and may be operated throughout the year or only during the winter. Both types may be fastened to, or form part of, the pile, or, if the pile is a sealed unit (e.g., a steel pipe), the pile itself may serve as a heat-removal device as well as a structural unit. Thermal piles are used to decrease the time for and ensure freezeback of the slurry and ground around piles, to prevent or control long-term permafrost degradation, and to decrease the existing ground temperatures around piles, particularly in warm temperature permafrost areas."@en;
  skos:topConceptOf <https://w3id.org/permafrost/v/nrcglossary/scheme> .

<https://w3id.org/permafrost/v/nrcglossary/t0363> a skos:Concept;
  dct:identifier "t0363"^^xsd:token;
  dct:source "https://nrc-publications.canada.ca/eng/view/object/?id=69fb8993-1baa-4225-b33a-6a02341d383d"^^xsd:anyURI,
    "https://nrc-publications.canada.ca/fra/voir/objet/?id=549123c3-092c-4fca-8dea-99d53eac06dd"^^xsd:anyURI;
  skos:definition "The properties of the ground governing the flow of heat through it, and its freezing and thawing conditions."@en;
  skos:inScheme <https://w3id.org/permafrost/v/nrcglossary/scheme>;
  skos:prefLabel "propriétés thermiques du gélisol"@fr, "thermal properties of frozen ground"@en;
  skos:scopeNote "The position of the interface between thawed and frozen soil with respect to the ground surface, for a given surface-temperature regime, depends on the thermal properties of the strata located above and immediately below the interface. The basic thermal properties of frozen ground are thermal conductivity, heat capacity and latent heat of fusion. Thermal conductivity is a measure of the quantity of heat that will flow through a unit area of a substance in unit time under a unit temperature gradient. Heat capacity (specific heat) is the amount of heat required to raise the temperature of a unit mass of a substance by one degree (sensible heat capacity). Volumetric heat capacity is the amount of heat required to raise the temperature of a unit volume of a substance by one degree. It is equal to the heat capacity multiplied by the density. Because the phase change in frozen soils is often gradual and continuous, the term \"apparent heat capacity\" is introduced to designate the rate of change of the total heat content (sensible plus latent heat) with temperature. The volumetric latent heat of fusion is the amount of heat required to melt the ice (or freeze the water) in a unit volume of soil. When phase change occurs over a temperature range, the latent heat manifests itself as an apparent (large) increase in heat capacity. Thermal diffusivity is defined as the ratio of the thermal conductivity to the volumetric heat capacity. It expresses the facility with which a material will undergo temperature change. These thermal properties vary with phase composition and hence temperature, soil type, total water content, porosity, degree of saturation, density and organic content."@en;
  skos:topConceptOf <https://w3id.org/permafrost/v/nrcglossary/scheme> .

<https://w3id.org/permafrost/v/nrcglossary/t0364> a skos:Concept;
  dct:identifier "t0364"^^xsd:token;
  dct:source "https://nrc-publications.canada.ca/eng/view/object/?id=69fb8993-1baa-4225-b33a-6a02341d383d"^^xsd:anyURI,
    "https://nrc-publications.canada.ca/fra/voir/objet/?id=549123c3-092c-4fca-8dea-99d53eac06dd"^^xsd:anyURI;
  skos:definition "A general term encompassing the temperature distribution and heat flows in the ground and their time-dependence (see Figure 2)."@en;
  skos:inScheme <https://w3id.org/permafrost/v/nrcglossary/scheme>;
  skos:prefLabel "thermal regime of the ground"@en;
  skos:scopeNote "Permafrost exists as a result of thermal conditions that maintain a ground temperature that does not rise above 0°C for at least two years. The ground temperature distribution is complicated, varying with depth from the surface and with time. Ground temperatures fluctuate in cyclical patterns on a daily and a yearly basis, in response to the heat losses and gains at the ground surface. The heat balance at the ground surface (which is indicated by the surface temperature) is highly variable with time, being affected by terrain and climate conditions as well by as the thermal properties of the ground itself. Changes in surface temperature impose a response that decays while travelling downwards. The rate of decay depends on the time scale involved, on the soil thermal properties and on the occurrence of freezing and thawing phenomena. The depth beyond which ground temperature fluctuations can be considered insignificant is the depth of zero annual amplitude. The effects of daily temperature variations at the ground surface penetrate to only a few centimetres; those due to weekly variations (e.g., transient weather systems) penetrate to perhaps several metres; and annual variations penetrate to a depth of about 10 to 20 metres. Longer-term changes in surface temperature caused by changes in climate and surface conditions may modify the thermal regime of the ground to much greater depths. Permafrost exists if the mean annual surface temperature is perennially below 0°C. Although the mean annual surface temperature may be below 0°C, the surface temperature will fluctuate during the year, causing a layer of ground immediately beneath the surface to thaw in the summer and freeze in the winter (the active layer). Small changes in the annual range of surface temperature and in the mean annual surface temperature from year to year, or over a period of a few years, may cause a layer of ground between the bottom of the active layer and the permafrost table to remain at a temperature above 0°C, creating a talik or residual thaw layer. The mean annual ground temperature usually increases with depth below the surface. In some northern areas, however, it is not uncommon to find that the mean annual ground temperature decreases in the upper 50 to 100 metres below the ground surface as a result of past changes in surface and climate conditions. Below that depth, it will increase as a result of heat flow from the interior of the earth. The rate of change of temperature with depth in the earth is known as the geothermal gradient. The geothermal gradient at a specific location can be determined from accurate measurements of ground temperature made at several depths to obtain the temperature profile over a period of time. A rough approximation of the mean annual surface temperature can be made by extrapolating the geothermal gradient to the ground surface. In permafrost areas, extrapolation of the gradient downwards to the point where the ground temperature changes from below to above 0°C will provide an estimate of the depth to the permafrost base. The thermal regime of the ground at various locations is often assessed using the mean annual ground temperature at the depth of zero annual amplitude. The geothermal heat flux is the amount of heat moving steadily outward from the interior of the earth by conduction through a unit area in unit time. It is generally calculated as the product of the geothermal gradient and the thermal conductivity of the earth materials at a given depth; its value is very small."@en;
  skos:topConceptOf <https://w3id.org/permafrost/v/nrcglossary/scheme> .

<https://w3id.org/permafrost/v/nrcglossary/t0365> a skos:Concept;
  dct:identifier "t0365"^^xsd:token;
  dct:source "https://nrc-publications.canada.ca/eng/view/object/?id=69fb8993-1baa-4225-b33a-6a02341d383d"^^xsd:anyURI,
    "https://nrc-publications.canada.ca/fra/voir/objet/?id=549123c3-092c-4fca-8dea-99d53eac06dd"^^xsd:anyURI;
  skos:definition "A layer or body of unfrozen ground (in a permafrost area) in which the temperature is above 0°C due to the local thermal regime of the ground."@en;
  skos:inScheme <https://w3id.org/permafrost/v/nrcglossary/scheme>;
  skos:prefLabel "thermal talik"@en;
  skos:scopeNote "The seasonally thawed ground in the active layer is a thermal talik."@en;
  skos:topConceptOf <https://w3id.org/permafrost/v/nrcglossary/scheme> .

<https://w3id.org/permafrost/v/nrcglossary/t0366> a skos:Concept;
  dct:identifier "t0366"^^xsd:token;
  dct:source "https://nrc-publications.canada.ca/eng/view/object/?id=69fb8993-1baa-4225-b33a-6a02341d383d"^^xsd:anyURI,
    "https://nrc-publications.canada.ca/fra/voir/objet/?id=549123c3-092c-4fca-8dea-99d53eac06dd"^^xsd:anyURI;
  skos:definition "The usually steep, horseshoe-shaped headwall of a retrogressive thaw slump."@en;
  skos:inScheme <https://w3id.org/permafrost/v/nrcglossary/scheme>;
  skos:prefLabel "thermo-erosional cirque"@en;
  skos:topConceptOf <https://w3id.org/permafrost/v/nrcglossary/scheme> .

<https://w3id.org/permafrost/v/nrcglossary/t0367> a skos:Concept;
  dct:identifier "t0367"^^xsd:token;
  dct:source "https://nrc-publications.canada.ca/eng/view/object/?id=69fb8993-1baa-4225-b33a-6a02341d383d"^^xsd:anyURI,
    "https://nrc-publications.canada.ca/fra/voir/objet/?id=549123c3-092c-4fca-8dea-99d53eac06dd"^^xsd:anyURI;
  skos:definition "A recess at the base of a river bank or coastal bluff, produced by thermal erosion of ice-bonded permafrost (see Figure 22d)."@en;
  skos:inScheme <https://w3id.org/permafrost/v/nrcglossary/scheme>;
  skos:prefLabel "niche d'érosion thermique"@fr, "thermo-erosional niche"@en;
  skos:scopeNote "A niche may extend more than 10 m into a river bank or coastal bluff.Subsequently, the undercut sediments may collapse along a line of weakness, such as an ice wedge, destroying the niche. Niche development and bank/bluff collapse is a unique mechanism of erosion in permafrost regions. Very rapid coastal or bank retreat can occur if collapse debris is removed by waves or water currents."@en;
  skos:topConceptOf <https://w3id.org/permafrost/v/nrcglossary/scheme> .

<https://w3id.org/permafrost/v/nrcglossary/t0368> a skos:Concept;
  dct:identifier "t0368"^^xsd:token;
  dct:source "https://nrc-publications.canada.ca/eng/view/object/?id=69fb8993-1baa-4225-b33a-6a02341d383d"^^xsd:anyURI,
    "https://nrc-publications.canada.ca/fra/voir/objet/?id=549123c3-092c-4fca-8dea-99d53eac06dd"^^xsd:anyURI;
  skos:definition "The process by which characteristic landforms result from the thawing of ice-rich permafrost or the melting of massive ice."@en;
  skos:inScheme <https://w3id.org/permafrost/v/nrcglossary/scheme>;
  skos:prefLabel "thermokarst"@en, "thermokarst"@fr;
  skos:scopeNote "Landforms found in thermokarst terrain include alasses, thermokarst lakes, and thermokarst mounds."@en;
  skos:topConceptOf <https://w3id.org/permafrost/v/nrcglossary/scheme> .

<https://w3id.org/permafrost/v/nrcglossary/t0369> a skos:Concept;
  dct:identifier "t0369"^^xsd:token;
  dct:source "https://nrc-publications.canada.ca/eng/view/object/?id=69fb8993-1baa-4225-b33a-6a02341d383d"^^xsd:anyURI,
    "https://nrc-publications.canada.ca/fra/voir/objet/?id=549123c3-092c-4fca-8dea-99d53eac06dd"^^xsd:anyURI;
  skos:definition "A lake occupying a closed depression formed by settlement of the ground following thawing of ice-rich permafrost or the melting of massive ice (see Figure 22c)."@en;
  skos:hiddenLabel "cave-in lake"@en, "thaw lake"@en;
  skos:inScheme <https://w3id.org/permafrost/v/nrcglossary/scheme>;
  skos:prefLabel "lac de thermokarst"@fr, "thermokarst lake"@en;
  skos:scopeNote "Thermokarst lakes are generally shallow. The depressions may expand by active-layer failure processes (see alas); the lakes may expand by thermokarst processes (see also oriented lake). In glaciated terrain they may be similar in appearance to kettle lakes."@en;
  skos:topConceptOf <https://w3id.org/permafrost/v/nrcglossary/scheme> .

<https://w3id.org/permafrost/v/nrcglossary/t0370> a skos:Concept;
  dct:identifier "t0370"^^xsd:token;
  dct:source "https://nrc-publications.canada.ca/eng/view/object/?id=69fb8993-1baa-4225-b33a-6a02341d383d"^^xsd:anyURI,
    "https://nrc-publications.canada.ca/fra/voir/objet/?id=549123c3-092c-4fca-8dea-99d53eac06dd"^^xsd:anyURI;
  skos:definition "A hummock remaining after melting of the ice wedges surrounding an ice- wedge polygon (see Figure 22e)."@en;
  skos:hiddenLabel "baydzherakh"@en, "cemetery mound"@en, "graveyard mound"@en;
  skos:inScheme <https://w3id.org/permafrost/v/nrcglossary/scheme>;
  skos:prefLabel "thermokarst mound"@en;
  skos:scopeNote "Thermokarst mounds occur in groups forming a distinctive surficial network of regularly shaped mounds separated by troughs formed by the melting of ice wedges."@en;
  skos:topConceptOf <https://w3id.org/permafrost/v/nrcglossary/scheme> .

<https://w3id.org/permafrost/v/nrcglossary/t0371> a skos:Concept;
  dct:identifier "t0371"^^xsd:token;
  dct:source "https://nrc-publications.canada.ca/eng/view/object/?id=69fb8993-1baa-4225-b33a-6a02341d383d"^^xsd:anyURI,
    "https://nrc-publications.canada.ca/fra/voir/objet/?id=549123c3-092c-4fca-8dea-99d53eac06dd"^^xsd:anyURI;
  skos:definition "The often irregular topography resulting from the melting of excess ground ice and subsequent thaw settlement (see Figure 22)."@en;
  skos:inScheme <https://w3id.org/permafrost/v/nrcglossary/scheme>;
  skos:prefLabel "modelé de thermokarst"@fr, "thermokarst terrain"@en;
  skos:scopeNote "Thermokarst terrain is so named because of its superficial resemblance to the karst topography typical of limestone regions. The melting of ground ice may be initiated by climatic change, destruction of an insulating vegetation cover by fire, animals or man, or by any other disturbance of the thermal regime of the ground, including the acceleration of the rate of thawing by moving water. Annual thawing of the active layer does not produce thermokarst terrain. Morphological features of thermokarst topography include depressions (see alas); lakes (see oriented lake; thermokarst lake); mounds (see thermokarst mound); and small, more or less equidimensional depressions or pits. Thermokarst landforms may be divided into active and inactive forms. Inactive thermokarst indicates that thermal equilibrium has been regained, whereas active thermokarst indicates continuing thermal disequilibrium. Except for thaw sinks there may be little underground drainage in thermokarst terrain."@en;
  skos:topConceptOf <https://w3id.org/permafrost/v/nrcglossary/scheme> .

<https://w3id.org/permafrost/v/nrcglossary/t0372> a skos:Concept;
  dct:identifier "t0372"^^xsd:token;
  dct:source "https://nrc-publications.canada.ca/eng/view/object/?id=69fb8993-1baa-4225-b33a-6a02341d383d"^^xsd:anyURI,
    "https://nrc-publications.canada.ca/fra/voir/objet/?id=549123c3-092c-4fca-8dea-99d53eac06dd"^^xsd:anyURI;
  skos:definition "A passive heat transfer device installed to remove heat from the ground (see Figure 24)."@en;
  skos:inScheme <https://w3id.org/permafrost/v/nrcglossary/scheme>;
  skos:prefLabel "thermosiphon"@fr, "thermosyphon"@en;
  skos:scopeNote "A thermosyphon, also called thermotube, or heat pipe, usually consists of a sealed tube, with a small radiator above the ground surface, containing a liquid and/or gas. These devices have no moving parts, require no external power for operation, and function only when air temperatures are lower than the ground temperature. They may be either single- or two-phase systems. A single-phase thermosyphon is usually liquid- or air-filled. During the winter, heat from the soil surrounding the embedded portion of the pipe is absorbed by and thus warms the working fluid, which rises to the above-ground radiator section of the pipe exposed to the cooler air and loses its heat by conduction and natural convection. A two-phase thermosyphon contains a working fluid that can be in either the liquid or vapour phase, depending on its temperature. When the air temperature falls below the ground temperature, the vapour condenses in the radiator section of the tube, the pressure in the tube is reduced and the liquid in the lower section starts to boil. The resulting cycle of boiling, vapour movement up the tube, condensation, and return of the condensate by gravity flow is an effective way of transferring heat up the tube, thus cooling the ground."@en;
  skos:topConceptOf <https://w3id.org/permafrost/v/nrcglossary/scheme> .

<https://w3id.org/permafrost/v/nrcglossary/t0373> a skos:Concept;
  dct:identifier "t0373"^^xsd:token;
  dct:source "https://nrc-publications.canada.ca/eng/view/object/?id=69fb8993-1baa-4225-b33a-6a02341d383d"^^xsd:anyURI,
    "https://nrc-publications.canada.ca/fra/voir/objet/?id=549123c3-092c-4fca-8dea-99d53eac06dd"^^xsd:anyURI;
  skos:definition "Perennial hummocks formed in either the active layer in permafrost areas, or in the seasonally frozen ground in non-permafrost areas, during freezing of the ground (see Figure 20d)."@en;
  skos:inScheme <https://w3id.org/permafrost/v/nrcglossary/scheme>;
  skos:prefLabel "thufur"@en, "thufur"@fr;
  skos:scopeNote "Thufur (an Icelandic term, plural of \"thufa\") can be formed in the warmer part of the zone of discontinuous permafrost and also under conditions of maritime seasonal frost. The hummocks may be as much as 50 cm in height and 160 cm in diameter and can reform within 20 years following destruction. Growth is favoured by silty sediments, a maritime climate and reasonably good drainage."@en;
  skos:topConceptOf <https://w3id.org/permafrost/v/nrcglossary/scheme> .

<https://w3id.org/permafrost/v/nrcglossary/t0374> a skos:Concept;
  dct:identifier "t0374"^^xsd:token;
  dct:source "https://nrc-publications.canada.ca/eng/view/object/?id=69fb8993-1baa-4225-b33a-6a02341d383d"^^xsd:anyURI,
    "https://nrc-publications.canada.ca/fra/voir/objet/?id=549123c3-092c-4fca-8dea-99d53eac06dd"^^xsd:anyURI;
  skos:definition "The cumulative number of degree-days, calculated by adding all the negative mean daily air temperatures (?C) for a specific station during a calendar year."@en;
  skos:inScheme <https://w3id.org/permafrost/v/nrcglossary/scheme>;
  skos:prefLabel "total annual freezing index"@en;
  skos:topConceptOf <https://w3id.org/permafrost/v/nrcglossary/scheme> .

<https://w3id.org/permafrost/v/nrcglossary/t0375> a skos:Concept;
  dct:identifier "t0375"^^xsd:token;
  dct:source "https://nrc-publications.canada.ca/eng/view/object/?id=69fb8993-1baa-4225-b33a-6a02341d383d"^^xsd:anyURI,
    "https://nrc-publications.canada.ca/fra/voir/objet/?id=549123c3-092c-4fca-8dea-99d53eac06dd"^^xsd:anyURI;
  skos:definition "The cumulative number of degree-days, calculated by adding all the positive mean daily air temperatures (?C) for a specific station during a calendar year."@en;
  skos:inScheme <https://w3id.org/permafrost/v/nrcglossary/scheme>;
  skos:prefLabel "total annual thawing index"@en;
  skos:topConceptOf <https://w3id.org/permafrost/v/nrcglossary/scheme> .

<https://w3id.org/permafrost/v/nrcglossary/t0376> a skos:Concept;
  dct:identifier "t0376"^^xsd:token;
  dct:source "https://nrc-publications.canada.ca/eng/view/object/?id=69fb8993-1baa-4225-b33a-6a02341d383d"^^xsd:anyURI,
    "https://nrc-publications.canada.ca/fra/voir/objet/?id=549123c3-092c-4fca-8dea-99d53eac06dd"^^xsd:anyURI;
  skos:definition "The total amount of water (unfrozen water plus ice) contained in soil or rock (see Figure 3)."@en;
  skos:inScheme <https://w3id.org/permafrost/v/nrcglossary/scheme>;
  skos:prefLabel "total water content (of frozen ground)"@en;
  skos:scopeNote "When no ice is present, the total water content is usually referred to as \"water content\" or \"moisture content\". The total water content of a soil or rock sample includes free water, interfacial (adsorbed) water, and water absorbed by organic material. Water of crystallization or hydration (e.g., in gypsum) is usually not included. The total water content is normally determined in one of two ways: 1. on a dry-weight basis (gravimetric total water content), as the ratio of the mass of the water and ice in a sample to the dry mass of the sample, expressed as a percentage; or 2. on a volume basis (volumetric total water content), as the ratio of the volume of water and ice in a sample to the volume of the whole sample, expressed as a fraction (or, less commonly, as a percentage). Because of the way in which it is defined, the volumetric total water content cannot exceed unity, whereas the gravimetric total water content can greatly exceed 100 percent. During thawing of a sample of frozen ground the volumetric total water content decreases, but the gravimetric total water content remains constant."@en;
  skos:topConceptOf <https://w3id.org/permafrost/v/nrcglossary/scheme> .

<https://w3id.org/permafrost/v/nrcglossary/t0377> a skos:Concept;
  dct:identifier "t0377"^^xsd:token;
  dct:source "https://nrc-publications.canada.ca/eng/view/object/?id=69fb8993-1baa-4225-b33a-6a02341d383d"^^xsd:anyURI,
    "https://nrc-publications.canada.ca/fra/voir/objet/?id=549123c3-092c-4fca-8dea-99d53eac06dd"^^xsd:anyURI;
  skos:definition "A layer or body of unfrozen ground (in a permafrost area) that is gradually being eliminated by freezing (see Figure 11)."@en;
  skos:inScheme <https://w3id.org/permafrost/v/nrcglossary/scheme>;
  skos:prefLabel "transient talik"@en;
  skos:scopeNote "An example is the initially noncryotic closed talik below a small lake which, upon draining of the lake, is turned into a transient, isolated talik by permafrost aggradation."@en;
  skos:topConceptOf <https://w3id.org/permafrost/v/nrcglossary/scheme> .

<https://w3id.org/permafrost/v/nrcglossary/t0378> a skos:Concept;
  dct:identifier "t0378"^^xsd:token;
  dct:source "https://nrc-publications.canada.ca/eng/view/object/?id=69fb8993-1baa-4225-b33a-6a02341d383d"^^xsd:anyURI,
    "https://nrc-publications.canada.ca/fra/voir/objet/?id=549123c3-092c-4fca-8dea-99d53eac06dd"^^xsd:anyURI;
  skos:definition "Treeless terrain, with a continuous cover of vegetation, found at both high latitudes and high altitudes."@en;
  skos:inScheme <https://w3id.org/permafrost/v/nrcglossary/scheme>;
  skos:prefLabel "toundra"@fr, "tundra"@en;
  skos:scopeNote "Tundra vegetation comprises lichens, mosses, sedges, grasses, forbs and low shrubs, including heaths, and dwarf willows and birches. This vegetation cover occurs most widely in the zone immediately north of the boreal forest including the treeless parts of the forest-tundra ecotone adjacent to the treeline. In high altitudes, tundra occurs immediately above the forest zone, and the upper altitudinal timberline. The term \"tundra\" is used to refer to both the region and the vegetation growing in the region. It should not be used as an adjective to describe lakes, polygons or other physiographic features. Areas of discontinuous vegetation in the polar semi-desert of the High Arctic are better termed barrens. Unvegetated areas of polar desert may be caused by climatic (too cold or too dry) or edaphic (low soil nutrients or toxic substrate) factors or a combination of both."@en;
  skos:topConceptOf <https://w3id.org/permafrost/v/nrcglossary/scheme> .

<https://w3id.org/permafrost/v/nrcglossary/t0379> a skos:Concept;
  dct:identifier "t0379"^^xsd:token;
  dct:source "https://nrc-publications.canada.ca/eng/view/object/?id=69fb8993-1baa-4225-b33a-6a02341d383d"^^xsd:anyURI,
    "https://nrc-publications.canada.ca/fra/voir/objet/?id=549123c3-092c-4fca-8dea-99d53eac06dd"^^xsd:anyURI;
  skos:definition "A mineral soil showing marked evidence of cryoturbation, as indicated by broken horizons and displaced material."@en;
  skos:inScheme <https://w3id.org/permafrost/v/nrcglossary/scheme>;
  skos:prefLabel "turbic cryosol"@en;
  skos:scopeNote "Turbic cryosols generally occur on patterned ground. They have mean annual ground temperatures below 0°C, with permafrost within 2 m below the surface."@en;
  skos:topConceptOf <https://w3id.org/permafrost/v/nrcglossary/scheme> .

<https://w3id.org/permafrost/v/nrcglossary/t0380> a skos:Concept;
  dct:identifier "t0380"^^xsd:token;
  dct:source "https://nrc-publications.canada.ca/eng/view/object/?id=69fb8993-1baa-4225-b33a-6a02341d383d"^^xsd:anyURI,
    "https://nrc-publications.canada.ca/fra/voir/objet/?id=549123c3-092c-4fca-8dea-99d53eac06dd"^^xsd:anyURI;
  skos:definition "A solifluction lobe with its front covered by a vegetation mat."@en;
  skos:inScheme <https://w3id.org/permafrost/v/nrcglossary/scheme>;
  skos:prefLabel "turf-banked (solifluction) lobe"@en;
  skos:topConceptOf <https://w3id.org/permafrost/v/nrcglossary/scheme> .

<https://w3id.org/permafrost/v/nrcglossary/t0381> a skos:Concept;
  dct:identifier "t0381"^^xsd:token;
  dct:source "https://nrc-publications.canada.ca/eng/view/object/?id=69fb8993-1baa-4225-b33a-6a02341d383d"^^xsd:anyURI,
    "https://nrc-publications.canada.ca/fra/voir/objet/?id=549123c3-092c-4fca-8dea-99d53eac06dd"^^xsd:anyURI;
  skos:definition "A solifluction terrace with its front covered by a vegetation mat."@en;
  skos:inScheme <https://w3id.org/permafrost/v/nrcglossary/scheme>;
  skos:prefLabel "turf-banked (solifluction) terrace"@en;
  skos:topConceptOf <https://w3id.org/permafrost/v/nrcglossary/scheme> .

<https://w3id.org/permafrost/v/nrcglossary/t0382> a skos:Concept;
  dct:identifier "t0382"^^xsd:token;
  dct:source "https://nrc-publications.canada.ca/eng/view/object/?id=69fb8993-1baa-4225-b33a-6a02341d383d"^^xsd:anyURI,
    "https://nrc-publications.canada.ca/fra/voir/objet/?id=549123c3-092c-4fca-8dea-99d53eac06dd"^^xsd:anyURI;
  skos:definition "A hummock consisting of vegetation and organic matter with or without a core of mineral soil or stones (see Figure 20c)."@en;
  skos:inScheme <https://w3id.org/permafrost/v/nrcglossary/scheme>;
  skos:prefLabel "turf hummock"@en;
  skos:topConceptOf <https://w3id.org/permafrost/v/nrcglossary/scheme> .

<https://w3id.org/permafrost/v/nrcglossary/t0383> a skos:Concept;
  dct:identifier "t0383"^^xsd:token;
  dct:source "https://nrc-publications.canada.ca/eng/view/object/?id=69fb8993-1baa-4225-b33a-6a02341d383d"^^xsd:anyURI,
    "https://nrc-publications.canada.ca/fra/voir/objet/?id=549123c3-092c-4fca-8dea-99d53eac06dd"^^xsd:anyURI;
  skos:definition "Ground in which two layers of permafrost are separated by a layer of unfrozen ground."@en;
  skos:inScheme <https://w3id.org/permafrost/v/nrcglossary/scheme>;
  skos:prefLabel "two-layer permafrost"@en;
  skos:scopeNote "In two-layer permafrost, the lower permafrost layer may represent relict permafrost remaining from an earlier cold period, whereas the upper permafrost layer represents more recent development of epigenetic permafrost. The intervening unfrozen layer could be a hydrothermal talik or a hydrochemical talik."@en;
  skos:topConceptOf <https://w3id.org/permafrost/v/nrcglossary/scheme> .

<https://w3id.org/permafrost/v/nrcglossary/t0384> a skos:Concept;
  dct:identifier "t0384"^^xsd:token;
  dct:source "https://nrc-publications.canada.ca/eng/view/object/?id=69fb8993-1baa-4225-b33a-6a02341d383d"^^xsd:anyURI,
    "https://nrc-publications.canada.ca/fra/voir/objet/?id=549123c3-092c-4fca-8dea-99d53eac06dd"^^xsd:anyURI;
  skos:definition "A passive heat transfer device, filled with a temperature-dependent liquid/vapour combination, installed to remove heat from the ground (see Figure 24)."@en;
  skos:inScheme <https://w3id.org/permafrost/v/nrcglossary/scheme>;
  skos:prefLabel "two-phase thermosyphon"@en;
  skos:scopeNote "A two-phase thermosyphon consists of a sealed tube with a small radiator above the ground surface, containing a working fluid that can be in either the liquid or vapour phase, depending on its temperature. These devices have no moving parts, and they require no external power for operation. When the air temperature falls below the ground temperature, the vapour condenses in the radiator section of the tube, the pressure in the tube is reduced and the liquid in the lower section starts to boil. The resulting cycle of boiling, vapour movement up the tube, condensation, and return of the condensate by gravity flow is an effective way of transferring heat up the tube, thus cooling the ground."@en;
  skos:topConceptOf <https://w3id.org/permafrost/v/nrcglossary/scheme> .

<https://w3id.org/permafrost/v/nrcglossary/t0385> a skos:Concept;
  dct:identifier "t0385"^^xsd:token;
  dct:source "https://nrc-publications.canada.ca/eng/view/object/?id=69fb8993-1baa-4225-b33a-6a02341d383d"^^xsd:anyURI,
    "https://nrc-publications.canada.ca/fra/voir/objet/?id=549123c3-092c-4fca-8dea-99d53eac06dd"^^xsd:anyURI;
  skos:definition "Soil or rock that does not contain any ice."@en;
  skos:inScheme <https://w3id.org/permafrost/v/nrcglossary/scheme>;
  skos:prefLabel "sol non gelé"@fr, "unfrozen ground"@en;
  skos:scopeNote "Unfrozen ground can be cryotic (T ? 0°C) if freezing-point depression prevents freezing of the pore water (see Figures 2 and 3), or if no water is available to freeze (e.g., in dry permafrost). It should not be called thawed ground, unless it is known that the ground has previously contained ice."@en;
  skos:topConceptOf <https://w3id.org/permafrost/v/nrcglossary/scheme> .

<https://w3id.org/permafrost/v/nrcglossary/t0386> a skos:Concept;
  dct:identifier "t0386"^^xsd:token;
  dct:source "https://nrc-publications.canada.ca/eng/view/object/?id=69fb8993-1baa-4225-b33a-6a02341d383d"^^xsd:anyURI,
    "https://nrc-publications.canada.ca/fra/voir/objet/?id=549123c3-092c-4fca-8dea-99d53eac06dd"^^xsd:anyURI;
  skos:definition "The amount of unfrozen (liquid) water contained in frozen soil or rock (see Figure 3)."@en;
  skos:hiddenLabel "liquid water content"@en;
  skos:inScheme <https://w3id.org/permafrost/v/nrcglossary/scheme>;
  skos:prefLabel "unfrozen water content"@en;
  skos:scopeNote "The unfrozen water content can include free water that can be moved by gravity, and/or interfacial (adsorbed) water that cannot be moved by gravity. The main factors controlling the unfrozen water content in frozen ground (or in partially frozen ground) are temperature, specific surface area of mineral particles, mineral type, pore size distribution, dissolved-solids content of the pore water, and kind of exchangeable ions. The unfrozen water content at temperatures below 0°C is highest in clays and decreases with decreasing temperature, clay content, and dissolved-solids content, and with increasing particle size. Unfrozen water content, like total water content, can be determined either gravimetrically or volumetrically."@en;
  skos:topConceptOf <https://w3id.org/permafrost/v/nrcglossary/scheme> .

<https://w3id.org/permafrost/v/nrcglossary/t0387> a skos:Concept;
  dct:identifier "t0387"^^xsd:token;
  dct:source "https://nrc-publications.canada.ca/eng/view/object/?id=69fb8993-1baa-4225-b33a-6a02341d383d"^^xsd:anyURI,
    "https://nrc-publications.canada.ca/fra/voir/objet/?id=549123c3-092c-4fca-8dea-99d53eac06dd"^^xsd:anyURI;
  skos:definition "The advance of a freezing front upwards from the permafrost table during annual freezing of the active layer."@en;
  skos:inScheme <https://w3id.org/permafrost/v/nrcglossary/scheme>;
  skos:prefLabel "upward freezing"@en;
  skos:scopeNote "Upward freezing can only occur where the active layer extends to the permafrost table."@en;
  skos:topConceptOf <https://w3id.org/permafrost/v/nrcglossary/scheme> .

<https://w3id.org/permafrost/v/nrcglossary/t0388> a skos:Concept;
  dct:identifier "t0388"^^xsd:token;
  dct:source "https://nrc-publications.canada.ca/eng/view/object/?id=69fb8993-1baa-4225-b33a-6a02341d383d"^^xsd:anyURI,
    "https://nrc-publications.canada.ca/fra/voir/objet/?id=549123c3-092c-4fca-8dea-99d53eac06dd"^^xsd:anyURI;
  skos:definition "A comprehensive term for ice of any origin occupying cracks in permafrost."@en;
  skos:inScheme <https://w3id.org/permafrost/v/nrcglossary/scheme>;
  skos:prefLabel "vein ice"@en;
  skos:scopeNote "Vein ice occurs in various forms, including horizontal layers or lenses, tabular sheets, wedges and reticulate nets."@en;
  skos:topConceptOf <https://w3id.org/permafrost/v/nrcglossary/scheme> .

<https://w3id.org/permafrost/v/nrcglossary/t0389> a skos:Concept;
  dct:identifier "t0389"^^xsd:token;
  dct:source "https://nrc-publications.canada.ca/eng/view/object/?id=69fb8993-1baa-4225-b33a-6a02341d383d"^^xsd:anyURI,
    "https://nrc-publications.canada.ca/fra/voir/objet/?id=549123c3-092c-4fca-8dea-99d53eac06dd"^^xsd:anyURI;
  skos:definition "The amount of heat required to raise the temperature of a unit volume of a substance by one degree."@en;
  skos:inScheme <https://w3id.org/permafrost/v/nrcglossary/scheme>;
  skos:prefLabel "volumetric heat capacity"@en;
  skos:scopeNote "The volumetric heat capacity of a material is equal to its (specific) heat capacity multiplied by the density of the material."@en;
  skos:topConceptOf <https://w3id.org/permafrost/v/nrcglossary/scheme> .

<https://w3id.org/permafrost/v/nrcglossary/t0390> a skos:Concept;
  dct:identifier "t0390"^^xsd:token;
  dct:source "https://nrc-publications.canada.ca/eng/view/object/?id=69fb8993-1baa-4225-b33a-6a02341d383d"^^xsd:anyURI,
    "https://nrc-publications.canada.ca/fra/voir/objet/?id=549123c3-092c-4fca-8dea-99d53eac06dd"^^xsd:anyURI;
  skos:definition "The amount of heat required to melt all the ice (or freeze all the pore water) in a unit volume of soil or rock."@en;
  skos:inScheme <https://w3id.org/permafrost/v/nrcglossary/scheme>;
  skos:prefLabel "volumetric latent heat of fusion"@en;
  skos:scopeNote "When the phase change occurs over a range of temperature, then the latent heat manifests itself as an apparent (large) increase in the heat capacity."@en;
  skos:topConceptOf <https://w3id.org/permafrost/v/nrcglossary/scheme> .

<https://w3id.org/permafrost/v/nrcglossary/t0391> a skos:Concept;
  dct:identifier "t0391"^^xsd:token;
  dct:source "https://nrc-publications.canada.ca/eng/view/object/?id=69fb8993-1baa-4225-b33a-6a02341d383d"^^xsd:anyURI,
    "https://nrc-publications.canada.ca/fra/voir/objet/?id=549123c3-092c-4fca-8dea-99d53eac06dd"^^xsd:anyURI;
  skos:definition "The ratio of the volume of the water and ice in a sample to the volume of the whole sample, expressed as a fraction (or, less commonly, as a percentage)."@en;
  skos:inScheme <https://w3id.org/permafrost/v/nrcglossary/scheme>;
  skos:prefLabel "volumetric (total) water content"@en;
  skos:scopeNote "Because of the way it is defined, the volumetric total water content cannot exceed unity (or 100 percent). During thawing of a sample of frozen ground the volumetric total water content decreases."@en;
  skos:topConceptOf <https://w3id.org/permafrost/v/nrcglossary/scheme> .

<https://w3id.org/permafrost/v/nrcglossary/t0392> a skos:Concept;
  dct:identifier "t0392"^^xsd:token;
  dct:source "https://nrc-publications.canada.ca/eng/view/object/?id=69fb8993-1baa-4225-b33a-6a02341d383d"^^xsd:anyURI,
    "https://nrc-publications.canada.ca/fra/voir/objet/?id=549123c3-092c-4fca-8dea-99d53eac06dd"^^xsd:anyURI;
  skos:definition "A water-filled depression surrounding a palsa."@en;
  skos:inScheme <https://w3id.org/permafrost/v/nrcglossary/scheme>;
  skos:prefLabel "waterbody encircling a palsa"@en;
  skos:topConceptOf <https://w3id.org/permafrost/v/nrcglossary/scheme> .

<https://w3id.org/permafrost/v/nrcglossary/t0393> a skos:Concept;
  dct:identifier "t0393"^^xsd:token;
  dct:source "https://nrc-publications.canada.ca/eng/view/object/?id=69fb8993-1baa-4225-b33a-6a02341d383d"^^xsd:anyURI,
    "https://nrc-publications.canada.ca/fra/voir/objet/?id=549123c3-092c-4fca-8dea-99d53eac06dd"^^xsd:anyURI;
  skos:definition "Ice occurring in an ice wedge (see Figure 17)."@en;
  skos:inScheme <https://w3id.org/permafrost/v/nrcglossary/scheme>;
  skos:prefLabel "wedge ice"@en;
  skos:scopeNote "Wedge ice comprises a series of ice veins formed in thermal contraction cracks at the same location over a period of time. The ice is vertically to subvertically banded and may be discoloured by sediments and contain air bubbles that tend to be arranged in nearly vertical bands. The presence of many small bubbles may give the ice a milky appearance. Individual bands of ice are a few millimetres to a centimetre in width."@en;
  skos:topConceptOf <https://w3id.org/permafrost/v/nrcglossary/scheme> .

<https://w3id.org/permafrost/v/nrcglossary/t0394> a skos:Concept;
  dct:identifier "t0394"^^xsd:token;
  dct:source "https://nrc-publications.canada.ca/eng/view/object/?id=69fb8993-1baa-4225-b33a-6a02341d383d"^^xsd:anyURI,
    "https://nrc-publications.canada.ca/fra/voir/objet/?id=549123c3-092c-4fca-8dea-99d53eac06dd"^^xsd:anyURI;
  skos:definition "Ice-bearing permafrost in which all the soil particles are held together by ice."@en;
  skos:inScheme <https://w3id.org/permafrost/v/nrcglossary/scheme>;
  skos:prefLabel "well-bonded permafrost"@en;
  skos:topConceptOf <https://w3id.org/permafrost/v/nrcglossary/scheme> .

<https://w3id.org/permafrost/v/nrcglossary/t0395> a skos:Concept;
  dct:identifier "t0395"^^xsd:token;
  dct:source "https://nrc-publications.canada.ca/eng/view/object/?id=69fb8993-1baa-4225-b33a-6a02341d383d"^^xsd:anyURI,
    "https://nrc-publications.canada.ca/fra/voir/objet/?id=549123c3-092c-4fca-8dea-99d53eac06dd"^^xsd:anyURI;
  skos:altLabel "elastic modulus"@en;
  skos:definition "The ratio of increase in stress acting on a test specimen, to the resulting increase in strain, under constant transverse stress."@en;
  skos:inScheme <https://w3id.org/permafrost/v/nrcglossary/scheme>;
  skos:prefLabel "Young's modulus"@en;
  skos:scopeNote "Limited to materials having a linear stress-strain relationship over the range of loading applied."@en;
  skos:topConceptOf <https://w3id.org/permafrost/v/nrcglossary/scheme> .

<https://w3id.org/permafrost/v/nrcglossary/t0396> a skos:Concept;
  dct:identifier "t0396"^^xsd:token;
  dct:source "https://nrc-publications.canada.ca/eng/view/object/?id=69fb8993-1baa-4225-b33a-6a02341d383d"^^xsd:anyURI,
    "https://nrc-publications.canada.ca/fra/voir/objet/?id=549123c3-092c-4fca-8dea-99d53eac06dd"^^xsd:anyURI;
  skos:definition "The persistence of a nearly constant temperature, very close to the freezing point, during annual freezing (and occasionally during thawing) of the active layer (see Figure 6)."@en;
  skos:inScheme <https://w3id.org/permafrost/v/nrcglossary/scheme>;
  skos:prefLabel "zero curtain"@en;
  skos:scopeNote "The zero curtain results from the dissipation of the latent heat of fusion of water during freezing or thawing of the ground. It can persist for several hours or several weeks depending largely on the total water content of the ground, snowcover and air temperatures. Although the zero curtain can occur in non- permafrost areas, it is most pronounced in permafrost areas, especially during freezing of the active layer. The zero curtain is not only evident in freezing and thawing of undisturbed natural terrain but is also an important factor with respect to frost action, refreezing of the ground (backfill or slurry) around foundations, etc. and can have a major effect on the thermal regime of the active layer and of the permafrost."@en;
  skos:topConceptOf <https://w3id.org/permafrost/v/nrcglossary/scheme> .

<https://w3id.org/permafrost/v/nrcglossary/t0397> a skos:Concept;
  dct:identifier "t0397"^^xsd:token;
  dct:source "https://nrc-publications.canada.ca/eng/view/object/?id=69fb8993-1baa-4225-b33a-6a02341d383d"^^xsd:anyURI,
    "https://nrc-publications.canada.ca/fra/voir/objet/?id=549123c3-092c-4fca-8dea-99d53eac06dd"^^xsd:anyURI;
  skos:definition "That portion of the subsurface where the conditions of temperature and pressure are suitable for the formation and preservation of gas hydrates."@en;
  skos:inScheme <https://w3id.org/permafrost/v/nrcglossary/scheme>;
  skos:prefLabel "zone of gas-hydrate stability"@en;
  skos:scopeNote "In permafrost regions, the zone of gas-hydrate stability is commonly found near the permafrost base."@en;
  skos:topConceptOf <https://w3id.org/permafrost/v/nrcglossary/scheme> .
